@prefix :     <https://w3id.org/foodpairing_inspire_kg#> .
@prefix dct:  <http://purl.org/dc/terms/> .
@prefix owl:  <http://www.w3.org/2002/07/owl#> .
@prefix rdf:  <http://www.w3.org/1999/02/22-rdf-syntax-ns#> .
@prefix rdfs: <http://www.w3.org/2000/01/rdf-schema#> .
@prefix skos: <http://www.w3.org/2004/02/skos/core#> .
@prefix xml:  <http://www.w3.org/XML/1998/namespace> .
@prefix xsd:  <http://www.w3.org/2001/XMLSchema#> .

:spicy  rdf:type        :AromaType ;
        skos:prefLabel  "Spicy"@en .

<https://w3id.org/foodpairing_inspire_kg>
        rdf:type         owl:Ontology ;
        rdfs:label       "Inspire KG"@en ;
        dct:contributor  <https://www.linkedin.com/in/marc-luis-cer%C3%B3n-a73825241/> ;
        dct:created      "2023-10-13"^^xsd:date ;
        dct:creator      <https://www.linkedin.com/in/peter-coucquyt-8922419/> , <https://www.linkedin.com/in/skontopo/> , <https://www.linkedin.com/in/bernardlahousse/> ;
        dct:description  "The Inspire Knowledge Graph contains (a) 102 food ingredients, (b) a 4-layer taxonomy of 139 ingredient categories, (c) sensory information for the ingredients (aromas, tastes, textures, trigeminals), (d) functional benefits of ingredients, (e) ingredient pairings."@en ;
        dct:license      <https://creativecommons.org/licenses/by/4.0/> ;
        dct:publisher    <https://www.foodpairing.com/> ;
        dct:title        "The Inspire Knowledge Graph"@en ;
        owl:imports      <http://www.w3.org/2004/02/skos/core> ;
        owl:versionInfo  "1.0.0" .

:caramel  rdf:type      :AromaType ;
        skos:prefLabel  "Caramel"@en .

:meaty_aroma  rdf:type  :Aroma ;
        skos:prefLabel  "Meaty Aroma"@en ;
        :hasAromaType   :animal .

:cookies_and_cakes  rdf:type  skos:Concept , :IngredientCategory ;
        skos:broader     :bakery_category ;
        skos:definition  "Refers to baked products made primarily from flour, water, and yeast or other leavening agents."@en ;
        skos:prefLabel   "Cookies And Cakes"@en .

:spirits  rdf:type       skos:Concept , :IngredientCategory ;
        skos:broader     :alcoholic_drink ;
        skos:definition  "Refers to a broad category of distilled alcoholic beverages, including liquors, whiskey, vodka, rum, gin, tequila, and others."@en ;
        skos:prefLabel   "Spirits"@en .

:breakfast_cereal  rdf:type  skos:Concept , :IngredientCategory ;
        skos:broader     :cereals_category ;
        skos:definition  "Encompasses processed cereal-based products typically consumed as breakfast, including flakes, granola, and oatmeal."@en ;
        skos:prefLabel   "Breakfast Cereal"@en .

:woody  rdf:type        :AromaType ;
        skos:prefLabel  "Woody"@en .

:8d06ddfc-2e8e-4eca-aadb-554cfab5aa6a
        rdf:type         :FunctionalBenefit ;
        skos:definition  "Prebiotics are dietary fibers that nourish beneficial gut bacteria, supporting a healthy digestive system." ;
        skos:prefLabel   "Prebiotic"@en .

:000110  rdf:type               :Ingredient ;
        rdfs:seeAlso            "http://www.wikidata.org/entity/Q1807269"^^xsd:anyURI ;
        skos:definition         "Pungent, stem vegetable with a mild onion flavor, commonly used in soups and salads."@en ;
        skos:prefLabel          "Leek"@en ;
        :hasFunctionalBenefit   :9521e144-95e4-4171-a421-9a468b1c62e5 , :8d06ddfc-2e8e-4eca-aadb-554cfab5aa6a ;
        :hasIngredientCategory  :stem_vegetables ;
        :pairsWith              :000047 .

:sea-grown_vegetables
        rdf:type         skos:Concept , :IngredientCategory ;
        skos:broader     :vegetable_category ;
        skos:definition  "Includes vegetables and algae that grow in the sea or saltwater environments, such as seaweed, kelp, or sea asparagus."@en ;
        skos:prefLabel   "Sea-grown Vegetables"@en .

:000472  rdf:type               :Ingredient ;
        rdfs:seeAlso            "http://www.wikidata.org/entity/Q131480"^^xsd:anyURI ;
        skos:definition         "Camembert is a soft, creamy cheese known for its rich, earthy flavor and velvety texture."@en ;
        skos:prefLabel          "Camembert"@en ;
        :hasAroma               :pungent_aroma , :cabbage_aroma , :buttery_aroma , :cheesy_aroma , :mushroom_aroma ;
        :hasIngredientCategory  :soft_cheese ;
        :hasTexture             :soft_texture , :creamy_texture ;
        :pairsWith              :005930 .

:000055  rdf:type               :Ingredient ;
        rdfs:seeAlso            "http://www.wikidata.org/entity/Q23374"^^xsd:anyURI ;
        skos:definition         "Spicy sausage made from ground pork and chili peppers, commonly used in Spanish and Mexican dishes."@en ;
        skos:prefLabel          "Chorizo"@en ;
        :hasAroma               :woody_aroma , :fatty_aroma , :animal_aroma , :meaty_aroma , :smoky_aroma , :spicy_aroma ;
        :hasIngredientCategory  :charcuterie ;
        :hasTaste               :fatty_taste .

:a5fee1e7-b975-44b2-b4dc-498e7c295bd4
        rdf:type         :FunctionalBenefit ;
        skos:definition  "Functional benefits related to antibacterial properties involve ingredients or products that help combat harmful bacteria." ;
        skos:prefLabel   "Antibacterial"@en .

:3674c0c7-026a-4337-a10c-bbe4ceff1870
        rdf:type         :FunctionalBenefit ;
        skos:definition  "Functional benefits related to aging focus on ingredients or products that may support healthy aging, including skin health and cognitive function." ;
        skos:prefLabel   "Ageing"@en .

:pepper_spices  rdf:type  skos:Concept , :IngredientCategory ;
        skos:broader     :pungent_spices ;
        skos:definition  "Includes spices derived from various pepper plants, such as black pepper, white pepper, or pink peppercorns, adding heat and pungency to dishes."@en ;
        skos:prefLabel   "Pepper Spices"@en .

:001696  rdf:type               :Ingredient ;
        rdfs:seeAlso            "http://www.wikidata.org/entity/Q10978"^^xsd:anyURI ;
        skos:definition         "Grapes are small, round fruits with a sweet and juicy flavor, commonly eaten fresh or used for making wine."@en ;
        skos:prefLabel          "Grape"@en ;
        :hasAroma               :grape_aroma , :melon_aroma , :berry_aroma , :floral_aroma ;
        :hasFunctionalBenefit   :a5fee1e7-b975-44b2-b4dc-498e7c295bd4 , :a910f718-6310-459f-976b-6c9c334adfe7 , :d1c71bca-dd90-47d3-9f3b-1e214ccaeb85 , :197f7339-d08a-4270-a44e-164cd5146dd4 , :be450163-d1fc-4eec-8e1b-ef10c6ddbfe2 , :e498450d-cced-4a4f-93dd-b3ef3d5e2d43 , :00541d6d-4dc5-4853-98f2-d176c27db355 , :aab0922c-eece-44ff-b800-92af6c07f55d , :1e883a46-9d0a-4f5a-aa3a-4e75a25e0eba , :8d06ddfc-2e8e-4eca-aadb-554cfab5aa6a , :787e979b-4d45-48b4-9f11-6fba2b367924 , :6a1a1d51-dfab-4237-aeac-a9ac4db26486 , :4b2e9d35-65b8-4a2e-96a4-6436e368f15f , :c6e9b1b9-673b-4038-a473-7c57181b9eec , :9521e144-95e4-4171-a421-9a468b1c62e5 , :c5a4476f-dc4e-417a-a47a-ede2655abb18 , :3674c0c7-026a-4337-a10c-bbe4ceff1870 , :1e86605f-2026-4f12-8293-e168aafc11e3 ;
        :hasIngredientCategory  :berries ;
        :hasTaste               :sweet_taste ;
        :hasTexture             :juicy_texture ;
        :pairsWith              :005569 , :007088 , :000148 , :000886 , :001755 , :000865 , :000149 , :000791 .

:000013  rdf:type               :Ingredient ;
        rdfs:seeAlso            "http://www.wikidata.org/entity/Q13317"^^xsd:anyURI ;
        skos:definition         "Dairy product with a high fat content, providing a creamy texture and rich flavor."@en ;
        skos:prefLabel          "Full-fat Yogurt"@en ;
        :hasAroma               :cheesy_aroma , :milk_aroma , :fatty_aroma , :acidic_aroma ;
        :hasFunctionalBenefit   :9521e144-95e4-4171-a421-9a468b1c62e5 , :c5a4476f-dc4e-417a-a47a-ede2655abb18 , :6a1a1d51-dfab-4237-aeac-a9ac4db26486 , :a910f718-6310-459f-976b-6c9c334adfe7 , :787e979b-4d45-48b4-9f11-6fba2b367924 , :00541d6d-4dc5-4853-98f2-d176c27db355 , :be450163-d1fc-4eec-8e1b-ef10c6ddbfe2 , :aab0922c-eece-44ff-b800-92af6c07f55d , :a5fee1e7-b975-44b2-b4dc-498e7c295bd4 , :8d06ddfc-2e8e-4eca-aadb-554cfab5aa6a , :d1c71bca-dd90-47d3-9f3b-1e214ccaeb85 , :c6e9b1b9-673b-4038-a473-7c57181b9eec , :1e883a46-9d0a-4f5a-aa3a-4e75a25e0eba , :e3f7dd51-c162-4746-8f72-cababacf8ace , :4b2e9d35-65b8-4a2e-96a4-6436e368f15f ;
        :hasIngredientCategory  :yoghurt ;
        :hasTaste               :fatty_taste , :sour_taste ;
        :pairsWith              :000791 .

:nutty_spices  rdf:type  skos:Concept , :IngredientCategory ;
        skos:broader     :spice_category ;
        skos:definition  "Includes spices with a nutty flavor profile, such as almonds, cashews, or hazelnuts, used to enhance the taste of dishes or desserts."@en ;
        skos:prefLabel   "Nutty Spices"@en .

:000148  rdf:type               :Ingredient ;
        rdfs:seeAlso            "http://www.wikidata.org/entity/Q169"^^xsd:anyURI ;
        skos:definition         "Mangoes are tropical fruits with a sweet, juicy flesh and a distinctive flavor, commonly eaten fresh or used in salsas and desserts."@en ;
        skos:prefLabel          "Mango"@en ;
        :hasAroma               :caramel_aroma , :pine_aroma , :tropical_aroma , :pineapple_aroma ;
        :hasFunctionalBenefit   :6a1a1d51-dfab-4237-aeac-a9ac4db26486 , :4b2e9d35-65b8-4a2e-96a4-6436e368f15f , :c5a4476f-dc4e-417a-a47a-ede2655abb18 , :1e86605f-2026-4f12-8293-e168aafc11e3 , :d1c71bca-dd90-47d3-9f3b-1e214ccaeb85 , :00541d6d-4dc5-4853-98f2-d176c27db355 , :aab0922c-eece-44ff-b800-92af6c07f55d , :c6e9b1b9-673b-4038-a473-7c57181b9eec , :787e979b-4d45-48b4-9f11-6fba2b367924 , :e498450d-cced-4a4f-93dd-b3ef3d5e2d43 , :9521e144-95e4-4171-a421-9a468b1c62e5 , :8d06ddfc-2e8e-4eca-aadb-554cfab5aa6a , :a910f718-6310-459f-976b-6c9c334adfe7 , :be450163-d1fc-4eec-8e1b-ef10c6ddbfe2 ;
        :hasIngredientCategory  :tropical_fruits ;
        :hasTaste               :sour_taste , :sweet_taste .

:hasFlavour  rdf:type    owl:ObjectProperty ;
        rdfs:domain      :Ingredient ;
        rdfs:range       :Flavour ;
        skos:definition  "Associates a flavour to an ingredient. This property is never used; instead, its subproperties are used."@en ;
        skos:prefLabel   "has flavour"@en .

:hot_sauce  rdf:type     skos:Concept , :IngredientCategory ;
        skos:broader     :table_sauces ;
        skos:definition  "Type of spicy table sauce made from chili peppers or chili pepper extracts."@en ;
        skos:prefLabel   "Hot Sauce"@en .

:plant-based_proteins
        rdf:type         skos:Concept , :IngredientCategory ;
        skos:broader     :protein_category ;
        skos:definition  "Encompasses protein-rich foods derived from plants, such as legumes, tofu, tempeh, seitan, and plant-based meat alternatives."@en ;
        skos:prefLabel   "Plant-based Proteins"@en .

dct:license  rdf:type  owl:AnnotationProperty .

:pastry  rdf:type        skos:Concept , :IngredientCategory ;
        skos:broader     :bakery_category ;
        skos:definition  "Refers to a type of pastry made from a yeast-leavened dough, including croissants, pain au chocolat, and Danish pastries."@en ;
        skos:prefLabel   "Pastry"@en .

:006821  rdf:type               :Ingredient ;
        rdfs:seeAlso            "http://www.wikidata.org/entity/Q277628"^^xsd:anyURI ;
        skos:definition         "Rich and bittersweet chocolate made from cocoa solids and sugar, known for its complex flavor profiles."@en ;
        skos:prefLabel          "Dark Chocolate"@en ;
        :hasAroma               :roasted_aroma , :nutty_aroma , :creamy_aroma , :caramel_aroma , :vanilla_aroma , :chocolate_aroma ;
        :hasIngredientCategory  :chocolate_category ;
        :hasTaste               :sweet_taste ;
        :hasTexture             :melting_texture , :hard_texture ;
        :pairsWith              :000101 .

:grains  rdf:type        skos:Concept , :IngredientCategory ;
        skos:broader     :cereals_category ;
        skos:definition  "Refers to various cereal grains used as staple foods, including wheat, rice, corn, oats, barley, and others."@en ;
        skos:prefLabel   "Grains"@en .

:95d1327c-5984-4045-b8b7-126a3d976bc0
        rdf:type         :FunctionalBenefit ;
        skos:definition  "Ingredients that provide a significant amount of calcium, vital for bone health." ;
        skos:prefLabel   "Calcium-source"@en .

:potato_aroma  rdf:type  :Aroma ;
        skos:prefLabel  "Potato Aroma"@en ;
        :hasAromaType   :vegetable .

:000101  rdf:type               :Ingredient ;
        rdfs:seeAlso            "http://www.wikidata.org/entity/Q932214"^^xsd:anyURI ;
        skos:definition         "Emmentaler is a Swiss cheese with a nutty flavor and distinctive holes, commonly used in cooking and sandwiches."@en ;
        skos:prefLabel          "Emmentaler"@en ;
        :hasAroma               :cheesy_aroma , :creamy_aroma , :nutty_aroma ;
        :hasIngredientCategory  :hard_cheese .

:lemon_aroma  rdf:type  :Aroma ;
        skos:prefLabel  "Lemon Aroma"@en ;
        :hasAromaType   :citrus .

:spice_category  rdf:type  skos:Concept , :IngredientCategory ;
        skos:definition  "Encompasses various spices and spice blends used to add flavor and aroma to dishes."@en ;
        skos:prefLabel   "Spice Category"@en .

:red_cheese  rdf:type    skos:Concept , :IngredientCategory ;
        skos:broader     :cheese ;
        skos:definition  "Refers to cheeses that have been colored or aged with the addition of red cultures or bacteria, resulting in distinct flavors."@en ;
        skos:prefLabel   "Red Cheese"@en .

:000083  rdf:type               :Ingredient ;
        rdfs:seeAlso            "http://www.wikidata.org/entity/Q106446932"^^xsd:anyURI ;
        skos:definition         "A vibrant red vegetable with a sweet and crunchy texture, used in salads, roasting, and cooking."@en ;
        skos:prefLabel          "Red Bell Pepper"@en ;
        :hasAroma               :bell_pepper_aroma , :green_aroma ;
        :hasFunctionalBenefit   :9521e144-95e4-4171-a421-9a468b1c62e5 ;
        :hasIngredientCategory  :fruit_vegetables ;
        :hasTaste               :bitter_taste ;
        :hasTexture             :crunchy_texture ;
        :pairsWith              :000141 , :000873 .

:000046  rdf:type               :Ingredient ;
        rdfs:seeAlso            "http://www.wikidata.org/entity/Q104248689"^^xsd:anyURI ;
        skos:definition         "Edible fungi with a mild flavor and smooth texture, often used in cooking."@en ;
        skos:prefLabel          "Champignon Mushroom"@en ;
        :hasAroma               :mushroom_aroma , :earthy_aroma ;
        :hasFunctionalBenefit   :d1c71bca-dd90-47d3-9f3b-1e214ccaeb85 , :787e979b-4d45-48b4-9f11-6fba2b367924 , :e498450d-cced-4a4f-93dd-b3ef3d5e2d43 , :1e86605f-2026-4f12-8293-e168aafc11e3 , :c6e9b1b9-673b-4038-a473-7c57181b9eec , :4b2e9d35-65b8-4a2e-96a4-6436e368f15f , :3674c0c7-026a-4337-a10c-bbe4ceff1870 , :aab0922c-eece-44ff-b800-92af6c07f55d , :9521e144-95e4-4171-a421-9a468b1c62e5 , :c5a4476f-dc4e-417a-a47a-ede2655abb18 , :6a1a1d51-dfab-4237-aeac-a9ac4db26486 , :a910f718-6310-459f-976b-6c9c334adfe7 , :1e883a46-9d0a-4f5a-aa3a-4e75a25e0eba , :00541d6d-4dc5-4853-98f2-d176c27db355 , :197f7339-d08a-4270-a44e-164cd5146dd4 , :f964c152-e1b0-4087-b7b9-6be16cec00ab , :8d06ddfc-2e8e-4eca-aadb-554cfab5aa6a ;
        :hasIngredientCategory  :mushroom_and_funghi .

:seeds  rdf:type         skos:Concept , :IngredientCategory ;
        skos:broader     :nuts_and_seeds_category ;
        skos:definition  "Includes small, edible plant embryos often used as ingredients in cooking, baking, or eaten as snacks, such as sesame seeds, chia seeds, and sunflower seeds."@en ;
        skos:prefLabel   "Seeds"@en .

:000801  rdf:type               :Ingredient ;
        rdfs:seeAlso            "http://www.wikidata.org/entity/Q208008"^^xsd:anyURI ;
        skos:definition         "Fine, brown powder made from roasted and ground cacao beans, commonly used in baking."@en ;
        skos:prefLabel          "Cocoa Powder"@en ;
        :hasFunctionalBenefit   :e3f7dd51-c162-4746-8f72-cababacf8ace , :f964c152-e1b0-4087-b7b9-6be16cec00ab , :d1c71bca-dd90-47d3-9f3b-1e214ccaeb85 , :c6e9b1b9-673b-4038-a473-7c57181b9eec , :9521e144-95e4-4171-a421-9a468b1c62e5 , :1e86605f-2026-4f12-8293-e168aafc11e3 , :6a1a1d51-dfab-4237-aeac-a9ac4db26486 , :4b2e9d35-65b8-4a2e-96a4-6436e368f15f , :1e883a46-9d0a-4f5a-aa3a-4e75a25e0eba , :197f7339-d08a-4270-a44e-164cd5146dd4 , :c5a4476f-dc4e-417a-a47a-ede2655abb18 , :aab0922c-eece-44ff-b800-92af6c07f55d , :a910f718-6310-459f-976b-6c9c334adfe7 , :3674c0c7-026a-4337-a10c-bbe4ceff1870 , :787e979b-4d45-48b4-9f11-6fba2b367924 , :e498450d-cced-4a4f-93dd-b3ef3d5e2d43 , :00541d6d-4dc5-4853-98f2-d176c27db355 , :be450163-d1fc-4eec-8e1b-ef10c6ddbfe2 , :ae69eda5-a1f9-41b4-b70e-1a7972de7c15 ;
        :hasIngredientCategory  :bakery_ingredients ;
        :pairsWith              :000141 .

:mezcal_and_tequila  rdf:type  skos:Concept , :IngredientCategory ;
        skos:broader     :spirits ;
        skos:definition  "Relates to distilled alcoholic beverages made specifically from agave plants, including mezcal and tequila."@en ;
        skos:prefLabel   "Mezcal And Tequila"@en .

:smoky_aroma  rdf:type  :Aroma ;
        skos:prefLabel  "Smoky Aroma"@en ;
        :hasAromaType   :woody .

:culinary_herbs  rdf:type  skos:Concept , :IngredientCategory ;
        skos:broader     :herbs_category ;
        skos:definition  "Encompasses herbs used primarily for cooking and flavoring dishes, such as basil, thyme, rosemary, and parsley."@en ;
        skos:prefLabel   "Culinary Herbs"@en .

:berries  rdf:type       skos:Concept , :IngredientCategory ;
        skos:broader     :fruit_category ;
        skos:definition  "Encompasses small, edible fruits, often colorful and packed with antioxidants, such as strawberries, blueberries, and raspberries."@en ;
        skos:prefLabel   "Berries"@en .

:fruit_vegetables  rdf:type  skos:Concept , :IngredientCategory ;
        skos:broader     :vegetable_category ;
        skos:definition  "Encompasses vegetables that are botanically classified as fruits, such as tomatoes, cucumbers, eggplants, or bell peppers."@en ;
        skos:prefLabel   "Fruit Vegetables"@en .

:flowers_category  rdf:type  skos:Concept , :IngredientCategory ;
        skos:definition  "Relates to edible flowers used in cooking, garnishing, or flavoring food and beverages."@en ;
        skos:prefLabel   "Flowers Category"@en .

:005760  rdf:type               :Ingredient ;
        rdfs:seeAlso            "http://www.wikidata.org/entity/Q957434"^^xsd:anyURI ;
        skos:definition         "Veal is tender, pale-pink meat from young calves, prized for its delicate flavor and tenderness, commonly used in gourmet cuisine."@en ;
        skos:prefLabel          "Veal"@en ;
        :hasAroma               :meaty_aroma , :roasted_aroma ;
        :hasIngredientCategory  :meats ;
        :pairsWith              :000873 , :005754 .

:grape_aroma  rdf:type  :Aroma ;
        skos:prefLabel  "Grape Aroma"@en ;
        :hasAromaType   :fruity .

:9521e144-95e4-4171-a421-9a468b1c62e5
        rdf:type         :FunctionalBenefit ;
        skos:definition  "Antioxidants help protect cells from damage caused by free radicals, which can contribute to aging and various diseases." ;
        skos:prefLabel   "Antioxidant"@en .

:000876  rdf:type               :Ingredient ;
        rdfs:seeAlso            "http://www.wikidata.org/entity/Q26877308"^^xsd:anyURI ;
        skos:definition         "Fortified wine flavored with botanicals, commonly used as a component in cocktails."@en ;
        skos:prefLabel          "Sweet Vermouth"@en ;
        :hasIngredientCategory  :wines .

:003290  rdf:type               :Ingredient ;
        rdfs:seeAlso            "http://www.wikidata.org/entity/Q193411"^^xsd:anyURI ;
        skos:definition         "Brie is a soft, creamy cheese known for its mild flavor and edible rind, commonly served as an appetizer."@en ;
        skos:prefLabel          "Brie"@en ;
        :hasAroma               :creamy_aroma , :buttery_aroma , :mushroom_aroma , :cheesy_aroma ;
        :hasIngredientCategory  :soft_cheese ;
        :hasTexture             :soft_texture , :creamy_texture ;
        :pairsWith              :000791 , :001755 , :007088 , :000013 , :000886 .

:007109  rdf:type               :Ingredient ;
        rdfs:seeAlso            "http://www.wikidata.org/entity/Q2746643"^^xsd:anyURI ;
        skos:definition         "Sweet, pear-shaped fruits with a unique texture and a mildly sweet flavor."@en ;
        skos:prefLabel          "Fig"@en ;
        :hasAroma               :herbal_aroma , :lemon_aroma , :fig_aroma ;
        :hasFunctionalBenefit   :be450163-d1fc-4eec-8e1b-ef10c6ddbfe2 , :197f7339-d08a-4270-a44e-164cd5146dd4 , :00541d6d-4dc5-4853-98f2-d176c27db355 , :6a1a1d51-dfab-4237-aeac-a9ac4db26486 , :1e883a46-9d0a-4f5a-aa3a-4e75a25e0eba , :9521e144-95e4-4171-a421-9a468b1c62e5 , :aab0922c-eece-44ff-b800-92af6c07f55d , :a910f718-6310-459f-976b-6c9c334adfe7 , :c6e9b1b9-673b-4038-a473-7c57181b9eec , :e3f7dd51-c162-4746-8f72-cababacf8ace , :c5a4476f-dc4e-417a-a47a-ede2655abb18 , :787e979b-4d45-48b4-9f11-6fba2b367924 , :4b2e9d35-65b8-4a2e-96a4-6436e368f15f , :d1c71bca-dd90-47d3-9f3b-1e214ccaeb85 , :e498450d-cced-4a4f-93dd-b3ef3d5e2d43 ;
        :hasIngredientCategory  :tropical_fruits ;
        :pairsWith              :000865 , :007088 , :003246 , :000873 .

:broths_and_fonds_category
        rdf:type         skos:Concept , :IngredientCategory ;
        skos:definition  "Broths and stocks are flavorful liquids used as a base for soups, sauces, and various dishes. They are created by simmering ingredients like meats, bones, vegetables, and seasonings in water to extract their flavors."@en ;
        skos:prefLabel   "Broths And Fonds Category"@en .

:flower_vegetables  rdf:type  skos:Concept , :IngredientCategory ;
        skos:broader     :vegetable_category ;
        skos:definition  "Refers to vegetables where the flowers or flower buds are consumed, such as broccoli, cauliflower, artichokes, or capers."@en ;
        skos:prefLabel   "Flower Vegetables"@en .

:fermented_aroma  rdf:type  :Aroma ;
        skos:prefLabel  "Fermented Aroma"@en ;
        :hasAromaType   :fruity .

:energy_drinks  rdf:type  skos:Concept , :IngredientCategory ;
        skos:broader     :non-alcoholic_drink ;
        skos:definition  "Refers to beverages containing stimulant ingredients like caffeine or taurine, often consumed to provide a temporary energy boost."@en ;
        skos:prefLabel   "Energy Drinks"@en .

:colouring  rdf:type     skos:Concept , :IngredientCategory ;
        skos:broader     :food_additives_category ;
        skos:definition  "Refers to substances used to add or enhance color in food and beverages, such as natural or synthetic food dyes."@en ;
        skos:prefLabel   "Colouring"@en .

:000357  rdf:type               :Ingredient ;
        rdfs:seeAlso            "http://www.wikidata.org/entity/Q92581152"^^xsd:anyURI ;
        skos:definition         "Oregano is a fragrant herb with a robust, slightly peppery flavor, often used to season Mediterranean and Italian dishes."@en ;
        skos:prefLabel          "Oregano"@en ;
        :hasAroma               :woody_aroma , :thyme_aroma ;
        :hasFunctionalBenefit   :c6e9b1b9-673b-4038-a473-7c57181b9eec , :9521e144-95e4-4171-a421-9a468b1c62e5 , :e498450d-cced-4a4f-93dd-b3ef3d5e2d43 , :787e979b-4d45-48b4-9f11-6fba2b367924 , :be450163-d1fc-4eec-8e1b-ef10c6ddbfe2 , :c5a4476f-dc4e-417a-a47a-ede2655abb18 , :d1c71bca-dd90-47d3-9f3b-1e214ccaeb85 , :4b2e9d35-65b8-4a2e-96a4-6436e368f15f , :00541d6d-4dc5-4853-98f2-d176c27db355 , :a910f718-6310-459f-976b-6c9c334adfe7 , :1e86605f-2026-4f12-8293-e168aafc11e3 ;
        :hasIngredientCategory  :culinary_herbs ;
        :pairsWith              :000123 , :000281 , :000109 , :000031 .

:bakery_category  rdf:type  skos:Concept , :IngredientCategory ;
        skos:definition  "Includes various baked goods like bread, cookies, cakes, pastries, and viennoiserie."@en ;
        skos:prefLabel   "Bakery Category"@en .

:bell_pepper_aroma  rdf:type  :Aroma ;
        skos:prefLabel  "Bell Pepper Aroma"@en ;
        :hasAromaType   :vegetable .

:sour_taste  rdf:type   :Taste ;
        skos:prefLabel  "Sour Taste"@en .

:e498450d-cced-4a4f-93dd-b3ef3d5e2d43
        rdf:type         :FunctionalBenefit ;
        skos:definition  "Functional benefits for the brain are properties that support cognitive function, memory, and overall mental well-being." ;
        skos:prefLabel   "Brain"@en .

:002530  rdf:type               :Ingredient ;
        rdfs:seeAlso            "http://www.wikidata.org/entity/Q7802"^^xsd:anyURI ;
        skos:definition         "Staple food made from flour, water, and yeast, commonly baked and consumed worldwide."@en ;
        skos:prefLabel          "Bread"@en ;
        :hasFunctionalBenefit   :e3f7dd51-c162-4746-8f72-cababacf8ace , :f964c152-e1b0-4087-b7b9-6be16cec00ab , :4b2e9d35-65b8-4a2e-96a4-6436e368f15f , :00541d6d-4dc5-4853-98f2-d176c27db355 , :d1c71bca-dd90-47d3-9f3b-1e214ccaeb85 , :1e883a46-9d0a-4f5a-aa3a-4e75a25e0eba , :aab0922c-eece-44ff-b800-92af6c07f55d , :be450163-d1fc-4eec-8e1b-ef10c6ddbfe2 , :a910f718-6310-459f-976b-6c9c334adfe7 , :9521e144-95e4-4171-a421-9a468b1c62e5 , :6a1a1d51-dfab-4237-aeac-a9ac4db26486 , :e498450d-cced-4a4f-93dd-b3ef3d5e2d43 , :3674c0c7-026a-4337-a10c-bbe4ceff1870 , :c6e9b1b9-673b-4038-a473-7c57181b9eec ;
        :hasIngredientCategory  :bread ;
        :pairsWith              :000013 , :007088 , :000791 , :003290 .

:rum    rdf:type         skos:Concept , :IngredientCategory ;
        skos:broader     :spirits ;
        skos:definition  "Refers to a distilled alcoholic beverage made from sugarcane byproducts, typically aged in oak barrels for flavor development."@en ;
        skos:prefLabel   "Rum"@en .

:milk_aroma  rdf:type   :Aroma ;
        skos:prefLabel  "Milk Aroma"@en ;
        :hasAromaType   :cheesy .

:000213  rdf:type               :Ingredient ;
        rdfs:seeAlso            "http://www.wikidata.org/entity/Q263203"^^xsd:anyURI ;
        skos:definition         "Crunchy and colorful vegetable used in salads and coleslaws for its vibrant hue and mild flavor."@en ;
        skos:prefLabel          "Red Cabbage"@en ;
        :hasAroma               :pungent_aroma , :onion_aroma , :mustard_aroma , :cabbage_aroma ;
        :hasFunctionalBenefit   :c6e9b1b9-673b-4038-a473-7c57181b9eec , :9521e144-95e4-4171-a421-9a468b1c62e5 , :787e979b-4d45-48b4-9f11-6fba2b367924 , :be450163-d1fc-4eec-8e1b-ef10c6ddbfe2 , :00541d6d-4dc5-4853-98f2-d176c27db355 ;
        :hasIngredientCategory  :leaves_vegetables .

:honeys  rdf:type        skos:Concept , :IngredientCategory ;
        skos:broader     :sweeteners_category ;
        skos:definition  "Refers to a sweet, viscous liquid produced by bees from flower nectar, often used as a natural sweetener and flavoring agent."@en ;
        skos:prefLabel   "Honeys"@en .

:fruity  rdf:type       :AromaType ;
        skos:prefLabel  "Fruity"@en .

:jasmin_aroma  rdf:type  :Aroma ;
        skos:prefLabel  "Jasmin Aroma"@en ;
        :hasAromaType   :floral .

:charcuterie  rdf:type   skos:Concept , :IngredientCategory ;
        skos:broader     :protein_category ;
        skos:definition  "Refers to a branch of cooking related to prepared meat products, such as cured meats, sausages, pâtés, and terrines."@en ;
        skos:prefLabel   "Charcuterie"@en .

:citrus_fruits  rdf:type  skos:Concept , :IngredientCategory ;
        skos:broader     :fruit_category ;
        skos:definition  "Refers to a group of fruits characterized by their acidic taste and high vitamin C content, including oranges, lemons, and grapefruits."@en ;
        skos:prefLabel   "Citrus Fruits"@en .

:clove_aroma  rdf:type  :Aroma ;
        skos:prefLabel  "Clove Aroma"@en ;
        :hasAromaType   :spicy .

:000306  rdf:type               :Ingredient ;
        rdfs:seeAlso            "http://www.wikidata.org/entity/Q188879"^^xsd:anyURI ;
        skos:definition         "Popular fish known for its tender, pink flesh and mild, slightly sweet flavor, making it a versatile choice for various culinary preparations."@en ;
        skos:prefLabel          "Atlantic Salmon"@en ;
        :hasAroma               :green_aroma , :fatty_aroma , :fishy_aroma ;
        :hasFunctionalBenefit   :aab0922c-eece-44ff-b800-92af6c07f55d , :a910f718-6310-459f-976b-6c9c334adfe7 , :d1c71bca-dd90-47d3-9f3b-1e214ccaeb85 , :00541d6d-4dc5-4853-98f2-d176c27db355 , :9521e144-95e4-4171-a421-9a468b1c62e5 , :c5a4476f-dc4e-417a-a47a-ede2655abb18 , :1e883a46-9d0a-4f5a-aa3a-4e75a25e0eba , :4b2e9d35-65b8-4a2e-96a4-6436e368f15f , :c6e9b1b9-673b-4038-a473-7c57181b9eec , :e498450d-cced-4a4f-93dd-b3ef3d5e2d43 ;
        :hasIngredientCategory  :fish ;
        :pairsWith              :000105 .

:hasKeyIngredient  rdf:type  owl:ObjectProperty ;
        rdfs:domain         :IngredientPairing ;
        rdfs:range          :Ingredient ;
        rdfs:subPropertyOf  :hasIngredient ;
        skos:definition     "Specifies the key ingredient in an ingredient pairing."@en ;
        skos:prefLabel      "has key ingredient"@en .

:relish_chutney  rdf:type  skos:Concept , :IngredientCategory ;
        skos:broader     :condiments_category ;
        skos:definition  "Relates to condiments made from fruits, vegetables, or herbs, typically used to add flavor and enhance dishes."@en ;
        skos:prefLabel   "Relish Chutney"@en .

:rice   rdf:type         skos:Concept , :IngredientCategory ;
        skos:broader     :cereals_category ;
        skos:definition  "Refers to the edible seeds of the rice plant, often consumed as a staple food in many cultures."@en ;
        skos:prefLabel   "Rice"@en .

:hasIngredient  rdf:type  owl:ObjectProperty ;
        rdfs:domain      :IngredientPairing ;
        rdfs:range       :Ingredient ;
        skos:definition  "Associates an ingredient pairing with one or more ingredients. This property is typically not used; instead, its subproperties are used."@en ;
        skos:prefLabel   "has ingredient"@en .

:infusion  rdf:type      skos:Concept , :IngredientCategory ;
        skos:broader     :non-alcoholic_drink ;
        skos:definition  "Refers to a beverage made by steeping ingredients like herbs, fruits, or flowers in hot water, creating flavored and aromatic drinks."@en ;
        skos:prefLabel   "Infusion"@en .

:flavor  rdf:type        skos:Concept , :IngredientCategory ;
        skos:broader     :food_additives_category ;
        skos:definition  "Relates to the distinct taste or aroma of a food or beverage, often achieved through natural or artificial flavorings."@en ;
        skos:prefLabel   "Flavor"@en .

:hasRelatedIngredient
        rdf:type            owl:ObjectProperty ;
        rdfs:domain         :IngredientPairing ;
        rdfs:range          :Ingredient ;
        rdfs:subPropertyOf  :hasIngredient ;
        skos:definition     "Specifies the related ingredient in an ingredient pairing."@en ;
        skos:prefLabel      "has related ingredient"@en .

:floral_aroma  rdf:type  :Aroma ;
        skos:prefLabel  "Floral Aroma"@en ;
        :hasAromaType   :floral .

:c5a4476f-dc4e-417a-a47a-ede2655abb18
        rdf:type         :FunctionalBenefit ;
        skos:definition  "Functional benefits for immunity involve ingredients or products that support the body's ability to defend against illnesses and infections." ;
        skos:prefLabel   "Immunity"@en .

:berry_aroma  rdf:type  :Aroma ;
        skos:prefLabel  "Berry Aroma"@en ;
        :hasAromaType   :fruity .

:meats  rdf:type         skos:Concept , :IngredientCategory ;
        skos:broader     :protein_category ;
        skos:definition  "Refers to the flesh of animals used as food, such as beef, pork, lamb, or poultry, which can be cooked in various ways."@en ;
        skos:prefLabel   "Meats"@en .

:herbal_aroma  rdf:type  :Aroma ;
        skos:prefLabel  "Herbal Aroma"@en ;
        :hasAromaType   :herbal .

:anise_aroma  rdf:type  :Aroma ;
        skos:prefLabel  "Anise Aroma"@en ;
        :hasAromaType   :spicy .

:vodka  rdf:type         skos:Concept , :IngredientCategory ;
        skos:broader     :spirits ;
        skos:definition  "Encompasses a neutral-tasting distilled spirit typically made from grains or potatoes, often used as a base for cocktails."@en ;
        skos:prefLabel   "Vodka"@en .

:rice_snacks  rdf:type   skos:Concept , :IngredientCategory ;
        skos:broader     :snacks_category ;
        skos:definition  "Encompasses snack foods made from rice, such as rice cakes, rice crackers, or puffed rice snacks, often flavored or seasoned."@en ;
        skos:prefLabel   "Rice Snacks"@en .

:plant-based_dairy  rdf:type  skos:Concept , :IngredientCategory ;
        skos:broader     :dairy_category ;
        skos:definition  "Includes dairy alternatives made from plant-based sources, such as almond milk, soy milk, or coconut milk."@en ;
        skos:prefLabel   "Plant-based Dairy"@en .

:6a1a1d51-dfab-4237-aeac-a9ac4db26486
        rdf:type         :FunctionalBenefit ;
        skos:definition  "Functional benefits for weight-loss involve ingredients or products that may aid in achieving and maintaining a healthy weight." ;
        skos:prefLabel   "Weight-loss"@en .

:000014  rdf:type               :Ingredient ;
        rdfs:seeAlso            "http://www.wikidata.org/entity/Q1062531"^^xsd:anyURI ;
        skos:definition         "An egg that has been cooked in boiling water, resulting in a firm white and a partially solid yolk."@en ;
        skos:prefLabel          "Boiled Egg"@en ;
        :hasAroma               :egg_aroma ;
        :hasFunctionalBenefit   :e3f7dd51-c162-4746-8f72-cababacf8ace , :4b2e9d35-65b8-4a2e-96a4-6436e368f15f , :c5a4476f-dc4e-417a-a47a-ede2655abb18 , :6a1a1d51-dfab-4237-aeac-a9ac4db26486 , :3674c0c7-026a-4337-a10c-bbe4ceff1870 , :1e86605f-2026-4f12-8293-e168aafc11e3 , :be450163-d1fc-4eec-8e1b-ef10c6ddbfe2 , :8d06ddfc-2e8e-4eca-aadb-554cfab5aa6a , :787e979b-4d45-48b4-9f11-6fba2b367924 , :95d1327c-5984-4045-b8b7-126a3d976bc0 , :e498450d-cced-4a4f-93dd-b3ef3d5e2d43 , :c6e9b1b9-673b-4038-a473-7c57181b9eec , :c19d9c65-c5d9-4b11-9762-8fd419f7ca5c , :197f7339-d08a-4270-a44e-164cd5146dd4 , :ae69eda5-a1f9-41b4-b70e-1a7972de7c15 , :1e883a46-9d0a-4f5a-aa3a-4e75a25e0eba , :9521e144-95e4-4171-a421-9a468b1c62e5 , :aab0922c-eece-44ff-b800-92af6c07f55d , :a910f718-6310-459f-976b-6c9c334adfe7 , :d1c71bca-dd90-47d3-9f3b-1e214ccaeb85 , :00541d6d-4dc5-4853-98f2-d176c27db355 ;
        :hasIngredientCategory  :dairy_category .

:sweeteners_category  rdf:type  skos:Concept , :IngredientCategory ;
        skos:definition  "Includes sweetening agents like sugars, syrups, and artificial sweeteners used to enhance the sweetness of food and drinks."@en ;
        skos:prefLabel   "Sweeteners Category"@en .

:bulb_vegetables  rdf:type  skos:Concept , :IngredientCategory ;
        skos:broader     :vegetable_category ;
        skos:definition  "Encompasses vegetables with edible bulbs, such as onions, garlic, shallots, or fennel, used as aromatic ingredients in cooking."@en ;
        skos:prefLabel   "Bulb Vegetables"@en .

:buttery_aroma  rdf:type  :Aroma ;
        skos:prefLabel  "Buttery Aroma"@en ;
        :hasAromaType   :cheesy .

:hasIngredientCategory
        rdf:type         owl:ObjectProperty ;
        rdfs:domain      :Ingredient ;
        rdfs:range       :IngredientCategory ;
        skos:definition  "Establishes a relationship between an individual ingredient and its corresponding ingredient category. This property serves to categorize and organize ingredients based on their shared attributes, facilitating structured representation and classification within the domain of food knowledge."@en ;
        skos:prefLabel   "has ingredient category"@en .

:fishy_aroma  rdf:type  :Aroma ;
        skos:prefLabel  "Fishy Aroma"@en ;
        :hasAromaType   :animal .

:pungent_aroma  rdf:type  :Aroma ;
        skos:prefLabel  "Pungent Aroma"@en ;
        :hasAromaType   :spicy .

:000149  rdf:type               :Ingredient ;
        rdfs:seeAlso            "http://www.wikidata.org/entity/Q503"^^xsd:anyURI ;
        skos:definition         "Yellow, curved fruits with a creamy texture and a sweet, mild flavor."@en ;
        skos:prefLabel          "Banana"@en ;
        :hasAroma               :banana_aroma , :tropical_aroma , :honey_aroma ;
        :hasFunctionalBenefit   :6a1a1d51-dfab-4237-aeac-a9ac4db26486 , :d1c71bca-dd90-47d3-9f3b-1e214ccaeb85 , :4b2e9d35-65b8-4a2e-96a4-6436e368f15f , :787e979b-4d45-48b4-9f11-6fba2b367924 , :1e883a46-9d0a-4f5a-aa3a-4e75a25e0eba , :c6e9b1b9-673b-4038-a473-7c57181b9eec , :a910f718-6310-459f-976b-6c9c334adfe7 , :8d06ddfc-2e8e-4eca-aadb-554cfab5aa6a , :197f7339-d08a-4270-a44e-164cd5146dd4 , :e498450d-cced-4a4f-93dd-b3ef3d5e2d43 , :c5a4476f-dc4e-417a-a47a-ede2655abb18 , :1e86605f-2026-4f12-8293-e168aafc11e3 , :9521e144-95e4-4171-a421-9a468b1c62e5 , :f964c152-e1b0-4087-b7b9-6be16cec00ab , :be450163-d1fc-4eec-8e1b-ef10c6ddbfe2 , :00541d6d-4dc5-4853-98f2-d176c27db355 , :aab0922c-eece-44ff-b800-92af6c07f55d ;
        :hasIngredientCategory  :tropical_fruits ;
        :hasTaste               :sweet_taste ;
        :pairsWith              :001696 , :005569 .

:197f7339-d08a-4270-a44e-164cd5146dd4
        rdf:type         :FunctionalBenefit ;
        skos:definition  "Involve ingredients or products that support healthy nerve function and transmission." ;
        skos:prefLabel   "Nervous-system"@en .

:roasted  rdf:type      :AromaType ;
        skos:prefLabel  "Roasted"@en .

:vinegar  rdf:type       skos:Concept , :IngredientCategory ;
        skos:broader     :condiments_category ;
        skos:definition  "Refers to a sour-tasting liquid produced through the fermentation of ethanol, often used as a condiment or preservative."@en ;
        skos:prefLabel   "Vinegar"@en .

:000181  rdf:type               :Ingredient ;
        rdfs:seeAlso            "http://www.wikidata.org/entity/Q36814998"^^xsd:anyURI ;
        skos:definition         "Dark leafy green vegetable known for its tender leaves and mild, slightly earthy taste, commonly used in salads, sautés, and as a versatile ingredient."@en ;
        skos:prefLabel          "Spinach"@en ;
        :hasAroma               :green_aroma , :potato_aroma , :earthy_aroma , :onion_aroma ;
        :hasFunctionalBenefit   :00541d6d-4dc5-4853-98f2-d176c27db355 , :6a1a1d51-dfab-4237-aeac-a9ac4db26486 , :9521e144-95e4-4171-a421-9a468b1c62e5 , :1e883a46-9d0a-4f5a-aa3a-4e75a25e0eba , :f964c152-e1b0-4087-b7b9-6be16cec00ab , :a910f718-6310-459f-976b-6c9c334adfe7 , :1e86605f-2026-4f12-8293-e168aafc11e3 , :d1c71bca-dd90-47d3-9f3b-1e214ccaeb85 , :787e979b-4d45-48b4-9f11-6fba2b367924 , :95d1327c-5984-4045-b8b7-126a3d976bc0 , :e498450d-cced-4a4f-93dd-b3ef3d5e2d43 , :c6e9b1b9-673b-4038-a473-7c57181b9eec ;
        :hasIngredientCategory  :leafy_greens ;
        :hasTaste               :bitter_taste ;
        :pairsWith              :000105 , :005754 , :000452 .

:dessert_category  rdf:type  skos:Concept , :IngredientCategory ;
        skos:definition  "Relates to sweet dishes, cakes, pastries, and other treats typically consumed after a meal."@en ;
        skos:prefLabel   "Dessert Category"@en .

:cheesy_aroma  rdf:type  :Aroma ;
        skos:prefLabel  "Cheesy Aroma"@en ;
        :hasAromaType   :cheesy .

:000144  rdf:type               :Ingredient ;
        rdfs:seeAlso            "http://www.wikidata.org/entity/Q12372598"^^xsd:anyURI ;
        skos:definition         "Juicy stone fruits with a sweet and tart flavor, commonly eaten fresh or used in jams and desserts."@en ;
        skos:prefLabel          "Plum"@en ;
        :hasAroma               :pineapple_aroma , :apple_aroma , :floral_aroma ;
        :hasFunctionalBenefit   :8d06ddfc-2e8e-4eca-aadb-554cfab5aa6a , :c5a4476f-dc4e-417a-a47a-ede2655abb18 , :e498450d-cced-4a4f-93dd-b3ef3d5e2d43 , :9521e144-95e4-4171-a421-9a468b1c62e5 , :a910f718-6310-459f-976b-6c9c334adfe7 , :00541d6d-4dc5-4853-98f2-d176c27db355 , :be450163-d1fc-4eec-8e1b-ef10c6ddbfe2 , :aab0922c-eece-44ff-b800-92af6c07f55d , :787e979b-4d45-48b4-9f11-6fba2b367924 , :a5fee1e7-b975-44b2-b4dc-498e7c295bd4 , :c6e9b1b9-673b-4038-a473-7c57181b9eec ;
        :hasIngredientCategory  :stone_fruits ;
        :hasTaste               :sour_taste , :sweet_taste ;
        :hasTrigeminal          :astringent_trigeminal_taste ;
        :pairsWith              :000141 .

:000886  rdf:type               :Ingredient ;
        rdfs:seeAlso            "http://www.wikidata.org/entity/Q281"^^xsd:anyURI ;
        skos:definition         "Distilled alcoholic beverage made from fermented grain mash, known for its complex flavor profiles."@en ;
        skos:prefLabel          "Whisky"@en ;
        :hasFunctionalBenefit   :00541d6d-4dc5-4853-98f2-d176c27db355 ;
        :hasIngredientCategory  :whisky ;
        :pairsWith              :001755 , :007088 , :000865 , :000791 .

:food_additives_category
        rdf:type         skos:Concept , :IngredientCategory ;
        skos:definition  "Includes substances added to food for various purposes like flavoring, coloring, preservation, and texture enhancement."@en ;
        skos:prefLabel   "Food Additives Category"@en .

:4b2e9d35-65b8-4a2e-96a4-6436e368f15f
        rdf:type         :FunctionalBenefit ;
        skos:definition  "Ingredients or products that may assist in increasing body mass and muscle." ;
        skos:prefLabel   "Weight-gain"@en .

:nuts   rdf:type         skos:Concept , :IngredientCategory ;
        skos:broader     :nuts_and_seeds_category ;
        skos:definition  "Includes edible seeds enclosed in a hard shell, such as almonds, walnuts, cashews, and peanuts, often consumed as snacks or used in cooking."@en ;
        skos:prefLabel   "Nuts"@en .

:seafoods  rdf:type      skos:Concept , :IngredientCategory ;
        skos:broader     :protein_category ;
        skos:definition  "Refers to various edible creatures from the sea, including fish, shellfish (such as shrimp, lobster, or crab), and mollusks (such as clams, oysters, or mussels)."@en ;
        skos:prefLabel   "Seafoods"@en .

:000107  rdf:type               :Ingredient ;
        rdfs:seeAlso            "http://www.wikidata.org/entity/Q2376488"^^xsd:anyURI ;
        skos:definition         "Gruyère is a Swiss cheese with a rich, nutty flavor, commonly used in cooking, baking, and as a topping."@en ;
        skos:prefLabel          "Gruyère"@en ;
        :hasAroma               :pungent_aroma , :creamy_aroma , :nutty_aroma , :cheesy_aroma ;
        :hasIngredientCategory  :hard_cheese ;
        :hasTaste               :umami_taste , :fatty_taste ;
        :hasTexture             :soft_texture , :creamy_texture .

:flavoured_waters  rdf:type  skos:Concept , :IngredientCategory ;
        skos:broader     :non-alcoholic_drink ;
        skos:definition  "Encompasses waters infused with flavors, often derived from fruits, herbs, or botanical extracts, offering a refreshing taste."@en ;
        skos:prefLabel   "Flavoured Waters"@en .

:honey_aroma  rdf:type  :Aroma ;
        skos:prefLabel  "Honey Aroma"@en ;
        :hasAromaType   :floral .

:hasTrigeminal  rdf:type    owl:ObjectProperty ;
        rdfs:domain         :Ingredient ;
        rdfs:range          :Trigeminal ;
        rdfs:seeAlso        <https://www.foodpairing.com/industry/glossary/definition/trigeminal-taste/> ;
        rdfs:subPropertyOf  :hasFlavour ;
        skos:definition     "Assigns a trigeminal taste to an ingredient."@en ;
        skos:prefLabel      "has trigeminal"@en .

:005483  rdf:type               :Ingredient ;
        rdfs:seeAlso            "http://www.wikidata.org/entity/Q104212"^^xsd:anyURI ;
        skos:definition         "Young, edible shoots of the hop plant, known for their mild and slightly bitter flavor."@en ;
        skos:prefLabel          "Humulus Shoot"@en ;
        :hasIngredientCategory  :sprouts .

:pineapple_aroma  rdf:type  :Aroma ;
        skos:prefLabel  "Pineapple Aroma"@en ;
        :hasAromaType   :fruity .

:starchy_texture  rdf:type  :Texture ;
        skos:prefLabel  "Starchy Texture"@en .

:hasAroma  rdf:type         owl:ObjectProperty ;
        rdfs:domain         :Ingredient ;
        rdfs:range          :Aroma ;
        rdfs:seeAlso        <https://www.foodpairing.com/industry/glossary/definition/aroma/> ;
        rdfs:subPropertyOf  :hasFlavour ;
        skos:definition     "Assigns an aroma to an ingredient."@en ;
        skos:prefLabel      "has aroma"@en .

:000047  rdf:type               :Ingredient ;
        rdfs:seeAlso            "http://www.wikidata.org/entity/Q21546392"^^xsd:anyURI ;
        skos:definition         "A pungent bulbous plant used for its aromatic and flavor-enhancing properties in various cuisines."@en ;
        skos:prefLabel          "Garlic"@en ;
        :hasAroma               :pungent_aroma , :garlic_aroma ;
        :hasFunctionalBenefit   :a910f718-6310-459f-976b-6c9c334adfe7 , :1e883a46-9d0a-4f5a-aa3a-4e75a25e0eba , :d1c71bca-dd90-47d3-9f3b-1e214ccaeb85 , :787e979b-4d45-48b4-9f11-6fba2b367924 , :e498450d-cced-4a4f-93dd-b3ef3d5e2d43 , :00541d6d-4dc5-4853-98f2-d176c27db355 , :4b2e9d35-65b8-4a2e-96a4-6436e368f15f , :c5a4476f-dc4e-417a-a47a-ede2655abb18 , :aab0922c-eece-44ff-b800-92af6c07f55d , :8d06ddfc-2e8e-4eca-aadb-554cfab5aa6a , :6a1a1d51-dfab-4237-aeac-a9ac4db26486 , :a5fee1e7-b975-44b2-b4dc-498e7c295bd4 , :be450163-d1fc-4eec-8e1b-ef10c6ddbfe2 , :c6e9b1b9-673b-4038-a473-7c57181b9eec , :1e86605f-2026-4f12-8293-e168aafc11e3 , :3674c0c7-026a-4337-a10c-bbe4ceff1870 , :9521e144-95e4-4171-a421-9a468b1c62e5 ;
        :hasIngredientCategory  :bulb_vegetables ;
        :pairsWith              :000110 , :000096 .

:insects  rdf:type       skos:Concept , :IngredientCategory ;
        skos:broader     :protein_category ;
        skos:definition  "Includes edible insects consumed as food, such as crickets, mealworms, or grasshoppers, which are part of some cultural cuisines."@en ;
        skos:prefLabel   "Insects"@en .

:c19d9c65-c5d9-4b11-9762-8fd419f7ca5c
        rdf:type         :FunctionalBenefit ;
        skos:definition  "Functional benefits for muscle gain involve ingredients or products that support the development and maintenance of lean muscle mass." ;
        skos:prefLabel   "Muscle-gain"@en .

:ae69eda5-a1f9-41b4-b70e-1a7972de7c15
        rdf:type         :FunctionalBenefit ;
        skos:definition  "Functional benefits for skin health involve ingredients or products that promote a healthy complexion and address skin-related issues." ;
        skos:prefLabel   "Skin-health"@en .

:herbs_category  rdf:type  skos:Concept , :IngredientCategory ;
        skos:definition  "Encompasses culinary and medicinal herbs used for flavoring, garnishing, or as natural remedies."@en ;
        skos:prefLabel   "Herbs Category"@en .

:creamy_texture  rdf:type  :Texture ;
        skos:prefLabel  "Creamy Texture"@en .

:aab0922c-eece-44ff-b800-92af6c07f55d
        rdf:type         :FunctionalBenefit ;
        skos:definition  "Functional benefits for cardiovascular health support the heart and circulatory system, reducing the risk of heart-related conditions." ;
        skos:prefLabel   "Cardiovascular"@en .

:000515  rdf:type               :Ingredient ;
        rdfs:seeAlso            "http://www.wikidata.org/entity/Q186451"^^xsd:anyURI ;
        skos:definition         "Edible fungi with a delicate flavor and tender texture, often used in cooking."@en ;
        skos:prefLabel          "Oyster Mushroom"@en ;
        :hasFunctionalBenefit   :e498450d-cced-4a4f-93dd-b3ef3d5e2d43 , :9521e144-95e4-4171-a421-9a468b1c62e5 , :c6e9b1b9-673b-4038-a473-7c57181b9eec , :787e979b-4d45-48b4-9f11-6fba2b367924 , :c5a4476f-dc4e-417a-a47a-ede2655abb18 , :d1c71bca-dd90-47d3-9f3b-1e214ccaeb85 ;
        :hasIngredientCategory  :mushroom_and_funghi .

:000135  rdf:type               :Ingredient ;
        rdfs:seeAlso            "http://www.wikidata.org/entity/Q13179"^^xsd:anyURI ;
        skos:definition         "Raspberries are small, red or black berries with a tart and sweet flavor, used in various culinary applications."@en ;
        skos:prefLabel          "Raspberry"@en ;
        :hasAroma               :green_aroma , :berry_aroma , :honey_aroma , :rose_aroma ;
        :hasFunctionalBenefit   :e498450d-cced-4a4f-93dd-b3ef3d5e2d43 , :6a1a1d51-dfab-4237-aeac-a9ac4db26486 , :e3f7dd51-c162-4746-8f72-cababacf8ace , :c6e9b1b9-673b-4038-a473-7c57181b9eec , :d1c71bca-dd90-47d3-9f3b-1e214ccaeb85 , :1e86605f-2026-4f12-8293-e168aafc11e3 , :aab0922c-eece-44ff-b800-92af6c07f55d , :8d06ddfc-2e8e-4eca-aadb-554cfab5aa6a , :787e979b-4d45-48b4-9f11-6fba2b367924 , :be450163-d1fc-4eec-8e1b-ef10c6ddbfe2 , :a5fee1e7-b975-44b2-b4dc-498e7c295bd4 , :9521e144-95e4-4171-a421-9a468b1c62e5 , :00541d6d-4dc5-4853-98f2-d176c27db355 ;
        :hasIngredientCategory  :berries ;
        :hasTaste               :sweet_taste , :sour_taste ;
        :hasTexture             :soft_texture ;
        :hasTrigeminal          :astringent_trigeminal_taste ;
        :pairsWith              :000101 .

:leafy_greens  rdf:type  skos:Concept , :IngredientCategory ;
        skos:broader     :leaves_vegetables ;
        skos:definition  "Includes a variety of edible leafy vegetables, such as spinach, lettuce, kale, or Swiss chard, often used in salads or cooked as side dishes."@en ;
        skos:prefLabel   "Leafy Greens"@en .

:herbal  rdf:type       :AromaType ;
        skos:prefLabel  "Herbal"@en .

:stone_fruits  rdf:type  skos:Concept , :IngredientCategory ;
        skos:broader     :fruit_category ;
        skos:definition  "Includes fruits with a single hard seed or pit surrounded by juicy flesh, such as peaches, plums, cherries, and apricots."@en ;
        skos:prefLabel   "Stone Fruits"@en .

:FunctionalBenefit  rdf:type  owl:Class ;
        skos:definition  "Represents the effects or advantages that a food ingredient or product provides beyond basic nutrition. These benefits may include specific health-promoting properties, culinary enhancements, or other functional attributes that contribute to overall well-being or enhance the overall quality of a food item."@en ;
        skos:prefLabel   "Functional Benefit"@en .

:1e883a46-9d0a-4f5a-aa3a-4e75a25e0eba
        rdf:type         :FunctionalBenefit ;
        skos:definition  "Functional benefits related to vitamins involve ingredients that are rich in essential vitamins necessary for overall health." ;
        skos:prefLabel   "Vitamins"@en .

:sport_drinks  rdf:type  skos:Concept , :IngredientCategory ;
        skos:broader     :non-alcoholic_drink ;
        skos:definition  "Refers to a specific type of beverage designed to replenish fluids, electrolytes, and provide carbohydrates during or after intense physical activity."@en ;
        skos:prefLabel   "Sport Drinks"@en .

:007105  rdf:type               :Ingredient ;
        rdfs:seeAlso            "http://www.wikidata.org/entity/Q10403913"^^xsd:anyURI ;
        skos:definition         "Light-colored, mild-flavored honey produced by bees that collect nectar from acacia flowers."@en ;
        skos:prefLabel          "Acacia Honey"@en ;
        :hasFunctionalBenefit   :be450163-d1fc-4eec-8e1b-ef10c6ddbfe2 , :8d06ddfc-2e8e-4eca-aadb-554cfab5aa6a , :9521e144-95e4-4171-a421-9a468b1c62e5 ;
        :hasIngredientCategory  :honeys ;
        :pairsWith              :005754 , :005483 .

:fatty_aroma  rdf:type  :Aroma ;
        skos:prefLabel  "Fatty Aroma"@en ;
        :hasAromaType   :green .

:fruit_category  rdf:type  skos:Concept , :IngredientCategory ;
        skos:definition  "Refers to a diverse range of fruits, including citrus fruits, berries, tropical fruits, and other fruit varieties."@en ;
        skos:prefLabel   "Fruit Category"@en .

:005622  rdf:type               :Ingredient ;
        rdfs:seeAlso            "http://www.wikidata.org/entity/Q1311395"^^xsd:anyURI ;
        skos:definition         "A type of shellfish known for its sweet and delicate flavor, commonly eaten raw."@en ;
        skos:prefLabel          "Scallop Saint Jacques"@en ;
        :hasFunctionalBenefit   :c6e9b1b9-673b-4038-a473-7c57181b9eec ;
        :hasIngredientCategory  :seafoods .

:000413  rdf:type               :Ingredient ;
        rdfs:seeAlso            "http://www.wikidata.org/entity/Q41778389"^^xsd:anyURI ;
        skos:definition         "A variety of apple known for their crisp texture and sweet-tart flavor, commonly eaten fresh."@en ;
        skos:prefLabel          "Apple 'Jonagold'"@en ;
        :hasAroma               :apple_aroma , :lemon_aroma , :fruity_aroma ;
        :hasFunctionalBenefit   :e3f7dd51-c162-4746-8f72-cababacf8ace , :c6e9b1b9-673b-4038-a473-7c57181b9eec , :4b2e9d35-65b8-4a2e-96a4-6436e368f15f , :a5fee1e7-b975-44b2-b4dc-498e7c295bd4 , :00541d6d-4dc5-4853-98f2-d176c27db355 , :c5a4476f-dc4e-417a-a47a-ede2655abb18 , :8d06ddfc-2e8e-4eca-aadb-554cfab5aa6a , :1e86605f-2026-4f12-8293-e168aafc11e3 , :aab0922c-eece-44ff-b800-92af6c07f55d , :e498450d-cced-4a4f-93dd-b3ef3d5e2d43 , :a910f718-6310-459f-976b-6c9c334adfe7 , :f964c152-e1b0-4087-b7b9-6be16cec00ab , :787e979b-4d45-48b4-9f11-6fba2b367924 , :9521e144-95e4-4171-a421-9a468b1c62e5 , :3674c0c7-026a-4337-a10c-bbe4ceff1870 , :be450163-d1fc-4eec-8e1b-ef10c6ddbfe2 , :6a1a1d51-dfab-4237-aeac-a9ac4db26486 ;
        :hasIngredientCategory  :pome_fruits ;
        :hasTaste               :sour_taste , :sweet_taste ;
        :hasTexture             :crispy_texture ;
        :pairsWith              :005483 .

:sugar_confections  rdf:type  skos:Concept , :IngredientCategory ;
        skos:broader     :confectionary_category ;
        skos:definition  "Refers to confectionery products with a high sugar content, including candies, gummies, and marshmallows."@en ;
        skos:prefLabel   "Sugar Confections"@en .

:table_sauces  rdf:type  skos:Concept , :IngredientCategory ;
        skos:broader     :condiments_category ;
        skos:definition  "Includes various sauces used as condiments on the dining table, such as ketchup, mustard, and mayonnaise."@en ;
        skos:prefLabel   "Table Sauces"@en .

:SensoryDescriptor  rdf:type  owl:Class ;
        rdfs:seeAlso     <https://www.foodpairing.com/industry/glossary/definition/sensory-descriptor/> ;
        skos:definition  "A sensory descriptor is a label used to describe a specific sensory property of an ingredient. We differentiate between 4 types: (a) Aroma descriptors contain properties like 'almond', 'cherry' and 'mustard'; (b) Texture descriptors contain properties like 'crunchy', 'hard' and 'gooey'; (c) Taste descriptors contain the five basic tastes 'salt', 'sour', 'sweet', 'bitter', and 'umami' and three additional descriptors 'fatty' (or 'oleogustus'), 'astringent', and 'pungent'; (d) Trigeminal taste descriptors contain taste sensations 'astringent', 'pungent', 'cooling' and 'tingling'."@en ;
        skos:prefLabel   "Sensory Descriptor"@en .

:005942  rdf:type               :Ingredient ;
        rdfs:seeAlso            "http://www.wikidata.org/entity/Q208172"^^xsd:anyURI ;
        skos:definition         "A long, slender loaf of French bread known for its crisp crust and soft interior."@en ;
        skos:prefLabel          "Baguette"@en ;
        :hasIngredientCategory  :bread .

:sea_vegetables  rdf:type  skos:Concept , :IngredientCategory ;
        skos:broader     :sea-grown_vegetables ;
        skos:definition  "Includes edible vegetables that grow in the sea or saltwater environments, such as seaweed, kelp, or sea asparagus, often used in Asian cuisines."@en ;
        skos:prefLabel   "Sea Vegetables"@en .

:000163  rdf:type               :Ingredient ;
        rdfs:seeAlso            "http://www.wikidata.org/entity/Q61858403"^^xsd:anyURI ;
        skos:definition         "A sweet and aromatic fruit with orange flesh, commonly eaten fresh or used in salads."@en ;
        skos:prefLabel          "Cantaloupe Melon"@en ;
        :hasAroma               :caramel_aroma , :fruity_aroma , :melon_aroma , :floral_aroma ;
        :hasFunctionalBenefit   :be450163-d1fc-4eec-8e1b-ef10c6ddbfe2 ;
        :hasIngredientCategory  :pepo_fruits ;
        :hasTaste               :sweet_taste , :sour_taste ;
        :pairsWith              :005569 , :000155 , :000873 , :000141 , :005483 , :000082 , :000083 , :000144 .

:pome_fruits  rdf:type   skos:Concept , :IngredientCategory ;
        skos:broader     :fruit_category ;
        skos:definition  "Relates to fruits with a central core containing seeds, often sweet and juicy, such as apples, pears, and quinces."@en ;
        skos:prefLabel   "Pome Fruits"@en .

:semi-soft_cheese  rdf:type  skos:Concept , :IngredientCategory ;
        skos:broader     :cheese ;
        skos:definition  "Encompasses cheeses with a semi-soft or springy texture, offering a balance between firmness and creaminess."@en ;
        skos:prefLabel   "Semi-soft Cheese"@en .

:bakery_ingredients  rdf:type  skos:Concept , :IngredientCategory ;
        skos:broader     :bakery_category ;
        skos:definition  "Relates to a category of baked goods made with dough or pastry dough, often used for pies, tarts, and pastries."@en ;
        skos:prefLabel   "Bakery Ingredients"@en .

:hasFunctionalBenefit
        rdf:type         owl:ObjectProperty ;
        rdfs:domain      :Ingredient ;
        rdfs:range       :FunctionalBenefit ;
        skos:definition  "Establishes a relationship between a food ingredient and a specific functional benefit."@en ;
        skos:prefLabel   "has functional benefit"@en .

:beers  rdf:type         skos:Concept , :IngredientCategory ;
        skos:broader     :alcoholic_drink ;
        skos:definition  "Encompasses a wide range of fermented alcoholic beverages made from grains, typically barley, flavored with hops and yeast."@en ;
        skos:prefLabel   "Beers"@en .

:protein_category  rdf:type  skos:Concept , :IngredientCategory ;
        skos:definition  "Refers to protein-rich foods such as meat, fish, seafood, plant-based proteins, and insect-based products."@en ;
        skos:prefLabel   "Protein Category"@en .

:vegetable  rdf:type    :AromaType ;
        skos:prefLabel  "Vegetable"@en .

:000311  rdf:type               :Ingredient ;
        rdfs:seeAlso            "http://www.wikidata.org/entity/Q167893"^^xsd:anyURI ;
        skos:definition         "Creamy condiment made from eggs, oil, and vinegar or lemon juice, commonly used in salads and sandwiches."@en ;
        skos:prefLabel          "Mayonnaise"@en ;
        :hasAroma               :lemon_aroma , :fatty_aroma , :acidic_aroma ;
        :hasFunctionalBenefit   :c6e9b1b9-673b-4038-a473-7c57181b9eec ;
        :hasIngredientCategory  :table_sauces ;
        :hasTaste               :fatty_taste .

:007170  rdf:type               :Ingredient ;
        rdfs:seeAlso            "http://www.wikidata.org/entity/Q122195"^^xsd:anyURI ;
        skos:definition         "A type of tequila known for its clear color and pure, unaged flavor."@en ;
        skos:prefLabel          "Tequila Silver"@en ;
        :hasAroma               :earthy_aroma , :ethanol_aroma , :herbal_aroma , :woody_aroma , :green_aroma , :smoky_aroma , :roasted_aroma ;
        :hasIngredientCategory  :mezcal_and_tequila ;
        :pairsWith              :000101 , :007088 .

:warm_spices  rdf:type   skos:Concept , :IngredientCategory ;
        skos:broader     :spice_category ;
        skos:definition  "Encompasses spices that create a warm and cozy flavor profile, often associated with fall or winter dishes, such as cloves, ginger, or allspice."@en ;
        skos:prefLabel   "Warm Spices"@en .

:soft_texture  rdf:type  :Texture ;
        skos:prefLabel  "Soft Texture"@en .

:006002  rdf:type               :Ingredient ;
        rdfs:seeAlso            "http://www.wikidata.org/entity/Q178"^^xsd:anyURI ;
        skos:definition         "Pasta noodles that have been cooked in boiling water, resulting in a tender and chewy texture."@en ;
        skos:prefLabel          "Pasta"@en ;
        :hasFunctionalBenefit   :9521e144-95e4-4171-a421-9a468b1c62e5 , :d1c71bca-dd90-47d3-9f3b-1e214ccaeb85 , :e3f7dd51-c162-4746-8f72-cababacf8ace , :aab0922c-eece-44ff-b800-92af6c07f55d , :be450163-d1fc-4eec-8e1b-ef10c6ddbfe2 , :6a1a1d51-dfab-4237-aeac-a9ac4db26486 , :c6e9b1b9-673b-4038-a473-7c57181b9eec , :4b2e9d35-65b8-4a2e-96a4-6436e368f15f , :1e883a46-9d0a-4f5a-aa3a-4e75a25e0eba , :a910f718-6310-459f-976b-6c9c334adfe7 , :00541d6d-4dc5-4853-98f2-d176c27db355 ;
        :hasIngredientCategory  :pasta ;
        :pairsWith              :000072 , :000215 , :000281 , :000109 , :000873 .

:000993  rdf:type               :Ingredient ;
        rdfs:seeAlso            "http://www.wikidata.org/entity/Q335016"^^xsd:anyURI ;
        skos:definition         "Tabasco is a brand of hot sauce made from tabasco peppers, commonly used to add heat and flavor to dishes."@en ;
        skos:prefLabel          "Tabasco"@en ;
        :hasAroma               :acidic_aroma , :fermented_aroma , :fruity_aroma ;
        :hasIngredientCategory  :hot_sauce ;
        :hasTaste               :sour_taste , :pungent_taste ;
        :pairsWith              :000791 , :000148 , :000101 .

:creamy_aroma  rdf:type  :Aroma ;
        skos:prefLabel  "Creamy Aroma"@en ;
        :hasAromaType   :cheesy .

:hasSensoryDescriptor
        rdf:type         owl:ObjectProperty ;
        rdfs:domain      :Flavour ;
        rdfs:range       :SensoryDescriptor ;
        skos:definition  "Associates a flavour (aroma, taste, texture, trigeminal) to a sensory descriptor."@en ;
        skos:prefLabel   "has sensory descriptor"@en .

:soft_cheese  rdf:type   skos:Concept , :IngredientCategory ;
        skos:broader     :cheese ;
        skos:definition  "Refers to cheeses with a soft and spreadable texture, often creamy and mild in flavor."@en ;
        skos:prefLabel   "Soft Cheese"@en .

:000159  rdf:type               :Ingredient ;
        rdfs:seeAlso            "http://www.wikidata.org/entity/Q21552830"^^xsd:anyURI ;
        skos:definition         "Yellow grapefruits are citrus fruits with a tangy-sweet flavor, commonly eaten fresh or used in juices. Their taste is slightly more bitter when compared to pink and red grapefruit."@en ;
        skos:prefLabel          "Yellow Grapefruit"@en ;
        :hasAroma               :orange_aroma , :lemon_aroma , :grapefruit_aroma , :pine_aroma ;
        :hasFunctionalBenefit   :a910f718-6310-459f-976b-6c9c334adfe7 , :e498450d-cced-4a4f-93dd-b3ef3d5e2d43 , :08d9e289-6d3a-4aa6-b70d-75b9c6c4c2cd , :aab0922c-eece-44ff-b800-92af6c07f55d , :c6e9b1b9-673b-4038-a473-7c57181b9eec , :1e86605f-2026-4f12-8293-e168aafc11e3 , :be450163-d1fc-4eec-8e1b-ef10c6ddbfe2 , :6a1a1d51-dfab-4237-aeac-a9ac4db26486 , :787e979b-4d45-48b4-9f11-6fba2b367924 , :00541d6d-4dc5-4853-98f2-d176c27db355 , :9521e144-95e4-4171-a421-9a468b1c62e5 ;
        :hasIngredientCategory  :citrus_fruits ;
        :hasTaste               :bitter_taste , :sour_taste , :sweet_taste ;
        :hasTexture             :juicy_texture ;
        :hasTrigeminal          :astringent_trigeminal_taste ;
        :pairsWith              :000123 , :000109 , :000281 .

:seed_vegetables  rdf:type  skos:Concept , :IngredientCategory ;
        skos:broader     :vegetable_category ;
        skos:definition  "Encompasses vegetables where the seeds or seed pods are the primary edible part, such as beans, peas, or corn."@en ;
        skos:prefLabel   "Seed Vegetables"@en .

:003143  rdf:type               :Ingredient ;
        rdfs:seeAlso            "http://www.wikidata.org/entity/Q1245530"^^xsd:anyURI ;
        skos:definition         "French blue cheese known for its creamy texture and distinctive blue veining."@en ;
        skos:prefLabel          "Fourme D'Ambert"@en ;
        :hasIngredientCategory  :blue_cheese .

:a910f718-6310-459f-976b-6c9c334adfe7
        rdf:type         :FunctionalBenefit ;
        skos:definition  "Involve ingredients or products that support the development and maintenance of strong bones." ;
        skos:prefLabel   "Bone"@en .

:pine_aroma  rdf:type   :Aroma ;
        skos:prefLabel  "Pine Aroma"@en ;
        :hasAromaType   :woody .

:000117  rdf:type               :Ingredient ;
        rdfs:seeAlso            "http://www.wikidata.org/entity/Q25237"^^xsd:anyURI ;
        skos:definition         "Fresh peas are small, round, green legumes with a sweet and tender taste, commonly used in cooking."@en ;
        skos:prefLabel          "Pea"@en ;
        :hasFunctionalBenefit   :8d06ddfc-2e8e-4eca-aadb-554cfab5aa6a , :787e979b-4d45-48b4-9f11-6fba2b367924 , :be450163-d1fc-4eec-8e1b-ef10c6ddbfe2 , :1e883a46-9d0a-4f5a-aa3a-4e75a25e0eba , :6a1a1d51-dfab-4237-aeac-a9ac4db26486 , :d1c71bca-dd90-47d3-9f3b-1e214ccaeb85 , :9521e144-95e4-4171-a421-9a468b1c62e5 , :00541d6d-4dc5-4853-98f2-d176c27db355 , :e3f7dd51-c162-4746-8f72-cababacf8ace , :3674c0c7-026a-4337-a10c-bbe4ceff1870 , :c5a4476f-dc4e-417a-a47a-ede2655abb18 , :aab0922c-eece-44ff-b800-92af6c07f55d , :4b2e9d35-65b8-4a2e-96a4-6436e368f15f , :1e86605f-2026-4f12-8293-e168aafc11e3 , :a910f718-6310-459f-976b-6c9c334adfe7 , :c6e9b1b9-673b-4038-a473-7c57181b9eec , :e498450d-cced-4a4f-93dd-b3ef3d5e2d43 , :197f7339-d08a-4270-a44e-164cd5146dd4 ;
        :hasIngredientCategory  :seed_vegetables ;
        :pairsWith              :005569 , :007109 , :000141 , :000142 .

:mushroom_and_funghi  rdf:type  skos:Concept , :IngredientCategory ;
        skos:broader     :vegetable_category ;
        skos:definition  "Encompasses various edible fungi, including mushrooms, truffles, and other types of fungi used in culinary preparations."@en ;
        skos:prefLabel   "Mushroom And Funghi"@en .

:coconut_aroma  rdf:type  :Aroma ;
        skos:prefLabel  "Coconut Aroma"@en ;
        :hasAromaType   :fruity .

:crunchy_texture  rdf:type  :Texture ;
        skos:prefLabel  "Crunchy Texture"@en .

:hazelnut_aroma  rdf:type  :Aroma ;
        skos:prefLabel  "Hazelnut Aroma"@en ;
        :hasAromaType   :nutty .

:00541d6d-4dc5-4853-98f2-d176c27db355
        rdf:type         :FunctionalBenefit ;
        skos:definition  "Involve ingredients or products that aid in the breakdown and absorption of nutrients in the digestive tract." ;
        skos:prefLabel   "Digestion"@en .

:caramels  rdf:type      skos:Concept , :IngredientCategory ;
        skos:broader     :sweeteners_category ;
        skos:definition  "Encompasses confectionery products made by heating sugar, often combined with butter, cream, or milk, resulting in a sweet and chewy treat."@en ;
        skos:prefLabel   "Caramels"@en .

:root_vegetables  rdf:type  skos:Concept , :IngredientCategory ;
        skos:broader     :vegetable_category ;
        skos:definition  "Refers to vegetables where the root portion is consumed, such as carrots, potatoes, turnips, or radishes, often used in soups or stews."@en ;
        skos:prefLabel   "Root Vegetables"@en .

:matchScore  rdf:type    owl:DatatypeProperty ;
        rdfs:domain      :IngredientPairing ;
        rdfs:range       xsd:double ;
        rdfs:seeAlso     <https://www.foodpairing.com/industry/glossary/definition/relative-matching-score/> , <https://www.foodpairing.com/industry/glossary/definition/matching-score/> ;
        skos:definition  "A metric measuring how well two ingredients match together in an ingredient pairing. It corresponds to the relative matching score of one ingredient with another and is dependent on the highest absolute matching score of a specific ingredient. The absolute matching score is transformed into a percentage relative to the highest absolute score for that specific product. The matching score in the Foodpairing® Flavor Database is a relative matching score. The best matching ingredient of the Foodpairing® Flavor Database for a customer product has a 100% match. The matching score of the other ingredients is relative to the aroma score of the best matching ingredient."@en ;
        skos:prefLabel   "Foodpairing match score"@en .

:IngredientCategory  rdf:type  owl:Class ;
        skos:definition  "An ingredient category is a broad classification of related food components based on shared characteristics, used for organizing and understanding various ingredients in culinary and nutritional contexts."@en ;
        skos:prefLabel   "Ingredient Category"@en .

:000182  rdf:type               :Ingredient ;
        rdfs:seeAlso            "http://www.wikidata.org/entity/Q23012379"^^xsd:anyURI ;
        skos:definition         "Crisp, green vegetable with a mild, earthy flavor, often used in salads, soups, and as a crunchy snack."@en ;
        skos:prefLabel          "Celery"@en ;
        :hasAroma               :celery_aroma , :potato_aroma , :anise_aroma ;
        :hasFunctionalBenefit   :1e883a46-9d0a-4f5a-aa3a-4e75a25e0eba , :e498450d-cced-4a4f-93dd-b3ef3d5e2d43 , :787e979b-4d45-48b4-9f11-6fba2b367924 , :1e86605f-2026-4f12-8293-e168aafc11e3 , :aab0922c-eece-44ff-b800-92af6c07f55d , :6a1a1d51-dfab-4237-aeac-a9ac4db26486 , :c6e9b1b9-673b-4038-a473-7c57181b9eec , :00541d6d-4dc5-4853-98f2-d176c27db355 , :9521e144-95e4-4171-a421-9a468b1c62e5 , :d1c71bca-dd90-47d3-9f3b-1e214ccaeb85 ;
        :hasIngredientCategory  :stem_vegetables ;
        :hasTaste               :sweet_taste ;
        :hasTexture             :crunchy_texture ;
        :pairsWith              :000157 .

:maple_aroma  rdf:type  :Aroma ;
        skos:prefLabel  "Maple Aroma"@en ;
        :hasAromaType   :caramel .

:000887  rdf:type               :Ingredient ;
        rdfs:seeAlso            "http://www.wikidata.org/entity/Q742385"^^xsd:anyURI ;
        skos:definition         "A creamy confection made from cocoa butter, sugar, and milk solids, known for its sweet and rich flavor."@en ;
        skos:prefLabel          "White Chocolate"@en ;
        :hasAroma               :vanilla_aroma , :milk_aroma , :cocoa_aroma , :buttery_aroma ;
        :hasFunctionalBenefit   :be450163-d1fc-4eec-8e1b-ef10c6ddbfe2 , :9521e144-95e4-4171-a421-9a468b1c62e5 , :c6e9b1b9-673b-4038-a473-7c57181b9eec ;
        :hasIngredientCategory  :chocolate_category ;
        :hasTaste               :sweet_taste .

:rose_aroma  rdf:type   :Aroma ;
        skos:prefLabel  "Rose Aroma"@en ;
        :hasAromaType   :floral .

:popcorn  rdf:type       skos:Concept , :IngredientCategory ;
        skos:broader     :snacks_category ;
        skos:definition  "Refers to a type of corn kernel that puffs up and becomes light and crispy when heated, commonly consumed as a snack."@en ;
        skos:prefLabel   "Popcorn"@en .

:000520  rdf:type               :Ingredient ;
        rdfs:seeAlso            "http://www.wikidata.org/entity/Q150463"^^xsd:anyURI ;
        skos:definition         "Small, green cruciferous vegetables with a mild, nutty flavor, commonly used in side dishes."@en ;
        skos:prefLabel          "Brussels Sprouts"@en ;
        :hasIngredientCategory  :leaves_vegetables .

:IngredientPairing  rdf:type  owl:Class ;
        rdfs:seeAlso     <https://www.foodpairing.com/industry/glossary/definition/foodpairing-match/> ;
        skos:definition  "A pairing between two ingredients that share one or more key aroma molecules. The pairing has a key ingredient and a related ingredient."@en ;
        skos:prefLabel   "Ingredient Pairing"@en .

:jam_and_jelly  rdf:type  skos:Concept , :IngredientCategory ;
        skos:broader     :condiments_category ;
        skos:definition  "Refers to sweet spreads made from fruit or fruit juice, typically preserved with sugar and pectin."@en ;
        skos:prefLabel   "Jam And Jelly"@en .

:Taste  rdf:type         owl:Class ;
        rdfs:seeAlso     <https://www.foodpairing.com/industry/glossary/definition/taste/> ;
        rdfs:subClassOf  :Flavour ;
        skos:definition  "Taste is the perception produced or stimulated when a substance in the mouth reacts chemically with taste receptor cells located on taste buds in the oral cavity, mostly on the tongue. Taste, along with olfaction and trigeminal nerve stimulation (registering texture, pain, and temperature), determines flavors of food and other substances. A taste is how the taste buds experience the 5 taste types - sweet, sour, bitter, salty and umami. Additional descriptors pungent, astringent and fatty also apply. A food is usually a blend of tastes, each in different concentrations."@en ;
        skos:prefLabel   "Taste"@en .

:ethanol_aroma  rdf:type  :Aroma ;
        skos:prefLabel  "Ethanol Aroma"@en ;
        :hasAromaType   :chemical .

:crispy_texture  rdf:type  :Texture ;
        skos:prefLabel  "Crispy Texture"@en .

:000840  rdf:type               :Ingredient ;
        rdfs:seeAlso            "http://www.wikidata.org/entity/Q62076228"^^xsd:anyURI ;
        skos:definition         "A type of gin known for its dry and juniper-forward flavor, commonly used in cocktails."@en ;
        skos:prefLabel          "London Dry Gin"@en ;
        :hasAroma               :ethanol_aroma , :juniper_aroma , :spicy_aroma , :pine_aroma , :camphor_aroma , :lemon_aroma ;
        :hasIngredientCategory  :gin_and_jenever .

:melon_aroma  rdf:type  :Aroma ;
        skos:prefLabel  "Melon Aroma"@en ;
        :hasAromaType   :fruity .

:000938  rdf:type               :Ingredient ;
        rdfs:seeAlso            "http://www.wikidata.org/entity/Q22806705"^^xsd:anyURI ;
        skos:definition         "White asparagus is a milder, sweeter variety of asparagus with pale stalks, commonly enjoyed steamed or roasted as a delicacy."@en ;
        skos:prefLabel          "White Asparagus"@en ;
        :hasAroma               :asparagus_aroma , :potato_aroma ;
        :hasIngredientCategory  :stem_vegetables .

:banana_aroma  rdf:type  :Aroma ;
        skos:prefLabel  "Banana Aroma"@en ;
        :hasAromaType   :fruity .

:leaves_vegetables  rdf:type  skos:Concept , :IngredientCategory ;
        skos:broader     :vegetable_category ;
        skos:definition  "Includes vegetables where the leaves are the primary edible part, such as cabbage, Swiss chard, or bok choy."@en ;
        skos:prefLabel   "Leaves Vegetables"@en .

:caramel_aroma  rdf:type  :Aroma ;
        skos:prefLabel  "Caramel Aroma"@en ;
        :hasAromaType   :caramel .

:alcoholic_drink  rdf:type  skos:Concept , :IngredientCategory ;
        skos:broader     :drinks_category ;
        skos:definition  "Refers to beverages containing alcohol, including various types of beer, wine, spirits, and cocktails."@en ;
        skos:prefLabel   "Alcoholic Drink"@en .

:dip_and_spread  rdf:type  skos:Concept , :IngredientCategory ;
        skos:broader     :condiments_category ;
        skos:definition  "Includes savory preparations used for dipping or spreading on other foods, such as hummus, guacamole, and cheese spreads."@en ;
        skos:prefLabel   "Dip And Spread"@en .

:soft_drinks  rdf:type   skos:Concept , :IngredientCategory ;
        skos:broader     :non-alcoholic_drink ;
        skos:definition  "Refers to non-alcoholic carbonated beverages, commonly known as sodas or pop, with a wide range of flavors and sweetness levels."@en ;
        skos:prefLabel   "Soft Drinks"@en .

:chips_and_crisps  rdf:type  skos:Concept , :IngredientCategory ;
        skos:broader     :snacks_category ;
        skos:definition  "Includes crispy snack foods made from potatoes, corn, or other vegetables, often flavored and fried or baked."@en ;
        skos:prefLabel   "Chips And Crisps"@en .

:000136  rdf:type               :Ingredient ;
        rdfs:seeAlso            "http://www.wikidata.org/entity/Q5812410"^^xsd:anyURI ;
        skos:definition         "Blueberries are small, round, and dark blue berries known for their sweet and slightly tart taste."@en ;
        skos:prefLabel          "Blueberry"@en ;
        :hasAroma               :green_aroma , :apple_aroma , :rose_aroma ;
        :hasFunctionalBenefit   :c6e9b1b9-673b-4038-a473-7c57181b9eec , :be450163-d1fc-4eec-8e1b-ef10c6ddbfe2 , :a5fee1e7-b975-44b2-b4dc-498e7c295bd4 , :4b2e9d35-65b8-4a2e-96a4-6436e368f15f , :1e883a46-9d0a-4f5a-aa3a-4e75a25e0eba , :00541d6d-4dc5-4853-98f2-d176c27db355 , :e498450d-cced-4a4f-93dd-b3ef3d5e2d43 , :aab0922c-eece-44ff-b800-92af6c07f55d , :1e86605f-2026-4f12-8293-e168aafc11e3 , :6a1a1d51-dfab-4237-aeac-a9ac4db26486 , :a910f718-6310-459f-976b-6c9c334adfe7 , :787e979b-4d45-48b4-9f11-6fba2b367924 , :9521e144-95e4-4171-a421-9a468b1c62e5 , :3674c0c7-026a-4337-a10c-bbe4ceff1870 ;
        :hasIngredientCategory  :berries ;
        :hasTaste               :sweet_taste , :sour_taste ;
        :pairsWith              :005483 .

:chemical  rdf:type     :AromaType ;
        skos:prefLabel  "Chemical"@en .

:006471  rdf:type               :Ingredient ;
        rdfs:seeAlso            "http://www.wikidata.org/entity/Q81"^^xsd:anyURI ;
        skos:definition         "Crunchy, orange root vegetables with a sweet and earthy flavor, commonly eaten fresh."@en ;
        skos:prefLabel          "Carrot"@en ;
        :hasAroma               :rose_aroma , :fruity_aroma ;
        :hasFunctionalBenefit   :1e883a46-9d0a-4f5a-aa3a-4e75a25e0eba , :00541d6d-4dc5-4853-98f2-d176c27db355 , :be450163-d1fc-4eec-8e1b-ef10c6ddbfe2 , :d1c71bca-dd90-47d3-9f3b-1e214ccaeb85 , :e3f7dd51-c162-4746-8f72-cababacf8ace , :a910f718-6310-459f-976b-6c9c334adfe7 , :8d06ddfc-2e8e-4eca-aadb-554cfab5aa6a , :e498450d-cced-4a4f-93dd-b3ef3d5e2d43 , :c6e9b1b9-673b-4038-a473-7c57181b9eec , :6a1a1d51-dfab-4237-aeac-a9ac4db26486 , :1e86605f-2026-4f12-8293-e168aafc11e3 , :f964c152-e1b0-4087-b7b9-6be16cec00ab , :aab0922c-eece-44ff-b800-92af6c07f55d , :9521e144-95e4-4171-a421-9a468b1c62e5 , :787e979b-4d45-48b4-9f11-6fba2b367924 ;
        :hasIngredientCategory  :root_vegetables ;
        :hasTaste               :sweet_taste ;
        :hasTexture             :crunchy_texture , :hard_texture ;
        :pairsWith              :000840 .

:woody_aroma  rdf:type  :Aroma ;
        skos:prefLabel  "Woody Aroma"@en ;
        :hasAromaType   :woody .

:000873  rdf:type               :Ingredient ;
        rdfs:seeAlso            "http://www.wikidata.org/entity/Q165137"^^xsd:anyURI ;
        skos:definition         "Sweet cherries are plump, red or dark purple fruits with a juicy and sweet flavor, commonly eaten fresh."@en ;
        skos:prefLabel          "Sweet Cherry"@en ;
        :hasAroma               :berry_aroma , :violet_aroma , :caramel_aroma ;
        :hasIngredientCategory  :berries ;
        :hasTaste               :sweet_taste , :sour_taste ;
        :hasTexture             :juicy_texture ;
        :pairsWith              :001755 , :000155 , :007088 , :007109 .

:tea_aroma  rdf:type    :Aroma ;
        skos:prefLabel  "Tea Aroma"@en ;
        :hasAromaType   :herbal .

:cocoa_aroma  rdf:type  :Aroma ;
        skos:prefLabel  "Cocoa Aroma"@en ;
        :hasAromaType   :roasted .

:08d9e289-6d3a-4aa6-b70d-75b9c6c4c2cd
        rdf:type         :FunctionalBenefit ;
        skos:definition  "Functional benefits of aromatherapy involve the use of aromatic compounds from plants to promote relaxation, well-being, and mental clarity." ;
        skos:prefLabel   "Aromatherapy"@en .

:cookies  rdf:type       skos:Concept , :IngredientCategory ;
        skos:broader     :snacks_category ;
        skos:definition  "Cookies are small, sweet, baked treats, typically made from a mixture of flour, sugar, butter, and other ingredients. Cookies come in a wide variety of flavors, shapes, and textures, and are enjoyed as a snack."@en ;
        skos:prefLabel   "Cookies"@en .

:007088  rdf:type               :Ingredient ;
        rdfs:seeAlso            "http://www.wikidata.org/entity/Q503252"^^xsd:anyURI ;
        skos:definition         "Armagnac is a French brandy from the Gascony region, known for its robust and fruity flavor."@en ;
        skos:prefLabel          "Armagnac"@en ;
        :hasIngredientCategory  :grape-based_spirits ;
        :pairsWith              :000791 .

:semi-hard_cheese  rdf:type  skos:Concept , :IngredientCategory ;
        skos:broader     :cheese ;
        skos:definition  "Relates to cheeses with a semi-firm texture and flavors that range from mild to sharp, often suitable for slicing or grating."@en ;
        skos:prefLabel   "Semi-hard Cheese"@en .

:tropical_fruits  rdf:type  skos:Concept , :IngredientCategory ;
        skos:broader     :fruit_category ;
        skos:definition  "Refers to a diverse group of fruits grown in tropical regions, often exotic in appearance and flavors, such as mangoes, pineapples, and papayas."@en ;
        skos:prefLabel   "Tropical Fruits"@en .

:fats   rdf:type         skos:Concept , :IngredientCategory ;
        skos:broader     :fats_and_oils_category ;
        skos:definition  "Refers to macronutrients that are a concentrated source of energy, such as butter, lard, and oils, used in cooking and baking."@en ;
        skos:prefLabel   "Fats"@en .

:mustard_aroma  rdf:type  :Aroma ;
        skos:prefLabel  "Mustard Aroma"@en ;
        :hasAromaType   :spicy .

:pasta  rdf:type         skos:Concept , :IngredientCategory ;
        skos:broader     :cereals_category ;
        skos:definition  "Encompasses various types of noodles and pasta products made from wheat flour, water, and sometimes eggs."@en ;
        skos:prefLabel   "Pasta"@en .

:juices  rdf:type        skos:Concept , :IngredientCategory ;
        skos:broader     :non-alcoholic_drink ;
        skos:definition  "Includes the extracted liquids from fruits or vegetables, often consumed as beverages or used as ingredients in recipes."@en ;
        skos:prefLabel   "Juices"@en .

:green  rdf:type        :AromaType ;
        skos:prefLabel  "Green"@en .

:nutty  rdf:type        :AromaType ;
        skos:prefLabel  "Nutty"@en .

:001448  rdf:type               :Ingredient ;
        rdfs:seeAlso            "http://www.wikidata.org/entity/Q60855"^^xsd:anyURI ;
        skos:definition         "Fragrant tea made by infusing green tea leaves with jasmine flowers, known for its floral aroma."@en ;
        skos:prefLabel          "Jasmine Tea"@en ;
        :hasAroma               :tea_aroma , :jasmin_aroma , :apple_aroma ;
        :hasIngredientCategory  :tea ;
        :pairsWith              :007088 , :000791 .

:animal  rdf:type       :AromaType ;
        skos:prefLabel  "Animal"@en .

:asparagus_aroma  rdf:type  :Aroma ;
        skos:prefLabel  "Asparagus Aroma"@en ;
        :hasAromaType   :vegetable .

:cream  rdf:type         skos:Concept , :IngredientCategory ;
        skos:broader     :dairy_category ;
        skos:definition  "Refers to the high-fat layer that forms on top of milk, often used in cooking, baking, or as a topping for desserts."@en ;
        skos:prefLabel   "Cream"@en .

:sensoryValue  rdf:type  owl:DatatypeProperty ;
        rdfs:domain      :Flavour ;
        rdfs:range       [ rdf:type     rdfs:Datatype ;
                           owl:unionOf  ( xsd:boolean xsd:double )
                         ] ;
        skos:definition  "Represents the sensory value for certain descriptors."@en ;
        skos:prefLabel   "sensory value"@en .

:garlic_aroma  rdf:type  :Aroma ;
        skos:prefLabel  "Garlic Aroma"@en ;
        :hasAromaType   :vegetable .

dct:created  rdf:type  owl:AnnotationProperty .

:003246  rdf:type               :Ingredient ;
        rdfs:seeAlso            "http://www.wikidata.org/entity/Q14088"^^xsd:anyURI ;
        skos:definition         "Soft, mild cheese made from cow's milk, commonly used in salads and pizzas."@en ;
        skos:prefLabel          "Cow Mozzarella"@en ;
        :hasAroma               :milk_aroma ;
        :hasIngredientCategory  :fresh_cheese ;
        :hasTexture             :soft_texture ;
        :pairsWith              :007109 .

:juniper_aroma  rdf:type  :Aroma ;
        skos:prefLabel  "Juniper Aroma"@en ;
        :hasAromaType   :spicy .

:hard_cheese  rdf:type   skos:Concept , :IngredientCategory ;
        skos:broader     :cheese ;
        skos:definition  "Encompasses aged cheeses with a firm and dry texture, typically characterized by intense flavors and a long aging process."@en ;
        skos:prefLabel   "Hard Cheese"@en .

:000252  rdf:type               :Ingredient ;
        rdfs:seeAlso            "http://www.wikidata.org/entity/Q37937"^^xsd:anyURI ;
        skos:definition         "Sweet potatoes are starchy, orange-fleshed tubers with a naturally sweet taste, commonly baked, mashed, or used in various culinary preparations."@en ;
        skos:prefLabel          "Sweet Potato"@en ;
        :hasAroma               :banana_aroma , :potato_aroma , :floral_aroma , :fruity_aroma ;
        :hasIngredientCategory  :tuber_vegetables ;
        :hasTexture             :starchy_texture ;
        :pairsWith              :007088 , :000865 .

:tea    rdf:type         skos:Concept , :IngredientCategory ;
        skos:broader     :non-alcoholic_drink ;
        skos:definition  "Encompasses beverages made from the leaves of the Camellia sinensis plant, offering various flavors and caffeine content."@en ;
        skos:prefLabel   "Tea"@en .

:corn_snacks  rdf:type   skos:Concept , :IngredientCategory ;
        skos:broader     :snacks_category ;
        skos:definition  "Refers to crispy or puffed snack foods made from corn; often flavored or seasoned."@en ;
        skos:prefLabel   "Corn Snacks"@en .

:000215  rdf:type               :Ingredient ;
        rdfs:seeAlso            "http://www.wikidata.org/entity/Q99548274"^^xsd:anyURI ;
        skos:definition         "A sweet, earthy root vegetable often used in salads and as a natural food coloring."@en ;
        skos:prefLabel          "Beetroot"@en ;
        :hasFunctionalBenefit   :c6e9b1b9-673b-4038-a473-7c57181b9eec , :9521e144-95e4-4171-a421-9a468b1c62e5 , :be450163-d1fc-4eec-8e1b-ef10c6ddbfe2 , :1e883a46-9d0a-4f5a-aa3a-4e75a25e0eba , :00541d6d-4dc5-4853-98f2-d176c27db355 , :d1c71bca-dd90-47d3-9f3b-1e214ccaeb85 , :3674c0c7-026a-4337-a10c-bbe4ceff1870 , :e498450d-cced-4a4f-93dd-b3ef3d5e2d43 , :aab0922c-eece-44ff-b800-92af6c07f55d , :a910f718-6310-459f-976b-6c9c334adfe7 ;
        :hasIngredientCategory  :root_vegetables .

:syrups  rdf:type        skos:Concept , :IngredientCategory ;
        skos:broader     :sweeteners_category ;
        skos:definition  "Includes thick, sweet liquids made by dissolving sugar in water or other liquids, often used as sweeteners or flavorings in beverages or desserts."@en ;
        skos:prefLabel   "Syrups"@en .

:cooling_trigeminal_taste
        rdf:type        :Trigeminal ;
        skos:prefLabel  "Cooling Trigeminal Taste"@en .

:pungent_taste  rdf:type  :Taste ;
        skos:prefLabel  "Pungent Taste"@en .

:nut_drink  rdf:type     skos:Concept , :IngredientCategory ;
        skos:broader     :nuts_and_seeds_category ;
        skos:definition  "Refers to plant-based beverages made from nuts, such as almond milk or cashew milk, often used as a dairy milk substitute."@en ;
        skos:prefLabel   "Nut Drink"@en .

:cheesy  rdf:type       :AromaType ;
        skos:prefLabel  "Cheesy"@en .

:floral  rdf:type       :AromaType ;
        skos:prefLabel  "Floral"@en .

:000155  rdf:type               :Ingredient ;
        rdfs:seeAlso            "http://www.wikidata.org/entity/Q13195"^^xsd:anyURI ;
        skos:definition         "Limes are small, green citrus fruits with a tart and tangy flavor, commonly used in cooking and beverages."@en ;
        skos:prefLabel          "Lime"@en ;
        :hasAroma               :citrus_aroma , :pine_aroma , :lemon_aroma , :herbal_aroma ;
        :hasFunctionalBenefit   :00541d6d-4dc5-4853-98f2-d176c27db355 , :c6e9b1b9-673b-4038-a473-7c57181b9eec , :4b2e9d35-65b8-4a2e-96a4-6436e368f15f , :c5a4476f-dc4e-417a-a47a-ede2655abb18 , :9521e144-95e4-4171-a421-9a468b1c62e5 , :6a1a1d51-dfab-4237-aeac-a9ac4db26486 , :d1c71bca-dd90-47d3-9f3b-1e214ccaeb85 , :a910f718-6310-459f-976b-6c9c334adfe7 , :e498450d-cced-4a4f-93dd-b3ef3d5e2d43 , :8d06ddfc-2e8e-4eca-aadb-554cfab5aa6a ;
        :hasIngredientCategory  :citrus_fruits ;
        :hasTaste               :sour_taste ;
        :hasTexture             :juicy_texture ;
        :pairsWith              :000840 , :000159 , :000281 , :000109 , :000873 , :000031 , :000072 , :000123 .

:nutty_aroma  rdf:type  :Aroma ;
        skos:prefLabel  "Nutty Aroma"@en ;
        :hasAromaType   :nutty .

:001624  rdf:type               :Ingredient ;
        rdfs:seeAlso            "http://www.wikidata.org/entity/Q374"^^xsd:anyURI ;
        skos:definition         "Colorless and flavorless distilled spirit made from fermented grains or potatoes, commonly used in cocktails."@en ;
        skos:prefLabel          "Vodka"@en ;
        :hasAroma               :oat_flakes_cereal_aroma , :ethanol_aroma , :buttery_aroma , :vanilla_aroma ;
        :hasFunctionalBenefit   :be450163-d1fc-4eec-8e1b-ef10c6ddbfe2 , :e3f7dd51-c162-4746-8f72-cababacf8ace , :c6e9b1b9-673b-4038-a473-7c57181b9eec , :787e979b-4d45-48b4-9f11-6fba2b367924 ;
        :hasIngredientCategory  :vodka ;
        :pairsWith              :005942 , :000109 .

:citrus  rdf:type       :AromaType ;
        skos:prefLabel  "Citrus"@en .

:rice_aroma  rdf:type   :Aroma ;
        skos:prefLabel  "Rice Aroma"@en ;
        :hasAromaType   :green .

:celery_aroma  rdf:type  :Aroma ;
        skos:prefLabel  "Celery Aroma"@en ;
        :hasAromaType   :vegetable .

:grape-based_spirits  rdf:type  skos:Concept , :IngredientCategory ;
        skos:broader     :spirits ;
        skos:definition  "Refers to distilled spirits made from fermented grapes, such as brandy, cognac, and pisco."@en ;
        skos:prefLabel   "Grape-based Spirits"@en .

:000475  rdf:type               :Ingredient ;
        rdfs:seeAlso            "http://www.wikidata.org/entity/Q1119911"^^xsd:anyURI ;
        skos:definition         "Buttery, oval-shaped nuts with a rich and nutty flavor, commonly used in baking and desserts."@en ;
        skos:prefLabel          "Pecan Nut"@en ;
        :hasAroma               :fatty_aroma , :honey_aroma , :nutty_aroma , :almond_aroma , :green_aroma ;
        :hasFunctionalBenefit   :9521e144-95e4-4171-a421-9a468b1c62e5 ;
        :hasIngredientCategory  :nuts ;
        :hasTexture             :hard_texture .

:umami_taste  rdf:type  :Taste ;
        skos:prefLabel  "Umami Taste"@en .

:sweet_taste  rdf:type  :Taste ;
        skos:prefLabel  "Sweet Taste"@en .

:d1c71bca-dd90-47d3-9f3b-1e214ccaeb85
        rdf:type         :FunctionalBenefit ;
        skos:definition  "Functional benefits related to minerals focus on ingredients that provide essential minerals necessary for various bodily functions." ;
        skos:prefLabel   "Minerals"@en .

:000090  rdf:type               :Ingredient ;
        rdfs:seeAlso            "http://www.wikidata.org/entity/Q217525"^^xsd:anyURI ;
        skos:definition         "A type of cheese known for its sharp and tangy flavor, commonly used in cooking and as a topping."@en ;
        skos:prefLabel          "Cheddar"@en ;
        :hasAroma               :fruity_aroma , :buttery_aroma , :cheesy_aroma ;
        :hasFunctionalBenefit   :1e86605f-2026-4f12-8293-e168aafc11e3 , :00541d6d-4dc5-4853-98f2-d176c27db355 , :e498450d-cced-4a4f-93dd-b3ef3d5e2d43 , :9521e144-95e4-4171-a421-9a468b1c62e5 ;
        :hasIngredientCategory  :hard_cheese ;
        :hasTaste               :fatty_taste , :salt_taste ;
        :hasTexture             :soft_texture , :creamy_texture ;
        :pairsWith              :000101 .

:hasAromaType  rdf:type  owl:ObjectProperty ;
        rdfs:domain      :SensoryDescriptor ;
        rdfs:range       :AromaType ;
        rdfs:seeAlso     <https://www.foodpairing.com/industry/glossary/definition/aroma-types/> ;
        skos:definition  "Specifies the aroma type of the sensory descriptor."@en ;
        skos:prefLabel   "has aroma type"@en .

:cheese  rdf:type        skos:Concept , :IngredientCategory ;
        skos:broader     :dairy_category ;
        skos:definition  "Encompasses a wide variety of dairy products made from curdled milk, with different textures, flavors, and production methods."@en ;
        skos:prefLabel   "Cheese"@en .

:chocolate_aroma  rdf:type  :Aroma ;
        skos:prefLabel  "Chocolate Aroma"@en ;
        :hasAromaType   :roasted .

:c6e9b1b9-673b-4038-a473-7c57181b9eec
        rdf:type         :FunctionalBenefit ;
        skos:definition  "Ingredients or products with energy-related functional benefits provide a source of sustenance and vitality for the body." ;
        skos:prefLabel   "Energy"@en .

:vegetable_category  rdf:type  skos:Concept , :IngredientCategory ;
        skos:definition  "Refers to a wide range of edible vegetables, including bulb vegetables, leafy greens, root vegetables, and sea-grown vegetables."@en ;
        skos:prefLabel   "Vegetable Category"@en .

:animal_aroma  rdf:type  :Aroma ;
        skos:prefLabel  "Animal Aroma"@en ;
        :hasAromaType   :animal .

:005545  rdf:type               :Ingredient ;
        rdfs:seeAlso            "http://www.wikidata.org/entity/Q27855"^^xsd:anyURI ;
        skos:definition         "Shellfish with tender, sweet meat, commonly steamed or cooked in various sauces, appreciated for their delicate sea flavor."@en ;
        skos:prefLabel          "Mussel"@en ;
        :hasFunctionalBenefit   :e498450d-cced-4a4f-93dd-b3ef3d5e2d43 , :9521e144-95e4-4171-a421-9a468b1c62e5 , :a910f718-6310-459f-976b-6c9c334adfe7 , :197f7339-d08a-4270-a44e-164cd5146dd4 , :c6e9b1b9-673b-4038-a473-7c57181b9eec ;
        :hasIngredientCategory  :seafoods ;
        :pairsWith              :006473 , :000101 .

:thyme_aroma  rdf:type  :Aroma ;
        skos:prefLabel  "Thyme Aroma"@en ;
        :hasAromaType   :herbal .

:000109  rdf:type               :Ingredient ;
        rdfs:seeAlso            "http://www.wikidata.org/entity/Q65522654"^^xsd:anyURI ;
        skos:definition         "A basil leaf is a fragrant, green leaf with a strong, sweet aroma, often used as a herb in cooking."@en ;
        skos:prefLabel          "Basil Leaf"@en ;
        :hasAroma               :lemon_aroma , :camphor_aroma , :green_aroma , :clove_aroma ;
        :hasFunctionalBenefit   :c5a4476f-dc4e-417a-a47a-ede2655abb18 , :c6e9b1b9-673b-4038-a473-7c57181b9eec , :e498450d-cced-4a4f-93dd-b3ef3d5e2d43 , :787e979b-4d45-48b4-9f11-6fba2b367924 , :be450163-d1fc-4eec-8e1b-ef10c6ddbfe2 , :00541d6d-4dc5-4853-98f2-d176c27db355 , :d1c71bca-dd90-47d3-9f3b-1e214ccaeb85 , :aab0922c-eece-44ff-b800-92af6c07f55d , :1e86605f-2026-4f12-8293-e168aafc11e3 , :a5fee1e7-b975-44b2-b4dc-498e7c295bd4 , :9521e144-95e4-4171-a421-9a468b1c62e5 ;
        :hasIngredientCategory  :culinary_herbs .

:000141  rdf:type               :Ingredient ;
        rdfs:seeAlso            "http://www.wikidata.org/entity/Q13202263"^^xsd:anyURI ;
        skos:definition         "Juicy, stone fruits with a sweet and fragrant flavor, commonly eaten fresh or used in desserts."@en ;
        skos:prefLabel          "Yellow Peach"@en ;
        :hasAroma               :citrus_aroma , :pineapple_aroma , :honey_aroma , :peach_aroma ;
        :hasFunctionalBenefit   :a910f718-6310-459f-976b-6c9c334adfe7 , :00541d6d-4dc5-4853-98f2-d176c27db355 , :e498450d-cced-4a4f-93dd-b3ef3d5e2d43 , :c5a4476f-dc4e-417a-a47a-ede2655abb18 , :c6e9b1b9-673b-4038-a473-7c57181b9eec , :be450163-d1fc-4eec-8e1b-ef10c6ddbfe2 , :aab0922c-eece-44ff-b800-92af6c07f55d , :9521e144-95e4-4171-a421-9a468b1c62e5 , :787e979b-4d45-48b4-9f11-6fba2b367924 , :6a1a1d51-dfab-4237-aeac-a9ac4db26486 , :d1c71bca-dd90-47d3-9f3b-1e214ccaeb85 ;
        :hasIngredientCategory  :stone_fruits ;
        :hasTaste               :sour_taste , :sweet_taste ;
        :hasTexture             :juicy_texture ;
        :pairsWith              :000142 .

:juicy_texture  rdf:type  :Texture ;
        skos:prefLabel  "Juicy Texture"@en .

:000104  rdf:type               :Ingredient ;
        rdfs:seeAlso            "http://www.wikidata.org/entity/Q198815"^^xsd:anyURI ;
        skos:definition         "Creamy and tangy cheese made from goat's milk, known for its distinct flavor and versatility."@en ;
        skos:prefLabel          "Goat Cheese"@en ;
        :hasFunctionalBenefit   :00541d6d-4dc5-4853-98f2-d176c27db355 , :aab0922c-eece-44ff-b800-92af6c07f55d ;
        :hasIngredientCategory  :dairy_category ;
        :pairsWith              :000101 .

:001008  rdf:type               :Ingredient ;
        rdfs:seeAlso            "http://www.wikidata.org/entity/Q2164820"^^xsd:anyURI ;
        skos:definition         "Milk chocolate is a smooth, creamy chocolate made from cocoa solids, milk, and sugar, known for its sweet flavor."@en ;
        skos:prefLabel          "Milk Chocolate"@en ;
        :hasAroma               :buttery_aroma , :milk_aroma , :chocolate_aroma , :caramel_aroma , :hazelnut_aroma , :vanilla_aroma ;
        :hasFunctionalBenefit   :9521e144-95e4-4171-a421-9a468b1c62e5 , :c6e9b1b9-673b-4038-a473-7c57181b9eec ;
        :hasIngredientCategory  :chocolate_category ;
        :hasTaste               :sweet_taste ;
        :hasTexture             :melting_texture , :hard_texture .

:citrus_spices  rdf:type  skos:Concept , :IngredientCategory ;
        skos:broader     :spice_category ;
        skos:definition  "Encompasses spices derived from citrus fruits, such as lemon zest, orange peel, or lime leaves, adding tangy and aromatic notes."@en ;
        skos:prefLabel   "Citrus Spices"@en .

:005675  rdf:type               :Ingredient ;
        rdfs:seeAlso            "http://www.wikidata.org/entity/Q4200953"^^xsd:anyURI ;
        skos:definition         "Turkey meat is lean, white poultry with a mild, slightly gamey flavor, commonly roasted, grilled, or used in a variety of dishes."@en ;
        skos:prefLabel          "Turkey"@en ;
        :hasFunctionalBenefit   :9521e144-95e4-4171-a421-9a468b1c62e5 , :c5a4476f-dc4e-417a-a47a-ede2655abb18 , :6a1a1d51-dfab-4237-aeac-a9ac4db26486 , :a910f718-6310-459f-976b-6c9c334adfe7 , :be450163-d1fc-4eec-8e1b-ef10c6ddbfe2 , :197f7339-d08a-4270-a44e-164cd5146dd4 , :00541d6d-4dc5-4853-98f2-d176c27db355 , :e498450d-cced-4a4f-93dd-b3ef3d5e2d43 , :4b2e9d35-65b8-4a2e-96a4-6436e368f15f , :aab0922c-eece-44ff-b800-92af6c07f55d , :1e883a46-9d0a-4f5a-aa3a-4e75a25e0eba , :e3f7dd51-c162-4746-8f72-cababacf8ace , :c6e9b1b9-673b-4038-a473-7c57181b9eec , :787e979b-4d45-48b4-9f11-6fba2b367924 , :d1c71bca-dd90-47d3-9f3b-1e214ccaeb85 ;
        :hasIngredientCategory  :meats .

:bitter_taste  rdf:type  :Taste ;
        skos:prefLabel  "Bitter Taste"@en .

:fresh_cheese  rdf:type  skos:Concept , :IngredientCategory ;
        skos:broader     :cheese ;
        skos:definition  "Refers to soft, unripened cheeses with a high moisture content, often mild and creamy in flavor."@en ;
        skos:prefLabel   "Fresh Cheese"@en .

:pear_aroma  rdf:type   :Aroma ;
        skos:prefLabel  "Pear Aroma"@en ;
        :hasAromaType   :fruity .

:earthy_aroma  rdf:type  :Aroma ;
        skos:prefLabel  "Earthy Aroma"@en ;
        :hasAromaType   :roasted .

:fruit_confections  rdf:type  skos:Concept , :IngredientCategory ;
        skos:broader     :sugar_confections ;
        skos:definition  "Encompasses confectionery products made primarily from fruits, such as fruit jellies, fruit gummies, and fruit-filled chocolates."@en ;
        skos:prefLabel   "Fruit Confections"@en .

:blue_cheese  rdf:type   skos:Concept , :IngredientCategory ;
        skos:broader     :cheese ;
        skos:definition  "Encompasses a type of cheese characterized by the presence of blue or green veins of mold, known for its distinct flavor."@en ;
        skos:prefLabel   "Blue Cheese"@en .

:tuber_vegetables  rdf:type  skos:Concept , :IngredientCategory ;
        skos:broader     :vegetable_category ;
        skos:definition  "Refers to vegetables where the enlarged underground stem or tuber is consumed, such as potatoes, yams, or taro."@en ;
        skos:prefLabel   "Tuber Vegetables"@en .

:tropical_aroma  rdf:type  :Aroma ;
        skos:prefLabel  "Tropical Aroma"@en ;
        :hasAromaType   :fruity .

:butter  rdf:type        skos:Concept , :IngredientCategory ;
        skos:broader     :dairy_category ;
        skos:definition  "Refers to a dairy product made by churning cream or milk, commonly used as a cooking fat or spread."@en ;
        skos:prefLabel   "Butter"@en .

:787e979b-4d45-48b4-9f11-6fba2b367924
        rdf:type         :FunctionalBenefit ;
        skos:definition  "Ingredients or products that can help regulate blood sugar levels." ;
        skos:prefLabel   "Diabetic"@en .

:apple_aroma  rdf:type  :Aroma ;
        skos:prefLabel  "Apple Aroma"@en ;
        :hasAromaType   :fruity .

:salt_taste  rdf:type   :Taste ;
        skos:prefLabel  "Salt Taste"@en .

:violet_aroma  rdf:type  :Aroma ;
        skos:prefLabel  "Violet Aroma"@en ;
        :hasAromaType   :floral .

:peach_aroma  rdf:type  :Aroma ;
        skos:prefLabel  "Peach Aroma"@en ;
        :hasAromaType   :fruity .

:001968  rdf:type               :Ingredient ;
        rdfs:seeAlso            "http://www.wikidata.org/entity/Q16976"^^xsd:anyURI ;
        skos:definition         "Pastis is an anise-flavored liqueur from France, commonly diluted with water before consumption."@en ;
        skos:prefLabel          "Pastis"@en ;
        :hasIngredientCategory  :non-grape-based_spirits .

:hard_texture  rdf:type  :Texture ;
        skos:prefLabel  "Hard Texture"@en .

:wines  rdf:type         skos:Concept , :IngredientCategory ;
        skos:broader     :alcoholic_drink ;
        skos:definition  "Includes alcoholic beverages produced by fermenting grapes or other fruits, offering a wide range of flavors, colors, and styles."@en ;
        skos:prefLabel   "Wines"@en .

:strawberry_aroma  rdf:type  :Aroma ;
        skos:prefLabel  "Strawberry Aroma"@en ;
        :hasAromaType   :fruity .

:algae  rdf:type         skos:Concept , :IngredientCategory ;
        skos:broader     :sea-grown_vegetables ;
        skos:definition  "Refers to various types of photosynthetic organisms that grow in water, such as seaweed or microalgae, which can be consumed as food or used as ingredients."@en ;
        skos:prefLabel   "Algae"@en .

:oat_flakes_cereal_aroma
        rdf:type        :Aroma ;
        skos:prefLabel  "Oat Flakes Cereal Aroma"@en ;
        :hasAromaType   :green .

:non-grape-based_spirits
        rdf:type         skos:Concept , :IngredientCategory ;
        skos:broader     :spirits ;
        skos:definition  "Encompasses distilled spirits made from sources other than grapes, such as whiskey, rum, vodka, and tequila."@en ;
        skos:prefLabel   "Non-grape-based Spirits"@en .

:000452  rdf:type               :Ingredient ;
        rdfs:seeAlso            "http://www.wikidata.org/entity/Q165308"^^xsd:anyURI ;
        skos:definition         "Vibrant orange squash with a mildly sweet, nutty flavor, used in both savory and sweet recipes, especially during autumn."@en ;
        skos:prefLabel          "Pumpkin"@en ;
        :hasAroma               :beany_aroma , :nutty_aroma , :fruity_aroma , :potato_aroma ;
        :hasFunctionalBenefit   :e498450d-cced-4a4f-93dd-b3ef3d5e2d43 , :d1c71bca-dd90-47d3-9f3b-1e214ccaeb85 , :787e979b-4d45-48b4-9f11-6fba2b367924 , :1e86605f-2026-4f12-8293-e168aafc11e3 , :be450163-d1fc-4eec-8e1b-ef10c6ddbfe2 , :c6e9b1b9-673b-4038-a473-7c57181b9eec , :1e883a46-9d0a-4f5a-aa3a-4e75a25e0eba , :a910f718-6310-459f-976b-6c9c334adfe7 , :00541d6d-4dc5-4853-98f2-d176c27db355 , :4b2e9d35-65b8-4a2e-96a4-6436e368f15f , :9521e144-95e4-4171-a421-9a468b1c62e5 ;
        :hasIngredientCategory  :fruit_vegetables ;
        :hasTexture             :starchy_texture ;
        :pairsWith              :000101 , :000873 .

:000072  rdf:type               :Ingredient ;
        rdfs:seeAlso            "http://www.wikidata.org/entity/Q1093742"^^xsd:anyURI ;
        skos:definition         "Citrus fruit with a sour and tangy flavor, commonly used in cooking, baking, and beverages."@en ;
        skos:prefLabel          "Lemon"@en ;
        :hasAroma               :lemon_aroma , :herbal_aroma ;
        :hasFunctionalBenefit   :6a1a1d51-dfab-4237-aeac-a9ac4db26486 , :e3f7dd51-c162-4746-8f72-cababacf8ace , :00541d6d-4dc5-4853-98f2-d176c27db355 , :e498450d-cced-4a4f-93dd-b3ef3d5e2d43 , :aab0922c-eece-44ff-b800-92af6c07f55d , :d1c71bca-dd90-47d3-9f3b-1e214ccaeb85 , :a5fee1e7-b975-44b2-b4dc-498e7c295bd4 , :a910f718-6310-459f-976b-6c9c334adfe7 , :8d06ddfc-2e8e-4eca-aadb-554cfab5aa6a , :c5a4476f-dc4e-417a-a47a-ede2655abb18 , :787e979b-4d45-48b4-9f11-6fba2b367924 , :1e86605f-2026-4f12-8293-e168aafc11e3 , :be450163-d1fc-4eec-8e1b-ef10c6ddbfe2 , :c6e9b1b9-673b-4038-a473-7c57181b9eec , :9521e144-95e4-4171-a421-9a468b1c62e5 ;
        :hasIngredientCategory  :citrus_fruits ;
        :hasTaste               :sweet_taste , :sour_taste ;
        :hasTexture             :juicy_texture ;
        :pairsWith              :000155 .

:fig_aroma  rdf:type    :Aroma ;
        skos:prefLabel  "Fig Aroma"@en ;
        :hasAromaType   :fruity .

:spicy_aroma  rdf:type  :Aroma ;
        skos:prefLabel  "Spicy Aroma"@en ;
        :hasAromaType   :spicy .

:vanilla_aroma  rdf:type  :Aroma ;
        skos:prefLabel  "Vanilla Aroma"@en ;
        :hasAromaType   :spicy .

:008970  rdf:type               :Ingredient ;
        rdfs:seeAlso            "http://www.wikidata.org/entity/Q1155703"^^xsd:anyURI ;
        skos:definition         "Beverage made by steeping ground coffee beans in hot water, known for its stimulating effect."@en ;
        skos:prefLabel          "Brewed Coffee"@en ;
        :hasAroma               :maple_aroma , :roasted_aroma , :coffee_aroma , :nutty_aroma , :chocolate_aroma , :woody_aroma ;
        :hasFunctionalBenefit   :9521e144-95e4-4171-a421-9a468b1c62e5 , :d1c71bca-dd90-47d3-9f3b-1e214ccaeb85 , :e498450d-cced-4a4f-93dd-b3ef3d5e2d43 , :ae69eda5-a1f9-41b4-b70e-1a7972de7c15 , :a910f718-6310-459f-976b-6c9c334adfe7 , :00541d6d-4dc5-4853-98f2-d176c27db355 , :e3f7dd51-c162-4746-8f72-cababacf8ace , :c6e9b1b9-673b-4038-a473-7c57181b9eec , :be450163-d1fc-4eec-8e1b-ef10c6ddbfe2 , :3674c0c7-026a-4337-a10c-bbe4ceff1870 , :197f7339-d08a-4270-a44e-164cd5146dd4 , :6a1a1d51-dfab-4237-aeac-a9ac4db26486 , :1e883a46-9d0a-4f5a-aa3a-4e75a25e0eba , :aab0922c-eece-44ff-b800-92af6c07f55d , :787e979b-4d45-48b4-9f11-6fba2b367924 , :8d06ddfc-2e8e-4eca-aadb-554cfab5aa6a , :4b2e9d35-65b8-4a2e-96a4-6436e368f15f ;
        :hasIngredientCategory  :coffees .

:005569  rdf:type               :Ingredient ;
        rdfs:seeAlso            "http://www.wikidata.org/entity/Q13099586"^^xsd:anyURI ;
        skos:definition         "Juicy, sweet fruits with a crisp texture, commonly eaten fresh or used in desserts."@en ;
        skos:prefLabel          "Pear"@en ;
        :hasAroma               :floral_aroma , :pear_aroma , :honey_aroma , :lemon_aroma ;
        :hasFunctionalBenefit   :c6e9b1b9-673b-4038-a473-7c57181b9eec , :a910f718-6310-459f-976b-6c9c334adfe7 , :9521e144-95e4-4171-a421-9a468b1c62e5 , :be450163-d1fc-4eec-8e1b-ef10c6ddbfe2 , :00541d6d-4dc5-4853-98f2-d176c27db355 , :1e86605f-2026-4f12-8293-e168aafc11e3 , :aab0922c-eece-44ff-b800-92af6c07f55d , :d1c71bca-dd90-47d3-9f3b-1e214ccaeb85 , :6a1a1d51-dfab-4237-aeac-a9ac4db26486 , :787e979b-4d45-48b4-9f11-6fba2b367924 , :e3f7dd51-c162-4746-8f72-cababacf8ace , :e498450d-cced-4a4f-93dd-b3ef3d5e2d43 ;
        :hasIngredientCategory  :pome_fruits ;
        :hasTaste               :sweet_taste ;
        :hasTexture             :soft_texture , :juicy_texture .

:000030  rdf:type               :Ingredient ;
        rdfs:seeAlso            "http://www.wikidata.org/entity/Q15046077"^^xsd:anyURI ;
        skos:definition         "A spicy and aromatic root commonly used in cooking and known for its distinctive flavor."@en ;
        skos:prefLabel          "Ginger"@en ;
        :hasAroma               :camphor_aroma , :lemon_aroma , :spicy_aroma ;
        :hasFunctionalBenefit   :c5a4476f-dc4e-417a-a47a-ede2655abb18 , :3674c0c7-026a-4337-a10c-bbe4ceff1870 , :d1c71bca-dd90-47d3-9f3b-1e214ccaeb85 , :1e86605f-2026-4f12-8293-e168aafc11e3 , :e3f7dd51-c162-4746-8f72-cababacf8ace , :1e883a46-9d0a-4f5a-aa3a-4e75a25e0eba , :e498450d-cced-4a4f-93dd-b3ef3d5e2d43 , :6a1a1d51-dfab-4237-aeac-a9ac4db26486 , :197f7339-d08a-4270-a44e-164cd5146dd4 , :787e979b-4d45-48b4-9f11-6fba2b367924 , :a910f718-6310-459f-976b-6c9c334adfe7 , :4b2e9d35-65b8-4a2e-96a4-6436e368f15f , :a5fee1e7-b975-44b2-b4dc-498e7c295bd4 , :be450163-d1fc-4eec-8e1b-ef10c6ddbfe2 , :8d06ddfc-2e8e-4eca-aadb-554cfab5aa6a , :00541d6d-4dc5-4853-98f2-d176c27db355 , :aab0922c-eece-44ff-b800-92af6c07f55d , :c6e9b1b9-673b-4038-a473-7c57181b9eec , :9521e144-95e4-4171-a421-9a468b1c62e5 ;
        :hasIngredientCategory  :citrus_spices ;
        :hasTaste               :pungent_taste ;
        :hasTrigeminal          :tingling_trigeminal_taste , :cooling_trigeminal_taste ;
        :pairsWith              :000840 , :000155 , :000109 , :000159 , :000031 .

:yoghurt  rdf:type       skos:Concept , :IngredientCategory ;
        skos:broader     :dairy_category ;
        skos:definition  "Refers to a fermented dairy product made from milk, typically with added bacterial cultures, offering a creamy and tangy taste."@en ;
        skos:prefLabel   "Yoghurt"@en .

:corn_aroma  rdf:type   :Aroma ;
        skos:prefLabel  "Corn Aroma"@en ;
        :hasAromaType   :vegetable .

:acidic_aroma  rdf:type  :Aroma ;
        skos:prefLabel  "Acidic Aroma"@en ;
        :hasAromaType   :cheesy .

:dish_category  rdf:type  skos:Concept , :IngredientCategory ;
        skos:definition  "A dish refers to a prepared and cooked food item that is intended to be consumed as a single serving. It can consist of one or more ingredients that have been combined and cooked together to create a specific flavor, texture, and presentation."@en ;
        skos:prefLabel   "Dish Category"@en .

:additives  rdf:type     skos:Concept , :IngredientCategory ;
        skos:broader     :food_additives_category ;
        skos:definition  "Encompasses substances added to food products to enhance taste, texture, appearance, or extend shelf life, such as preservatives or emulsifiers."@en ;
        skos:prefLabel   "Additives"@en .

:005754  rdf:type               :Ingredient ;
        rdfs:seeAlso            "http://www.wikidata.org/entity/Q6663"^^xsd:anyURI ;
        skos:definition         "Ground meat formed into a patty and cooked in an oven, resulting in a flavorful and juicy burger."@en ;
        skos:prefLabel          "Hamburger"@en ;
        :hasFunctionalBenefit   :c6e9b1b9-673b-4038-a473-7c57181b9eec ;
        :hasIngredientCategory  :meats ;
        :pairsWith              :000101 , :005483 .

:000355  rdf:type               :Ingredient ;
        rdfs:seeAlso            "http://www.wikidata.org/entity/Q18966"^^xsd:anyURI ;
        skos:definition         "A type of maize known for its tender, sweet kernels, enjoyed as a vegetable when fresh and often used in a variety of dishes."@en ;
        skos:prefLabel          "Sweet Corn"@en ;
        :hasAroma               :corn_aroma , :milk_aroma , :pea_aroma ;
        :hasFunctionalBenefit   :1e883a46-9d0a-4f5a-aa3a-4e75a25e0eba , :c6e9b1b9-673b-4038-a473-7c57181b9eec , :9521e144-95e4-4171-a421-9a468b1c62e5 , :be450163-d1fc-4eec-8e1b-ef10c6ddbfe2 ;
        :hasIngredientCategory  :fruit_vegetables ;
        :pairsWith              :000452 , :000520 , :000313 .

:snacks_category  rdf:type  skos:Concept , :IngredientCategory ;
        skos:definition  "Includes a wide range of snack foods like chips, crisps, popcorn, and rice snacks."@en ;
        skos:prefLabel   "Snacks Category"@en .

:000920  rdf:type               :Ingredient ;
        rdfs:seeAlso            "http://www.wikidata.org/entity/Q2735883"^^xsd:anyURI ;
        skos:definition         "Crisp, green vegetables with a mild and refreshing flavor, commonly eaten fresh or pickled."@en ;
        skos:prefLabel          "Cucumber"@en ;
        :hasAroma               :cucumber_aroma , :green_aroma ;
        :hasFunctionalBenefit   :aab0922c-eece-44ff-b800-92af6c07f55d , :e498450d-cced-4a4f-93dd-b3ef3d5e2d43 , :197f7339-d08a-4270-a44e-164cd5146dd4 , :d1c71bca-dd90-47d3-9f3b-1e214ccaeb85 , :6a1a1d51-dfab-4237-aeac-a9ac4db26486 , :c6e9b1b9-673b-4038-a473-7c57181b9eec , :be450163-d1fc-4eec-8e1b-ef10c6ddbfe2 , :4b2e9d35-65b8-4a2e-96a4-6436e368f15f , :c5a4476f-dc4e-417a-a47a-ede2655abb18 , :1e86605f-2026-4f12-8293-e168aafc11e3 , :00541d6d-4dc5-4853-98f2-d176c27db355 , :9521e144-95e4-4171-a421-9a468b1c62e5 , :a910f718-6310-459f-976b-6c9c334adfe7 , :8d06ddfc-2e8e-4eca-aadb-554cfab5aa6a ;
        :hasIngredientCategory  :fruit_vegetables ;
        :pairsWith              :000163 , :000133 , :005942 .

:chili_spices  rdf:type  skos:Concept , :IngredientCategory ;
        skos:broader     :pungent_spices ;
        skos:definition  "Refers to spices made from chili peppers, offering varying levels of heat and flavors, often used in spicy dishes or hot sauces."@en ;
        skos:prefLabel   "Chili Spices"@en .

:000313  rdf:type               :Ingredient ;
        rdfs:seeAlso            "http://www.wikidata.org/entity/Q10987"^^xsd:anyURI ;
        skos:definition         "A sweet, natural substance produced by bees from flower nectar, commonly used as a sweetener."@en ;
        skos:prefLabel          "Honey"@en ;
        :hasAroma               :honey_aroma ;
        :hasFunctionalBenefit   :00541d6d-4dc5-4853-98f2-d176c27db355 , :197f7339-d08a-4270-a44e-164cd5146dd4 , :c5a4476f-dc4e-417a-a47a-ede2655abb18 , :a910f718-6310-459f-976b-6c9c334adfe7 , :e3f7dd51-c162-4746-8f72-cababacf8ace , :d1c71bca-dd90-47d3-9f3b-1e214ccaeb85 , :787e979b-4d45-48b4-9f11-6fba2b367924 , :a5fee1e7-b975-44b2-b4dc-498e7c295bd4 , :4b2e9d35-65b8-4a2e-96a4-6436e368f15f , :c6e9b1b9-673b-4038-a473-7c57181b9eec , :1e883a46-9d0a-4f5a-aa3a-4e75a25e0eba , :aab0922c-eece-44ff-b800-92af6c07f55d , :1e86605f-2026-4f12-8293-e168aafc11e3 , :6a1a1d51-dfab-4237-aeac-a9ac4db26486 , :e498450d-cced-4a4f-93dd-b3ef3d5e2d43 , :be450163-d1fc-4eec-8e1b-ef10c6ddbfe2 , :3674c0c7-026a-4337-a10c-bbe4ceff1870 , :8d06ddfc-2e8e-4eca-aadb-554cfab5aa6a , :9521e144-95e4-4171-a421-9a468b1c62e5 ;
        :hasIngredientCategory  :honeys ;
        :hasTaste               :sweet_taste .

:000123  rdf:type               :Ingredient ;
        rdfs:seeAlso            "http://www.wikidata.org/entity/Q68315046"^^xsd:anyURI ;
        skos:definition         "A small, fragrant branch of the herb rosemary, used to impart flavor to dishes."@en ;
        skos:prefLabel          "Rosemary"@en ;
        :hasAroma               :woody_aroma , :pine_aroma , :camphor_aroma , :citrus_aroma , :thyme_aroma ;
        :hasFunctionalBenefit   :a910f718-6310-459f-976b-6c9c334adfe7 , :c5a4476f-dc4e-417a-a47a-ede2655abb18 , :197f7339-d08a-4270-a44e-164cd5146dd4 , :9521e144-95e4-4171-a421-9a468b1c62e5 , :e498450d-cced-4a4f-93dd-b3ef3d5e2d43 , :aab0922c-eece-44ff-b800-92af6c07f55d , :e3f7dd51-c162-4746-8f72-cababacf8ace , :6a1a1d51-dfab-4237-aeac-a9ac4db26486 , :d1c71bca-dd90-47d3-9f3b-1e214ccaeb85 , :787e979b-4d45-48b4-9f11-6fba2b367924 , :c6e9b1b9-673b-4038-a473-7c57181b9eec , :00541d6d-4dc5-4853-98f2-d176c27db355 , :a5fee1e7-b975-44b2-b4dc-498e7c295bd4 , :be450163-d1fc-4eec-8e1b-ef10c6ddbfe2 ;
        :hasIngredientCategory  :culinary_herbs ;
        :pairsWith              :000159 , :000109 , :006471 , :000357 , :000840 , :000155 .

:sauces_category  rdf:type  skos:Concept , :IngredientCategory ;
        skos:definition  "Encompasses different types of sauces used for flavoring and enhancing the taste of dishes."@en ;
        skos:prefLabel   "Sauces Category"@en .

:grapefruit_aroma  rdf:type  :Aroma ;
        skos:prefLabel  "Grapefruit Aroma"@en ;
        :hasAromaType   :citrus .

:001959  rdf:type               :Ingredient ;
        rdfs:seeAlso            "http://www.wikidata.org/entity/Q693078"^^xsd:anyURI ;
        skos:definition         "Grappa is an Italian brandy made from grape pomace, known for its strong and distinctive flavor."@en ;
        skos:prefLabel          "Grappa"@en ;
        :hasIngredientCategory  :grape-based_spirits ;
        :pairsWith              :007088 , :000886 , :001696 , :000148 , :000865 , :000791 , :001755 .

:000865  rdf:type               :Ingredient ;
        rdfs:seeAlso            "http://www.wikidata.org/entity/Q170219"^^xsd:anyURI ;
        skos:definition         "Sake is a Japanese rice wine with a mild and slightly sweet flavor, commonly consumed as a beverage."@en ;
        skos:prefLabel          "Sake"@en ;
        :hasAroma               :rice_aroma , :fermented_aroma , :fruity_aroma ;
        :hasFunctionalBenefit   :00541d6d-4dc5-4853-98f2-d176c27db355 , :e498450d-cced-4a4f-93dd-b3ef3d5e2d43 ;
        :hasIngredientCategory  :drinks_category ;
        :pairsWith              :007088 , :000791 .

:confectionary_category
        rdf:type         skos:Concept , :IngredientCategory ;
        skos:definition  "Encompasses sweet treats like chocolate confections, milk confections, sugar confections, and fruit confections."@en ;
        skos:prefLabel   "Confectionary Category"@en .

:005842  rdf:type               :Ingredient ;
        rdfs:seeAlso            "http://www.wikidata.org/entity/Q21546392"^^xsd:anyURI ;
        skos:definition         "Smooth, concentrated paste made from roasted garlic cloves, providing a mellow, aromatic essence to a wide range of recipes."@en ;
        skos:prefLabel          "Garlic Puree"@en ;
        :hasIngredientCategory  :bulb_vegetables ;
        :pairsWith              :000133 .

:bitter_spices  rdf:type  skos:Concept , :IngredientCategory ;
        skos:broader     :spice_category ;
        skos:definition  "Refers to spices with a bitter taste, often used in small quantities to add complexity and depth of flavor to dishes."@en ;
        skos:prefLabel   "Bitter Spices"@en .

:green_aroma  rdf:type  :Aroma ;
        skos:prefLabel  "Green Aroma"@en ;
        :hasAromaType   :green .

:fruity_aroma  rdf:type  :Aroma ;
        skos:prefLabel  "Fruity Aroma"@en ;
        :hasAromaType   :fruity .

:sweet_spices  rdf:type  skos:Concept , :IngredientCategory ;
        skos:broader     :spice_category ;
        skos:definition  "Refers to spices with a sweet taste or aroma, such as cinnamon, vanilla, or nutmeg, often used in desserts, baked goods, or sweet beverages."@en ;
        skos:prefLabel   "Sweet Spices"@en .

:chocolate_category  rdf:type  skos:Concept , :IngredientCategory ;
        skos:definition  "Encompasses products made from or containing chocolate, including confections and desserts."@en ;
        skos:prefLabel   "Chocolate Category"@en .

:000021  rdf:type               :Ingredient ;
        rdfs:seeAlso            "http://www.wikidata.org/entity/Q545985"^^xsd:anyURI ;
        skos:definition         "Pungent condiment made from fermented fish, commonly used in Southeast Asian cuisine for its savory flavor."@en ;
        skos:prefLabel          "Fish Sauce"@en ;
        :hasAroma               :fishy_aroma , :caramel_aroma , :roasted_aroma , :cheesy_aroma ;
        :hasFunctionalBenefit   :c6e9b1b9-673b-4038-a473-7c57181b9eec , :9521e144-95e4-4171-a421-9a468b1c62e5 ;
        :hasIngredientCategory  :table_sauces ;
        :hasTaste               :salt_taste , :umami_taste .

:gin_and_jenever  rdf:type  skos:Concept , :IngredientCategory ;
        skos:broader     :spirits ;
        skos:definition  "Includes distilled spirits flavored with juniper berries and other botanical ingredients, such as gin and jenever."@en ;
        skos:prefLabel   "Gin And Jenever"@en .

:Ingredient  rdf:type    owl:Class ;
        rdfs:seeAlso     <https://www.foodpairing.com/industry/glossary/definition/ingredient/> ;
        skos:definition  "An ingredient is an individual food entity or elaboration thereof (e.g. apple & apple jam)."@en ;
        skos:prefLabel   "Ingredient"@en .

:milk_confections  rdf:type  skos:Concept , :IngredientCategory ;
        skos:broader     :confectionary_category ;
        skos:definition  "Includes confectionery products made with milk or milk-derived ingredients, such as fudge, caramels, and milk chocolates."@en ;
        skos:prefLabel   "Milk Confections"@en .

:lettuces  rdf:type      skos:Concept , :IngredientCategory ;
        skos:broader     :leaves_vegetables ;
        skos:definition  "Encompasses different types of lettuce, such as romaine, iceberg, or butterhead, often used in salads or as a bed for other ingredients."@en ;
        skos:prefLabel   "Lettuces"@en .

:bread  rdf:type         skos:Concept , :IngredientCategory ;
        skos:broader     :bakery_category ;
        skos:definition  "Bread is a staple food made from a combination of flour and water, along with other ingredients such as yeast, salt, and sometimes sweeteners or fats. The dough is typically baked."@en ;
        skos:prefLabel   "Bread"@en .

:fish   rdf:type         skos:Concept , :IngredientCategory ;
        skos:broader     :protein_category ;
        skos:definition  "Encompasses various edible aquatic creatures, often prepared as food, such as salmon, tuna, cod, or trout."@en ;
        skos:prefLabel   "Fish"@en .

dct:publisher  rdf:type  owl:AnnotationProperty .

:005930  rdf:type               :Ingredient ;
        rdfs:seeAlso            "http://www.wikidata.org/entity/Q8495"^^xsd:anyURI ;
        skos:definition         "A white, nutrient-rich liquid produced by mammals, commonly consumed as a beverage and used in cooking."@en ;
        skos:prefLabel          "Milk"@en ;
        :hasAroma               :milk_aroma ;
        :hasFunctionalBenefit   :c5a4476f-dc4e-417a-a47a-ede2655abb18 , :ae69eda5-a1f9-41b4-b70e-1a7972de7c15 , :e3f7dd51-c162-4746-8f72-cababacf8ace , :6a1a1d51-dfab-4237-aeac-a9ac4db26486 , :1e86605f-2026-4f12-8293-e168aafc11e3 , :a5fee1e7-b975-44b2-b4dc-498e7c295bd4 , :787e979b-4d45-48b4-9f11-6fba2b367924 , :3674c0c7-026a-4337-a10c-bbe4ceff1870 , :9521e144-95e4-4171-a421-9a468b1c62e5 , :aab0922c-eece-44ff-b800-92af6c07f55d , :1e883a46-9d0a-4f5a-aa3a-4e75a25e0eba , :4b2e9d35-65b8-4a2e-96a4-6436e368f15f , :e498450d-cced-4a4f-93dd-b3ef3d5e2d43 , :00541d6d-4dc5-4853-98f2-d176c27db355 , :95d1327c-5984-4045-b8b7-126a3d976bc0 , :a910f718-6310-459f-976b-6c9c334adfe7 , :8d06ddfc-2e8e-4eca-aadb-554cfab5aa6a , :197f7339-d08a-4270-a44e-164cd5146dd4 , :d1c71bca-dd90-47d3-9f3b-1e214ccaeb85 , :c6e9b1b9-673b-4038-a473-7c57181b9eec , :be450163-d1fc-4eec-8e1b-ef10c6ddbfe2 ;
        :hasIngredientCategory  :milk ;
        :hasTaste               :sweet_taste ;
        :hasTexture             :creamy_texture ;
        :pairsWith              :000101 .

:000151  rdf:type               :Ingredient ;
        rdfs:seeAlso            "http://www.wikidata.org/entity/Q10817602"^^xsd:anyURI ;
        skos:definition         "Pineapples are tropical fruits with a spiky skin and a sweet, tangy flavor, commonly eaten fresh or used in desserts."@en ;
        skos:prefLabel          "Pineapple"@en ;
        :hasAroma               :grass_aroma , :caramel_aroma , :citrus_aroma , :pineapple_aroma ;
        :hasFunctionalBenefit   :c5a4476f-dc4e-417a-a47a-ede2655abb18 , :9521e144-95e4-4171-a421-9a468b1c62e5 , :00541d6d-4dc5-4853-98f2-d176c27db355 , :1e86605f-2026-4f12-8293-e168aafc11e3 , :787e979b-4d45-48b4-9f11-6fba2b367924 , :be450163-d1fc-4eec-8e1b-ef10c6ddbfe2 , :4b2e9d35-65b8-4a2e-96a4-6436e368f15f , :1e883a46-9d0a-4f5a-aa3a-4e75a25e0eba , :c6e9b1b9-673b-4038-a473-7c57181b9eec , :8d06ddfc-2e8e-4eca-aadb-554cfab5aa6a , :d1c71bca-dd90-47d3-9f3b-1e214ccaeb85 , :a5fee1e7-b975-44b2-b4dc-498e7c295bd4 ;
        :hasIngredientCategory  :tropical_fruits ;
        :hasTaste               :sweet_taste , :sour_taste ;
        :hasTexture             :juicy_texture ;
        :pairsWith              :000141 , :000101 , :000148 .

:000096  rdf:type               :Ingredient ;
        rdfs:seeAlso            "http://www.wikidata.org/entity/Q61046162"^^xsd:anyURI ;
        skos:definition         "Chives are thin, green herbs with a mild onion flavor, often used as a garnish or flavoring in various dishes."@en ;
        skos:prefLabel          "Chives"@en ;
        :hasAroma               :pungent_aroma , :onion_aroma , :garlic_aroma , :green_aroma ;
        :hasFunctionalBenefit   :9521e144-95e4-4171-a421-9a468b1c62e5 ;
        :hasIngredientCategory  :culinary_herbs ;
        :pairsWith              :000110 , :000047 .

:egg_aroma  rdf:type    :Aroma ;
        skos:prefLabel  "Egg Aroma"@en ;
        :hasAromaType   :cheesy .

:mushroom_aroma  rdf:type  :Aroma ;
        skos:prefLabel  "Mushroom Aroma"@en ;
        :hasAromaType   :vegetable .

:000059  rdf:type               :Ingredient ;
        rdfs:seeAlso            "http://www.wikidata.org/entity/Q23900272"^^xsd:anyURI ;
        skos:definition         "A cruciferous vegetable known for its mild flavor and versatility in cooking."@en ;
        skos:prefLabel          "Cauliflower"@en ;
        :hasAroma               :mustard_aroma , :onion_aroma ;
        :hasFunctionalBenefit   :a910f718-6310-459f-976b-6c9c334adfe7 , :9521e144-95e4-4171-a421-9a468b1c62e5 , :c5a4476f-dc4e-417a-a47a-ede2655abb18 , :c6e9b1b9-673b-4038-a473-7c57181b9eec , :e498450d-cced-4a4f-93dd-b3ef3d5e2d43 , :00541d6d-4dc5-4853-98f2-d176c27db355 , :be450163-d1fc-4eec-8e1b-ef10c6ddbfe2 ;
        :hasIngredientCategory  :flower_vegetables ;
        :hasTexture             :hard_texture .

:pungent_spices  rdf:type  skos:Concept , :IngredientCategory ;
        skos:broader     :spice_category ;
        skos:definition  "Refers to spices with a strong, sharp, or intense taste, often used to add heat or spiciness to foods, such as chili peppers or mustard seeds."@en ;
        skos:prefLabel   "Pungent Spices"@en .

:001755  rdf:type               :Ingredient ;
        rdfs:seeAlso            "http://www.wikidata.org/entity/Q1051699"^^xsd:anyURI ;
        skos:definition         "Cava is a sparkling wine from Catalonia, Spain, known for its crisp and effervescent quality."@en ;
        skos:prefLabel          "Cava"@en ;
        :hasIngredientCategory  :wines ;
        :pairsWith              :007088 , :000791 , :000886 , :000865 , :001959 .

:000281  rdf:type               :Ingredient ;
        rdfs:seeAlso            "http://www.wikidata.org/entity/Q20856764"^^xsd:anyURI ;
        skos:definition         "Coriander seeds are the dried fruits of the coriander plant, imparting a warm, citrusy flavor to dishes and frequently used in spice blends."@en ;
        skos:prefLabel          "Coriander Seed"@en ;
        :hasAroma               :citrus_aroma , :woody_aroma , :orange_aroma , :floral_aroma ;
        :hasFunctionalBenefit   :be450163-d1fc-4eec-8e1b-ef10c6ddbfe2 , :1e86605f-2026-4f12-8293-e168aafc11e3 , :6a1a1d51-dfab-4237-aeac-a9ac4db26486 , :aab0922c-eece-44ff-b800-92af6c07f55d , :9521e144-95e4-4171-a421-9a468b1c62e5 , :4b2e9d35-65b8-4a2e-96a4-6436e368f15f , :c6e9b1b9-673b-4038-a473-7c57181b9eec , :e498450d-cced-4a4f-93dd-b3ef3d5e2d43 , :787e979b-4d45-48b4-9f11-6fba2b367924 ;
        :hasIngredientCategory  :citrus_spices ;
        :pairsWith              :000840 , :000159 , :000109 .

:chocolate_confections
        rdf:type         skos:Concept , :IngredientCategory ;
        skos:broader     :confectionary_category ;
        skos:definition  "Encompasses confectionery products made primarily from chocolate, including chocolate bars, truffles, and pralines."@en ;
        skos:prefLabel   "Chocolate Confections"@en .

:000091  rdf:type               :Ingredient ;
        rdfs:seeAlso            "http://www.wikidata.org/entity/Q21281535"^^xsd:anyURI ;
        skos:definition         "Delicate herb with a mild, anise-like flavor, used to add a fresh and aromatic touch to dishes."@en ;
        skos:prefLabel          "Chervil"@en ;
        :hasAroma               :green_aroma , :anise_aroma ;
        :hasIngredientCategory  :culinary_herbs ;
        :hasTrigeminal          :cooling_trigeminal_taste ;
        :pairsWith              :000031 , :000123 , :000109 , :000840 , :000281 , :006471 .

:camphor_aroma  rdf:type  :Aroma ;
        skos:prefLabel  "Camphor Aroma"@en ;
        :hasAromaType   :spicy .

:f964c152-e1b0-4087-b7b9-6be16cec00ab
        rdf:type         :FunctionalBenefit ;
        skos:definition  "Ingredients or products with satiety-related functional benefits help promote feelings of fullness and satisfaction after eating." ;
        skos:prefLabel   "Satiety"@en .

:milk   rdf:type         skos:Concept , :IngredientCategory ;
        skos:broader     :dairy_category ;
        skos:definition  "Relates to the white liquid produced by mammals' mammary glands, often consumed as a beverage or used in various recipes."@en ;
        skos:prefLabel   "Milk"@en .

:Texture  rdf:type       owl:Class ;
        rdfs:seeAlso     <https://www.foodpairing.com/industry/glossary/definition/texture/> ;
        rdfs:subClassOf  :Flavour ;
        skos:definition  "Textures are the qualities of a food item that can be sensed through mouthfeel; i.e. the degree to which something is rough or smooth, or soft or hard."@en ;
        skos:prefLabel   "Texture"@en .

:roasted_aroma  rdf:type  :Aroma ;
        skos:prefLabel  "Roasted Aroma"@en ;
        :hasAromaType   :roasted .

:pepo_fruits  rdf:type   skos:Concept , :IngredientCategory ;
        skos:broader     :fruit_category ;
        skos:definition  "Encompasses fruits with a hard, outer rind and soft inner flesh, such as melons, cucumbers, and squash."@en ;
        skos:prefLabel   "Pepo Fruits"@en .

:cereals_category  rdf:type  skos:Concept , :IngredientCategory ;
        skos:definition  "Refers to grains and breakfast cereals such as oats, rice, pasta, and other grain-based products."@en ;
        skos:prefLabel   "Cereals Category"@en .

:grass_aroma  rdf:type  :Aroma ;
        skos:prefLabel  "Grass Aroma"@en ;
        :hasAromaType   :green .

:000017  rdf:type               :Ingredient ;
        rdfs:seeAlso            "http://www.wikidata.org/entity/Q20638126"^^xsd:anyURI ;
        skos:definition         "A red, yellowish, green, or even purple fruit with a juicy pulp, commonly used in salads, sauces, and various culinary dishes."@en ;
        skos:prefLabel          "Tomato"@en ;
        :hasAroma               :fruity_aroma , :green_aroma ;
        :hasFunctionalBenefit   :1e883a46-9d0a-4f5a-aa3a-4e75a25e0eba , :e3f7dd51-c162-4746-8f72-cababacf8ace , :aab0922c-eece-44ff-b800-92af6c07f55d , :a910f718-6310-459f-976b-6c9c334adfe7 , :6a1a1d51-dfab-4237-aeac-a9ac4db26486 , :be450163-d1fc-4eec-8e1b-ef10c6ddbfe2 , :c6e9b1b9-673b-4038-a473-7c57181b9eec , :e498450d-cced-4a4f-93dd-b3ef3d5e2d43 , :9521e144-95e4-4171-a421-9a468b1c62e5 , :c5a4476f-dc4e-417a-a47a-ede2655abb18 , :00541d6d-4dc5-4853-98f2-d176c27db355 , :197f7339-d08a-4270-a44e-164cd5146dd4 , :d1c71bca-dd90-47d3-9f3b-1e214ccaeb85 , :f964c152-e1b0-4087-b7b9-6be16cec00ab , :3674c0c7-026a-4337-a10c-bbe4ceff1870 , :787e979b-4d45-48b4-9f11-6fba2b367924 , :4b2e9d35-65b8-4a2e-96a4-6436e368f15f ;
        :hasIngredientCategory  :fruit_vegetables ;
        :hasTaste               :sour_taste ;
        :hasTexture             :juicy_texture .

:popcorn_aroma  rdf:type  :Aroma ;
        skos:prefLabel  "Popcorn Aroma"@en ;
        :hasAromaType   :roasted .

:000791  rdf:type               :Ingredient ;
        rdfs:seeAlso            "http://www.wikidata.org/entity/Q3268"^^xsd:anyURI ;
        skos:definition         "Apple brandy from the Normandy region of France, known for its fruity and robust flavor."@en ;
        skos:prefLabel          "Calvados"@en ;
        :hasIngredientCategory  :non-grape-based_spirits ;
        :pairsWith              :007088 .

:Trigeminal  rdf:type    owl:Class ;
        rdfs:seeAlso     <https://www.foodpairing.com/industry/glossary/definition/trigeminal-taste/> ;
        rdfs:subClassOf  :Flavour ;
        skos:definition  "Trigeminal tastes (“other tastes”) are a set of tastes which are perceived as triggers sent to the brain via the trigeminal nerve, creating the conscious perception of touch-position and pain-temperature information. Trigeminal sensations are often associated with compounds found in certain foods; menthol for cooling is found in mint, spilanthol comes from a variety of plants, causing a tingling effect on the tongue (think wine and green tea) and capsaicin in chilies is what gives them their signature spiciness."@en ;
        skos:prefLabel   "Trigeminal"@en .

:tingling_trigeminal_taste
        rdf:type        :Trigeminal ;
        skos:prefLabel  "Tingling Trigeminal Taste"@en .

:sugars  rdf:type        skos:Concept , :IngredientCategory ;
        skos:broader     :sweeteners_category ;
        skos:definition  "Refers to sweet-tasting, soluble carbohydrates added to foods and beverages to provide sweetness, flavor and energy. Includes natural and synthetic sugars."@en ;
        skos:prefLabel   "Sugars"@en .

:hasTaste  rdf:type         owl:ObjectProperty ;
        rdfs:domain         :Ingredient ;
        rdfs:range          :Taste ;
        rdfs:seeAlso        <https://www.foodpairing.com/industry/glossary/definition/taste/> ;
        rdfs:subPropertyOf  :hasFlavour ;
        skos:definition     "Assigns a taste to an ingredient."@en ;
        skos:prefLabel      "has taste"@en .

:005509  rdf:type               :Ingredient ;
        rdfs:seeAlso            "http://www.wikidata.org/entity/Q67594028"^^xsd:anyURI ;
        skos:definition         "Rice grains that have been cooked in boiling water, resulting in a fluffy and separate texture."@en ;
        skos:prefLabel          "Long-Grain Rice"@en ;
        :hasFunctionalBenefit   :c6e9b1b9-673b-4038-a473-7c57181b9eec , :be450163-d1fc-4eec-8e1b-ef10c6ddbfe2 , :00541d6d-4dc5-4853-98f2-d176c27db355 , :6a1a1d51-dfab-4237-aeac-a9ac4db26486 , :1e86605f-2026-4f12-8293-e168aafc11e3 , :197f7339-d08a-4270-a44e-164cd5146dd4 , :f964c152-e1b0-4087-b7b9-6be16cec00ab , :4b2e9d35-65b8-4a2e-96a4-6436e368f15f , :d1c71bca-dd90-47d3-9f3b-1e214ccaeb85 , :1e883a46-9d0a-4f5a-aa3a-4e75a25e0eba , :e3f7dd51-c162-4746-8f72-cababacf8ace , :8d06ddfc-2e8e-4eca-aadb-554cfab5aa6a , :787e979b-4d45-48b4-9f11-6fba2b367924 , :e498450d-cced-4a4f-93dd-b3ef3d5e2d43 , :aab0922c-eece-44ff-b800-92af6c07f55d , :c5a4476f-dc4e-417a-a47a-ede2655abb18 , :9521e144-95e4-4171-a421-9a468b1c62e5 , :3674c0c7-026a-4337-a10c-bbe4ceff1870 , :a910f718-6310-459f-976b-6c9c334adfe7 ;
        :hasIngredientCategory  :rice ;
        :pairsWith              :000046 .

:fats_and_oils_category
        rdf:type         skos:Concept , :IngredientCategory ;
        skos:definition  "Encompasses various fats and oils used in cooking and food preparation."@en ;
        skos:prefLabel   "Fats And Oils Category"@en .

:melting_texture  rdf:type  :Texture ;
        skos:prefLabel  "Melting Texture"@en .

:000142  rdf:type               :Ingredient ;
        rdfs:seeAlso            "http://www.wikidata.org/entity/Q841156"^^xsd:anyURI ;
        skos:definition         "Yellow nectarines are similar to peaches but have smooth skin and a sweet, juicy flavor."@en ;
        skos:prefLabel          "Yellow Nectarine"@en ;
        :hasAroma               :citrus_aroma , :peach_aroma , :coconut_aroma , :floral_aroma ;
        :hasFunctionalBenefit   :c6e9b1b9-673b-4038-a473-7c57181b9eec , :be450163-d1fc-4eec-8e1b-ef10c6ddbfe2 ;
        :hasIngredientCategory  :stone_fruits ;
        :hasTaste               :sour_taste , :sweet_taste ;
        :hasTexture             :juicy_texture ;
        :pairsWith              :005569 , :000141 .

:000105  rdf:type               :Ingredient ;
        rdfs:seeAlso            "http://www.wikidata.org/entity/Q2987371"^^xsd:anyURI ;
        skos:definition         "Crisp, slender pods with a fresh and slightly sweet taste, commonly used in various dishes."@en ;
        skos:prefLabel          "Green Bean"@en ;
        :hasFunctionalBenefit   :9521e144-95e4-4171-a421-9a468b1c62e5 ;
        :hasIngredientCategory  :seed_vegetables ;
        :pairsWith              :000873 .

:bitter  rdf:type        skos:Concept , :IngredientCategory ;
        skos:broader     :alcoholic_drink ;
        skos:definition  "Refers to a category of alcoholic beverages characterized by a bitter taste, often produced by botanical ingredients or hops."@en ;
        skos:prefLabel   "Bitter"@en .

:AromaType  rdf:type     owl:Class ;
        rdfs:seeAlso     <https://www.foodpairing.com/industry/glossary/definition/aroma-types/> ;
        skos:definition  "An aroma type serves as a fundamental category within the broader aroma profile. It is further subdivided into aroma descriptors, which constitute a group of diverse molecules sharing a distinct olfactory characteristic."@en ;
        skos:prefLabel   "Aroma Type"@en .

:chili  rdf:type         skos:Concept , :IngredientCategory ;
        skos:broader     :fruit_vegetables ;
        skos:definition  "Refers to spicy peppers, often used as a seasoning or ingredient to add heat and flavor to dishes."@en ;
        skos:prefLabel   "Chili"@en .

:000082  rdf:type               :Ingredient ;
        rdfs:seeAlso            "http://www.wikidata.org/entity/Q1474"^^xsd:anyURI ;
        skos:definition         "A leafy vegetable with a slightly bitter taste, commonly used in salads and cooked dishes."@en ;
        skos:prefLabel          "Belgian Endive"@en ;
        :hasFunctionalBenefit   :9521e144-95e4-4171-a421-9a468b1c62e5 ;
        :hasIngredientCategory  :leaves_vegetables ;
        :pairsWith              :000083 , :000520 , :000163 , :000141 , :000873 .

:drinks_category  rdf:type  skos:Concept , :IngredientCategory ;
        skos:definition  "Refers to a wide range of beverages, including alcoholic and non-alcoholic drinks like juices, soft drinks, coffee, tea, and flavored waters."@en ;
        skos:prefLabel   "Drinks Category"@en .

:herbal_and_spicy_confections
        rdf:type         skos:Concept , :IngredientCategory ;
        skos:broader     :sugar_confections ;
        skos:definition  "Relates to confectionery products infused with herbs or spices, often creating unique flavor combinations."@en ;
        skos:prefLabel   "Herbal And Spicy Confections"@en .

:000787  rdf:type               :Ingredient ;
        rdfs:seeAlso            "http://www.wikidata.org/entity/Q13241"^^xsd:anyURI ;
        skos:definition         "A variety of vanilla known for its rich and aromatic flavor, commonly used in baking."@en ;
        skos:prefLabel          "Vanilla 'Bourbon'"@en ;
        :hasFunctionalBenefit   :9521e144-95e4-4171-a421-9a468b1c62e5 , :be450163-d1fc-4eec-8e1b-ef10c6ddbfe2 , :c6e9b1b9-673b-4038-a473-7c57181b9eec , :a910f718-6310-459f-976b-6c9c334adfe7 , :e498450d-cced-4a4f-93dd-b3ef3d5e2d43 , :e3f7dd51-c162-4746-8f72-cababacf8ace ;
        :hasIngredientCategory  :sweet_spices ;
        :pairsWith              :000133 , :000791 .

:orange_aroma  rdf:type  :Aroma ;
        skos:prefLabel  "Orange Aroma"@en ;
        :hasAromaType   :citrus .

:be450163-d1fc-4eec-8e1b-ef10c6ddbfe2
        rdf:type         :FunctionalBenefit ;
        skos:definition  "Ingredients or products that may help reduce or manage stress levels in the body." ;
        skos:prefLabel   "Stress"@en .

:000040  rdf:type               :Ingredient ;
        rdfs:seeAlso            "http://www.wikidata.org/entity/Q131748"^^xsd:anyURI ;
        skos:definition         "Pungent condiment made from ground mustard seeds, commonly used to add flavor and heat to dishes."@en ;
        skos:prefLabel          "Mustard"@en ;
        :hasAroma               :acidic_aroma , :mustard_aroma ;
        :hasFunctionalBenefit   :9521e144-95e4-4171-a421-9a468b1c62e5 , :c5a4476f-dc4e-417a-a47a-ede2655abb18 , :d1c71bca-dd90-47d3-9f3b-1e214ccaeb85 , :e3f7dd51-c162-4746-8f72-cababacf8ace , :1e86605f-2026-4f12-8293-e168aafc11e3 , :e498450d-cced-4a4f-93dd-b3ef3d5e2d43 , :6a1a1d51-dfab-4237-aeac-a9ac4db26486 , :787e979b-4d45-48b4-9f11-6fba2b367924 , :197f7339-d08a-4270-a44e-164cd5146dd4 , :a910f718-6310-459f-976b-6c9c334adfe7 , :4b2e9d35-65b8-4a2e-96a4-6436e368f15f , :00541d6d-4dc5-4853-98f2-d176c27db355 , :aab0922c-eece-44ff-b800-92af6c07f55d , :c6e9b1b9-673b-4038-a473-7c57181b9eec , :be450163-d1fc-4eec-8e1b-ef10c6ddbfe2 ;
        :hasIngredientCategory  :table_sauces ;
        :hasTaste               :sour_taste ;
        :pairsWith              :000873 , :007109 , :001755 , :000865 .

:nuts_and_seeds_category
        rdf:type         skos:Concept , :IngredientCategory ;
        skos:definition  "Includes various types of nuts and seeds used as ingredients or snacks."@en ;
        skos:prefLabel   "Nuts And Seeds Category"@en .

:oat    rdf:type         skos:Concept , :IngredientCategory ;
        skos:broader     :grains ;
        skos:definition  "Relates to oats, a type of cereal grain commonly used in breakfast cereals, porridge, and baked goods."@en ;
        skos:prefLabel   "Oat"@en .

:Aroma  rdf:type         owl:Class ;
        rdfs:seeAlso     <https://www.foodpairing.com/industry/glossary/definition/aroma/> ;
        rdfs:subClassOf  :Flavour ;
        skos:definition  "An aroma refers to the collective scent of ingredients, such as passion fruit. It comprises aroma molecules, each possessing a distinct smell, like a lactone that imparts a peach-like fragrance."@en ;
        skos:prefLabel   "Aroma"@en .

:pea_aroma  rdf:type    :Aroma ;
        skos:prefLabel  "Pea Aroma"@en ;
        :hasAromaType   :vegetable .

:citrus_aroma  rdf:type  :Aroma ;
        skos:prefLabel  "Citrus Aroma"@en ;
        :hasAromaType   :citrus .

:dairy_category  rdf:type  skos:Concept , :IngredientCategory ;
        skos:definition  "Involves dairy products like butter, cheese, cream, milk, plant-based dairy alternatives, and yogurt."@en ;
        skos:prefLabel   "Dairy Category"@en .

:1e86605f-2026-4f12-8293-e168aafc11e3
        rdf:type         :FunctionalBenefit ;
        skos:definition  "Probiotics are live microorganisms that provide health benefits when consumed, particularly in aiding digestion and supporting a healthy gut microbiome." ;
        skos:prefLabel   "Probiotic"@en .

:006473  rdf:type               :Ingredient ;
        rdfs:seeAlso            "http://www.wikidata.org/entity/Q1747334"^^xsd:anyURI ;
        skos:definition         "Shellfish known for their delicate and briny flavor, commonly eaten raw or cooked."@en ;
        skos:prefLabel          "Oyster"@en ;
        :hasFunctionalBenefit   :95d1327c-5984-4045-b8b7-126a3d976bc0 , :00541d6d-4dc5-4853-98f2-d176c27db355 , :be450163-d1fc-4eec-8e1b-ef10c6ddbfe2 , :d1c71bca-dd90-47d3-9f3b-1e214ccaeb85 , :a910f718-6310-459f-976b-6c9c334adfe7 , :c5a4476f-dc4e-417a-a47a-ede2655abb18 , :c6e9b1b9-673b-4038-a473-7c57181b9eec , :e498450d-cced-4a4f-93dd-b3ef3d5e2d43 , :aab0922c-eece-44ff-b800-92af6c07f55d , :197f7339-d08a-4270-a44e-164cd5146dd4 , :9521e144-95e4-4171-a421-9a468b1c62e5 ;
        :hasIngredientCategory  :seafoods .

:fatty_taste  rdf:type  :Taste ;
        skos:prefLabel  "Fatty Taste"@en .

:almond_aroma  rdf:type  :Aroma ;
        skos:prefLabel  "Almond Aroma"@en ;
        :hasAromaType   :nutty .

:000133  rdf:type               :Ingredient ;
        rdfs:seeAlso            "http://www.wikidata.org/entity/Q14458220"^^xsd:anyURI ;
        skos:definition         "Strawberries are sweet, red berries with a juicy texture, commonly used in desserts, salads, and beverages."@en ;
        skos:prefLabel          "Strawberry"@en ;
        :hasAroma               :orange_aroma , :strawberry_aroma , :caramel_aroma ;
        :hasFunctionalBenefit   :787e979b-4d45-48b4-9f11-6fba2b367924 , :00541d6d-4dc5-4853-98f2-d176c27db355 , :d1c71bca-dd90-47d3-9f3b-1e214ccaeb85 , :1e86605f-2026-4f12-8293-e168aafc11e3 , :f964c152-e1b0-4087-b7b9-6be16cec00ab , :a910f718-6310-459f-976b-6c9c334adfe7 , :c5a4476f-dc4e-417a-a47a-ede2655abb18 , :197f7339-d08a-4270-a44e-164cd5146dd4 , :9521e144-95e4-4171-a421-9a468b1c62e5 , :e498450d-cced-4a4f-93dd-b3ef3d5e2d43 , :6a1a1d51-dfab-4237-aeac-a9ac4db26486 , :aab0922c-eece-44ff-b800-92af6c07f55d , :c6e9b1b9-673b-4038-a473-7c57181b9eec ;
        :hasIngredientCategory  :berries ;
        :hasTaste               :sour_taste , :sweet_taste ;
        :hasTexture             :juicy_texture ;
        :pairsWith              :005842 .

:viennoiserie  rdf:type  skos:Concept , :IngredientCategory ;
        skos:broader     :bakery_category ;
        skos:definition  "Encompasses sweet baked goods like cookies and cakes, typically made from a combination of flour, sugar, eggs, and flavorings."@en ;
        skos:prefLabel   "Viennoiserie"@en .

:stem_vegetables  rdf:type  skos:Concept , :IngredientCategory ;
        skos:broader     :vegetable_category ;
        skos:definition  "Includes vegetables where the stem or stalk portion is consumed, such as asparagus, celery, or rhubarb."@en ;
        skos:prefLabel   "Stem Vegetables"@en .

:000078  rdf:type               :Ingredient ;
        rdfs:seeAlso            "http://www.wikidata.org/entity/Q961769"^^xsd:anyURI ;
        skos:definition         "A creamy, green fruit with a buttery texture, often used in salads, spreads, and various dishes."@en ;
        skos:prefLabel          "Avocado"@en ;
        :hasAroma               :fruity_aroma , :green_aroma , :fatty_aroma , :cucumber_aroma ;
        :hasFunctionalBenefit   :787e979b-4d45-48b4-9f11-6fba2b367924 , :1e883a46-9d0a-4f5a-aa3a-4e75a25e0eba , :e498450d-cced-4a4f-93dd-b3ef3d5e2d43 , :c6e9b1b9-673b-4038-a473-7c57181b9eec , :d1c71bca-dd90-47d3-9f3b-1e214ccaeb85 , :00541d6d-4dc5-4853-98f2-d176c27db355 , :a910f718-6310-459f-976b-6c9c334adfe7 , :aab0922c-eece-44ff-b800-92af6c07f55d , :f964c152-e1b0-4087-b7b9-6be16cec00ab , :1e86605f-2026-4f12-8293-e168aafc11e3 , :be450163-d1fc-4eec-8e1b-ef10c6ddbfe2 ;
        :hasIngredientCategory  :fruit_vegetables ;
        :pairsWith              :000873 , :000141 , :000520 , :000149 , :007109 .

:cucumber_aroma  rdf:type  :Aroma ;
        skos:prefLabel  "Cucumber Aroma"@en ;
        :hasAromaType   :green .

:001394  rdf:type               :Ingredient ;
        rdfs:seeAlso            "http://www.wikidata.org/entity/Q165112"^^xsd:anyURI ;
        skos:definition         "Popcorn is a type of corn that puffs up when heated, resulting in a light and crunchy snack."@en ;
        skos:prefLabel          "Popcorn"@en ;
        :hasAroma               :nutty_aroma , :fatty_aroma , :roasted_aroma , :popcorn_aroma ;
        :hasFunctionalBenefit   :f964c152-e1b0-4087-b7b9-6be16cec00ab , :c6e9b1b9-673b-4038-a473-7c57181b9eec , :a910f718-6310-459f-976b-6c9c334adfe7 , :9521e144-95e4-4171-a421-9a468b1c62e5 , :e498450d-cced-4a4f-93dd-b3ef3d5e2d43 ;
        :hasIngredientCategory  :popcorn ;
        :hasTexture             :crunchy_texture ;
        :pairsWith              :005754 .

:onion_aroma  rdf:type  :Aroma ;
        skos:prefLabel  "Onion Aroma"@en ;
        :hasAromaType   :vegetable .

:Flavour  rdf:type       owl:Class ;
        rdfs:seeAlso     <https://www.foodpairing.com/industry/glossary/definition/flavor/> ;
        skos:definition  "The sensory experience of consuming food and beverages formed by the chemical sensations of taste and smell alongside other sensations like texture."@en ;
        skos:prefLabel   "Flavour"@en .

:pickles  rdf:type       skos:Concept , :IngredientCategory ;
        skos:broader     :condiments_category ;
        skos:definition  "Encompasses preserved vegetables or fruits, often soaked in a brine or vinegar solution to impart a tangy flavor."@en ;
        skos:prefLabel   "Pickles"@en .

:sprouts  rdf:type       skos:Concept , :IngredientCategory ;
        skos:broader     :vegetable_category ;
        skos:definition  "Refers to young, tender shoots or germinated seeds of various vegetables, often used as a fresh ingredient in salads or sandwiches."@en ;
        skos:prefLabel   "Sprouts"@en .

:astringent_trigeminal_taste
        rdf:type        :Trigeminal ;
        skos:prefLabel  "Astringent Trigeminal Taste"@en .

:sour_and_fruity_spices
        rdf:type         skos:Concept , :IngredientCategory ;
        skos:broader     :spice_category ;
        skos:definition  "Encompasses spices with a tangy or fruity flavor, such as tamarind, sumac, or dried berries, used to enhance sweet or savory dishes."@en ;
        skos:prefLabel   "Sour And Fruity Spices"@en .

:000031  rdf:type               :Ingredient ;
        rdfs:seeAlso            "http://www.wikidata.org/entity/Q33913"^^xsd:anyURI ;
        skos:definition         "A fragrant herb with a lemony scent, often used in Asian cuisine to add a citrusy flavor to dishes."@en ;
        skos:prefLabel          "Lemongrass"@en ;
        :hasAroma               :citrus_aroma , :lemon_aroma ;
        :hasFunctionalBenefit   :e3f7dd51-c162-4746-8f72-cababacf8ace , :c6e9b1b9-673b-4038-a473-7c57181b9eec , :9521e144-95e4-4171-a421-9a468b1c62e5 , :c5a4476f-dc4e-417a-a47a-ede2655abb18 , :be450163-d1fc-4eec-8e1b-ef10c6ddbfe2 ;
        :hasIngredientCategory  :culinary_herbs ;
        :pairsWith              :000159 , :000072 , :000840 , :000155 .

:beany_aroma  rdf:type  :Aroma ;
        skos:prefLabel  "Beany Aroma"@en ;
        :hasAromaType   :vegetable .

:non-alcoholic_drink  rdf:type  skos:Concept , :IngredientCategory ;
        skos:broader     :drinks_category ;
        skos:definition  "Includes beverages without alcohol, such as soft drinks, juices, water, coffee, tea, and non-alcoholic cocktails."@en ;
        skos:prefLabel   "Non-alcoholic Drink"@en .

:coffees  rdf:type       skos:Concept , :IngredientCategory ;
        skos:broader     :non-alcoholic_drink ;
        skos:definition  "Includes various coffee products, such as whole beans, ground coffee, instant coffee, and coffee-based beverages."@en ;
        skos:prefLabel   "Coffees"@en .

:hasTexture  rdf:type       owl:ObjectProperty ;
        rdfs:domain         :Ingredient ;
        rdfs:range          :Texture ;
        rdfs:seeAlso        <https://www.foodpairing.com/industry/glossary/definition/texture/> ;
        rdfs:subPropertyOf  :hasFlavour ;
        skos:definition     "Assigns a texture to an ingredient."@en ;
        skos:prefLabel      "has texture"@en .

:000161  rdf:type               :Ingredient ;
        rdfs:seeAlso            "http://www.wikidata.org/entity/Q38645"^^xsd:anyURI ;
        skos:definition         "A juicy and refreshing fruit with a sweet, hydrating taste, commonly eaten fresh."@en ;
        skos:prefLabel          "Watermelon"@en ;
        :hasAroma               :orange_aroma , :caramel_aroma , :fruity_aroma , :cucumber_aroma ;
        :hasFunctionalBenefit   :d1c71bca-dd90-47d3-9f3b-1e214ccaeb85 , :c5a4476f-dc4e-417a-a47a-ede2655abb18 , :e498450d-cced-4a4f-93dd-b3ef3d5e2d43 , :9521e144-95e4-4171-a421-9a468b1c62e5 , :f964c152-e1b0-4087-b7b9-6be16cec00ab , :aab0922c-eece-44ff-b800-92af6c07f55d , :00541d6d-4dc5-4853-98f2-d176c27db355 , :c6e9b1b9-673b-4038-a473-7c57181b9eec , :be450163-d1fc-4eec-8e1b-ef10c6ddbfe2 , :a910f718-6310-459f-976b-6c9c334adfe7 , :1e883a46-9d0a-4f5a-aa3a-4e75a25e0eba ;
        :hasIngredientCategory  :pepo_fruits ;
        :hasTaste               :sweet_taste , :sour_taste ;
        :hasTexture             :juicy_texture , :soft_texture .

:001218  rdf:type               :Ingredient ;
        rdfs:seeAlso            "http://www.wikidata.org/entity/Q13194939"^^xsd:anyURI ;
        skos:definition         "White fish with a mild flavor and flaky texture, commonly used in a variety of culinary dishes."@en ;
        skos:prefLabel          "Cod"@en ;
        :hasFunctionalBenefit   :c5a4476f-dc4e-417a-a47a-ede2655abb18 , :197f7339-d08a-4270-a44e-164cd5146dd4 , :9521e144-95e4-4171-a421-9a468b1c62e5 , :a910f718-6310-459f-976b-6c9c334adfe7 , :d1c71bca-dd90-47d3-9f3b-1e214ccaeb85 , :4b2e9d35-65b8-4a2e-96a4-6436e368f15f , :c6e9b1b9-673b-4038-a473-7c57181b9eec , :aab0922c-eece-44ff-b800-92af6c07f55d , :be450163-d1fc-4eec-8e1b-ef10c6ddbfe2 , :6a1a1d51-dfab-4237-aeac-a9ac4db26486 , :00541d6d-4dc5-4853-98f2-d176c27db355 , :e498450d-cced-4a4f-93dd-b3ef3d5e2d43 , :1e883a46-9d0a-4f5a-aa3a-4e75a25e0eba ;
        :hasIngredientCategory  :fish ;
        :pairsWith              :000101 , :000873 .

:whisky  rdf:type        skos:Concept , :IngredientCategory ;
        skos:broader     :spirits ;
        skos:definition  "Relates to distilled alcoholic beverages made from fermented grain mash, aged in wooden casks, and varying in flavor profiles."@en ;
        skos:prefLabel   "Whisky"@en .

:condiments_category  rdf:type  skos:Concept , :IngredientCategory ;
        skos:definition  "Includes various sauces, dips, spreads, and pickled products used to enhance the flavor of food."@en ;
        skos:prefLabel   "Condiments Category"@en .

:cabbage_aroma  rdf:type  :Aroma ;
        skos:prefLabel  "Cabbage Aroma"@en ;
        :hasAromaType   :vegetable .

:oils   rdf:type         skos:Concept , :IngredientCategory ;
        skos:broader     :fats_and_oils_category ;
        skos:definition  "Includes various liquid fats derived from plants or animals, often used for cooking, frying, and as dressings or flavorings."@en ;
        skos:prefLabel   "Oils"@en .

:spice_mixes  rdf:type   skos:Concept , :IngredientCategory ;
        skos:broader     :spice_category ;
        skos:definition  "Includes blends of different spices and herbs, often used to season various dishes or add flavor to sauces, marinades, or rubs."@en ;
        skos:prefLabel   "Spice Mixes"@en .

:coffee_aroma  rdf:type  :Aroma ;
        skos:prefLabel  "Coffee Aroma"@en ;
        :hasAromaType   :roasted .

:pairsWith  rdf:type    owl:ObjectProperty ;
        rdfs:domain     :Ingredient ;
        rdfs:range      :Ingredient ;
        skos:prefLabel  "pairs with"@en .

:e3f7dd51-c162-4746-8f72-cababacf8ace
        rdf:type         :FunctionalBenefit ;
        skos:definition  "Ingredients or products that may promote better sleep quality and duration." ;
        skos:prefLabel   "Sleep"@en .

:liquors  rdf:type       skos:Concept , :IngredientCategory ;
        skos:broader     :alcoholic_drink ;
        skos:definition  "Encompasses distilled alcoholic beverages with a higher alcohol content, often flavored and consumed in small quantities."@en ;
        skos:prefLabel   "Liquors"@en .

:nut_butter  rdf:type    skos:Concept , :IngredientCategory ;
        skos:broader     :nuts_and_seeds_category ;
        skos:definition  "Encompasses spreads made from ground nuts, such as peanut butter, almond butter, or hazelnut spread."@en ;
        skos:prefLabel   "Nut Butter"@en .

:anise_and_liquorice_spices
        rdf:type         skos:Concept , :IngredientCategory ;
        skos:broader     :spice_category ;
        skos:definition  "Includes spices derived from anise and licorice plants, offering distinctive flavors often used in culinary and confectionery preparations."@en ;
        skos:prefLabel   "Anise And Liquorice Spices"@en .

:iced_tea  rdf:type      skos:Concept , :IngredientCategory ;
        skos:broader     :soft_drinks ;
        skos:definition  "Encompasses chilled tea-based beverages, often served with ice, and may be sweetened or flavored with fruits or herbs."@en ;
        skos:prefLabel   "Iced Tea"@en .

:000157  rdf:type               :Ingredient ;
        rdfs:seeAlso            "http://www.wikidata.org/entity/Q13191"^^xsd:anyURI ;
        skos:definition         "Oranges are round, citrus fruits with a sweet and tangy flavor, commonly eaten fresh or used in juices and desserts."@en ;
        skos:prefLabel          "Orange"@en ;
        :hasAroma               :orange_aroma , :fruity_aroma , :pineapple_aroma ;
        :hasFunctionalBenefit   :00541d6d-4dc5-4853-98f2-d176c27db355 , :9521e144-95e4-4171-a421-9a468b1c62e5 , :a5fee1e7-b975-44b2-b4dc-498e7c295bd4 , :d1c71bca-dd90-47d3-9f3b-1e214ccaeb85 , :a910f718-6310-459f-976b-6c9c334adfe7 , :e3f7dd51-c162-4746-8f72-cababacf8ace , :f964c152-e1b0-4087-b7b9-6be16cec00ab , :197f7339-d08a-4270-a44e-164cd5146dd4 , :e498450d-cced-4a4f-93dd-b3ef3d5e2d43 , :4b2e9d35-65b8-4a2e-96a4-6436e368f15f , :c5a4476f-dc4e-417a-a47a-ede2655abb18 , :c6e9b1b9-673b-4038-a473-7c57181b9eec , :1e883a46-9d0a-4f5a-aa3a-4e75a25e0eba , :aab0922c-eece-44ff-b800-92af6c07f55d , :1e86605f-2026-4f12-8293-e168aafc11e3 , :8d06ddfc-2e8e-4eca-aadb-554cfab5aa6a , :6a1a1d51-dfab-4237-aeac-a9ac4db26486 , :787e979b-4d45-48b4-9f11-6fba2b367924 , :3674c0c7-026a-4337-a10c-bbe4ceff1870 , :be450163-d1fc-4eec-8e1b-ef10c6ddbfe2 ;
        :hasIngredientCategory  :citrus_fruits ;
        :hasTaste               :sour_taste , :sweet_taste ;
        :hasTexture             :juicy_texture ;
        :pairsWith              :000159 , :000148 .

:medicinal_herbs  rdf:type  skos:Concept , :IngredientCategory ;
        skos:broader     :herbs_category ;
        skos:definition  "Refers to herbs used for their potential health benefits or medicinal properties, such as chamomile, echinacea, and ginseng."@en ;
        skos:prefLabel   "Medicinal Herbs"@en .
