<?xml version="1.0"?>
<rdf:RDF xmlns="http://www.foodpairing.com/ontologies/inspire-kg#"
     xml:base="http://www.foodpairing.com/ontologies/inspire-kg"
     xmlns:owl="http://www.w3.org/2002/07/owl#"
     xmlns:rdf="http://www.w3.org/1999/02/22-rdf-syntax-ns#"
     xmlns:xml="http://www.w3.org/XML/1998/namespace"
     xmlns:xsd="http://www.w3.org/2001/XMLSchema#"
     xmlns:rdfs="http://www.w3.org/2000/01/rdf-schema#"
     xmlns:skos="http://www.w3.org/2004/02/skos/core#"
     xmlns:terms="http://purl.org/dc/terms/"
     xmlns:foodpairing-kg="http://www.foodpairing.com/ontologies/foodpairing-kg#">
    <owl:Ontology rdf:about="http://www.foodpairing.com/ontologies/inspire-kg">
        <owl:imports rdf:resource="http://www.w3.org/2004/02/skos/core"/>
        <terms:contributor rdf:resource="https://www.linkedin.com/in/marc-luis-cer%C3%B3n-a73825241/"/>
        <terms:created rdf:datatype="http://www.w3.org/2001/XMLSchema#date">2023-10-10</terms:created>
        <terms:creator rdf:resource="https://www.linkedin.com/in/bernardlahousse/"/>
        <terms:creator rdf:resource="https://www.linkedin.com/in/peter-coucquyt-8922419/"/>
        <terms:creator rdf:resource="https://www.linkedin.com/in/skontopo/"/>
        <terms:description xml:lang="en">The Inspire Knowledge Graph contains (a) 102 food ingredients, (b) a 4-layer taxonomy of 150 ingredient categories, (c) sensory information for the ingredients (aromas, tastes, textures, trigeminals), (d) functional benefits of ingredients, (e) ingredient pairings.</terms:description>
        <terms:license rdf:resource="https://creativecommons.org/licenses/by/4.0/"/>
        <terms:publisher rdf:resource="https://www.foodpairing.com/"/>
        <terms:title xml:lang="en">The Inspire Knowledge Graph</terms:title>
        <rdfs:label xml:lang="en">Inspire KG</rdfs:label>
        <owl:versionInfo>1.0.0</owl:versionInfo>
    </owl:Ontology>
    


    <!-- 
    ///////////////////////////////////////////////////////////////////////////////////////
    //
    // Annotation properties
    //
    ///////////////////////////////////////////////////////////////////////////////////////
     -->


    


    <!-- http://purl.org/dc/terms/created -->


    <owl:AnnotationProperty rdf:about="http://purl.org/dc/terms/created"/>
    


    <!-- http://purl.org/dc/terms/license -->


    <owl:AnnotationProperty rdf:about="http://purl.org/dc/terms/license"/>
    


    <!-- http://purl.org/dc/terms/publisher -->


    <owl:AnnotationProperty rdf:about="http://purl.org/dc/terms/publisher"/>
    


    <!-- 
    ///////////////////////////////////////////////////////////////////////////////////////
    //
    // Datatypes
    //
    ///////////////////////////////////////////////////////////////////////////////////////
     -->


    


    <!-- http://www.w3.org/2001/XMLSchema#date -->


    <rdfs:Datatype rdf:about="http://www.w3.org/2001/XMLSchema#date"/>
    


    <!-- 
    ///////////////////////////////////////////////////////////////////////////////////////
    //
    // Object Properties
    //
    ///////////////////////////////////////////////////////////////////////////////////////
     -->


    


    <!-- http://www.foodpairing.com/ontologies/foodpairing-kg#hasAroma -->


    <owl:ObjectProperty rdf:about="http://www.foodpairing.com/ontologies/foodpairing-kg#hasAroma">
        <rdfs:subPropertyOf rdf:resource="http://www.foodpairing.com/ontologies/foodpairing-kg#hasFlavour"/>
        <rdfs:domain rdf:resource="http://www.foodpairing.com/ontologies/foodpairing-kg#Ingredient"/>
        <rdfs:range rdf:resource="http://www.foodpairing.com/ontologies/foodpairing-kg#Aroma"/>
        <rdfs:seeAlso rdf:resource="https://www.foodpairing.com/industry/glossary/definition/aroma/"/>
        <skos:definition xml:lang="en">Associates an ingredient to an aroma.</skos:definition>
        <skos:prefLabel xml:lang="en">has aroma</skos:prefLabel>
    </owl:ObjectProperty>
    


    <!-- http://www.foodpairing.com/ontologies/foodpairing-kg#hasAromaType -->


    <owl:ObjectProperty rdf:about="http://www.foodpairing.com/ontologies/foodpairing-kg#hasAromaType">
        <rdfs:domain rdf:resource="http://www.foodpairing.com/ontologies/foodpairing-kg#SensoryDescriptor"/>
        <rdfs:range rdf:resource="http://www.foodpairing.com/ontologies/foodpairing-kg#AromaType"/>
        <rdfs:seeAlso rdf:resource="https://www.foodpairing.com/industry/glossary/definition/aroma-types/"/>
        <skos:definition xml:lang="en">Specifies the aroma type of the sensory descriptor.</skos:definition>
        <skos:prefLabel xml:lang="en">has aroma type</skos:prefLabel>
    </owl:ObjectProperty>
    


    <!-- http://www.foodpairing.com/ontologies/foodpairing-kg#hasFlavour -->


    <owl:ObjectProperty rdf:about="http://www.foodpairing.com/ontologies/foodpairing-kg#hasFlavour">
        <rdfs:domain rdf:resource="http://www.foodpairing.com/ontologies/foodpairing-kg#Ingredient"/>
        <rdfs:range rdf:resource="http://www.foodpairing.com/ontologies/foodpairing-kg#Flavour"/>
        <skos:definition xml:lang="en">Associates a flavour to an ingredient. This property is never used; instead, its subproperties are used.</skos:definition>
        <skos:prefLabel xml:lang="en">has flavour</skos:prefLabel>
    </owl:ObjectProperty>
    


    <!-- http://www.foodpairing.com/ontologies/foodpairing-kg#hasFunctionalBenefit -->


    <owl:ObjectProperty rdf:about="http://www.foodpairing.com/ontologies/foodpairing-kg#hasFunctionalBenefit">
        <rdfs:domain rdf:resource="http://www.foodpairing.com/ontologies/foodpairing-kg#Ingredient"/>
        <rdfs:range rdf:resource="http://www.foodpairing.com/ontologies/foodpairing-kg#FunctionalBenefit"/>
        <skos:definition xml:lang="en">Establishes a relationship between a food ingredient and a specific functional benefit.</skos:definition>
        <skos:prefLabel xml:lang="en">has functional benefit</skos:prefLabel>
    </owl:ObjectProperty>
    


    <!-- http://www.foodpairing.com/ontologies/foodpairing-kg#hasIngredient -->


    <owl:ObjectProperty rdf:about="http://www.foodpairing.com/ontologies/foodpairing-kg#hasIngredient">
        <rdfs:domain rdf:resource="http://www.foodpairing.com/ontologies/foodpairing-kg#IngredientPairing"/>
        <rdfs:range rdf:resource="http://www.foodpairing.com/ontologies/foodpairing-kg#Ingredient"/>
        <skos:definition xml:lang="en">Associates an ingredient pairing with one or more ingredients.</skos:definition>
        <skos:prefLabel xml:lang="en">has ingredient</skos:prefLabel>
    </owl:ObjectProperty>
    


    <!-- http://www.foodpairing.com/ontologies/foodpairing-kg#hasIngredientCategory -->


    <owl:ObjectProperty rdf:about="http://www.foodpairing.com/ontologies/foodpairing-kg#hasIngredientCategory">
        <rdfs:domain rdf:resource="http://www.foodpairing.com/ontologies/foodpairing-kg#Ingredient"/>
        <rdfs:range rdf:resource="http://www.foodpairing.com/ontologies/foodpairing-kg#IngredientCategory"/>
        <skos:definition xml:lang="en">Establishes a relationship between an individual ingredient and its corresponding ingredient category. This property serves to categorize and organize ingredients based on their shared attributes, facilitating structured representation and classification within the domain of food knowledge.</skos:definition>
        <skos:prefLabel xml:lang="en">has ingredient category</skos:prefLabel>
    </owl:ObjectProperty>
    


    <!-- http://www.foodpairing.com/ontologies/foodpairing-kg#hasKeyIngredient -->


    <owl:ObjectProperty rdf:about="http://www.foodpairing.com/ontologies/foodpairing-kg#hasKeyIngredient">
        <rdfs:subPropertyOf rdf:resource="http://www.foodpairing.com/ontologies/foodpairing-kg#hasIngredient"/>
        <rdfs:domain rdf:resource="http://www.foodpairing.com/ontologies/foodpairing-kg#IngredientPairing"/>
        <rdfs:range rdf:resource="http://www.foodpairing.com/ontologies/foodpairing-kg#Ingredient"/>
        <skos:definition xml:lang="en">Specifies the key ingredient in an ingredient pairing.</skos:definition>
        <skos:prefLabel xml:lang="en">has key ingredient</skos:prefLabel>
    </owl:ObjectProperty>
    


    <!-- http://www.foodpairing.com/ontologies/foodpairing-kg#hasRelatedIngredient -->


    <owl:ObjectProperty rdf:about="http://www.foodpairing.com/ontologies/foodpairing-kg#hasRelatedIngredient">
        <rdfs:subPropertyOf rdf:resource="http://www.foodpairing.com/ontologies/foodpairing-kg#hasIngredient"/>
        <rdfs:domain rdf:resource="http://www.foodpairing.com/ontologies/foodpairing-kg#IngredientPairing"/>
        <rdfs:range rdf:resource="http://www.foodpairing.com/ontologies/foodpairing-kg#Ingredient"/>
        <skos:definition xml:lang="en">Specifies the related ingredient in an ingredient pairing.</skos:definition>
        <skos:prefLabel xml:lang="en">has related ingredient</skos:prefLabel>
    </owl:ObjectProperty>
    


    <!-- http://www.foodpairing.com/ontologies/foodpairing-kg#hasSensoryDescriptor -->


    <owl:ObjectProperty rdf:about="http://www.foodpairing.com/ontologies/foodpairing-kg#hasSensoryDescriptor">
        <rdfs:domain rdf:resource="http://www.foodpairing.com/ontologies/foodpairing-kg#Flavour"/>
        <rdfs:range rdf:resource="http://www.foodpairing.com/ontologies/foodpairing-kg#SensoryDescriptor"/>
        <skos:definition xml:lang="en">Associates a flavour (aroma, taste, texture, trigeminal) to a sensory descriptor.</skos:definition>
        <skos:prefLabel xml:lang="en">has sensory descriptor</skos:prefLabel>
    </owl:ObjectProperty>
    


    <!-- http://www.foodpairing.com/ontologies/foodpairing-kg#hasTaste -->


    <owl:ObjectProperty rdf:about="http://www.foodpairing.com/ontologies/foodpairing-kg#hasTaste">
        <rdfs:subPropertyOf rdf:resource="http://www.foodpairing.com/ontologies/foodpairing-kg#hasFlavour"/>
        <rdfs:domain rdf:resource="http://www.foodpairing.com/ontologies/foodpairing-kg#Ingredient"/>
        <rdfs:range rdf:resource="http://www.foodpairing.com/ontologies/foodpairing-kg#Taste"/>
        <rdfs:seeAlso rdf:resource="https://www.foodpairing.com/industry/glossary/definition/taste/"/>
        <skos:definition xml:lang="en">Associates an ingredient to a taste.</skos:definition>
        <skos:prefLabel xml:lang="en">has taste</skos:prefLabel>
    </owl:ObjectProperty>
    


    <!-- http://www.foodpairing.com/ontologies/foodpairing-kg#hasTexture -->


    <owl:ObjectProperty rdf:about="http://www.foodpairing.com/ontologies/foodpairing-kg#hasTexture">
        <rdfs:subPropertyOf rdf:resource="http://www.foodpairing.com/ontologies/foodpairing-kg#hasFlavour"/>
        <rdfs:domain rdf:resource="http://www.foodpairing.com/ontologies/foodpairing-kg#Ingredient"/>
        <rdfs:range rdf:resource="http://www.foodpairing.com/ontologies/foodpairing-kg#Texture"/>
        <rdfs:seeAlso rdf:resource="https://www.foodpairing.com/industry/glossary/definition/texture/"/>
        <skos:definition xml:lang="en">Associates an ingredient to a texture.</skos:definition>
        <skos:prefLabel xml:lang="en">has texture</skos:prefLabel>
    </owl:ObjectProperty>
    


    <!-- http://www.foodpairing.com/ontologies/foodpairing-kg#hasTrigeminal -->


    <owl:ObjectProperty rdf:about="http://www.foodpairing.com/ontologies/foodpairing-kg#hasTrigeminal">
        <rdfs:subPropertyOf rdf:resource="http://www.foodpairing.com/ontologies/foodpairing-kg#hasFlavour"/>
        <rdfs:domain rdf:resource="http://www.foodpairing.com/ontologies/foodpairing-kg#Ingredient"/>
        <rdfs:range rdf:resource="http://www.foodpairing.com/ontologies/foodpairing-kg#Trigeminal"/>
        <rdfs:seeAlso rdf:resource="https://www.foodpairing.com/industry/glossary/definition/trigeminal-taste/"/>
        <skos:definition xml:lang="en">Associates an ingredient to a trigeminal taste.</skos:definition>
        <skos:prefLabel xml:lang="en">has trigeminal</skos:prefLabel>
    </owl:ObjectProperty>
    


    <!-- 
    ///////////////////////////////////////////////////////////////////////////////////////
    //
    // Data properties
    //
    ///////////////////////////////////////////////////////////////////////////////////////
     -->


    


    <!-- http://www.foodpairing.com/ontologies/foodpairing-kg#aromaIntensity -->


    <owl:DatatypeProperty rdf:about="http://www.foodpairing.com/ontologies/foodpairing-kg#aromaIntensity">
        <rdfs:domain rdf:resource="http://www.foodpairing.com/ontologies/foodpairing-kg#SensoryDescriptor"/>
        <rdfs:range rdf:resource="http://www.w3.org/2001/XMLSchema#double"/>
        <rdfs:seeAlso rdf:resource="https://www.foodpairing.com/industry/glossary/definition/aroma-intensity-comparison/"/>
        <skos:definition xml:lang="en">Expresses how strongly a certain aroma is perceived by a person, based on Foodpairing benchmarking.</skos:definition>
        <skos:prefLabel xml:lang="en">aroma intensity</skos:prefLabel>
    </owl:DatatypeProperty>
    


    <!-- http://www.foodpairing.com/ontologies/foodpairing-kg#matchScore -->


    <owl:DatatypeProperty rdf:about="http://www.foodpairing.com/ontologies/foodpairing-kg#matchScore">
        <rdfs:domain rdf:resource="http://www.foodpairing.com/ontologies/foodpairing-kg#IngredientPairing"/>
        <rdfs:range rdf:resource="http://www.w3.org/2001/XMLSchema#double"/>
        <rdfs:seeAlso rdf:resource="https://www.foodpairing.com/industry/glossary/definition/matching-score/"/>
        <rdfs:seeAlso rdf:resource="https://www.foodpairing.com/industry/glossary/definition/relative-matching-score/"/>
        <skos:definition xml:lang="en">A metric measuring how well two ingredients match together in an ingredient pairing. It corresponds to the relative matching score of one ingredient with another and is dependent on the highest absolute matching score of a specific ingredient. The absolute matching score is transformed into a percentage relative to the highest absolute score for that specific product. The matching score in the Foodpairing® Flavor Database is a relative matching score. The best matching ingredient of the Foodpairing® Flavor Database for a customer product has a 100% match. The matching score of the other ingredients is relative to the aroma score of the best matching ingredient.</skos:definition>
        <skos:prefLabel xml:lang="en">Foodpairing match score</skos:prefLabel>
    </owl:DatatypeProperty>
    


    <!-- http://www.foodpairing.com/ontologies/foodpairing-kg#sensoryValue -->


    <owl:DatatypeProperty rdf:about="http://www.foodpairing.com/ontologies/foodpairing-kg#sensoryValue">
        <rdfs:domain rdf:resource="http://www.foodpairing.com/ontologies/foodpairing-kg#Flavour"/>
        <rdfs:range>
            <rdfs:Datatype>
                <owl:unionOf rdf:parseType="Collection">
                    <rdf:Description rdf:about="http://www.w3.org/2001/XMLSchema#boolean"/>
                    <rdf:Description rdf:about="http://www.w3.org/2001/XMLSchema#double"/>
                </owl:unionOf>
            </rdfs:Datatype>
        </rdfs:range>
        <skos:definition xml:lang="en">Represents the &apos;raw&apos; sensory value for certain descriptors.</skos:definition>
        <skos:prefLabel xml:lang="en">sensory value</skos:prefLabel>
    </owl:DatatypeProperty>
    


    <!-- 
    ///////////////////////////////////////////////////////////////////////////////////////
    //
    // Classes
    //
    ///////////////////////////////////////////////////////////////////////////////////////
     -->


    


    <!-- http://www.foodpairing.com/ontologies/foodpairing-kg#Aroma -->


    <owl:Class rdf:about="http://www.foodpairing.com/ontologies/foodpairing-kg#Aroma">
        <rdfs:subClassOf rdf:resource="http://www.foodpairing.com/ontologies/foodpairing-kg#Flavour"/>
        <rdfs:seeAlso rdf:resource="https://www.foodpairing.com/industry/glossary/definition/aroma/"/>
        <skos:definition xml:lang="en">Aromas are the odorants or smells present in a food product. Aroma molecules are perceived through the mouth and the nose and are translated by our olfactory system. Aroma defines on average 80% of our flavor experience.</skos:definition>
        <skos:prefLabel xml:lang="en">Aroma</skos:prefLabel>
    </owl:Class>
    


    <!-- http://www.foodpairing.com/ontologies/foodpairing-kg#AromaType -->


    <owl:Class rdf:about="http://www.foodpairing.com/ontologies/foodpairing-kg#AromaType">
        <rdfs:seeAlso rdf:resource="https://www.foodpairing.com/industry/glossary/definition/aroma-types/"/>
        <skos:definition xml:lang="en">The aroma types represent the key odorants in the aroma profile of a customer product. There are 14 standard aroma types that can be found, e.g. fruity, floral, spicy, green, roasted, etc. Each of the aroma types are further defined by different aroma descriptors, e.g fruity-coconut or vegetable-potato.</skos:definition>
        <skos:prefLabel xml:lang="en">Aroma Type</skos:prefLabel>
    </owl:Class>
    


    <!-- http://www.foodpairing.com/ontologies/foodpairing-kg#Flavour -->


    <owl:Class rdf:about="http://www.foodpairing.com/ontologies/foodpairing-kg#Flavour">
        <rdfs:seeAlso rdf:resource="https://www.foodpairing.com/industry/glossary/definition/flavor/"/>
        <skos:definition xml:lang="en">The sensory experience of consuming food and beverages formed by the chemical sensations of taste and smell alongside other sensations like texture.</skos:definition>
        <skos:prefLabel xml:lang="en">Flavour</skos:prefLabel>
    </owl:Class>
    


    <!-- http://www.foodpairing.com/ontologies/foodpairing-kg#FunctionalBenefit -->


    <owl:Class rdf:about="http://www.foodpairing.com/ontologies/foodpairing-kg#FunctionalBenefit">
        <skos:definition xml:lang="en">Represents the effects or advantages that a food ingredient or product provides beyond basic nutrition. These benefits may include specific health-promoting properties, culinary enhancements, or other functional attributes that contribute to overall well-being or enhance the overall quality of a food item.</skos:definition>
        <skos:prefLabel xml:lang="en">Functional Benefit</skos:prefLabel>
    </owl:Class>
    


    <!-- http://www.foodpairing.com/ontologies/foodpairing-kg#Ingredient -->


    <owl:Class rdf:about="http://www.foodpairing.com/ontologies/foodpairing-kg#Ingredient">
        <rdfs:seeAlso rdf:resource="https://www.foodpairing.com/industry/glossary/definition/ingredient/"/>
        <skos:definition xml:lang="en">An ingredient is an individual food entity or elaboration thereof (e.g. apple &amp; apple jam).</skos:definition>
        <skos:prefLabel xml:lang="en">Ingredient</skos:prefLabel>
    </owl:Class>
    


    <!-- http://www.foodpairing.com/ontologies/foodpairing-kg#IngredientCategory -->


    <owl:Class rdf:about="http://www.foodpairing.com/ontologies/foodpairing-kg#IngredientCategory">
        <skos:definition xml:lang="en">An ingredient category is a broad classification of related food components based on shared characteristics, used for organizing and understanding various ingredients in culinary and nutritional contexts.</skos:definition>
        <skos:prefLabel xml:lang="en">Ingredient Category</skos:prefLabel>
    </owl:Class>
    


    <!-- http://www.foodpairing.com/ontologies/foodpairing-kg#IngredientPairing -->


    <owl:Class rdf:about="http://www.foodpairing.com/ontologies/foodpairing-kg#IngredientPairing">
        <rdfs:seeAlso rdf:resource="https://www.foodpairing.com/industry/glossary/definition/foodpairing-match/"/>
        <skos:definition xml:lang="en">A pairing between two ingredients that share one or more key aroma molecules. The pairing has a key ingredient and a related ingredient.</skos:definition>
        <skos:prefLabel xml:lang="en">Ingredient Pairing</skos:prefLabel>
    </owl:Class>
    


    <!-- http://www.foodpairing.com/ontologies/foodpairing-kg#SensoryDescriptor -->


    <owl:Class rdf:about="http://www.foodpairing.com/ontologies/foodpairing-kg#SensoryDescriptor">
        <rdfs:seeAlso rdf:resource="https://www.foodpairing.com/industry/glossary/definition/sensory-descriptor/"/>
        <skos:definition xml:lang="en">A sensory descriptor is a label used to describe a specific sensory property of an ingredient. We differentiate between 4 types: (a) Aroma descriptors contain properties like &apos;almond&apos;, &apos;cherry&apos; and &apos;mustard&apos;; (b) Texture descriptors contain properties like &apos;crunchy&apos;, &apos;hard&apos; and &apos;gooey&apos;; (c) Taste descriptors contain the five basic tastes &apos;salt&apos;, &apos;sour&apos;, &apos;sweet&apos;, &apos;bitter&apos;, and &apos;umami&apos; and three additional descriptors &apos;fatty&apos; (or &apos;oleogustus&apos;), &apos;astringent&apos;, and &apos;pungent&apos;; (d) Trigeminal taste descriptors contain taste sensations &apos;astringent&apos;, &apos;pungent&apos;, &apos;cooling&apos; and &apos;tingling&apos;.</skos:definition>
        <skos:prefLabel xml:lang="en">Sensory Descriptor</skos:prefLabel>
    </owl:Class>
    


    <!-- http://www.foodpairing.com/ontologies/foodpairing-kg#Taste -->


    <owl:Class rdf:about="http://www.foodpairing.com/ontologies/foodpairing-kg#Taste">
        <rdfs:subClassOf rdf:resource="http://www.foodpairing.com/ontologies/foodpairing-kg#Flavour"/>
        <rdfs:seeAlso rdf:resource="https://www.foodpairing.com/industry/glossary/definition/taste/"/>
        <skos:definition xml:lang="en">Taste is the perception produced or stimulated when a substance in the mouth reacts chemically with taste receptor cells located on taste buds in the oral cavity, mostly on the tongue. Taste, along with olfaction and trigeminal nerve stimulation (registering texture, pain, and temperature), determines flavors of food and other substances. A taste is how the taste buds experience the 5 taste types - sweet, sour, bitter, salty and umami. Additional descriptors pungent, astringent and fatty also apply. A food is usually a blend of tastes, each in different concentrations.</skos:definition>
        <skos:prefLabel xml:lang="en">Taste</skos:prefLabel>
    </owl:Class>
    


    <!-- http://www.foodpairing.com/ontologies/foodpairing-kg#Texture -->


    <owl:Class rdf:about="http://www.foodpairing.com/ontologies/foodpairing-kg#Texture">
        <rdfs:subClassOf rdf:resource="http://www.foodpairing.com/ontologies/foodpairing-kg#Flavour"/>
        <rdfs:seeAlso rdf:resource="https://www.foodpairing.com/industry/glossary/definition/texture/"/>
        <skos:definition xml:lang="en">Textures are the qualities of a food item that can be sensed through touch; i.e. the degree to which something is rough or smooth, or soft or hard.</skos:definition>
        <skos:prefLabel xml:lang="en">Texture</skos:prefLabel>
    </owl:Class>
    


    <!-- http://www.foodpairing.com/ontologies/foodpairing-kg#Trigeminal -->


    <owl:Class rdf:about="http://www.foodpairing.com/ontologies/foodpairing-kg#Trigeminal">
        <rdfs:subClassOf rdf:resource="http://www.foodpairing.com/ontologies/foodpairing-kg#Flavour"/>
        <rdfs:seeAlso rdf:resource="https://www.foodpairing.com/industry/glossary/definition/trigeminal-taste/"/>
        <skos:definition xml:lang="en">Trigeminal taste (“other tastes”) are a set of tastes which are perceived as triggers sent to the brain via the trigeminal nerve, creating the conscious perception of touch-position and pain-temperature information. Trigeminal sensations are often associated with compounds found in certain foods; menthol for cooling is found in mint, spilanthol comes from a variety of plants, causing a tingling effect on the tongue (think wine and green tea) and capsaicin in chilies is what gives them their signature spiciness.</skos:definition>
        <skos:prefLabel xml:lang="en">Trigeminal</skos:prefLabel>
    </owl:Class>
    


    <!-- 
    ///////////////////////////////////////////////////////////////////////////////////////
    //
    // Individuals
    //
    ///////////////////////////////////////////////////////////////////////////////////////
     -->


    


    <!-- http://www.foodpairing.com/ontologies/foodpairing-kg#Ageing -->


    <owl:NamedIndividual rdf:about="http://www.foodpairing.com/ontologies/foodpairing-kg#Ageing">
        <rdf:type rdf:resource="http://www.foodpairing.com/ontologies/foodpairing-kg#FunctionalBenefit"/>
        <skos:definition>Functional benefits related to aging focus on ingredients or products that may support healthy aging, including skin health and cognitive function.</skos:definition>
        <skos:prefLabel xml:lang="en">Ageing</skos:prefLabel>
    </owl:NamedIndividual>
    


    <!-- http://www.foodpairing.com/ontologies/foodpairing-kg#Antibacterial -->


    <owl:NamedIndividual rdf:about="http://www.foodpairing.com/ontologies/foodpairing-kg#Antibacterial">
        <rdf:type rdf:resource="http://www.foodpairing.com/ontologies/foodpairing-kg#FunctionalBenefit"/>
        <skos:definition>Functional benefits related to antibacterial properties involve ingredients or products that help combat harmful bacteria.</skos:definition>
        <skos:prefLabel xml:lang="en">Antibacterial</skos:prefLabel>
    </owl:NamedIndividual>
    


    <!-- http://www.foodpairing.com/ontologies/foodpairing-kg#Antioxidant -->


    <owl:NamedIndividual rdf:about="http://www.foodpairing.com/ontologies/foodpairing-kg#Antioxidant">
        <rdf:type rdf:resource="http://www.foodpairing.com/ontologies/foodpairing-kg#FunctionalBenefit"/>
        <skos:definition>Antioxidants help protect cells from damage caused by free radicals, which can contribute to aging and various diseases.</skos:definition>
        <skos:prefLabel xml:lang="en">Antioxidant</skos:prefLabel>
    </owl:NamedIndividual>
    


    <!-- http://www.foodpairing.com/ontologies/foodpairing-kg#Aromatherapy -->


    <owl:NamedIndividual rdf:about="http://www.foodpairing.com/ontologies/foodpairing-kg#Aromatherapy">
        <rdf:type rdf:resource="http://www.foodpairing.com/ontologies/foodpairing-kg#FunctionalBenefit"/>
        <skos:definition>Functional benefits of aromatherapy involve the use of aromatic compounds from plants to promote relaxation, well-being, and mental clarity.</skos:definition>
        <skos:prefLabel xml:lang="en">Aromatherapy</skos:prefLabel>
    </owl:NamedIndividual>
    


    <!-- http://www.foodpairing.com/ontologies/foodpairing-kg#Bone -->


    <owl:NamedIndividual rdf:about="http://www.foodpairing.com/ontologies/foodpairing-kg#Bone">
        <rdf:type rdf:resource="http://www.foodpairing.com/ontologies/foodpairing-kg#FunctionalBenefit"/>
        <skos:definition>Involve ingredients or products that support the development and maintenance of strong bones.</skos:definition>
        <skos:prefLabel xml:lang="en">Bone</skos:prefLabel>
    </owl:NamedIndividual>
    


    <!-- http://www.foodpairing.com/ontologies/foodpairing-kg#Brain -->


    <owl:NamedIndividual rdf:about="http://www.foodpairing.com/ontologies/foodpairing-kg#Brain">
        <rdf:type rdf:resource="http://www.foodpairing.com/ontologies/foodpairing-kg#FunctionalBenefit"/>
        <skos:definition>Functional benefits for the brain are properties that support cognitive function, memory, and overall mental well-being.</skos:definition>
        <skos:prefLabel xml:lang="en">Brain</skos:prefLabel>
    </owl:NamedIndividual>
    


    <!-- http://www.foodpairing.com/ontologies/foodpairing-kg#Calcium-source -->


    <owl:NamedIndividual rdf:about="http://www.foodpairing.com/ontologies/foodpairing-kg#Calcium-source">
        <rdf:type rdf:resource="http://www.foodpairing.com/ontologies/foodpairing-kg#FunctionalBenefit"/>
        <skos:definition>Ingredients that provide a significant amount of calcium, vital for bone health.</skos:definition>
        <skos:prefLabel xml:lang="en">Calcium-source</skos:prefLabel>
    </owl:NamedIndividual>
    


    <!-- http://www.foodpairing.com/ontologies/foodpairing-kg#Cardiovascular -->


    <owl:NamedIndividual rdf:about="http://www.foodpairing.com/ontologies/foodpairing-kg#Cardiovascular">
        <rdf:type rdf:resource="http://www.foodpairing.com/ontologies/foodpairing-kg#FunctionalBenefit"/>
        <skos:definition>Functional benefits for cardiovascular health support the heart and circulatory system, reducing the risk of heart-related conditions.</skos:definition>
        <skos:prefLabel xml:lang="en">Cardiovascular</skos:prefLabel>
    </owl:NamedIndividual>
    


    <!-- http://www.foodpairing.com/ontologies/foodpairing-kg#Diabetic -->


    <owl:NamedIndividual rdf:about="http://www.foodpairing.com/ontologies/foodpairing-kg#Diabetic">
        <rdf:type rdf:resource="http://www.foodpairing.com/ontologies/foodpairing-kg#FunctionalBenefit"/>
        <skos:definition>Ingredients or products that can help regulate blood sugar levels.</skos:definition>
        <skos:prefLabel xml:lang="en">Diabetic</skos:prefLabel>
    </owl:NamedIndividual>
    


    <!-- http://www.foodpairing.com/ontologies/foodpairing-kg#Digestion -->


    <owl:NamedIndividual rdf:about="http://www.foodpairing.com/ontologies/foodpairing-kg#Digestion">
        <rdf:type rdf:resource="http://www.foodpairing.com/ontologies/foodpairing-kg#FunctionalBenefit"/>
        <skos:definition>Involve ingredients or products that aid in the breakdown and absorption of nutrients in the digestive tract.</skos:definition>
        <skos:prefLabel xml:lang="en">Digestion</skos:prefLabel>
    </owl:NamedIndividual>
    


    <!-- http://www.foodpairing.com/ontologies/foodpairing-kg#Energy -->


    <owl:NamedIndividual rdf:about="http://www.foodpairing.com/ontologies/foodpairing-kg#Energy">
        <rdf:type rdf:resource="http://www.foodpairing.com/ontologies/foodpairing-kg#FunctionalBenefit"/>
        <skos:definition>Ingredients or products with energy-related functional benefits provide a source of sustenance and vitality for the body.</skos:definition>
        <skos:prefLabel xml:lang="en">Energy</skos:prefLabel>
    </owl:NamedIndividual>
    


    <!-- http://www.foodpairing.com/ontologies/foodpairing-kg#Immunity -->


    <owl:NamedIndividual rdf:about="http://www.foodpairing.com/ontologies/foodpairing-kg#Immunity">
        <rdf:type rdf:resource="http://www.foodpairing.com/ontologies/foodpairing-kg#FunctionalBenefit"/>
        <skos:definition>Functional benefits for immunity involve ingredients or products that support the body&apos;s ability to defend against illnesses and infections.</skos:definition>
        <skos:prefLabel xml:lang="en">Immunity</skos:prefLabel>
    </owl:NamedIndividual>
    


    <!-- http://www.foodpairing.com/ontologies/foodpairing-kg#Minerals -->


    <owl:NamedIndividual rdf:about="http://www.foodpairing.com/ontologies/foodpairing-kg#Minerals">
        <rdf:type rdf:resource="http://www.foodpairing.com/ontologies/foodpairing-kg#FunctionalBenefit"/>
        <skos:definition>Functional benefits related to minerals focus on ingredients that provide essential minerals necessary for various bodily functions.</skos:definition>
        <skos:prefLabel xml:lang="en">Minerals</skos:prefLabel>
    </owl:NamedIndividual>
    


    <!-- http://www.foodpairing.com/ontologies/foodpairing-kg#Muscle-gain -->


    <owl:NamedIndividual rdf:about="http://www.foodpairing.com/ontologies/foodpairing-kg#Muscle-gain">
        <rdf:type rdf:resource="http://www.foodpairing.com/ontologies/foodpairing-kg#FunctionalBenefit"/>
        <skos:definition>Functional benefits for muscle gain involve ingredients or products that support the development and maintenance of lean muscle mass.</skos:definition>
        <skos:prefLabel xml:lang="en">Muscle-gain</skos:prefLabel>
    </owl:NamedIndividual>
    


    <!-- http://www.foodpairing.com/ontologies/foodpairing-kg#Nervous-system -->


    <owl:NamedIndividual rdf:about="http://www.foodpairing.com/ontologies/foodpairing-kg#Nervous-system">
        <rdf:type rdf:resource="http://www.foodpairing.com/ontologies/foodpairing-kg#FunctionalBenefit"/>
        <skos:definition>Involve ingredients or products that support healthy nerve function and transmission.</skos:definition>
        <skos:prefLabel xml:lang="en">Nervous-system</skos:prefLabel>
    </owl:NamedIndividual>
    


    <!-- http://www.foodpairing.com/ontologies/foodpairing-kg#Prebiotic -->


    <owl:NamedIndividual rdf:about="http://www.foodpairing.com/ontologies/foodpairing-kg#Prebiotic">
        <rdf:type rdf:resource="http://www.foodpairing.com/ontologies/foodpairing-kg#FunctionalBenefit"/>
        <skos:definition>Prebiotics are dietary fibers that nourish beneficial gut bacteria, supporting a healthy digestive system.</skos:definition>
        <skos:prefLabel xml:lang="en">Prebiotic</skos:prefLabel>
    </owl:NamedIndividual>
    


    <!-- http://www.foodpairing.com/ontologies/foodpairing-kg#Probiotic -->


    <owl:NamedIndividual rdf:about="http://www.foodpairing.com/ontologies/foodpairing-kg#Probiotic">
        <rdf:type rdf:resource="http://www.foodpairing.com/ontologies/foodpairing-kg#FunctionalBenefit"/>
        <skos:definition>Probiotics are live microorganisms that provide health benefits when consumed, particularly in aiding digestion and supporting a healthy gut microbiome.</skos:definition>
        <skos:prefLabel xml:lang="en">Probiotic</skos:prefLabel>
    </owl:NamedIndividual>
    


    <!-- http://www.foodpairing.com/ontologies/foodpairing-kg#Satiety -->


    <owl:NamedIndividual rdf:about="http://www.foodpairing.com/ontologies/foodpairing-kg#Satiety">
        <rdf:type rdf:resource="http://www.foodpairing.com/ontologies/foodpairing-kg#FunctionalBenefit"/>
        <skos:definition>Ingredients or products with satiety-related functional benefits help promote feelings of fullness and satisfaction after eating.</skos:definition>
        <skos:prefLabel xml:lang="en">Satiety</skos:prefLabel>
    </owl:NamedIndividual>
    


    <!-- http://www.foodpairing.com/ontologies/foodpairing-kg#Skin-health -->


    <owl:NamedIndividual rdf:about="http://www.foodpairing.com/ontologies/foodpairing-kg#Skin-health">
        <rdf:type rdf:resource="http://www.foodpairing.com/ontologies/foodpairing-kg#FunctionalBenefit"/>
        <skos:definition>Functional benefits for skin health involve ingredients or products that promote a healthy complexion and address skin-related issues.</skos:definition>
        <skos:prefLabel xml:lang="en">Skin-health</skos:prefLabel>
    </owl:NamedIndividual>
    


    <!-- http://www.foodpairing.com/ontologies/foodpairing-kg#Sleep -->


    <owl:NamedIndividual rdf:about="http://www.foodpairing.com/ontologies/foodpairing-kg#Sleep">
        <rdf:type rdf:resource="http://www.foodpairing.com/ontologies/foodpairing-kg#FunctionalBenefit"/>
        <skos:definition>Ingredients or products that may promote better sleep quality and duration.</skos:definition>
        <skos:prefLabel xml:lang="en">Sleep</skos:prefLabel>
    </owl:NamedIndividual>
    


    <!-- http://www.foodpairing.com/ontologies/foodpairing-kg#Stress -->


    <owl:NamedIndividual rdf:about="http://www.foodpairing.com/ontologies/foodpairing-kg#Stress">
        <rdf:type rdf:resource="http://www.foodpairing.com/ontologies/foodpairing-kg#FunctionalBenefit"/>
        <skos:definition>Ingredients or products that may help reduce or manage stress levels in the body.</skos:definition>
        <skos:prefLabel xml:lang="en">Stress</skos:prefLabel>
    </owl:NamedIndividual>
    


    <!-- http://www.foodpairing.com/ontologies/foodpairing-kg#Vitamins -->


    <owl:NamedIndividual rdf:about="http://www.foodpairing.com/ontologies/foodpairing-kg#Vitamins">
        <rdf:type rdf:resource="http://www.foodpairing.com/ontologies/foodpairing-kg#FunctionalBenefit"/>
        <skos:definition>Functional benefits related to vitamins involve ingredients that are rich in essential vitamins necessary for overall health.</skos:definition>
        <skos:prefLabel xml:lang="en">Vitamins</skos:prefLabel>
    </owl:NamedIndividual>
    


    <!-- http://www.foodpairing.com/ontologies/foodpairing-kg#Weight-gain -->


    <owl:NamedIndividual rdf:about="http://www.foodpairing.com/ontologies/foodpairing-kg#Weight-gain">
        <rdf:type rdf:resource="http://www.foodpairing.com/ontologies/foodpairing-kg#FunctionalBenefit"/>
        <skos:definition>Ingredients or products that may assist in increasing body mass and muscle.</skos:definition>
        <skos:prefLabel xml:lang="en">Weight-gain</skos:prefLabel>
    </owl:NamedIndividual>
    


    <!-- http://www.foodpairing.com/ontologies/foodpairing-kg#Weight-loss -->


    <owl:NamedIndividual rdf:about="http://www.foodpairing.com/ontologies/foodpairing-kg#Weight-loss">
        <rdf:type rdf:resource="http://www.foodpairing.com/ontologies/foodpairing-kg#FunctionalBenefit"/>
        <skos:definition>Functional benefits for weight-loss involve ingredients or products that may aid in achieving and maintaining a healthy weight.</skos:definition>
        <skos:prefLabel xml:lang="en">Weight-loss</skos:prefLabel>
    </owl:NamedIndividual>
    


    <!-- http://www.foodpairing.com/ontologies/foodpairing-kg#000013 -->


    <owl:NamedIndividual rdf:about="http://www.foodpairing.com/ontologies/foodpairing-kg#000013">
        <rdf:type rdf:resource="http://www.foodpairing.com/ontologies/foodpairing-kg#Ingredient"/>
        <foodpairing-kg:hasIngredientCategory rdf:resource="http://www.foodpairing.com/ontologies/foodpairing-kg#icat:000052"/>
        <rdfs:seeAlso rdf:datatype="http://www.w3.org/2001/XMLSchema#anyURI">http://www.wikidata.org/entity/Q13317</rdfs:seeAlso>
        <skos:definition xml:lang="en">Dairy product with a high fat content, providing a creamy texture and rich flavor.</skos:definition>
        <skos:prefLabel xml:lang="en">Full-fat Yogurt</skos:prefLabel>
    </owl:NamedIndividual>
    


    <!-- http://www.foodpairing.com/ontologies/foodpairing-kg#000014 -->


    <owl:NamedIndividual rdf:about="http://www.foodpairing.com/ontologies/foodpairing-kg#000014">
        <rdf:type rdf:resource="http://www.foodpairing.com/ontologies/foodpairing-kg#Ingredient"/>
        <foodpairing-kg:hasIngredientCategory rdf:resource="http://www.foodpairing.com/ontologies/foodpairing-kg#icat:000007"/>
        <rdfs:seeAlso rdf:datatype="http://www.w3.org/2001/XMLSchema#anyURI">http://www.wikidata.org/entity/Q1062531</rdfs:seeAlso>
        <skos:definition xml:lang="en">An egg that has been cooked in boiling water, resulting in a firm white and a partially solid yolk.</skos:definition>
        <skos:prefLabel xml:lang="en">Boiled Egg</skos:prefLabel>
    </owl:NamedIndividual>
    


    <!-- http://www.foodpairing.com/ontologies/foodpairing-kg#000017 -->


    <owl:NamedIndividual rdf:about="http://www.foodpairing.com/ontologies/foodpairing-kg#000017">
        <rdf:type rdf:resource="http://www.foodpairing.com/ontologies/foodpairing-kg#Ingredient"/>
        <foodpairing-kg:hasIngredientCategory rdf:resource="http://www.foodpairing.com/ontologies/foodpairing-kg#icat:000129"/>
        <rdfs:seeAlso rdf:datatype="http://www.w3.org/2001/XMLSchema#anyURI">http://www.wikidata.org/entity/Q20638126</rdfs:seeAlso>
        <skos:definition xml:lang="en">A red, yellowish, green, or even purple fruit with a juicy pulp, commonly used in salads, sauces, and various culinary dishes.</skos:definition>
        <skos:prefLabel xml:lang="en">Tomato</skos:prefLabel>
    </owl:NamedIndividual>
    


    <!-- http://www.foodpairing.com/ontologies/foodpairing-kg#000021 -->


    <owl:NamedIndividual rdf:about="http://www.foodpairing.com/ontologies/foodpairing-kg#000021">
        <rdf:type rdf:resource="http://www.foodpairing.com/ontologies/foodpairing-kg#Ingredient"/>
        <foodpairing-kg:hasIngredientCategory rdf:resource="http://www.foodpairing.com/ontologies/foodpairing-kg#icat:000040"/>
        <rdfs:seeAlso rdf:datatype="http://www.w3.org/2001/XMLSchema#anyURI">http://www.wikidata.org/entity/Q545985</rdfs:seeAlso>
        <skos:definition xml:lang="en">Pungent condiment made from fermented fish, commonly used in Southeast Asian cuisine for its savory flavor.</skos:definition>
        <skos:prefLabel xml:lang="en">Fish Sauce</skos:prefLabel>
    </owl:NamedIndividual>
    


    <!-- http://www.foodpairing.com/ontologies/foodpairing-kg#000030 -->


    <owl:NamedIndividual rdf:about="http://www.foodpairing.com/ontologies/foodpairing-kg#000030">
        <rdf:type rdf:resource="http://www.foodpairing.com/ontologies/foodpairing-kg#Ingredient"/>
        <foodpairing-kg:hasIngredientCategory rdf:resource="http://www.foodpairing.com/ontologies/foodpairing-kg#icat:000115"/>
        <rdfs:seeAlso rdf:datatype="http://www.w3.org/2001/XMLSchema#anyURI">http://www.wikidata.org/entity/Q15046077</rdfs:seeAlso>
        <skos:definition xml:lang="en">A spicy and aromatic root commonly used in cooking and known for its distinctive flavor.</skos:definition>
        <skos:prefLabel xml:lang="en">Ginger</skos:prefLabel>
    </owl:NamedIndividual>
    


    <!-- http://www.foodpairing.com/ontologies/foodpairing-kg#000031 -->


    <owl:NamedIndividual rdf:about="http://www.foodpairing.com/ontologies/foodpairing-kg#000031">
        <rdf:type rdf:resource="http://www.foodpairing.com/ontologies/foodpairing-kg#Ingredient"/>
        <foodpairing-kg:hasIngredientCategory rdf:resource="http://www.foodpairing.com/ontologies/foodpairing-kg#icat:000094"/>
        <rdfs:seeAlso rdf:datatype="http://www.w3.org/2001/XMLSchema#anyURI">http://www.wikidata.org/entity/Q33913</rdfs:seeAlso>
        <skos:definition xml:lang="en">A fragrant herb with a lemony scent, often used in Asian cuisine to add a citrusy flavor to dishes.</skos:definition>
        <skos:prefLabel xml:lang="en">Lemongrass</skos:prefLabel>
    </owl:NamedIndividual>
    


    <!-- http://www.foodpairing.com/ontologies/foodpairing-kg#000040 -->


    <owl:NamedIndividual rdf:about="http://www.foodpairing.com/ontologies/foodpairing-kg#000040">
        <rdf:type rdf:resource="http://www.foodpairing.com/ontologies/foodpairing-kg#Ingredient"/>
        <foodpairing-kg:hasIngredientCategory rdf:resource="http://www.foodpairing.com/ontologies/foodpairing-kg#icat:000040"/>
        <rdfs:seeAlso rdf:datatype="http://www.w3.org/2001/XMLSchema#anyURI">http://www.wikidata.org/entity/Q131748</rdfs:seeAlso>
        <skos:definition xml:lang="en">Pungent condiment made from ground mustard seeds, commonly used to add flavor and heat to dishes.</skos:definition>
        <skos:prefLabel xml:lang="en">Mustard</skos:prefLabel>
    </owl:NamedIndividual>
    


    <!-- http://www.foodpairing.com/ontologies/foodpairing-kg#000046 -->


    <owl:NamedIndividual rdf:about="http://www.foodpairing.com/ontologies/foodpairing-kg#000046">
        <rdf:type rdf:resource="http://www.foodpairing.com/ontologies/foodpairing-kg#Ingredient"/>
        <foodpairing-kg:hasIngredientCategory rdf:resource="http://www.foodpairing.com/ontologies/foodpairing-kg#icat:000131"/>
        <rdfs:seeAlso rdf:datatype="http://www.w3.org/2001/XMLSchema#anyURI">http://www.wikidata.org/entity/Q104248689</rdfs:seeAlso>
        <skos:definition xml:lang="en">Edible fungi with a mild flavor and smooth texture, often used in cooking.</skos:definition>
        <skos:prefLabel xml:lang="en">Champignon Mushroom</skos:prefLabel>
    </owl:NamedIndividual>
    


    <!-- http://www.foodpairing.com/ontologies/foodpairing-kg#000047 -->


    <owl:NamedIndividual rdf:about="http://www.foodpairing.com/ontologies/foodpairing-kg#000047">
        <rdf:type rdf:resource="http://www.foodpairing.com/ontologies/foodpairing-kg#Ingredient"/>
        <foodpairing-kg:hasIngredientCategory rdf:resource="http://www.foodpairing.com/ontologies/foodpairing-kg#icat:000127"/>
        <rdfs:seeAlso rdf:datatype="http://www.w3.org/2001/XMLSchema#anyURI">http://www.wikidata.org/entity/Q21546392</rdfs:seeAlso>
        <skos:definition xml:lang="en">A pungent bulbous plant used for its aromatic and flavor-enhancing properties in various cuisines.</skos:definition>
        <skos:prefLabel xml:lang="en">Garlic</skos:prefLabel>
    </owl:NamedIndividual>
    


    <!-- http://www.foodpairing.com/ontologies/foodpairing-kg#000055 -->


    <owl:NamedIndividual rdf:about="http://www.foodpairing.com/ontologies/foodpairing-kg#000055">
        <rdf:type rdf:resource="http://www.foodpairing.com/ontologies/foodpairing-kg#Ingredient"/>
        <foodpairing-kg:hasIngredientCategory rdf:resource="http://www.foodpairing.com/ontologies/foodpairing-kg#icat:000104"/>
        <rdfs:seeAlso rdf:datatype="http://www.w3.org/2001/XMLSchema#anyURI">http://www.wikidata.org/entity/Q23374</rdfs:seeAlso>
        <skos:definition xml:lang="en">Spicy sausage made from ground pork and chili peppers, commonly used in Spanish and Mexican dishes.</skos:definition>
        <skos:prefLabel xml:lang="en">Chorizo</skos:prefLabel>
    </owl:NamedIndividual>
    


    <!-- http://www.foodpairing.com/ontologies/foodpairing-kg#000059 -->


    <owl:NamedIndividual rdf:about="http://www.foodpairing.com/ontologies/foodpairing-kg#000059">
        <rdf:type rdf:resource="http://www.foodpairing.com/ontologies/foodpairing-kg#Ingredient"/>
        <foodpairing-kg:hasIngredientCategory rdf:resource="http://www.foodpairing.com/ontologies/foodpairing-kg#icat:000128"/>
        <rdfs:seeAlso rdf:datatype="http://www.w3.org/2001/XMLSchema#anyURI">http://www.wikidata.org/entity/Q23900272</rdfs:seeAlso>
        <skos:definition xml:lang="en">A cruciferous vegetable known for its mild flavor and versatility in cooking.</skos:definition>
        <skos:prefLabel xml:lang="en">Cauliflower</skos:prefLabel>
    </owl:NamedIndividual>
    


    <!-- http://www.foodpairing.com/ontologies/foodpairing-kg#000072 -->


    <owl:NamedIndividual rdf:about="http://www.foodpairing.com/ontologies/foodpairing-kg#000072">
        <rdf:type rdf:resource="http://www.foodpairing.com/ontologies/foodpairing-kg#Ingredient"/>
        <foodpairing-kg:hasIngredientCategory rdf:resource="http://www.foodpairing.com/ontologies/foodpairing-kg#icat:000089"/>
        <rdfs:seeAlso rdf:datatype="http://www.w3.org/2001/XMLSchema#anyURI">http://www.wikidata.org/entity/Q1093742</rdfs:seeAlso>
        <skos:definition xml:lang="en">Citrus fruit with a sour and tangy flavor, commonly used in cooking, baking, and beverages.</skos:definition>
        <skos:prefLabel xml:lang="en">Lemon</skos:prefLabel>
    </owl:NamedIndividual>
    


    <!-- http://www.foodpairing.com/ontologies/foodpairing-kg#000078 -->


    <owl:NamedIndividual rdf:about="http://www.foodpairing.com/ontologies/foodpairing-kg#000078">
        <rdf:type rdf:resource="http://www.foodpairing.com/ontologies/foodpairing-kg#Ingredient"/>
        <foodpairing-kg:hasIngredientCategory rdf:resource="http://www.foodpairing.com/ontologies/foodpairing-kg#icat:000129"/>
        <rdfs:seeAlso rdf:datatype="http://www.w3.org/2001/XMLSchema#anyURI">http://www.wikidata.org/entity/Q961769</rdfs:seeAlso>
        <skos:definition xml:lang="en">A creamy, green fruit with a buttery texture, often used in salads, spreads, and various dishes.</skos:definition>
        <skos:prefLabel xml:lang="en">Avocado</skos:prefLabel>
    </owl:NamedIndividual>
    


    <!-- http://www.foodpairing.com/ontologies/foodpairing-kg#000082 -->


    <owl:NamedIndividual rdf:about="http://www.foodpairing.com/ontologies/foodpairing-kg#000082">
        <rdf:type rdf:resource="http://www.foodpairing.com/ontologies/foodpairing-kg#Ingredient"/>
        <foodpairing-kg:hasIngredientCategory rdf:resource="http://www.foodpairing.com/ontologies/foodpairing-kg#icat:000130"/>
        <rdfs:seeAlso rdf:datatype="http://www.w3.org/2001/XMLSchema#anyURI">http://www.wikidata.org/entity/Q1474</rdfs:seeAlso>
        <skos:definition xml:lang="en">A leafy vegetable with a slightly bitter taste, commonly used in salads and cooked dishes.</skos:definition>
        <skos:prefLabel xml:lang="en">Belgian Endive</skos:prefLabel>
    </owl:NamedIndividual>
    


    <!-- http://www.foodpairing.com/ontologies/foodpairing-kg#000083 -->


    <owl:NamedIndividual rdf:about="http://www.foodpairing.com/ontologies/foodpairing-kg#000083">
        <rdf:type rdf:resource="http://www.foodpairing.com/ontologies/foodpairing-kg#Ingredient"/>
        <foodpairing-kg:hasIngredientCategory rdf:resource="http://www.foodpairing.com/ontologies/foodpairing-kg#icat:000129"/>
        <rdfs:seeAlso rdf:datatype="http://www.w3.org/2001/XMLSchema#anyURI">http://www.wikidata.org/entity/Q106446932</rdfs:seeAlso>
        <skos:definition xml:lang="en">A vibrant red vegetable with a sweet and crunchy texture, used in salads, roasting, and cooking.</skos:definition>
        <skos:prefLabel xml:lang="en">Red Bell Pepper</skos:prefLabel>
    </owl:NamedIndividual>
    


    <!-- http://www.foodpairing.com/ontologies/foodpairing-kg#000090 -->


    <owl:NamedIndividual rdf:about="http://www.foodpairing.com/ontologies/foodpairing-kg#000090">
        <rdf:type rdf:resource="http://www.foodpairing.com/ontologies/foodpairing-kg#Ingredient"/>
        <foodpairing-kg:hasIngredientCategory rdf:resource="http://www.foodpairing.com/ontologies/foodpairing-kg#icat:000055"/>
        <rdfs:seeAlso rdf:datatype="http://www.w3.org/2001/XMLSchema#anyURI">http://www.wikidata.org/entity/Q217525</rdfs:seeAlso>
        <skos:definition xml:lang="en">A type of cheese known for its sharp and tangy flavor, commonly used in cooking and as a topping.</skos:definition>
        <skos:prefLabel xml:lang="en">Cheddar</skos:prefLabel>
    </owl:NamedIndividual>
    


    <!-- http://www.foodpairing.com/ontologies/foodpairing-kg#000091 -->


    <owl:NamedIndividual rdf:about="http://www.foodpairing.com/ontologies/foodpairing-kg#000091">
        <rdf:type rdf:resource="http://www.foodpairing.com/ontologies/foodpairing-kg#Ingredient"/>
        <foodpairing-kg:hasIngredientCategory rdf:resource="http://www.foodpairing.com/ontologies/foodpairing-kg#icat:000094"/>
        <rdfs:seeAlso rdf:datatype="http://www.w3.org/2001/XMLSchema#anyURI">http://www.wikidata.org/entity/Q21281535</rdfs:seeAlso>
        <skos:definition xml:lang="en">Delicate herb with a mild, anise-like flavor, used to add a fresh and aromatic touch to dishes.</skos:definition>
        <skos:prefLabel xml:lang="en">Chervil</skos:prefLabel>
    </owl:NamedIndividual>
    


    <!-- http://www.foodpairing.com/ontologies/foodpairing-kg#000096 -->


    <owl:NamedIndividual rdf:about="http://www.foodpairing.com/ontologies/foodpairing-kg#000096">
        <rdf:type rdf:resource="http://www.foodpairing.com/ontologies/foodpairing-kg#Ingredient"/>
        <foodpairing-kg:hasIngredientCategory rdf:resource="http://www.foodpairing.com/ontologies/foodpairing-kg#icat:000094"/>
        <rdfs:seeAlso rdf:datatype="http://www.w3.org/2001/XMLSchema#anyURI">http://www.wikidata.org/entity/Q61046162</rdfs:seeAlso>
        <skos:definition xml:lang="en">Chives are thin, green herbs with a mild onion flavor, often used as a garnish or flavoring in various dishes.</skos:definition>
        <skos:prefLabel xml:lang="en">Chives</skos:prefLabel>
    </owl:NamedIndividual>
    


    <!-- http://www.foodpairing.com/ontologies/foodpairing-kg#000101 -->


    <owl:NamedIndividual rdf:about="http://www.foodpairing.com/ontologies/foodpairing-kg#000101">
        <rdf:type rdf:resource="http://www.foodpairing.com/ontologies/foodpairing-kg#Ingredient"/>
        <foodpairing-kg:hasIngredientCategory rdf:resource="http://www.foodpairing.com/ontologies/foodpairing-kg#icat:000055"/>
        <rdfs:seeAlso rdf:datatype="http://www.w3.org/2001/XMLSchema#anyURI">http://www.wikidata.org/entity/Q932214</rdfs:seeAlso>
        <skos:definition xml:lang="en">Emmentaler is a Swiss cheese with a nutty flavor and distinctive holes, commonly used in cooking and sandwiches.</skos:definition>
        <skos:prefLabel xml:lang="en">Emmentaler</skos:prefLabel>
    </owl:NamedIndividual>
    


    <!-- http://www.foodpairing.com/ontologies/foodpairing-kg#000104 -->


    <owl:NamedIndividual rdf:about="http://www.foodpairing.com/ontologies/foodpairing-kg#000104">
        <rdf:type rdf:resource="http://www.foodpairing.com/ontologies/foodpairing-kg#Ingredient"/>
        <foodpairing-kg:hasIngredientCategory rdf:resource="http://www.foodpairing.com/ontologies/foodpairing-kg#icat:000007"/>
        <rdfs:seeAlso rdf:datatype="http://www.w3.org/2001/XMLSchema#anyURI">http://www.wikidata.org/entity/Q198815</rdfs:seeAlso>
        <skos:definition xml:lang="en">Creamy and tangy cheese made from goat&apos;s milk, known for its distinct flavor and versatility.</skos:definition>
        <skos:prefLabel xml:lang="en">Goat Cheese</skos:prefLabel>
    </owl:NamedIndividual>
    


    <!-- http://www.foodpairing.com/ontologies/foodpairing-kg#000105 -->


    <owl:NamedIndividual rdf:about="http://www.foodpairing.com/ontologies/foodpairing-kg#000105">
        <rdf:type rdf:resource="http://www.foodpairing.com/ontologies/foodpairing-kg#Ingredient"/>
        <foodpairing-kg:hasIngredientCategory rdf:resource="http://www.foodpairing.com/ontologies/foodpairing-kg#icat:000134"/>
        <rdfs:seeAlso rdf:datatype="http://www.w3.org/2001/XMLSchema#anyURI">http://www.wikidata.org/entity/Q2987371</rdfs:seeAlso>
        <skos:definition xml:lang="en">Crisp, slender pods with a fresh and slightly sweet taste, commonly used in various dishes.</skos:definition>
        <skos:prefLabel xml:lang="en">Green Bean</skos:prefLabel>
    </owl:NamedIndividual>
    


    <!-- http://www.foodpairing.com/ontologies/foodpairing-kg#000107 -->


    <owl:NamedIndividual rdf:about="http://www.foodpairing.com/ontologies/foodpairing-kg#000107">
        <rdf:type rdf:resource="http://www.foodpairing.com/ontologies/foodpairing-kg#Ingredient"/>
        <foodpairing-kg:hasIngredientCategory rdf:resource="http://www.foodpairing.com/ontologies/foodpairing-kg#icat:000055"/>
        <rdfs:seeAlso rdf:datatype="http://www.w3.org/2001/XMLSchema#anyURI">http://www.wikidata.org/entity/Q2376488</rdfs:seeAlso>
        <skos:definition xml:lang="en">Gruyère is a Swiss cheese with a rich, nutty flavor, commonly used in cooking, baking, and as a topping.</skos:definition>
        <skos:prefLabel xml:lang="en">Gruyère</skos:prefLabel>
    </owl:NamedIndividual>
    


    <!-- http://www.foodpairing.com/ontologies/foodpairing-kg#000109 -->


    <owl:NamedIndividual rdf:about="http://www.foodpairing.com/ontologies/foodpairing-kg#000109">
        <rdf:type rdf:resource="http://www.foodpairing.com/ontologies/foodpairing-kg#Ingredient"/>
        <foodpairing-kg:hasIngredientCategory rdf:resource="http://www.foodpairing.com/ontologies/foodpairing-kg#icat:000094"/>
        <rdfs:seeAlso rdf:datatype="http://www.w3.org/2001/XMLSchema#anyURI">http://www.wikidata.org/entity/Q65522654</rdfs:seeAlso>
        <skos:definition xml:lang="en">A basil leaf is a fragrant, green leaf with a strong, sweet aroma, often used as a herb in cooking.</skos:definition>
        <skos:prefLabel xml:lang="en">Basil Leaf</skos:prefLabel>
    </owl:NamedIndividual>
    


    <!-- http://www.foodpairing.com/ontologies/foodpairing-kg#000110 -->


    <owl:NamedIndividual rdf:about="http://www.foodpairing.com/ontologies/foodpairing-kg#000110">
        <rdf:type rdf:resource="http://www.foodpairing.com/ontologies/foodpairing-kg#Ingredient"/>
        <foodpairing-kg:hasIngredientCategory rdf:resource="http://www.foodpairing.com/ontologies/foodpairing-kg#icat:000136"/>
        <rdfs:seeAlso rdf:datatype="http://www.w3.org/2001/XMLSchema#anyURI">http://www.wikidata.org/entity/Q1807269</rdfs:seeAlso>
        <skos:definition xml:lang="en">Pungent, stem vegetable with a mild onion flavor, commonly used in soups and salads.</skos:definition>
        <skos:prefLabel xml:lang="en">Leek</skos:prefLabel>
    </owl:NamedIndividual>
    


    <!-- http://www.foodpairing.com/ontologies/foodpairing-kg#000117 -->


    <owl:NamedIndividual rdf:about="http://www.foodpairing.com/ontologies/foodpairing-kg#000117">
        <rdf:type rdf:resource="http://www.foodpairing.com/ontologies/foodpairing-kg#Ingredient"/>
        <foodpairing-kg:hasIngredientCategory rdf:resource="http://www.foodpairing.com/ontologies/foodpairing-kg#icat:000134"/>
        <rdfs:seeAlso rdf:datatype="http://www.w3.org/2001/XMLSchema#anyURI">http://www.wikidata.org/entity/Q25237</rdfs:seeAlso>
        <skos:definition xml:lang="en">Fresh peas are small, round, green legumes with a sweet and tender taste, commonly used in cooking.</skos:definition>
        <skos:prefLabel xml:lang="en">Pea</skos:prefLabel>
    </owl:NamedIndividual>
    


    <!-- http://www.foodpairing.com/ontologies/foodpairing-kg#000123 -->


    <owl:NamedIndividual rdf:about="http://www.foodpairing.com/ontologies/foodpairing-kg#000123">
        <rdf:type rdf:resource="http://www.foodpairing.com/ontologies/foodpairing-kg#Ingredient"/>
        <foodpairing-kg:hasIngredientCategory rdf:resource="http://www.foodpairing.com/ontologies/foodpairing-kg#icat:000094"/>
        <rdfs:seeAlso rdf:datatype="http://www.w3.org/2001/XMLSchema#anyURI">http://www.wikidata.org/entity/Q68315046</rdfs:seeAlso>
        <skos:definition xml:lang="en">A small, fragrant branch of the herb rosemary, used to impart flavor to dishes.</skos:definition>
        <skos:prefLabel xml:lang="en">Rosemary</skos:prefLabel>
    </owl:NamedIndividual>
    


    <!-- http://www.foodpairing.com/ontologies/foodpairing-kg#000133 -->


    <owl:NamedIndividual rdf:about="http://www.foodpairing.com/ontologies/foodpairing-kg#000133">
        <rdf:type rdf:resource="http://www.foodpairing.com/ontologies/foodpairing-kg#Ingredient"/>
        <foodpairing-kg:hasIngredientCategory rdf:resource="http://www.foodpairing.com/ontologies/foodpairing-kg#icat:000088"/>
        <rdfs:seeAlso rdf:datatype="http://www.w3.org/2001/XMLSchema#anyURI">http://www.wikidata.org/entity/Q14458220</rdfs:seeAlso>
        <skos:definition xml:lang="en">Strawberries are sweet, red berries with a juicy texture, commonly used in desserts, salads, and beverages.</skos:definition>
        <skos:prefLabel xml:lang="en">Strawberry</skos:prefLabel>
    </owl:NamedIndividual>
    


    <!-- http://www.foodpairing.com/ontologies/foodpairing-kg#000135 -->


    <owl:NamedIndividual rdf:about="http://www.foodpairing.com/ontologies/foodpairing-kg#000135">
        <rdf:type rdf:resource="http://www.foodpairing.com/ontologies/foodpairing-kg#Ingredient"/>
        <foodpairing-kg:hasIngredientCategory rdf:resource="http://www.foodpairing.com/ontologies/foodpairing-kg#icat:000088"/>
        <rdfs:seeAlso rdf:datatype="http://www.w3.org/2001/XMLSchema#anyURI">http://www.wikidata.org/entity/Q13179</rdfs:seeAlso>
        <skos:definition xml:lang="en">Raspberries are small, red or black berries with a tart and sweet flavor, used in various culinary applications.</skos:definition>
        <skos:prefLabel xml:lang="en">Raspberry</skos:prefLabel>
    </owl:NamedIndividual>
    


    <!-- http://www.foodpairing.com/ontologies/foodpairing-kg#000136 -->


    <owl:NamedIndividual rdf:about="http://www.foodpairing.com/ontologies/foodpairing-kg#000136">
        <rdf:type rdf:resource="http://www.foodpairing.com/ontologies/foodpairing-kg#Ingredient"/>
        <foodpairing-kg:hasIngredientCategory rdf:resource="http://www.foodpairing.com/ontologies/foodpairing-kg#icat:000088"/>
        <rdfs:seeAlso rdf:datatype="http://www.w3.org/2001/XMLSchema#anyURI">http://www.wikidata.org/entity/Q5812410</rdfs:seeAlso>
        <skos:definition xml:lang="en">Blueberries are small, round, and dark blue berries known for their sweet and slightly tart taste.</skos:definition>
        <skos:prefLabel xml:lang="en">Blueberry</skos:prefLabel>
    </owl:NamedIndividual>
    


    <!-- http://www.foodpairing.com/ontologies/foodpairing-kg#000141 -->


    <owl:NamedIndividual rdf:about="http://www.foodpairing.com/ontologies/foodpairing-kg#000141">
        <rdf:type rdf:resource="http://www.foodpairing.com/ontologies/foodpairing-kg#Ingredient"/>
        <foodpairing-kg:hasIngredientCategory rdf:resource="http://www.foodpairing.com/ontologies/foodpairing-kg#icat:000092"/>
        <rdfs:seeAlso rdf:datatype="http://www.w3.org/2001/XMLSchema#anyURI">http://www.wikidata.org/entity/Q13202263</rdfs:seeAlso>
        <skos:definition xml:lang="en">Juicy, stone fruits with a sweet and fragrant flavor, commonly eaten fresh or used in desserts.</skos:definition>
        <skos:prefLabel xml:lang="en">Yellow Peach</skos:prefLabel>
    </owl:NamedIndividual>
    


    <!-- http://www.foodpairing.com/ontologies/foodpairing-kg#000142 -->


    <owl:NamedIndividual rdf:about="http://www.foodpairing.com/ontologies/foodpairing-kg#000142">
        <rdf:type rdf:resource="http://www.foodpairing.com/ontologies/foodpairing-kg#Ingredient"/>
        <foodpairing-kg:hasIngredientCategory rdf:resource="http://www.foodpairing.com/ontologies/foodpairing-kg#icat:000092"/>
        <rdfs:seeAlso rdf:datatype="http://www.w3.org/2001/XMLSchema#anyURI">http://www.wikidata.org/entity/Q841156</rdfs:seeAlso>
        <skos:definition xml:lang="en">Yellow nectarines are similar to peaches but have smooth skin and a sweet, juicy flavor.</skos:definition>
        <skos:prefLabel xml:lang="en">Yellow Nectarine</skos:prefLabel>
    </owl:NamedIndividual>
    


    <!-- http://www.foodpairing.com/ontologies/foodpairing-kg#000144 -->


    <owl:NamedIndividual rdf:about="http://www.foodpairing.com/ontologies/foodpairing-kg#000144">
        <rdf:type rdf:resource="http://www.foodpairing.com/ontologies/foodpairing-kg#Ingredient"/>
        <foodpairing-kg:hasIngredientCategory rdf:resource="http://www.foodpairing.com/ontologies/foodpairing-kg#icat:000092"/>
        <rdfs:seeAlso rdf:datatype="http://www.w3.org/2001/XMLSchema#anyURI">http://www.wikidata.org/entity/Q12372598</rdfs:seeAlso>
        <skos:definition xml:lang="en">Juicy stone fruits with a sweet and tart flavor, commonly eaten fresh or used in jams and desserts.</skos:definition>
        <skos:prefLabel xml:lang="en">Plum</skos:prefLabel>
    </owl:NamedIndividual>
    


    <!-- http://www.foodpairing.com/ontologies/foodpairing-kg#000148 -->


    <owl:NamedIndividual rdf:about="http://www.foodpairing.com/ontologies/foodpairing-kg#000148">
        <rdf:type rdf:resource="http://www.foodpairing.com/ontologies/foodpairing-kg#Ingredient"/>
        <foodpairing-kg:hasIngredientCategory rdf:resource="http://www.foodpairing.com/ontologies/foodpairing-kg#icat:000093"/>
        <rdfs:seeAlso rdf:datatype="http://www.w3.org/2001/XMLSchema#anyURI">http://www.wikidata.org/entity/Q169</rdfs:seeAlso>
        <skos:definition xml:lang="en">Mangoes are tropical fruits with a sweet, juicy flesh and a distinctive flavor, commonly eaten fresh or used in salsas and desserts.</skos:definition>
        <skos:prefLabel xml:lang="en">Mango</skos:prefLabel>
    </owl:NamedIndividual>
    


    <!-- http://www.foodpairing.com/ontologies/foodpairing-kg#000149 -->


    <owl:NamedIndividual rdf:about="http://www.foodpairing.com/ontologies/foodpairing-kg#000149">
        <rdf:type rdf:resource="http://www.foodpairing.com/ontologies/foodpairing-kg#Ingredient"/>
        <foodpairing-kg:hasIngredientCategory rdf:resource="http://www.foodpairing.com/ontologies/foodpairing-kg#icat:000093"/>
        <rdfs:seeAlso rdf:datatype="http://www.w3.org/2001/XMLSchema#anyURI">http://www.wikidata.org/entity/Q503</rdfs:seeAlso>
        <skos:definition xml:lang="en">Yellow, curved fruits with a creamy texture and a sweet, mild flavor.</skos:definition>
        <skos:prefLabel xml:lang="en">Banana</skos:prefLabel>
    </owl:NamedIndividual>
    


    <!-- http://www.foodpairing.com/ontologies/foodpairing-kg#000151 -->


    <owl:NamedIndividual rdf:about="http://www.foodpairing.com/ontologies/foodpairing-kg#000151">
        <rdf:type rdf:resource="http://www.foodpairing.com/ontologies/foodpairing-kg#Ingredient"/>
        <foodpairing-kg:hasIngredientCategory rdf:resource="http://www.foodpairing.com/ontologies/foodpairing-kg#icat:000093"/>
        <rdfs:seeAlso rdf:datatype="http://www.w3.org/2001/XMLSchema#anyURI">http://www.wikidata.org/entity/Q10817602</rdfs:seeAlso>
        <skos:definition xml:lang="en">Pineapples are tropical fruits with a spiky skin and a sweet, tangy flavor, commonly eaten fresh or used in desserts.</skos:definition>
        <skos:prefLabel xml:lang="en">Pineapple</skos:prefLabel>
    </owl:NamedIndividual>
    


    <!-- http://www.foodpairing.com/ontologies/foodpairing-kg#000155 -->


    <owl:NamedIndividual rdf:about="http://www.foodpairing.com/ontologies/foodpairing-kg#000155">
        <rdf:type rdf:resource="http://www.foodpairing.com/ontologies/foodpairing-kg#Ingredient"/>
        <foodpairing-kg:hasIngredientCategory rdf:resource="http://www.foodpairing.com/ontologies/foodpairing-kg#icat:000089"/>
        <rdfs:seeAlso rdf:datatype="http://www.w3.org/2001/XMLSchema#anyURI">http://www.wikidata.org/entity/Q13195</rdfs:seeAlso>
        <skos:definition xml:lang="en">Limes are small, green citrus fruits with a tart and tangy flavor, commonly used in cooking and beverages.</skos:definition>
        <skos:prefLabel xml:lang="en">Lime</skos:prefLabel>
    </owl:NamedIndividual>
    


    <!-- http://www.foodpairing.com/ontologies/foodpairing-kg#000157 -->


    <owl:NamedIndividual rdf:about="http://www.foodpairing.com/ontologies/foodpairing-kg#000157">
        <rdf:type rdf:resource="http://www.foodpairing.com/ontologies/foodpairing-kg#Ingredient"/>
        <foodpairing-kg:hasIngredientCategory rdf:resource="http://www.foodpairing.com/ontologies/foodpairing-kg#icat:000089"/>
        <rdfs:seeAlso rdf:datatype="http://www.w3.org/2001/XMLSchema#anyURI">http://www.wikidata.org/entity/Q13191</rdfs:seeAlso>
        <skos:definition xml:lang="en">Oranges are round, citrus fruits with a sweet and tangy flavor, commonly eaten fresh or used in juices and desserts.</skos:definition>
        <skos:prefLabel xml:lang="en">Orange</skos:prefLabel>
    </owl:NamedIndividual>
    


    <!-- http://www.foodpairing.com/ontologies/foodpairing-kg#000159 -->


    <owl:NamedIndividual rdf:about="http://www.foodpairing.com/ontologies/foodpairing-kg#000159">
        <rdf:type rdf:resource="http://www.foodpairing.com/ontologies/foodpairing-kg#Ingredient"/>
        <foodpairing-kg:hasIngredientCategory rdf:resource="http://www.foodpairing.com/ontologies/foodpairing-kg#icat:000089"/>
        <rdfs:seeAlso rdf:datatype="http://www.w3.org/2001/XMLSchema#anyURI">http://www.wikidata.org/entity/Q21552830</rdfs:seeAlso>
        <skos:definition xml:lang="en">Yellow grapefruits are citrus fruits with a tangy-sweet flavor, commonly eaten fresh or used in juices. Their taste is slightly more bitter when compared to pink and red grapefruit.</skos:definition>
        <skos:prefLabel xml:lang="en">Yellow Grapefruit</skos:prefLabel>
    </owl:NamedIndividual>
    


    <!-- http://www.foodpairing.com/ontologies/foodpairing-kg#000161 -->


    <owl:NamedIndividual rdf:about="http://www.foodpairing.com/ontologies/foodpairing-kg#000161">
        <rdf:type rdf:resource="http://www.foodpairing.com/ontologies/foodpairing-kg#Ingredient"/>
        <foodpairing-kg:hasIngredientCategory rdf:resource="http://www.foodpairing.com/ontologies/foodpairing-kg#icat:000090"/>
        <rdfs:seeAlso rdf:datatype="http://www.w3.org/2001/XMLSchema#anyURI">http://www.wikidata.org/entity/Q38645</rdfs:seeAlso>
        <skos:definition xml:lang="en">A juicy and refreshing fruit with a sweet, hydrating taste, commonly eaten fresh.</skos:definition>
        <skos:prefLabel xml:lang="en">Watermelon</skos:prefLabel>
    </owl:NamedIndividual>
    


    <!-- http://www.foodpairing.com/ontologies/foodpairing-kg#000163 -->


    <owl:NamedIndividual rdf:about="http://www.foodpairing.com/ontologies/foodpairing-kg#000163">
        <rdf:type rdf:resource="http://www.foodpairing.com/ontologies/foodpairing-kg#Ingredient"/>
        <foodpairing-kg:hasIngredientCategory rdf:resource="http://www.foodpairing.com/ontologies/foodpairing-kg#icat:000090"/>
        <rdfs:seeAlso rdf:datatype="http://www.w3.org/2001/XMLSchema#anyURI">http://www.wikidata.org/entity/Q61858403</rdfs:seeAlso>
        <skos:definition xml:lang="en">A sweet and aromatic fruit with orange flesh, commonly eaten fresh or used in salads.</skos:definition>
        <skos:prefLabel xml:lang="en">Cantaloupe Melon</skos:prefLabel>
    </owl:NamedIndividual>
    


    <!-- http://www.foodpairing.com/ontologies/foodpairing-kg#000181 -->


    <owl:NamedIndividual rdf:about="http://www.foodpairing.com/ontologies/foodpairing-kg#000181">
        <rdf:type rdf:resource="http://www.foodpairing.com/ontologies/foodpairing-kg#Ingredient"/>
        <foodpairing-kg:hasIngredientCategory rdf:resource="http://www.foodpairing.com/ontologies/foodpairing-kg#icat:000139"/>
        <rdfs:seeAlso rdf:datatype="http://www.w3.org/2001/XMLSchema#anyURI">http://www.wikidata.org/entity/Q36814998</rdfs:seeAlso>
        <skos:definition xml:lang="en">Dark leafy green vegetable known for its tender leaves and mild, slightly earthy taste, commonly used in salads, sautés, and as a versatile ingredient.</skos:definition>
        <skos:prefLabel xml:lang="en">Spinach</skos:prefLabel>
    </owl:NamedIndividual>
    


    <!-- http://www.foodpairing.com/ontologies/foodpairing-kg#000182 -->


    <owl:NamedIndividual rdf:about="http://www.foodpairing.com/ontologies/foodpairing-kg#000182">
        <rdf:type rdf:resource="http://www.foodpairing.com/ontologies/foodpairing-kg#Ingredient"/>
        <foodpairing-kg:hasIngredientCategory rdf:resource="http://www.foodpairing.com/ontologies/foodpairing-kg#icat:000136"/>
        <rdfs:seeAlso rdf:datatype="http://www.w3.org/2001/XMLSchema#anyURI">http://www.wikidata.org/entity/Q23012379</rdfs:seeAlso>
        <skos:definition xml:lang="en">Crisp, green vegetable with a mild, earthy flavor, often used in salads, soups, and as a crunchy snack.</skos:definition>
        <skos:prefLabel xml:lang="en">Celery</skos:prefLabel>
    </owl:NamedIndividual>
    


    <!-- http://www.foodpairing.com/ontologies/foodpairing-kg#000213 -->


    <owl:NamedIndividual rdf:about="http://www.foodpairing.com/ontologies/foodpairing-kg#000213">
        <rdf:type rdf:resource="http://www.foodpairing.com/ontologies/foodpairing-kg#Ingredient"/>
        <foodpairing-kg:hasIngredientCategory rdf:resource="http://www.foodpairing.com/ontologies/foodpairing-kg#icat:000130"/>
        <rdfs:seeAlso rdf:datatype="http://www.w3.org/2001/XMLSchema#anyURI">http://www.wikidata.org/entity/Q263203</rdfs:seeAlso>
        <skos:definition xml:lang="en">Crunchy and colorful vegetable used in salads and coleslaws for its vibrant hue and mild flavor.</skos:definition>
        <skos:prefLabel xml:lang="en">Red Cabbage</skos:prefLabel>
    </owl:NamedIndividual>
    


    <!-- http://www.foodpairing.com/ontologies/foodpairing-kg#000215 -->


    <owl:NamedIndividual rdf:about="http://www.foodpairing.com/ontologies/foodpairing-kg#000215">
        <rdf:type rdf:resource="http://www.foodpairing.com/ontologies/foodpairing-kg#Ingredient"/>
        <foodpairing-kg:hasIngredientCategory rdf:resource="http://www.foodpairing.com/ontologies/foodpairing-kg#icat:000132"/>
        <rdfs:seeAlso rdf:datatype="http://www.w3.org/2001/XMLSchema#anyURI">http://www.wikidata.org/entity/Q99548274</rdfs:seeAlso>
        <skos:definition xml:lang="en">A sweet, earthy root vegetable often used in salads and as a natural food coloring.</skos:definition>
        <skos:prefLabel xml:lang="en">Beetroot</skos:prefLabel>
    </owl:NamedIndividual>
    


    <!-- http://www.foodpairing.com/ontologies/foodpairing-kg#000252 -->


    <owl:NamedIndividual rdf:about="http://www.foodpairing.com/ontologies/foodpairing-kg#000252">
        <rdf:type rdf:resource="http://www.foodpairing.com/ontologies/foodpairing-kg#Ingredient"/>
        <foodpairing-kg:hasIngredientCategory rdf:resource="http://www.foodpairing.com/ontologies/foodpairing-kg#icat:000137"/>
        <rdfs:seeAlso rdf:datatype="http://www.w3.org/2001/XMLSchema#anyURI">http://www.wikidata.org/entity/Q37937</rdfs:seeAlso>
        <skos:definition xml:lang="en">Sweet potatoes are starchy, orange-fleshed tubers with a naturally sweet taste, commonly baked, mashed, or used in various culinary preparations.</skos:definition>
        <skos:prefLabel xml:lang="en">Sweet Potato</skos:prefLabel>
    </owl:NamedIndividual>
    


    <!-- http://www.foodpairing.com/ontologies/foodpairing-kg#000281 -->


    <owl:NamedIndividual rdf:about="http://www.foodpairing.com/ontologies/foodpairing-kg#000281">
        <rdf:type rdf:resource="http://www.foodpairing.com/ontologies/foodpairing-kg#Ingredient"/>
        <foodpairing-kg:hasIngredientCategory rdf:resource="http://www.foodpairing.com/ontologies/foodpairing-kg#icat:000115"/>
        <rdfs:seeAlso rdf:datatype="http://www.w3.org/2001/XMLSchema#anyURI">http://www.wikidata.org/entity/Q20856764</rdfs:seeAlso>
        <skos:definition xml:lang="en">Coriander seeds are the dried fruits of the coriander plant, imparting a warm, citrusy flavor to dishes and frequently used in spice blends.</skos:definition>
        <skos:prefLabel xml:lang="en">Coriander Seed</skos:prefLabel>
    </owl:NamedIndividual>
    


    <!-- http://www.foodpairing.com/ontologies/foodpairing-kg#000306 -->


    <owl:NamedIndividual rdf:about="http://www.foodpairing.com/ontologies/foodpairing-kg#000306">
        <rdf:type rdf:resource="http://www.foodpairing.com/ontologies/foodpairing-kg#Ingredient"/>
        <foodpairing-kg:hasIngredientCategory rdf:resource="http://www.foodpairing.com/ontologies/foodpairing-kg#icat:000105"/>
        <rdfs:seeAlso rdf:datatype="http://www.w3.org/2001/XMLSchema#anyURI">http://www.wikidata.org/entity/Q188879</rdfs:seeAlso>
        <skos:definition xml:lang="en">Popular fish known for its tender, pink flesh and mild, slightly sweet flavor, making it a versatile choice for various culinary preparations.</skos:definition>
        <skos:prefLabel xml:lang="en">Atlantic Salmon</skos:prefLabel>
    </owl:NamedIndividual>
    


    <!-- http://www.foodpairing.com/ontologies/foodpairing-kg#000311 -->


    <owl:NamedIndividual rdf:about="http://www.foodpairing.com/ontologies/foodpairing-kg#000311">
        <rdf:type rdf:resource="http://www.foodpairing.com/ontologies/foodpairing-kg#Ingredient"/>
        <foodpairing-kg:hasIngredientCategory rdf:resource="http://www.foodpairing.com/ontologies/foodpairing-kg#icat:000040"/>
        <rdfs:seeAlso rdf:datatype="http://www.w3.org/2001/XMLSchema#anyURI">http://www.wikidata.org/entity/Q167893</rdfs:seeAlso>
        <skos:definition xml:lang="en">Creamy condiment made from eggs, oil, and vinegar or lemon juice, commonly used in salads and sandwiches.</skos:definition>
        <skos:prefLabel xml:lang="en">Mayonnaise</skos:prefLabel>
    </owl:NamedIndividual>
    


    <!-- http://www.foodpairing.com/ontologies/foodpairing-kg#000313 -->


    <owl:NamedIndividual rdf:about="http://www.foodpairing.com/ontologies/foodpairing-kg#000313">
        <rdf:type rdf:resource="http://www.foodpairing.com/ontologies/foodpairing-kg#Ingredient"/>
        <foodpairing-kg:hasIngredientCategory rdf:resource="http://www.foodpairing.com/ontologies/foodpairing-kg#icat:000125"/>
        <rdfs:seeAlso rdf:datatype="http://www.w3.org/2001/XMLSchema#anyURI">http://www.wikidata.org/entity/Q10987</rdfs:seeAlso>
        <skos:definition xml:lang="en">A sweet, natural substance produced by bees from flower nectar, commonly used as a sweetener.</skos:definition>
        <skos:prefLabel xml:lang="en">Honey</skos:prefLabel>
    </owl:NamedIndividual>
    


    <!-- http://www.foodpairing.com/ontologies/foodpairing-kg#000355 -->


    <owl:NamedIndividual rdf:about="http://www.foodpairing.com/ontologies/foodpairing-kg#000355">
        <rdf:type rdf:resource="http://www.foodpairing.com/ontologies/foodpairing-kg#Ingredient"/>
        <foodpairing-kg:hasIngredientCategory rdf:resource="http://www.foodpairing.com/ontologies/foodpairing-kg#icat:000129"/>
        <rdfs:seeAlso rdf:datatype="http://www.w3.org/2001/XMLSchema#anyURI">http://www.wikidata.org/entity/Q18966</rdfs:seeAlso>
        <skos:definition xml:lang="en">A type of maize known for its tender, sweet kernels, enjoyed as a vegetable when fresh and often used in a variety of dishes.</skos:definition>
        <skos:prefLabel xml:lang="en">Sweet Corn</skos:prefLabel>
    </owl:NamedIndividual>
    


    <!-- http://www.foodpairing.com/ontologies/foodpairing-kg#000357 -->


    <owl:NamedIndividual rdf:about="http://www.foodpairing.com/ontologies/foodpairing-kg#000357">
        <rdf:type rdf:resource="http://www.foodpairing.com/ontologies/foodpairing-kg#Ingredient"/>
        <foodpairing-kg:hasIngredientCategory rdf:resource="http://www.foodpairing.com/ontologies/foodpairing-kg#icat:000094"/>
        <rdfs:seeAlso rdf:datatype="http://www.w3.org/2001/XMLSchema#anyURI">http://www.wikidata.org/entity/Q92581152</rdfs:seeAlso>
        <skos:definition xml:lang="en">Oregano is a fragrant herb with a robust, slightly peppery flavor, often used to season Mediterranean and Italian dishes.</skos:definition>
        <skos:prefLabel xml:lang="en">Oregano</skos:prefLabel>
    </owl:NamedIndividual>
    


    <!-- http://www.foodpairing.com/ontologies/foodpairing-kg#000413 -->


    <owl:NamedIndividual rdf:about="http://www.foodpairing.com/ontologies/foodpairing-kg#000413">
        <rdf:type rdf:resource="http://www.foodpairing.com/ontologies/foodpairing-kg#Ingredient"/>
        <foodpairing-kg:hasIngredientCategory rdf:resource="http://www.foodpairing.com/ontologies/foodpairing-kg#icat:000091"/>
        <rdfs:seeAlso rdf:datatype="http://www.w3.org/2001/XMLSchema#anyURI">http://www.wikidata.org/entity/Q41778389</rdfs:seeAlso>
        <skos:definition xml:lang="en">A variety of apple known for their crisp texture and sweet-tart flavor, commonly eaten fresh.</skos:definition>
        <skos:prefLabel xml:lang="en">Apple &apos;Jonagold&apos;</skos:prefLabel>
    </owl:NamedIndividual>
    


    <!-- http://www.foodpairing.com/ontologies/foodpairing-kg#000452 -->


    <owl:NamedIndividual rdf:about="http://www.foodpairing.com/ontologies/foodpairing-kg#000452">
        <rdf:type rdf:resource="http://www.foodpairing.com/ontologies/foodpairing-kg#Ingredient"/>
        <foodpairing-kg:hasIngredientCategory rdf:resource="http://www.foodpairing.com/ontologies/foodpairing-kg#icat:000129"/>
        <rdfs:seeAlso rdf:datatype="http://www.w3.org/2001/XMLSchema#anyURI">http://www.wikidata.org/entity/Q165308</rdfs:seeAlso>
        <skos:definition xml:lang="en">Vibrant orange squash with a mildly sweet, nutty flavor, used in both savory and sweet recipes, especially during autumn.</skos:definition>
        <skos:prefLabel xml:lang="en">Pumpkin</skos:prefLabel>
    </owl:NamedIndividual>
    


    <!-- http://www.foodpairing.com/ontologies/foodpairing-kg#000472 -->


    <owl:NamedIndividual rdf:about="http://www.foodpairing.com/ontologies/foodpairing-kg#000472">
        <rdf:type rdf:resource="http://www.foodpairing.com/ontologies/foodpairing-kg#Ingredient"/>
        <foodpairing-kg:hasIngredientCategory rdf:resource="http://www.foodpairing.com/ontologies/foodpairing-kg#icat:000059"/>
        <rdfs:seeAlso rdf:datatype="http://www.w3.org/2001/XMLSchema#anyURI">http://www.wikidata.org/entity/Q131480</rdfs:seeAlso>
        <skos:definition xml:lang="en">Camembert is a soft, creamy cheese known for its rich, earthy flavor and velvety texture.</skos:definition>
        <skos:prefLabel xml:lang="en">Camembert</skos:prefLabel>
    </owl:NamedIndividual>
    


    <!-- http://www.foodpairing.com/ontologies/foodpairing-kg#000475 -->


    <owl:NamedIndividual rdf:about="http://www.foodpairing.com/ontologies/foodpairing-kg#000475">
        <rdf:type rdf:resource="http://www.foodpairing.com/ontologies/foodpairing-kg#Ingredient"/>
        <foodpairing-kg:hasIngredientCategory rdf:resource="http://www.foodpairing.com/ontologies/foodpairing-kg#icat:000100"/>
        <rdfs:seeAlso rdf:datatype="http://www.w3.org/2001/XMLSchema#anyURI">http://www.wikidata.org/entity/Q1119911</rdfs:seeAlso>
        <skos:definition xml:lang="en">Buttery, oval-shaped nuts with a rich and nutty flavor, commonly used in baking and desserts.</skos:definition>
        <skos:prefLabel xml:lang="en">Pecan Nut</skos:prefLabel>
    </owl:NamedIndividual>
    


    <!-- http://www.foodpairing.com/ontologies/foodpairing-kg#000515 -->


    <owl:NamedIndividual rdf:about="http://www.foodpairing.com/ontologies/foodpairing-kg#000515">
        <rdf:type rdf:resource="http://www.foodpairing.com/ontologies/foodpairing-kg#Ingredient"/>
        <foodpairing-kg:hasIngredientCategory rdf:resource="http://www.foodpairing.com/ontologies/foodpairing-kg#icat:000131"/>
        <rdfs:seeAlso rdf:datatype="http://www.w3.org/2001/XMLSchema#anyURI">http://www.wikidata.org/entity/Q186451</rdfs:seeAlso>
        <skos:definition xml:lang="en">Edible fungi with a delicate flavor and tender texture, often used in cooking.</skos:definition>
        <skos:prefLabel xml:lang="en">Oyster Mushroom</skos:prefLabel>
    </owl:NamedIndividual>
    


    <!-- http://www.foodpairing.com/ontologies/foodpairing-kg#000520 -->


    <owl:NamedIndividual rdf:about="http://www.foodpairing.com/ontologies/foodpairing-kg#000520">
        <rdf:type rdf:resource="http://www.foodpairing.com/ontologies/foodpairing-kg#Ingredient"/>
        <foodpairing-kg:hasIngredientCategory rdf:resource="http://www.foodpairing.com/ontologies/foodpairing-kg#icat:000130"/>
        <rdfs:seeAlso rdf:datatype="http://www.w3.org/2001/XMLSchema#anyURI">http://www.wikidata.org/entity/Q150463</rdfs:seeAlso>
        <skos:definition xml:lang="en">Small, green cruciferous vegetables with a mild, nutty flavor, commonly used in side dishes.</skos:definition>
        <skos:prefLabel xml:lang="en">Brussels Sprouts</skos:prefLabel>
    </owl:NamedIndividual>
    


    <!-- http://www.foodpairing.com/ontologies/foodpairing-kg#000787 -->


    <owl:NamedIndividual rdf:about="http://www.foodpairing.com/ontologies/foodpairing-kg#000787">
        <rdf:type rdf:resource="http://www.foodpairing.com/ontologies/foodpairing-kg#Ingredient"/>
        <foodpairing-kg:hasIngredientCategory rdf:resource="http://www.foodpairing.com/ontologies/foodpairing-kg#icat:000120"/>
        <rdfs:seeAlso rdf:datatype="http://www.w3.org/2001/XMLSchema#anyURI">http://www.wikidata.org/entity/Q13241</rdfs:seeAlso>
        <skos:definition xml:lang="en">A variety of vanilla known for its rich and aromatic flavor, commonly used in baking.</skos:definition>
        <skos:prefLabel xml:lang="en">Vanilla &apos;Bourbon&apos;</skos:prefLabel>
    </owl:NamedIndividual>
    


    <!-- http://www.foodpairing.com/ontologies/foodpairing-kg#000791 -->


    <owl:NamedIndividual rdf:about="http://www.foodpairing.com/ontologies/foodpairing-kg#000791">
        <rdf:type rdf:resource="http://www.foodpairing.com/ontologies/foodpairing-kg#Ingredient"/>
        <foodpairing-kg:hasIngredientCategory rdf:resource="http://www.foodpairing.com/ontologies/foodpairing-kg#icat:000068"/>
        <rdfs:seeAlso rdf:datatype="http://www.w3.org/2001/XMLSchema#anyURI">http://www.wikidata.org/entity/Q3268</rdfs:seeAlso>
        <skos:definition xml:lang="en">Apple brandy from the Normandy region of France, known for its fruity and robust flavor.</skos:definition>
        <skos:prefLabel xml:lang="en">Calvados</skos:prefLabel>
    </owl:NamedIndividual>
    


    <!-- http://www.foodpairing.com/ontologies/foodpairing-kg#000801 -->


    <owl:NamedIndividual rdf:about="http://www.foodpairing.com/ontologies/foodpairing-kg#000801">
        <rdf:type rdf:resource="http://www.foodpairing.com/ontologies/foodpairing-kg#Ingredient"/>
        <foodpairing-kg:hasIngredientCategory rdf:resource="http://www.foodpairing.com/ontologies/foodpairing-kg#icat:000028"/>
        <rdfs:seeAlso rdf:datatype="http://www.w3.org/2001/XMLSchema#anyURI">http://www.wikidata.org/entity/Q208008</rdfs:seeAlso>
        <skos:definition xml:lang="en">Fine, brown powder made from roasted and ground cacao beans, commonly used in baking.</skos:definition>
        <skos:prefLabel xml:lang="en">Cocoa Powder</skos:prefLabel>
    </owl:NamedIndividual>
    


    <!-- http://www.foodpairing.com/ontologies/foodpairing-kg#000840 -->


    <owl:NamedIndividual rdf:about="http://www.foodpairing.com/ontologies/foodpairing-kg#000840">
        <rdf:type rdf:resource="http://www.foodpairing.com/ontologies/foodpairing-kg#Ingredient"/>
        <foodpairing-kg:hasIngredientCategory rdf:resource="http://www.foodpairing.com/ontologies/foodpairing-kg#icat:000070"/>
        <rdfs:seeAlso rdf:datatype="http://www.w3.org/2001/XMLSchema#anyURI">http://www.wikidata.org/entity/Q62076228</rdfs:seeAlso>
        <skos:definition xml:lang="en">A type of gin known for its dry and juniper-forward flavor, commonly used in cocktails.</skos:definition>
        <skos:prefLabel xml:lang="en">London Dry Gin</skos:prefLabel>
    </owl:NamedIndividual>
    


    <!-- http://www.foodpairing.com/ontologies/foodpairing-kg#000865 -->


    <owl:NamedIndividual rdf:about="http://www.foodpairing.com/ontologies/foodpairing-kg#000865">
        <rdf:type rdf:resource="http://www.foodpairing.com/ontologies/foodpairing-kg#Ingredient"/>
        <foodpairing-kg:hasIngredientCategory rdf:resource="http://www.foodpairing.com/ontologies/foodpairing-kg#icat:000009"/>
        <rdfs:seeAlso rdf:datatype="http://www.w3.org/2001/XMLSchema#anyURI">http://www.wikidata.org/entity/Q170219</rdfs:seeAlso>
        <skos:definition xml:lang="en">Sake is a Japanese rice wine with a mild and slightly sweet flavor, commonly consumed as a beverage.</skos:definition>
        <skos:prefLabel xml:lang="en">Sake</skos:prefLabel>
    </owl:NamedIndividual>
    


    <!-- http://www.foodpairing.com/ontologies/foodpairing-kg#000873 -->


    <owl:NamedIndividual rdf:about="http://www.foodpairing.com/ontologies/foodpairing-kg#000873">
        <rdf:type rdf:resource="http://www.foodpairing.com/ontologies/foodpairing-kg#Ingredient"/>
        <foodpairing-kg:hasIngredientCategory rdf:resource="http://www.foodpairing.com/ontologies/foodpairing-kg#icat:000088"/>
        <rdfs:seeAlso rdf:datatype="http://www.w3.org/2001/XMLSchema#anyURI">http://www.wikidata.org/entity/Q165137</rdfs:seeAlso>
        <skos:definition xml:lang="en">Sweet cherries are plump, red or dark purple fruits with a juicy and sweet flavor, commonly eaten fresh.</skos:definition>
        <skos:prefLabel xml:lang="en">Sweet Cherry</skos:prefLabel>
    </owl:NamedIndividual>
    


    <!-- http://www.foodpairing.com/ontologies/foodpairing-kg#000876 -->


    <owl:NamedIndividual rdf:about="http://www.foodpairing.com/ontologies/foodpairing-kg#000876">
        <rdf:type rdf:resource="http://www.foodpairing.com/ontologies/foodpairing-kg#Ingredient"/>
        <foodpairing-kg:hasIngredientCategory rdf:resource="http://www.foodpairing.com/ontologies/foodpairing-kg#icat:000066"/>
        <rdfs:seeAlso rdf:datatype="http://www.w3.org/2001/XMLSchema#anyURI">http://www.wikidata.org/entity/Q26877308</rdfs:seeAlso>
        <skos:definition xml:lang="en">Fortified wine flavored with botanicals, commonly used as a component in cocktails.</skos:definition>
        <skos:prefLabel xml:lang="en">Sweet Vermouth</skos:prefLabel>
    </owl:NamedIndividual>
    


    <!-- http://www.foodpairing.com/ontologies/foodpairing-kg#000886 -->


    <owl:NamedIndividual rdf:about="http://www.foodpairing.com/ontologies/foodpairing-kg#000886">
        <rdf:type rdf:resource="http://www.foodpairing.com/ontologies/foodpairing-kg#Ingredient"/>
        <foodpairing-kg:hasIngredientCategory rdf:resource="http://www.foodpairing.com/ontologies/foodpairing-kg#icat:000073"/>
        <rdfs:seeAlso rdf:datatype="http://www.w3.org/2001/XMLSchema#anyURI">http://www.wikidata.org/entity/Q281</rdfs:seeAlso>
        <skos:definition xml:lang="en">Distilled alcoholic beverage made from fermented grain mash, known for its complex flavor profiles.</skos:definition>
        <skos:prefLabel xml:lang="en">Whisky</skos:prefLabel>
    </owl:NamedIndividual>
    


    <!-- http://www.foodpairing.com/ontologies/foodpairing-kg#000887 -->


    <owl:NamedIndividual rdf:about="http://www.foodpairing.com/ontologies/foodpairing-kg#000887">
        <rdf:type rdf:resource="http://www.foodpairing.com/ontologies/foodpairing-kg#Ingredient"/>
        <foodpairing-kg:hasIngredientCategory rdf:resource="http://www.foodpairing.com/ontologies/foodpairing-kg#icat:000004"/>
        <rdfs:seeAlso rdf:datatype="http://www.w3.org/2001/XMLSchema#anyURI">http://www.wikidata.org/entity/Q742385</rdfs:seeAlso>
        <skos:definition xml:lang="en">A creamy confection made from cocoa butter, sugar, and milk solids, known for its sweet and rich flavor.</skos:definition>
        <skos:prefLabel xml:lang="en">White Chocolate</skos:prefLabel>
    </owl:NamedIndividual>
    


    <!-- http://www.foodpairing.com/ontologies/foodpairing-kg#000920 -->


    <owl:NamedIndividual rdf:about="http://www.foodpairing.com/ontologies/foodpairing-kg#000920">
        <rdf:type rdf:resource="http://www.foodpairing.com/ontologies/foodpairing-kg#Ingredient"/>
        <foodpairing-kg:hasIngredientCategory rdf:resource="http://www.foodpairing.com/ontologies/foodpairing-kg#icat:000129"/>
        <rdfs:seeAlso rdf:datatype="http://www.w3.org/2001/XMLSchema#anyURI">http://www.wikidata.org/entity/Q2735883</rdfs:seeAlso>
        <skos:definition xml:lang="en">Crisp, green vegetables with a mild and refreshing flavor, commonly eaten fresh or pickled.</skos:definition>
        <skos:prefLabel xml:lang="en">Cucumber</skos:prefLabel>
    </owl:NamedIndividual>
    


    <!-- http://www.foodpairing.com/ontologies/foodpairing-kg#000938 -->


    <owl:NamedIndividual rdf:about="http://www.foodpairing.com/ontologies/foodpairing-kg#000938">
        <rdf:type rdf:resource="http://www.foodpairing.com/ontologies/foodpairing-kg#Ingredient"/>
        <foodpairing-kg:hasIngredientCategory rdf:resource="http://www.foodpairing.com/ontologies/foodpairing-kg#icat:000136"/>
        <rdfs:seeAlso rdf:datatype="http://www.w3.org/2001/XMLSchema#anyURI">http://www.wikidata.org/entity/Q22806705</rdfs:seeAlso>
        <skos:definition xml:lang="en">White asparagus is a milder, sweeter variety of asparagus with pale stalks, commonly enjoyed steamed or roasted as a delicacy.</skos:definition>
        <skos:prefLabel xml:lang="en">White Asparagus</skos:prefLabel>
    </owl:NamedIndividual>
    


    <!-- http://www.foodpairing.com/ontologies/foodpairing-kg#000993 -->


    <owl:NamedIndividual rdf:about="http://www.foodpairing.com/ontologies/foodpairing-kg#000993">
        <rdf:type rdf:resource="http://www.foodpairing.com/ontologies/foodpairing-kg#Ingredient"/>
        <foodpairing-kg:hasIngredientCategory rdf:resource="http://www.foodpairing.com/ontologies/foodpairing-kg#icat:000147"/>
        <rdfs:seeAlso rdf:datatype="http://www.w3.org/2001/XMLSchema#anyURI">http://www.wikidata.org/entity/Q335016</rdfs:seeAlso>
        <skos:definition xml:lang="en">Tabasco is a brand of hot sauce made from tabasco peppers, commonly used to add heat and flavor to dishes.</skos:definition>
        <skos:prefLabel xml:lang="en">Tabasco</skos:prefLabel>
    </owl:NamedIndividual>
    


    <!-- http://www.foodpairing.com/ontologies/foodpairing-kg#001008 -->


    <owl:NamedIndividual rdf:about="http://www.foodpairing.com/ontologies/foodpairing-kg#001008">
        <rdf:type rdf:resource="http://www.foodpairing.com/ontologies/foodpairing-kg#Ingredient"/>
        <foodpairing-kg:hasIngredientCategory rdf:resource="http://www.foodpairing.com/ontologies/foodpairing-kg#icat:000004"/>
        <rdfs:seeAlso rdf:datatype="http://www.w3.org/2001/XMLSchema#anyURI">http://www.wikidata.org/entity/Q2164820</rdfs:seeAlso>
        <skos:definition xml:lang="en">Milk chocolate is a smooth, creamy chocolate made from cocoa solids, milk, and sugar, known for its sweet flavor.</skos:definition>
        <skos:prefLabel xml:lang="en">Milk Chocolate</skos:prefLabel>
    </owl:NamedIndividual>
    


    <!-- http://www.foodpairing.com/ontologies/foodpairing-kg#001218 -->


    <owl:NamedIndividual rdf:about="http://www.foodpairing.com/ontologies/foodpairing-kg#001218">
        <rdf:type rdf:resource="http://www.foodpairing.com/ontologies/foodpairing-kg#Ingredient"/>
        <foodpairing-kg:hasIngredientCategory rdf:resource="http://www.foodpairing.com/ontologies/foodpairing-kg#icat:000105"/>
        <rdfs:seeAlso rdf:datatype="http://www.w3.org/2001/XMLSchema#anyURI">http://www.wikidata.org/entity/Q13194939</rdfs:seeAlso>
        <skos:definition xml:lang="en">White fish with a mild flavor and flaky texture, commonly used in a variety of culinary dishes.</skos:definition>
        <skos:prefLabel xml:lang="en">Cod</skos:prefLabel>
    </owl:NamedIndividual>
    


    <!-- http://www.foodpairing.com/ontologies/foodpairing-kg#001394 -->


    <owl:NamedIndividual rdf:about="http://www.foodpairing.com/ontologies/foodpairing-kg#001394">
        <rdf:type rdf:resource="http://www.foodpairing.com/ontologies/foodpairing-kg#Ingredient"/>
        <foodpairing-kg:hasIngredientCategory rdf:resource="http://www.foodpairing.com/ontologies/foodpairing-kg#icat:000111"/>
        <rdfs:seeAlso rdf:datatype="http://www.w3.org/2001/XMLSchema#anyURI">http://www.wikidata.org/entity/Q165112</rdfs:seeAlso>
        <skos:definition xml:lang="en">Popcorn is a type of corn that puffs up when heated, resulting in a light and crunchy snack.</skos:definition>
        <skos:prefLabel xml:lang="en">Popcorn</skos:prefLabel>
    </owl:NamedIndividual>
    


    <!-- http://www.foodpairing.com/ontologies/foodpairing-kg#001448 -->


    <owl:NamedIndividual rdf:about="http://www.foodpairing.com/ontologies/foodpairing-kg#001448">
        <rdf:type rdf:resource="http://www.foodpairing.com/ontologies/foodpairing-kg#Ingredient"/>
        <foodpairing-kg:hasIngredientCategory rdf:resource="http://www.foodpairing.com/ontologies/foodpairing-kg#icat:000079"/>
        <rdfs:seeAlso rdf:datatype="http://www.w3.org/2001/XMLSchema#anyURI">http://www.wikidata.org/entity/Q60855</rdfs:seeAlso>
        <skos:definition xml:lang="en">Fragrant tea made by infusing green tea leaves with jasmine flowers, known for its floral aroma.</skos:definition>
        <skos:prefLabel xml:lang="en">Jasmine Tea</skos:prefLabel>
    </owl:NamedIndividual>
    


    <!-- http://www.foodpairing.com/ontologies/foodpairing-kg#001624 -->


    <owl:NamedIndividual rdf:about="http://www.foodpairing.com/ontologies/foodpairing-kg#001624">
        <rdf:type rdf:resource="http://www.foodpairing.com/ontologies/foodpairing-kg#Ingredient"/>
        <foodpairing-kg:hasIngredientCategory rdf:resource="http://www.foodpairing.com/ontologies/foodpairing-kg#icat:000072"/>
        <rdfs:seeAlso rdf:datatype="http://www.w3.org/2001/XMLSchema#anyURI">http://www.wikidata.org/entity/Q374</rdfs:seeAlso>
        <skos:definition xml:lang="en">Colorless and flavorless distilled spirit made from fermented grains or potatoes, commonly used in cocktails.</skos:definition>
        <skos:prefLabel xml:lang="en">Vodka</skos:prefLabel>
    </owl:NamedIndividual>
    


    <!-- http://www.foodpairing.com/ontologies/foodpairing-kg#001696 -->


    <owl:NamedIndividual rdf:about="http://www.foodpairing.com/ontologies/foodpairing-kg#001696">
        <rdf:type rdf:resource="http://www.foodpairing.com/ontologies/foodpairing-kg#Ingredient"/>
        <foodpairing-kg:hasIngredientCategory rdf:resource="http://www.foodpairing.com/ontologies/foodpairing-kg#icat:000088"/>
        <rdfs:seeAlso rdf:datatype="http://www.w3.org/2001/XMLSchema#anyURI">http://www.wikidata.org/entity/Q10978</rdfs:seeAlso>
        <skos:definition xml:lang="en">Grapes are small, round fruits with a sweet and juicy flavor, commonly eaten fresh or used for making wine.</skos:definition>
        <skos:prefLabel xml:lang="en">Grape</skos:prefLabel>
    </owl:NamedIndividual>
    


    <!-- http://www.foodpairing.com/ontologies/foodpairing-kg#001755 -->


    <owl:NamedIndividual rdf:about="http://www.foodpairing.com/ontologies/foodpairing-kg#001755">
        <rdf:type rdf:resource="http://www.foodpairing.com/ontologies/foodpairing-kg#Ingredient"/>
        <foodpairing-kg:hasIngredientCategory rdf:resource="http://www.foodpairing.com/ontologies/foodpairing-kg#icat:000066"/>
        <rdfs:seeAlso rdf:datatype="http://www.w3.org/2001/XMLSchema#anyURI">http://www.wikidata.org/entity/Q1051699</rdfs:seeAlso>
        <skos:definition xml:lang="en">Cava is a sparkling wine from Catalonia, Spain, known for its crisp and effervescent quality.</skos:definition>
        <skos:prefLabel xml:lang="en">Cava</skos:prefLabel>
    </owl:NamedIndividual>
    


    <!-- http://www.foodpairing.com/ontologies/foodpairing-kg#001959 -->


    <owl:NamedIndividual rdf:about="http://www.foodpairing.com/ontologies/foodpairing-kg#001959">
        <rdf:type rdf:resource="http://www.foodpairing.com/ontologies/foodpairing-kg#Ingredient"/>
        <foodpairing-kg:hasIngredientCategory rdf:resource="http://www.foodpairing.com/ontologies/foodpairing-kg#icat:000067"/>
        <rdfs:seeAlso rdf:datatype="http://www.w3.org/2001/XMLSchema#anyURI">http://www.wikidata.org/entity/Q693078</rdfs:seeAlso>
        <skos:definition xml:lang="en">Grappa is an Italian brandy made from grape pomace, known for its strong and distinctive flavor.</skos:definition>
        <skos:prefLabel xml:lang="en">Grappa</skos:prefLabel>
    </owl:NamedIndividual>
    


    <!-- http://www.foodpairing.com/ontologies/foodpairing-kg#001968 -->


    <owl:NamedIndividual rdf:about="http://www.foodpairing.com/ontologies/foodpairing-kg#001968">
        <rdf:type rdf:resource="http://www.foodpairing.com/ontologies/foodpairing-kg#Ingredient"/>
        <foodpairing-kg:hasIngredientCategory rdf:resource="http://www.foodpairing.com/ontologies/foodpairing-kg#icat:000068"/>
        <rdfs:seeAlso rdf:datatype="http://www.w3.org/2001/XMLSchema#anyURI">http://www.wikidata.org/entity/Q16976</rdfs:seeAlso>
        <skos:definition xml:lang="en">Pastis is an anise-flavored liqueur from France, commonly diluted with water before consumption.</skos:definition>
        <skos:prefLabel xml:lang="en">Pastis</skos:prefLabel>
    </owl:NamedIndividual>
    


    <!-- http://www.foodpairing.com/ontologies/foodpairing-kg#002530 -->


    <owl:NamedIndividual rdf:about="http://www.foodpairing.com/ontologies/foodpairing-kg#002530">
        <rdf:type rdf:resource="http://www.foodpairing.com/ontologies/foodpairing-kg#Ingredient"/>
        <foodpairing-kg:hasIngredientCategory rdf:resource="http://www.foodpairing.com/ontologies/foodpairing-kg#icat:000026"/>
        <rdfs:seeAlso rdf:datatype="http://www.w3.org/2001/XMLSchema#anyURI">http://www.wikidata.org/entity/Q7802</rdfs:seeAlso>
        <skos:definition xml:lang="en">Staple food made from flour, water, and yeast, commonly baked and consumed worldwide.</skos:definition>
        <skos:prefLabel xml:lang="en">Bread</skos:prefLabel>
    </owl:NamedIndividual>
    


    <!-- http://www.foodpairing.com/ontologies/foodpairing-kg#003143 -->


    <owl:NamedIndividual rdf:about="http://www.foodpairing.com/ontologies/foodpairing-kg#003143">
        <rdf:type rdf:resource="http://www.foodpairing.com/ontologies/foodpairing-kg#Ingredient"/>
        <foodpairing-kg:hasIngredientCategory rdf:resource="http://www.foodpairing.com/ontologies/foodpairing-kg#icat:000053"/>
        <rdfs:seeAlso rdf:datatype="http://www.w3.org/2001/XMLSchema#anyURI">http://www.wikidata.org/entity/Q1245530</rdfs:seeAlso>
        <skos:definition xml:lang="en">French blue cheese known for its creamy texture and distinctive blue veining.</skos:definition>
        <skos:prefLabel xml:lang="en">Fourme D&apos;Ambert</skos:prefLabel>
    </owl:NamedIndividual>
    


    <!-- http://www.foodpairing.com/ontologies/foodpairing-kg#003246 -->


    <owl:NamedIndividual rdf:about="http://www.foodpairing.com/ontologies/foodpairing-kg#003246">
        <rdf:type rdf:resource="http://www.foodpairing.com/ontologies/foodpairing-kg#Ingredient"/>
        <foodpairing-kg:hasIngredientCategory rdf:resource="http://www.foodpairing.com/ontologies/foodpairing-kg#icat:000054"/>
        <rdfs:seeAlso rdf:datatype="http://www.w3.org/2001/XMLSchema#anyURI">http://www.wikidata.org/entity/Q14088</rdfs:seeAlso>
        <skos:definition xml:lang="en">Soft, mild cheese made from cow&apos;s milk, commonly used in salads and pizzas.</skos:definition>
        <skos:prefLabel xml:lang="en">Cow Mozzarella</skos:prefLabel>
    </owl:NamedIndividual>
    


    <!-- http://www.foodpairing.com/ontologies/foodpairing-kg#003290 -->


    <owl:NamedIndividual rdf:about="http://www.foodpairing.com/ontologies/foodpairing-kg#003290">
        <rdf:type rdf:resource="http://www.foodpairing.com/ontologies/foodpairing-kg#Ingredient"/>
        <foodpairing-kg:hasIngredientCategory rdf:resource="http://www.foodpairing.com/ontologies/foodpairing-kg#icat:000059"/>
        <rdfs:seeAlso rdf:datatype="http://www.w3.org/2001/XMLSchema#anyURI">http://www.wikidata.org/entity/Q193411</rdfs:seeAlso>
        <skos:definition xml:lang="en">Brie is a soft, creamy cheese known for its mild flavor and edible rind, commonly served as an appetizer.</skos:definition>
        <skos:prefLabel xml:lang="en">Brie</skos:prefLabel>
    </owl:NamedIndividual>
    


    <!-- http://www.foodpairing.com/ontologies/foodpairing-kg#005483 -->


    <owl:NamedIndividual rdf:about="http://www.foodpairing.com/ontologies/foodpairing-kg#005483">
        <rdf:type rdf:resource="http://www.foodpairing.com/ontologies/foodpairing-kg#Ingredient"/>
        <foodpairing-kg:hasIngredientCategory rdf:resource="http://www.foodpairing.com/ontologies/foodpairing-kg#icat:000135"/>
        <rdfs:seeAlso rdf:datatype="http://www.w3.org/2001/XMLSchema#anyURI">http://www.wikidata.org/entity/Q104212</rdfs:seeAlso>
        <skos:definition xml:lang="en">Young, edible shoots of the hop plant, known for their mild and slightly bitter flavor.</skos:definition>
        <skos:prefLabel xml:lang="en">Humulus Shoot</skos:prefLabel>
    </owl:NamedIndividual>
    


    <!-- http://www.foodpairing.com/ontologies/foodpairing-kg#005509 -->


    <owl:NamedIndividual rdf:about="http://www.foodpairing.com/ontologies/foodpairing-kg#005509">
        <rdf:type rdf:resource="http://www.foodpairing.com/ontologies/foodpairing-kg#Ingredient"/>
        <foodpairing-kg:hasIngredientCategory rdf:resource="http://www.foodpairing.com/ontologies/foodpairing-kg#icat:000033"/>
        <rdfs:seeAlso rdf:datatype="http://www.w3.org/2001/XMLSchema#anyURI">http://www.wikidata.org/entity/Q67594028</rdfs:seeAlso>
        <skos:definition xml:lang="en">Rice grains that have been cooked in boiling water, resulting in a fluffy and separate texture.</skos:definition>
        <skos:prefLabel xml:lang="en">Long-Grain Rice</skos:prefLabel>
    </owl:NamedIndividual>
    


    <!-- http://www.foodpairing.com/ontologies/foodpairing-kg#005545 -->


    <owl:NamedIndividual rdf:about="http://www.foodpairing.com/ontologies/foodpairing-kg#005545">
        <rdf:type rdf:resource="http://www.foodpairing.com/ontologies/foodpairing-kg#Ingredient"/>
        <foodpairing-kg:hasIngredientCategory rdf:resource="http://www.foodpairing.com/ontologies/foodpairing-kg#icat:000109"/>
        <rdfs:seeAlso rdf:datatype="http://www.w3.org/2001/XMLSchema#anyURI">http://www.wikidata.org/entity/Q27855</rdfs:seeAlso>
        <skos:definition xml:lang="en">Shellfish with tender, sweet meat, commonly steamed or cooked in various sauces, appreciated for their delicate sea flavor.</skos:definition>
        <skos:prefLabel xml:lang="en">Mussel</skos:prefLabel>
    </owl:NamedIndividual>
    


    <!-- http://www.foodpairing.com/ontologies/foodpairing-kg#005569 -->


    <owl:NamedIndividual rdf:about="http://www.foodpairing.com/ontologies/foodpairing-kg#005569">
        <rdf:type rdf:resource="http://www.foodpairing.com/ontologies/foodpairing-kg#Ingredient"/>
        <foodpairing-kg:hasIngredientCategory rdf:resource="http://www.foodpairing.com/ontologies/foodpairing-kg#icat:000091"/>
        <rdfs:seeAlso rdf:datatype="http://www.w3.org/2001/XMLSchema#anyURI">http://www.wikidata.org/entity/Q13099586</rdfs:seeAlso>
        <skos:definition xml:lang="en">Juicy, sweet fruits with a crisp texture, commonly eaten fresh or used in desserts.</skos:definition>
        <skos:prefLabel xml:lang="en">Pear</skos:prefLabel>
    </owl:NamedIndividual>
    


    <!-- http://www.foodpairing.com/ontologies/foodpairing-kg#005622 -->


    <owl:NamedIndividual rdf:about="http://www.foodpairing.com/ontologies/foodpairing-kg#005622">
        <rdf:type rdf:resource="http://www.foodpairing.com/ontologies/foodpairing-kg#Ingredient"/>
        <foodpairing-kg:hasIngredientCategory rdf:resource="http://www.foodpairing.com/ontologies/foodpairing-kg#icat:000109"/>
        <rdfs:seeAlso rdf:datatype="http://www.w3.org/2001/XMLSchema#anyURI">http://www.wikidata.org/entity/Q1311395</rdfs:seeAlso>
        <skos:definition xml:lang="en">A type of shellfish known for its sweet and delicate flavor, commonly eaten raw.</skos:definition>
        <skos:prefLabel xml:lang="en">Scallop Saint Jacques</skos:prefLabel>
    </owl:NamedIndividual>
    


    <!-- http://www.foodpairing.com/ontologies/foodpairing-kg#005675 -->


    <owl:NamedIndividual rdf:about="http://www.foodpairing.com/ontologies/foodpairing-kg#005675">
        <rdf:type rdf:resource="http://www.foodpairing.com/ontologies/foodpairing-kg#Ingredient"/>
        <foodpairing-kg:hasIngredientCategory rdf:resource="http://www.foodpairing.com/ontologies/foodpairing-kg#icat:000107"/>
        <rdfs:seeAlso rdf:datatype="http://www.w3.org/2001/XMLSchema#anyURI">http://www.wikidata.org/entity/Q4200953</rdfs:seeAlso>
        <skos:definition xml:lang="en">Turkey meat is lean, white poultry with a mild, slightly gamey flavor, commonly roasted, grilled, or used in a variety of dishes.</skos:definition>
        <skos:prefLabel xml:lang="en">Turkey</skos:prefLabel>
    </owl:NamedIndividual>
    


    <!-- http://www.foodpairing.com/ontologies/foodpairing-kg#005754 -->


    <owl:NamedIndividual rdf:about="http://www.foodpairing.com/ontologies/foodpairing-kg#005754">
        <rdf:type rdf:resource="http://www.foodpairing.com/ontologies/foodpairing-kg#Ingredient"/>
        <foodpairing-kg:hasIngredientCategory rdf:resource="http://www.foodpairing.com/ontologies/foodpairing-kg#icat:000107"/>
        <rdfs:seeAlso rdf:datatype="http://www.w3.org/2001/XMLSchema#anyURI">http://www.wikidata.org/entity/Q6663</rdfs:seeAlso>
        <skos:definition xml:lang="en">Ground meat formed into a patty and cooked in an oven, resulting in a flavorful and juicy burger.</skos:definition>
        <skos:prefLabel xml:lang="en">Hamburger</skos:prefLabel>
    </owl:NamedIndividual>
    


    <!-- http://www.foodpairing.com/ontologies/foodpairing-kg#005760 -->


    <owl:NamedIndividual rdf:about="http://www.foodpairing.com/ontologies/foodpairing-kg#005760">
        <rdf:type rdf:resource="http://www.foodpairing.com/ontologies/foodpairing-kg#Ingredient"/>
        <foodpairing-kg:hasIngredientCategory rdf:resource="http://www.foodpairing.com/ontologies/foodpairing-kg#icat:000107"/>
        <rdfs:seeAlso rdf:datatype="http://www.w3.org/2001/XMLSchema#anyURI">http://www.wikidata.org/entity/Q957434</rdfs:seeAlso>
        <skos:definition xml:lang="en">Veal is tender, pale-pink meat from young calves, prized for its delicate flavor and tenderness, commonly used in gourmet cuisine.</skos:definition>
        <skos:prefLabel xml:lang="en">Veal</skos:prefLabel>
    </owl:NamedIndividual>
    


    <!-- http://www.foodpairing.com/ontologies/foodpairing-kg#005842 -->


    <owl:NamedIndividual rdf:about="http://www.foodpairing.com/ontologies/foodpairing-kg#005842">
        <rdf:type rdf:resource="http://www.foodpairing.com/ontologies/foodpairing-kg#Ingredient"/>
        <foodpairing-kg:hasIngredientCategory rdf:resource="http://www.foodpairing.com/ontologies/foodpairing-kg#icat:000127"/>
        <rdfs:seeAlso rdf:datatype="http://www.w3.org/2001/XMLSchema#anyURI">http://www.wikidata.org/entity/Q21546392</rdfs:seeAlso>
        <skos:definition xml:lang="en">Smooth, concentrated paste made from roasted garlic cloves, providing a mellow, aromatic essence to a wide range of recipes.</skos:definition>
        <skos:prefLabel xml:lang="en">Garlic Puree</skos:prefLabel>
    </owl:NamedIndividual>
    


    <!-- http://www.foodpairing.com/ontologies/foodpairing-kg#005930 -->


    <owl:NamedIndividual rdf:about="http://www.foodpairing.com/ontologies/foodpairing-kg#005930">
        <rdf:type rdf:resource="http://www.foodpairing.com/ontologies/foodpairing-kg#Ingredient"/>
        <foodpairing-kg:hasIngredientCategory rdf:resource="http://www.foodpairing.com/ontologies/foodpairing-kg#icat:000050"/>
        <rdfs:seeAlso rdf:datatype="http://www.w3.org/2001/XMLSchema#anyURI">http://www.wikidata.org/entity/Q8495</rdfs:seeAlso>
        <skos:definition xml:lang="en">A white, nutrient-rich liquid produced by mammals, commonly consumed as a beverage and used in cooking.</skos:definition>
        <skos:prefLabel xml:lang="en">Milk</skos:prefLabel>
    </owl:NamedIndividual>
    


    <!-- http://www.foodpairing.com/ontologies/foodpairing-kg#005942 -->


    <owl:NamedIndividual rdf:about="http://www.foodpairing.com/ontologies/foodpairing-kg#005942">
        <rdf:type rdf:resource="http://www.foodpairing.com/ontologies/foodpairing-kg#Ingredient"/>
        <foodpairing-kg:hasIngredientCategory rdf:resource="http://www.foodpairing.com/ontologies/foodpairing-kg#icat:000026"/>
        <rdfs:seeAlso rdf:datatype="http://www.w3.org/2001/XMLSchema#anyURI">http://www.wikidata.org/entity/Q208172</rdfs:seeAlso>
        <skos:definition xml:lang="en">A long, slender loaf of French bread known for its crisp crust and soft interior.</skos:definition>
        <skos:prefLabel xml:lang="en">Baguette</skos:prefLabel>
    </owl:NamedIndividual>
    


    <!-- http://www.foodpairing.com/ontologies/foodpairing-kg#006002 -->


    <owl:NamedIndividual rdf:about="http://www.foodpairing.com/ontologies/foodpairing-kg#006002">
        <rdf:type rdf:resource="http://www.foodpairing.com/ontologies/foodpairing-kg#Ingredient"/>
        <foodpairing-kg:hasIngredientCategory rdf:resource="http://www.foodpairing.com/ontologies/foodpairing-kg#icat:000034"/>
        <rdfs:seeAlso rdf:datatype="http://www.w3.org/2001/XMLSchema#anyURI">http://www.wikidata.org/entity/Q178</rdfs:seeAlso>
        <skos:definition xml:lang="en">Pasta noodles that have been cooked in boiling water, resulting in a tender and chewy texture.</skos:definition>
        <skos:prefLabel xml:lang="en">Pasta</skos:prefLabel>
    </owl:NamedIndividual>
    


    <!-- http://www.foodpairing.com/ontologies/foodpairing-kg#006471 -->


    <owl:NamedIndividual rdf:about="http://www.foodpairing.com/ontologies/foodpairing-kg#006471">
        <rdf:type rdf:resource="http://www.foodpairing.com/ontologies/foodpairing-kg#Ingredient"/>
        <foodpairing-kg:hasIngredientCategory rdf:resource="http://www.foodpairing.com/ontologies/foodpairing-kg#icat:000132"/>
        <rdfs:seeAlso rdf:datatype="http://www.w3.org/2001/XMLSchema#anyURI">http://www.wikidata.org/entity/Q81</rdfs:seeAlso>
        <skos:definition xml:lang="en">Crunchy, orange root vegetables with a sweet and earthy flavor, commonly eaten fresh.</skos:definition>
        <skos:prefLabel xml:lang="en">Carrot</skos:prefLabel>
    </owl:NamedIndividual>
    


    <!-- http://www.foodpairing.com/ontologies/foodpairing-kg#006473 -->


    <owl:NamedIndividual rdf:about="http://www.foodpairing.com/ontologies/foodpairing-kg#006473">
        <rdf:type rdf:resource="http://www.foodpairing.com/ontologies/foodpairing-kg#Ingredient"/>
        <foodpairing-kg:hasIngredientCategory rdf:resource="http://www.foodpairing.com/ontologies/foodpairing-kg#icat:000109"/>
        <rdfs:seeAlso rdf:datatype="http://www.w3.org/2001/XMLSchema#anyURI">http://www.wikidata.org/entity/Q1747334</rdfs:seeAlso>
        <skos:definition xml:lang="en">Shellfish known for their delicate and briny flavor, commonly eaten raw or cooked.</skos:definition>
        <skos:prefLabel xml:lang="en">Oyster</skos:prefLabel>
    </owl:NamedIndividual>
    


    <!-- http://www.foodpairing.com/ontologies/foodpairing-kg#006821 -->


    <owl:NamedIndividual rdf:about="http://www.foodpairing.com/ontologies/foodpairing-kg#006821">
        <rdf:type rdf:resource="http://www.foodpairing.com/ontologies/foodpairing-kg#Ingredient"/>
        <foodpairing-kg:hasIngredientCategory rdf:resource="http://www.foodpairing.com/ontologies/foodpairing-kg#icat:000004"/>
        <rdfs:seeAlso rdf:datatype="http://www.w3.org/2001/XMLSchema#anyURI">http://www.wikidata.org/entity/Q277628</rdfs:seeAlso>
        <skos:definition xml:lang="en">Rich and bittersweet chocolate made from cocoa solids and sugar, known for its complex flavor profiles.</skos:definition>
        <skos:prefLabel xml:lang="en">Dark Chocolate</skos:prefLabel>
    </owl:NamedIndividual>
    


    <!-- http://www.foodpairing.com/ontologies/foodpairing-kg#007088 -->


    <owl:NamedIndividual rdf:about="http://www.foodpairing.com/ontologies/foodpairing-kg#007088">
        <rdf:type rdf:resource="http://www.foodpairing.com/ontologies/foodpairing-kg#Ingredient"/>
        <foodpairing-kg:hasIngredientCategory rdf:resource="http://www.foodpairing.com/ontologies/foodpairing-kg#icat:000067"/>
        <rdfs:seeAlso rdf:datatype="http://www.w3.org/2001/XMLSchema#anyURI">http://www.wikidata.org/entity/Q503252</rdfs:seeAlso>
        <skos:definition xml:lang="en">Armagnac is a French brandy from the Gascony region, known for its robust and fruity flavor.</skos:definition>
        <skos:prefLabel xml:lang="en">Armagnac</skos:prefLabel>
    </owl:NamedIndividual>
    


    <!-- http://www.foodpairing.com/ontologies/foodpairing-kg#007105 -->


    <owl:NamedIndividual rdf:about="http://www.foodpairing.com/ontologies/foodpairing-kg#007105">
        <rdf:type rdf:resource="http://www.foodpairing.com/ontologies/foodpairing-kg#Ingredient"/>
        <foodpairing-kg:hasIngredientCategory rdf:resource="http://www.foodpairing.com/ontologies/foodpairing-kg#icat:000125"/>
        <rdfs:seeAlso rdf:datatype="http://www.w3.org/2001/XMLSchema#anyURI">http://www.wikidata.org/entity/Q10403913</rdfs:seeAlso>
        <skos:definition xml:lang="en">Light-colored, mild-flavored honey produced by bees that collect nectar from acacia flowers.</skos:definition>
        <skos:prefLabel xml:lang="en">Acacia Honey</skos:prefLabel>
    </owl:NamedIndividual>
    


    <!-- http://www.foodpairing.com/ontologies/foodpairing-kg#007109 -->


    <owl:NamedIndividual rdf:about="http://www.foodpairing.com/ontologies/foodpairing-kg#007109">
        <rdf:type rdf:resource="http://www.foodpairing.com/ontologies/foodpairing-kg#Ingredient"/>
        <foodpairing-kg:hasIngredientCategory rdf:resource="http://www.foodpairing.com/ontologies/foodpairing-kg#icat:000093"/>
        <rdfs:seeAlso rdf:datatype="http://www.w3.org/2001/XMLSchema#anyURI">http://www.wikidata.org/entity/Q2746643</rdfs:seeAlso>
        <skos:definition xml:lang="en">Sweet, pear-shaped fruits with a unique texture and a mildly sweet flavor.</skos:definition>
        <skos:prefLabel xml:lang="en">Fig</skos:prefLabel>
    </owl:NamedIndividual>
    


    <!-- http://www.foodpairing.com/ontologies/foodpairing-kg#007170 -->


    <owl:NamedIndividual rdf:about="http://www.foodpairing.com/ontologies/foodpairing-kg#007170">
        <rdf:type rdf:resource="http://www.foodpairing.com/ontologies/foodpairing-kg#Ingredient"/>
        <foodpairing-kg:hasIngredientCategory rdf:resource="http://www.foodpairing.com/ontologies/foodpairing-kg#icat:000069"/>
        <rdfs:seeAlso rdf:datatype="http://www.w3.org/2001/XMLSchema#anyURI">http://www.wikidata.org/entity/Q122195</rdfs:seeAlso>
        <skos:definition xml:lang="en">A type of tequila known for its clear color and pure, unaged flavor.</skos:definition>
        <skos:prefLabel xml:lang="en">Tequila Silver</skos:prefLabel>
    </owl:NamedIndividual>
    


    <!-- http://www.foodpairing.com/ontologies/foodpairing-kg#008970 -->


    <owl:NamedIndividual rdf:about="http://www.foodpairing.com/ontologies/foodpairing-kg#008970">
        <rdf:type rdf:resource="http://www.foodpairing.com/ontologies/foodpairing-kg#Ingredient"/>
        <foodpairing-kg:hasIngredientCategory rdf:resource="http://www.foodpairing.com/ontologies/foodpairing-kg#icat:000074"/>
        <rdfs:seeAlso rdf:datatype="http://www.w3.org/2001/XMLSchema#anyURI">http://www.wikidata.org/entity/Q1155703</rdfs:seeAlso>
        <skos:definition xml:lang="en">Beverage made by steeping ground coffee beans in hot water, known for its stimulating effect.</skos:definition>
        <skos:prefLabel xml:lang="en">Brewed Coffee</skos:prefLabel>
    </owl:NamedIndividual>
    


    <!-- http://www.foodpairing.com/ontologies/foodpairing-kg#icat:000001 -->


    <owl:NamedIndividual rdf:about="http://www.foodpairing.com/ontologies/foodpairing-kg#icat:000001">
        <rdf:type rdf:resource="http://www.foodpairing.com/ontologies/foodpairing-kg#IngredientCategory"/>
        <rdf:type rdf:resource="http://www.w3.org/2004/02/skos/core#Concept"/>
        <skos:definition xml:lang="en">Includes various baked goods like bread, cookies, cakes, pastries, and viennoiserie.</skos:definition>
        <skos:prefLabel xml:lang="en">Bakery Category</skos:prefLabel>
    </owl:NamedIndividual>
    


    <!-- http://www.foodpairing.com/ontologies/foodpairing-kg#icat:000002 -->


    <owl:NamedIndividual rdf:about="http://www.foodpairing.com/ontologies/foodpairing-kg#icat:000002">
        <rdf:type rdf:resource="http://www.foodpairing.com/ontologies/foodpairing-kg#IngredientCategory"/>
        <rdf:type rdf:resource="http://www.w3.org/2004/02/skos/core#Concept"/>
        <skos:definition xml:lang="en">Refers to grains and breakfast cereals such as oats, rice, pasta, and other grain-based products.</skos:definition>
        <skos:prefLabel xml:lang="en">Cereals Category</skos:prefLabel>
    </owl:NamedIndividual>
    


    <!-- http://www.foodpairing.com/ontologies/foodpairing-kg#icat:000003 -->


    <owl:NamedIndividual rdf:about="http://www.foodpairing.com/ontologies/foodpairing-kg#icat:000003">
        <rdf:type rdf:resource="http://www.foodpairing.com/ontologies/foodpairing-kg#IngredientCategory"/>
        <rdf:type rdf:resource="http://www.w3.org/2004/02/skos/core#Concept"/>
        <skos:definition xml:lang="en">Relates to sensory aspects and flavors associated with cigarettes.</skos:definition>
        <skos:prefLabel xml:lang="en">Cigarette Sensory Category</skos:prefLabel>
    </owl:NamedIndividual>
    


    <!-- http://www.foodpairing.com/ontologies/foodpairing-kg#icat:000004 -->


    <owl:NamedIndividual rdf:about="http://www.foodpairing.com/ontologies/foodpairing-kg#icat:000004">
        <rdf:type rdf:resource="http://www.foodpairing.com/ontologies/foodpairing-kg#IngredientCategory"/>
        <rdf:type rdf:resource="http://www.w3.org/2004/02/skos/core#Concept"/>
        <skos:definition xml:lang="en">Encompasses products made from or containing chocolate, including confections and desserts.</skos:definition>
        <skos:prefLabel xml:lang="en">Chocolate Category</skos:prefLabel>
    </owl:NamedIndividual>
    


    <!-- http://www.foodpairing.com/ontologies/foodpairing-kg#icat:000005 -->


    <owl:NamedIndividual rdf:about="http://www.foodpairing.com/ontologies/foodpairing-kg#icat:000005">
        <rdf:type rdf:resource="http://www.foodpairing.com/ontologies/foodpairing-kg#IngredientCategory"/>
        <rdf:type rdf:resource="http://www.w3.org/2004/02/skos/core#Concept"/>
        <skos:definition xml:lang="en">Includes various sauces, dips, spreads, and pickled products used to enhance the flavor of food.</skos:definition>
        <skos:prefLabel xml:lang="en">Condiments Category</skos:prefLabel>
    </owl:NamedIndividual>
    


    <!-- http://www.foodpairing.com/ontologies/foodpairing-kg#icat:000006 -->


    <owl:NamedIndividual rdf:about="http://www.foodpairing.com/ontologies/foodpairing-kg#icat:000006">
        <rdf:type rdf:resource="http://www.foodpairing.com/ontologies/foodpairing-kg#IngredientCategory"/>
        <rdf:type rdf:resource="http://www.w3.org/2004/02/skos/core#Concept"/>
        <skos:definition xml:lang="en">Encompasses sweet treats like chocolate confections, milk confections, sugar confections, and fruit confections.</skos:definition>
        <skos:prefLabel xml:lang="en">Confectionary Category</skos:prefLabel>
    </owl:NamedIndividual>
    


    <!-- http://www.foodpairing.com/ontologies/foodpairing-kg#icat:000007 -->


    <owl:NamedIndividual rdf:about="http://www.foodpairing.com/ontologies/foodpairing-kg#icat:000007">
        <rdf:type rdf:resource="http://www.foodpairing.com/ontologies/foodpairing-kg#IngredientCategory"/>
        <rdf:type rdf:resource="http://www.w3.org/2004/02/skos/core#Concept"/>
        <skos:definition xml:lang="en">Involves dairy products like butter, cheese, cream, milk, plant-based dairy alternatives, and yogurt.</skos:definition>
        <skos:prefLabel xml:lang="en">Dairy Category</skos:prefLabel>
    </owl:NamedIndividual>
    


    <!-- http://www.foodpairing.com/ontologies/foodpairing-kg#icat:000008 -->


    <owl:NamedIndividual rdf:about="http://www.foodpairing.com/ontologies/foodpairing-kg#icat:000008">
        <rdf:type rdf:resource="http://www.foodpairing.com/ontologies/foodpairing-kg#IngredientCategory"/>
        <rdf:type rdf:resource="http://www.w3.org/2004/02/skos/core#Concept"/>
        <skos:definition xml:lang="en">Relates to sweet dishes, cakes, pastries, and other treats typically consumed after a meal.</skos:definition>
        <skos:prefLabel xml:lang="en">Dessert Category</skos:prefLabel>
    </owl:NamedIndividual>
    


    <!-- http://www.foodpairing.com/ontologies/foodpairing-kg#icat:000009 -->


    <owl:NamedIndividual rdf:about="http://www.foodpairing.com/ontologies/foodpairing-kg#icat:000009">
        <rdf:type rdf:resource="http://www.foodpairing.com/ontologies/foodpairing-kg#IngredientCategory"/>
        <rdf:type rdf:resource="http://www.w3.org/2004/02/skos/core#Concept"/>
        <skos:definition xml:lang="en">Refers to a wide range of beverages, including alcoholic and non-alcoholic drinks like juices, soft drinks, coffee, tea, and flavored waters.</skos:definition>
        <skos:prefLabel xml:lang="en">Drinks Category</skos:prefLabel>
    </owl:NamedIndividual>
    


    <!-- http://www.foodpairing.com/ontologies/foodpairing-kg#icat:000010 -->


    <owl:NamedIndividual rdf:about="http://www.foodpairing.com/ontologies/foodpairing-kg#icat:000010">
        <rdf:type rdf:resource="http://www.foodpairing.com/ontologies/foodpairing-kg#IngredientCategory"/>
        <rdf:type rdf:resource="http://www.w3.org/2004/02/skos/core#Concept"/>
        <skos:definition xml:lang="en">Pertains to liquids used in electronic cigarettes or vaping devices for inhalation.</skos:definition>
        <skos:prefLabel xml:lang="en">E Liquids Category</skos:prefLabel>
    </owl:NamedIndividual>
    


    <!-- http://www.foodpairing.com/ontologies/foodpairing-kg#icat:000011 -->


    <owl:NamedIndividual rdf:about="http://www.foodpairing.com/ontologies/foodpairing-kg#icat:000011">
        <rdf:type rdf:resource="http://www.foodpairing.com/ontologies/foodpairing-kg#IngredientCategory"/>
        <rdf:type rdf:resource="http://www.w3.org/2004/02/skos/core#Concept"/>
        <skos:definition xml:lang="en">Encompasses various fats and oils used in cooking and food preparation.</skos:definition>
        <skos:prefLabel xml:lang="en">Fats And Oils Category</skos:prefLabel>
    </owl:NamedIndividual>
    


    <!-- http://www.foodpairing.com/ontologies/foodpairing-kg#icat:000012 -->


    <owl:NamedIndividual rdf:about="http://www.foodpairing.com/ontologies/foodpairing-kg#icat:000012">
        <rdf:type rdf:resource="http://www.foodpairing.com/ontologies/foodpairing-kg#IngredientCategory"/>
        <rdf:type rdf:resource="http://www.w3.org/2004/02/skos/core#Concept"/>
        <skos:definition xml:lang="en">Includes substances added to food for various purposes like flavoring, coloring, preservation, and texture enhancement.</skos:definition>
        <skos:prefLabel xml:lang="en">Food Additives Category</skos:prefLabel>
    </owl:NamedIndividual>
    


    <!-- http://www.foodpairing.com/ontologies/foodpairing-kg#icat:000013 -->


    <owl:NamedIndividual rdf:about="http://www.foodpairing.com/ontologies/foodpairing-kg#icat:000013">
        <rdf:type rdf:resource="http://www.foodpairing.com/ontologies/foodpairing-kg#IngredientCategory"/>
        <rdf:type rdf:resource="http://www.w3.org/2004/02/skos/core#Concept"/>
        <skos:definition xml:lang="en">Relates to edible flowers used in cooking, garnishing, or flavoring food and beverages.</skos:definition>
        <skos:prefLabel xml:lang="en">Flowers Category</skos:prefLabel>
    </owl:NamedIndividual>
    


    <!-- http://www.foodpairing.com/ontologies/foodpairing-kg#icat:000014 -->


    <owl:NamedIndividual rdf:about="http://www.foodpairing.com/ontologies/foodpairing-kg#icat:000014">
        <rdf:type rdf:resource="http://www.foodpairing.com/ontologies/foodpairing-kg#IngredientCategory"/>
        <rdf:type rdf:resource="http://www.w3.org/2004/02/skos/core#Concept"/>
        <skos:definition xml:lang="en">Refers to a diverse range of fruits, including citrus fruits, berries, tropical fruits, and other fruit varieties.</skos:definition>
        <skos:prefLabel xml:lang="en">Fruit Category</skos:prefLabel>
    </owl:NamedIndividual>
    


    <!-- http://www.foodpairing.com/ontologies/foodpairing-kg#icat:000015 -->


    <owl:NamedIndividual rdf:about="http://www.foodpairing.com/ontologies/foodpairing-kg#icat:000015">
        <rdf:type rdf:resource="http://www.foodpairing.com/ontologies/foodpairing-kg#IngredientCategory"/>
        <rdf:type rdf:resource="http://www.w3.org/2004/02/skos/core#Concept"/>
        <skos:definition xml:lang="en">Encompasses culinary and medicinal herbs used for flavoring, garnishing, or as natural remedies.</skos:definition>
        <skos:prefLabel xml:lang="en">Herbs Category</skos:prefLabel>
    </owl:NamedIndividual>
    


    <!-- http://www.foodpairing.com/ontologies/foodpairing-kg#icat:000016 -->


    <owl:NamedIndividual rdf:about="http://www.foodpairing.com/ontologies/foodpairing-kg#icat:000016">
        <rdf:type rdf:resource="http://www.foodpairing.com/ontologies/foodpairing-kg#IngredientCategory"/>
        <rdf:type rdf:resource="http://www.w3.org/2004/02/skos/core#Concept"/>
        <skos:definition xml:lang="en">Relates to items or substances not intended for human consumption, such as non-edible products or materials.</skos:definition>
        <skos:prefLabel xml:lang="en">Non-food Category</skos:prefLabel>
    </owl:NamedIndividual>
    


    <!-- http://www.foodpairing.com/ontologies/foodpairing-kg#icat:000017 -->


    <owl:NamedIndividual rdf:about="http://www.foodpairing.com/ontologies/foodpairing-kg#icat:000017">
        <rdf:type rdf:resource="http://www.foodpairing.com/ontologies/foodpairing-kg#IngredientCategory"/>
        <rdf:type rdf:resource="http://www.w3.org/2004/02/skos/core#Concept"/>
        <skos:definition xml:lang="en">Includes various types of nuts and seeds used as ingredients or snacks.</skos:definition>
        <skos:prefLabel xml:lang="en">Nuts And Seeds Category</skos:prefLabel>
    </owl:NamedIndividual>
    


    <!-- http://www.foodpairing.com/ontologies/foodpairing-kg#icat:000018 -->


    <owl:NamedIndividual rdf:about="http://www.foodpairing.com/ontologies/foodpairing-kg#icat:000018">
        <rdf:type rdf:resource="http://www.foodpairing.com/ontologies/foodpairing-kg#IngredientCategory"/>
        <rdf:type rdf:resource="http://www.w3.org/2004/02/skos/core#Concept"/>
        <skos:definition xml:lang="en">Relates to sensory aspects not covered by other specific categories</skos:definition>
        <skos:prefLabel xml:lang="en">Other Sensory Category</skos:prefLabel>
    </owl:NamedIndividual>
    


    <!-- http://www.foodpairing.com/ontologies/foodpairing-kg#icat:000019 -->


    <owl:NamedIndividual rdf:about="http://www.foodpairing.com/ontologies/foodpairing-kg#icat:000019">
        <rdf:type rdf:resource="http://www.foodpairing.com/ontologies/foodpairing-kg#IngredientCategory"/>
        <rdf:type rdf:resource="http://www.w3.org/2004/02/skos/core#Concept"/>
        <skos:definition xml:lang="en">Refers to protein-rich foods such as meat, fish, seafood, plant-based proteins, and insect-based products.</skos:definition>
        <skos:prefLabel xml:lang="en">Protein Category</skos:prefLabel>
    </owl:NamedIndividual>
    


    <!-- http://www.foodpairing.com/ontologies/foodpairing-kg#icat:000020 -->


    <owl:NamedIndividual rdf:about="http://www.foodpairing.com/ontologies/foodpairing-kg#icat:000020">
        <rdf:type rdf:resource="http://www.foodpairing.com/ontologies/foodpairing-kg#IngredientCategory"/>
        <rdf:type rdf:resource="http://www.w3.org/2004/02/skos/core#Concept"/>
        <skos:definition xml:lang="en">Encompasses different types of sauces used for flavoring and enhancing the taste of dishes.</skos:definition>
        <skos:prefLabel xml:lang="en">Sauces Category</skos:prefLabel>
    </owl:NamedIndividual>
    


    <!-- http://www.foodpairing.com/ontologies/foodpairing-kg#icat:000021 -->


    <owl:NamedIndividual rdf:about="http://www.foodpairing.com/ontologies/foodpairing-kg#icat:000021">
        <rdf:type rdf:resource="http://www.foodpairing.com/ontologies/foodpairing-kg#IngredientCategory"/>
        <rdf:type rdf:resource="http://www.w3.org/2004/02/skos/core#Concept"/>
        <skos:definition xml:lang="en">Includes a wide range of snack foods like chips, crisps, popcorn, and rice snacks.</skos:definition>
        <skos:prefLabel xml:lang="en">Snacks Category</skos:prefLabel>
    </owl:NamedIndividual>
    


    <!-- http://www.foodpairing.com/ontologies/foodpairing-kg#icat:000022 -->


    <owl:NamedIndividual rdf:about="http://www.foodpairing.com/ontologies/foodpairing-kg#icat:000022">
        <rdf:type rdf:resource="http://www.foodpairing.com/ontologies/foodpairing-kg#IngredientCategory"/>
        <rdf:type rdf:resource="http://www.w3.org/2004/02/skos/core#Concept"/>
        <skos:definition xml:lang="en">Pertains to moist powder tobacco products, usually placed under the lip for extended periods.</skos:definition>
        <skos:prefLabel xml:lang="en">Snus Category</skos:prefLabel>
    </owl:NamedIndividual>
    


    <!-- http://www.foodpairing.com/ontologies/foodpairing-kg#icat:000023 -->


    <owl:NamedIndividual rdf:about="http://www.foodpairing.com/ontologies/foodpairing-kg#icat:000023">
        <rdf:type rdf:resource="http://www.foodpairing.com/ontologies/foodpairing-kg#IngredientCategory"/>
        <rdf:type rdf:resource="http://www.w3.org/2004/02/skos/core#Concept"/>
        <skos:definition xml:lang="en">Encompasses various spices and spice blends used to add flavor and aroma to dishes.</skos:definition>
        <skos:prefLabel xml:lang="en">Spice Category</skos:prefLabel>
    </owl:NamedIndividual>
    


    <!-- http://www.foodpairing.com/ontologies/foodpairing-kg#icat:000024 -->


    <owl:NamedIndividual rdf:about="http://www.foodpairing.com/ontologies/foodpairing-kg#icat:000024">
        <rdf:type rdf:resource="http://www.foodpairing.com/ontologies/foodpairing-kg#IngredientCategory"/>
        <rdf:type rdf:resource="http://www.w3.org/2004/02/skos/core#Concept"/>
        <skos:definition xml:lang="en">Includes sweetening agents like sugars, syrups, and artificial sweeteners used to enhance the sweetness of food and drinks.</skos:definition>
        <skos:prefLabel xml:lang="en">Sweeteners Category</skos:prefLabel>
    </owl:NamedIndividual>
    


    <!-- http://www.foodpairing.com/ontologies/foodpairing-kg#icat:000025 -->


    <owl:NamedIndividual rdf:about="http://www.foodpairing.com/ontologies/foodpairing-kg#icat:000025">
        <rdf:type rdf:resource="http://www.foodpairing.com/ontologies/foodpairing-kg#IngredientCategory"/>
        <rdf:type rdf:resource="http://www.w3.org/2004/02/skos/core#Concept"/>
        <skos:definition xml:lang="en">Refers to a wide range of edible vegetables, including bulb vegetables, leafy greens, root vegetables, and sea-grown vegetables.</skos:definition>
        <skos:prefLabel xml:lang="en">Vegetable Category</skos:prefLabel>
    </owl:NamedIndividual>
    


    <!-- http://www.foodpairing.com/ontologies/foodpairing-kg#icat:000026 -->


    <owl:NamedIndividual rdf:about="http://www.foodpairing.com/ontologies/foodpairing-kg#icat:000026">
        <rdf:type rdf:resource="http://www.foodpairing.com/ontologies/foodpairing-kg#IngredientCategory"/>
        <rdf:type rdf:resource="http://www.w3.org/2004/02/skos/core#Concept"/>
        <skos:broader rdf:resource="http://www.foodpairing.com/ontologies/foodpairing-kg#icat:000001"/>
        <skos:definition xml:lang="en">Bread is a staple food made from a combination of flour and water, along with other ingredients such as yeast, salt, and sometimes sweeteners or fats. The dough is typically baked.</skos:definition>
        <skos:prefLabel xml:lang="en">Bread</skos:prefLabel>
    </owl:NamedIndividual>
    


    <!-- http://www.foodpairing.com/ontologies/foodpairing-kg#icat:000027 -->


    <owl:NamedIndividual rdf:about="http://www.foodpairing.com/ontologies/foodpairing-kg#icat:000027">
        <rdf:type rdf:resource="http://www.foodpairing.com/ontologies/foodpairing-kg#IngredientCategory"/>
        <rdf:type rdf:resource="http://www.w3.org/2004/02/skos/core#Concept"/>
        <skos:broader rdf:resource="http://www.foodpairing.com/ontologies/foodpairing-kg#icat:000001"/>
        <skos:definition xml:lang="en">Refers to baked products made primarily from flour, water, and yeast or other leavening agents.</skos:definition>
        <skos:prefLabel xml:lang="en">Cookies And Cakes</skos:prefLabel>
    </owl:NamedIndividual>
    


    <!-- http://www.foodpairing.com/ontologies/foodpairing-kg#icat:000028 -->


    <owl:NamedIndividual rdf:about="http://www.foodpairing.com/ontologies/foodpairing-kg#icat:000028">
        <rdf:type rdf:resource="http://www.foodpairing.com/ontologies/foodpairing-kg#IngredientCategory"/>
        <rdf:type rdf:resource="http://www.w3.org/2004/02/skos/core#Concept"/>
        <skos:broader rdf:resource="http://www.foodpairing.com/ontologies/foodpairing-kg#icat:000001"/>
        <skos:definition xml:lang="en">Relates to a category of baked goods made with dough or pastry dough, often used for pies, tarts, and pastries.</skos:definition>
        <skos:prefLabel xml:lang="en">Bakery Ingredients</skos:prefLabel>
    </owl:NamedIndividual>
    


    <!-- http://www.foodpairing.com/ontologies/foodpairing-kg#icat:000029 -->


    <owl:NamedIndividual rdf:about="http://www.foodpairing.com/ontologies/foodpairing-kg#icat:000029">
        <rdf:type rdf:resource="http://www.foodpairing.com/ontologies/foodpairing-kg#IngredientCategory"/>
        <rdf:type rdf:resource="http://www.w3.org/2004/02/skos/core#Concept"/>
        <skos:broader rdf:resource="http://www.foodpairing.com/ontologies/foodpairing-kg#icat:000001"/>
        <skos:definition xml:lang="en">Refers to a type of pastry made from a yeast-leavened dough, including croissants, pain au chocolat, and Danish pastries.</skos:definition>
        <skos:prefLabel xml:lang="en">Pastry</skos:prefLabel>
    </owl:NamedIndividual>
    


    <!-- http://www.foodpairing.com/ontologies/foodpairing-kg#icat:000030 -->


    <owl:NamedIndividual rdf:about="http://www.foodpairing.com/ontologies/foodpairing-kg#icat:000030">
        <rdf:type rdf:resource="http://www.foodpairing.com/ontologies/foodpairing-kg#IngredientCategory"/>
        <rdf:type rdf:resource="http://www.w3.org/2004/02/skos/core#Concept"/>
        <skos:broader rdf:resource="http://www.foodpairing.com/ontologies/foodpairing-kg#icat:000001"/>
        <skos:definition xml:lang="en">Encompasses sweet baked goods like cookies and cakes, typically made from a combination of flour, sugar, eggs, and flavorings.</skos:definition>
        <skos:prefLabel xml:lang="en">Viennoiserie</skos:prefLabel>
    </owl:NamedIndividual>
    


    <!-- http://www.foodpairing.com/ontologies/foodpairing-kg#icat:000031 -->


    <owl:NamedIndividual rdf:about="http://www.foodpairing.com/ontologies/foodpairing-kg#icat:000031">
        <rdf:type rdf:resource="http://www.foodpairing.com/ontologies/foodpairing-kg#IngredientCategory"/>
        <rdf:type rdf:resource="http://www.w3.org/2004/02/skos/core#Concept"/>
        <skos:broader rdf:resource="http://www.foodpairing.com/ontologies/foodpairing-kg#icat:000002"/>
        <skos:definition xml:lang="en">Encompasses processed cereal-based products typically consumed as breakfast, including flakes, granola, and oatmeal.</skos:definition>
        <skos:prefLabel xml:lang="en">Breakfast Cereal</skos:prefLabel>
    </owl:NamedIndividual>
    


    <!-- http://www.foodpairing.com/ontologies/foodpairing-kg#icat:000032 -->


    <owl:NamedIndividual rdf:about="http://www.foodpairing.com/ontologies/foodpairing-kg#icat:000032">
        <rdf:type rdf:resource="http://www.foodpairing.com/ontologies/foodpairing-kg#IngredientCategory"/>
        <rdf:type rdf:resource="http://www.w3.org/2004/02/skos/core#Concept"/>
        <skos:broader rdf:resource="http://www.foodpairing.com/ontologies/foodpairing-kg#icat:000002"/>
        <skos:definition xml:lang="en">Refers to various cereal grains used as staple foods, including wheat, rice, corn, oats, barley, and others.</skos:definition>
        <skos:prefLabel xml:lang="en">Grains</skos:prefLabel>
    </owl:NamedIndividual>
    


    <!-- http://www.foodpairing.com/ontologies/foodpairing-kg#icat:000033 -->


    <owl:NamedIndividual rdf:about="http://www.foodpairing.com/ontologies/foodpairing-kg#icat:000033">
        <rdf:type rdf:resource="http://www.foodpairing.com/ontologies/foodpairing-kg#IngredientCategory"/>
        <rdf:type rdf:resource="http://www.w3.org/2004/02/skos/core#Concept"/>
        <skos:broader rdf:resource="http://www.foodpairing.com/ontologies/foodpairing-kg#icat:000002"/>
        <skos:definition xml:lang="en">Refers to the edible seeds of the rice plant, often consumed as a staple food in many cultures.</skos:definition>
        <skos:prefLabel xml:lang="en">Rice</skos:prefLabel>
    </owl:NamedIndividual>
    


    <!-- http://www.foodpairing.com/ontologies/foodpairing-kg#icat:000034 -->


    <owl:NamedIndividual rdf:about="http://www.foodpairing.com/ontologies/foodpairing-kg#icat:000034">
        <rdf:type rdf:resource="http://www.foodpairing.com/ontologies/foodpairing-kg#IngredientCategory"/>
        <rdf:type rdf:resource="http://www.w3.org/2004/02/skos/core#Concept"/>
        <skos:broader rdf:resource="http://www.foodpairing.com/ontologies/foodpairing-kg#icat:000002"/>
        <skos:definition xml:lang="en">Encompasses various types of noodles and pasta products made from wheat flour, water, and sometimes eggs.</skos:definition>
        <skos:prefLabel xml:lang="en">Pasta</skos:prefLabel>
    </owl:NamedIndividual>
    


    <!-- http://www.foodpairing.com/ontologies/foodpairing-kg#icat:000035 -->


    <owl:NamedIndividual rdf:about="http://www.foodpairing.com/ontologies/foodpairing-kg#icat:000035">
        <rdf:type rdf:resource="http://www.foodpairing.com/ontologies/foodpairing-kg#IngredientCategory"/>
        <rdf:type rdf:resource="http://www.w3.org/2004/02/skos/core#Concept"/>
        <skos:broader rdf:resource="http://www.foodpairing.com/ontologies/foodpairing-kg#icat:000032"/>
        <skos:definition xml:lang="en">Relates to oats, a type of cereal grain commonly used in breakfast cereals, porridge, and baked goods.</skos:definition>
        <skos:prefLabel xml:lang="en">Oat</skos:prefLabel>
    </owl:NamedIndividual>
    


    <!-- http://www.foodpairing.com/ontologies/foodpairing-kg#icat:000036 -->


    <owl:NamedIndividual rdf:about="http://www.foodpairing.com/ontologies/foodpairing-kg#icat:000036">
        <rdf:type rdf:resource="http://www.foodpairing.com/ontologies/foodpairing-kg#IngredientCategory"/>
        <rdf:type rdf:resource="http://www.w3.org/2004/02/skos/core#Concept"/>
        <skos:broader rdf:resource="http://www.foodpairing.com/ontologies/foodpairing-kg#icat:000005"/>
        <skos:definition xml:lang="en">Includes savory preparations used for dipping or spreading on other foods, such as hummus, guacamole, and cheese spreads.</skos:definition>
        <skos:prefLabel xml:lang="en">Dip And Spread</skos:prefLabel>
    </owl:NamedIndividual>
    


    <!-- http://www.foodpairing.com/ontologies/foodpairing-kg#icat:000037 -->


    <owl:NamedIndividual rdf:about="http://www.foodpairing.com/ontologies/foodpairing-kg#icat:000037">
        <rdf:type rdf:resource="http://www.foodpairing.com/ontologies/foodpairing-kg#IngredientCategory"/>
        <rdf:type rdf:resource="http://www.w3.org/2004/02/skos/core#Concept"/>
        <skos:broader rdf:resource="http://www.foodpairing.com/ontologies/foodpairing-kg#icat:000005"/>
        <skos:definition xml:lang="en">Refers to sweet spreads made from fruit or fruit juice, typically preserved with sugar and pectin.</skos:definition>
        <skos:prefLabel xml:lang="en">Jam And Jelly</skos:prefLabel>
    </owl:NamedIndividual>
    


    <!-- http://www.foodpairing.com/ontologies/foodpairing-kg#icat:000038 -->


    <owl:NamedIndividual rdf:about="http://www.foodpairing.com/ontologies/foodpairing-kg#icat:000038">
        <rdf:type rdf:resource="http://www.foodpairing.com/ontologies/foodpairing-kg#IngredientCategory"/>
        <rdf:type rdf:resource="http://www.w3.org/2004/02/skos/core#Concept"/>
        <skos:broader rdf:resource="http://www.foodpairing.com/ontologies/foodpairing-kg#icat:000005"/>
        <skos:definition xml:lang="en">Encompasses preserved vegetables or fruits, often soaked in a brine or vinegar solution to impart a tangy flavor.</skos:definition>
        <skos:prefLabel xml:lang="en">Pickles</skos:prefLabel>
    </owl:NamedIndividual>
    


    <!-- http://www.foodpairing.com/ontologies/foodpairing-kg#icat:000039 -->


    <owl:NamedIndividual rdf:about="http://www.foodpairing.com/ontologies/foodpairing-kg#icat:000039">
        <rdf:type rdf:resource="http://www.foodpairing.com/ontologies/foodpairing-kg#IngredientCategory"/>
        <rdf:type rdf:resource="http://www.w3.org/2004/02/skos/core#Concept"/>
        <skos:broader rdf:resource="http://www.foodpairing.com/ontologies/foodpairing-kg#icat:000005"/>
        <skos:definition xml:lang="en">Relates to condiments made from fruits, vegetables, or herbs, typically used to add flavor and enhance dishes.</skos:definition>
        <skos:prefLabel xml:lang="en">Relish Chutney</skos:prefLabel>
    </owl:NamedIndividual>
    


    <!-- http://www.foodpairing.com/ontologies/foodpairing-kg#icat:000040 -->


    <owl:NamedIndividual rdf:about="http://www.foodpairing.com/ontologies/foodpairing-kg#icat:000040">
        <rdf:type rdf:resource="http://www.foodpairing.com/ontologies/foodpairing-kg#IngredientCategory"/>
        <rdf:type rdf:resource="http://www.w3.org/2004/02/skos/core#Concept"/>
        <skos:broader rdf:resource="http://www.foodpairing.com/ontologies/foodpairing-kg#icat:000005"/>
        <skos:definition xml:lang="en">Includes various sauces used as condiments on the dining table, such as ketchup, mustard, and mayonnaise.</skos:definition>
        <skos:prefLabel xml:lang="en">Table Sauces</skos:prefLabel>
    </owl:NamedIndividual>
    


    <!-- http://www.foodpairing.com/ontologies/foodpairing-kg#icat:000041 -->


    <owl:NamedIndividual rdf:about="http://www.foodpairing.com/ontologies/foodpairing-kg#icat:000041">
        <rdf:type rdf:resource="http://www.foodpairing.com/ontologies/foodpairing-kg#IngredientCategory"/>
        <rdf:type rdf:resource="http://www.w3.org/2004/02/skos/core#Concept"/>
        <skos:broader rdf:resource="http://www.foodpairing.com/ontologies/foodpairing-kg#icat:000005"/>
        <skos:definition xml:lang="en">Refers to a sour-tasting liquid produced through the fermentation of ethanol, often used as a condiment or preservative.</skos:definition>
        <skos:prefLabel xml:lang="en">Vinegar</skos:prefLabel>
    </owl:NamedIndividual>
    


    <!-- http://www.foodpairing.com/ontologies/foodpairing-kg#icat:000042 -->


    <owl:NamedIndividual rdf:about="http://www.foodpairing.com/ontologies/foodpairing-kg#icat:000042">
        <rdf:type rdf:resource="http://www.foodpairing.com/ontologies/foodpairing-kg#IngredientCategory"/>
        <rdf:type rdf:resource="http://www.w3.org/2004/02/skos/core#Concept"/>
        <skos:broader rdf:resource="http://www.foodpairing.com/ontologies/foodpairing-kg#icat:000006"/>
        <skos:definition xml:lang="en">Encompasses confectionery products made primarily from chocolate, including chocolate bars, truffles, and pralines.</skos:definition>
        <skos:prefLabel xml:lang="en">Chocolate Confections</skos:prefLabel>
    </owl:NamedIndividual>
    


    <!-- http://www.foodpairing.com/ontologies/foodpairing-kg#icat:000043 -->


    <owl:NamedIndividual rdf:about="http://www.foodpairing.com/ontologies/foodpairing-kg#icat:000043">
        <rdf:type rdf:resource="http://www.foodpairing.com/ontologies/foodpairing-kg#IngredientCategory"/>
        <rdf:type rdf:resource="http://www.w3.org/2004/02/skos/core#Concept"/>
        <skos:broader rdf:resource="http://www.foodpairing.com/ontologies/foodpairing-kg#icat:000006"/>
        <skos:definition xml:lang="en">Includes confectionery products made with milk or milk-derived ingredients, such as fudge, caramels, and milk chocolates.</skos:definition>
        <skos:prefLabel xml:lang="en">Milk Confections</skos:prefLabel>
    </owl:NamedIndividual>
    


    <!-- http://www.foodpairing.com/ontologies/foodpairing-kg#icat:000044 -->


    <owl:NamedIndividual rdf:about="http://www.foodpairing.com/ontologies/foodpairing-kg#icat:000044">
        <rdf:type rdf:resource="http://www.foodpairing.com/ontologies/foodpairing-kg#IngredientCategory"/>
        <rdf:type rdf:resource="http://www.w3.org/2004/02/skos/core#Concept"/>
        <skos:broader rdf:resource="http://www.foodpairing.com/ontologies/foodpairing-kg#icat:000006"/>
        <skos:definition xml:lang="en">Refers to confectionery products with a high sugar content, including candies, gummies, and marshmallows.</skos:definition>
        <skos:prefLabel xml:lang="en">Sugar Confections</skos:prefLabel>
    </owl:NamedIndividual>
    


    <!-- http://www.foodpairing.com/ontologies/foodpairing-kg#icat:000045 -->


    <owl:NamedIndividual rdf:about="http://www.foodpairing.com/ontologies/foodpairing-kg#icat:000045">
        <rdf:type rdf:resource="http://www.foodpairing.com/ontologies/foodpairing-kg#IngredientCategory"/>
        <rdf:type rdf:resource="http://www.w3.org/2004/02/skos/core#Concept"/>
        <skos:broader rdf:resource="http://www.foodpairing.com/ontologies/foodpairing-kg#icat:000044"/>
        <skos:definition xml:lang="en">Encompasses confectionery products made primarily from fruits, such as fruit jellies, fruit gummies, and fruit-filled chocolates.</skos:definition>
        <skos:prefLabel xml:lang="en">Fruit Confections</skos:prefLabel>
    </owl:NamedIndividual>
    


    <!-- http://www.foodpairing.com/ontologies/foodpairing-kg#icat:000046 -->


    <owl:NamedIndividual rdf:about="http://www.foodpairing.com/ontologies/foodpairing-kg#icat:000046">
        <rdf:type rdf:resource="http://www.foodpairing.com/ontologies/foodpairing-kg#IngredientCategory"/>
        <rdf:type rdf:resource="http://www.w3.org/2004/02/skos/core#Concept"/>
        <skos:broader rdf:resource="http://www.foodpairing.com/ontologies/foodpairing-kg#icat:000044"/>
        <skos:definition xml:lang="en">Relates to confectionery products infused with herbs or spices, often creating unique flavor combinations.</skos:definition>
        <skos:prefLabel xml:lang="en">Herbal And Spicy Confections</skos:prefLabel>
    </owl:NamedIndividual>
    


    <!-- http://www.foodpairing.com/ontologies/foodpairing-kg#icat:000047 -->


    <owl:NamedIndividual rdf:about="http://www.foodpairing.com/ontologies/foodpairing-kg#icat:000047">
        <rdf:type rdf:resource="http://www.foodpairing.com/ontologies/foodpairing-kg#IngredientCategory"/>
        <rdf:type rdf:resource="http://www.w3.org/2004/02/skos/core#Concept"/>
        <skos:broader rdf:resource="http://www.foodpairing.com/ontologies/foodpairing-kg#icat:000007"/>
        <skos:definition xml:lang="en">Refers to a dairy product made by churning cream or milk, commonly used as a cooking fat or spread.</skos:definition>
        <skos:prefLabel xml:lang="en">Butter</skos:prefLabel>
    </owl:NamedIndividual>
    


    <!-- http://www.foodpairing.com/ontologies/foodpairing-kg#icat:000048 -->


    <owl:NamedIndividual rdf:about="http://www.foodpairing.com/ontologies/foodpairing-kg#icat:000048">
        <rdf:type rdf:resource="http://www.foodpairing.com/ontologies/foodpairing-kg#IngredientCategory"/>
        <rdf:type rdf:resource="http://www.w3.org/2004/02/skos/core#Concept"/>
        <skos:broader rdf:resource="http://www.foodpairing.com/ontologies/foodpairing-kg#icat:000007"/>
        <skos:definition xml:lang="en">Encompasses a wide variety of dairy products made from curdled milk, with different textures, flavors, and production methods.</skos:definition>
        <skos:prefLabel xml:lang="en">Cheese</skos:prefLabel>
    </owl:NamedIndividual>
    


    <!-- http://www.foodpairing.com/ontologies/foodpairing-kg#icat:000049 -->


    <owl:NamedIndividual rdf:about="http://www.foodpairing.com/ontologies/foodpairing-kg#icat:000049">
        <rdf:type rdf:resource="http://www.foodpairing.com/ontologies/foodpairing-kg#IngredientCategory"/>
        <rdf:type rdf:resource="http://www.w3.org/2004/02/skos/core#Concept"/>
        <skos:broader rdf:resource="http://www.foodpairing.com/ontologies/foodpairing-kg#icat:000007"/>
        <skos:definition xml:lang="en">Refers to the high-fat layer that forms on top of milk, often used in cooking, baking, or as a topping for desserts.</skos:definition>
        <skos:prefLabel xml:lang="en">Cream</skos:prefLabel>
    </owl:NamedIndividual>
    


    <!-- http://www.foodpairing.com/ontologies/foodpairing-kg#icat:000050 -->


    <owl:NamedIndividual rdf:about="http://www.foodpairing.com/ontologies/foodpairing-kg#icat:000050">
        <rdf:type rdf:resource="http://www.foodpairing.com/ontologies/foodpairing-kg#IngredientCategory"/>
        <rdf:type rdf:resource="http://www.w3.org/2004/02/skos/core#Concept"/>
        <skos:broader rdf:resource="http://www.foodpairing.com/ontologies/foodpairing-kg#icat:000007"/>
        <skos:definition xml:lang="en">Relates to the white liquid produced by mammals&apos; mammary glands, often consumed as a beverage or used in various recipes.</skos:definition>
        <skos:prefLabel xml:lang="en">Milk</skos:prefLabel>
    </owl:NamedIndividual>
    


    <!-- http://www.foodpairing.com/ontologies/foodpairing-kg#icat:000051 -->


    <owl:NamedIndividual rdf:about="http://www.foodpairing.com/ontologies/foodpairing-kg#icat:000051">
        <rdf:type rdf:resource="http://www.foodpairing.com/ontologies/foodpairing-kg#IngredientCategory"/>
        <rdf:type rdf:resource="http://www.w3.org/2004/02/skos/core#Concept"/>
        <skos:broader rdf:resource="http://www.foodpairing.com/ontologies/foodpairing-kg#icat:000007"/>
        <skos:definition xml:lang="en">Includes dairy alternatives made from plant-based sources, such as almond milk, soy milk, or coconut milk.</skos:definition>
        <skos:prefLabel xml:lang="en">Plant-based Dairy</skos:prefLabel>
    </owl:NamedIndividual>
    


    <!-- http://www.foodpairing.com/ontologies/foodpairing-kg#icat:000052 -->


    <owl:NamedIndividual rdf:about="http://www.foodpairing.com/ontologies/foodpairing-kg#icat:000052">
        <rdf:type rdf:resource="http://www.foodpairing.com/ontologies/foodpairing-kg#IngredientCategory"/>
        <rdf:type rdf:resource="http://www.w3.org/2004/02/skos/core#Concept"/>
        <skos:broader rdf:resource="http://www.foodpairing.com/ontologies/foodpairing-kg#icat:000007"/>
        <skos:definition xml:lang="en">Refers to a fermented dairy product made from milk, typically with added bacterial cultures, offering a creamy and tangy taste.</skos:definition>
        <skos:prefLabel xml:lang="en">Yoghurt</skos:prefLabel>
    </owl:NamedIndividual>
    


    <!-- http://www.foodpairing.com/ontologies/foodpairing-kg#icat:000053 -->


    <owl:NamedIndividual rdf:about="http://www.foodpairing.com/ontologies/foodpairing-kg#icat:000053">
        <rdf:type rdf:resource="http://www.foodpairing.com/ontologies/foodpairing-kg#IngredientCategory"/>
        <rdf:type rdf:resource="http://www.w3.org/2004/02/skos/core#Concept"/>
        <skos:broader rdf:resource="http://www.foodpairing.com/ontologies/foodpairing-kg#icat:000048"/>
        <skos:definition xml:lang="en">Encompasses a type of cheese characterized by the presence of blue or green veins of mold, known for its distinct flavor.</skos:definition>
        <skos:prefLabel xml:lang="en">Blue Cheese</skos:prefLabel>
    </owl:NamedIndividual>
    


    <!-- http://www.foodpairing.com/ontologies/foodpairing-kg#icat:000054 -->


    <owl:NamedIndividual rdf:about="http://www.foodpairing.com/ontologies/foodpairing-kg#icat:000054">
        <rdf:type rdf:resource="http://www.foodpairing.com/ontologies/foodpairing-kg#IngredientCategory"/>
        <rdf:type rdf:resource="http://www.w3.org/2004/02/skos/core#Concept"/>
        <skos:broader rdf:resource="http://www.foodpairing.com/ontologies/foodpairing-kg#icat:000048"/>
        <skos:definition xml:lang="en">Refers to soft, unripened cheeses with a high moisture content, often mild and creamy in flavor.</skos:definition>
        <skos:prefLabel xml:lang="en">Fresh Cheese</skos:prefLabel>
    </owl:NamedIndividual>
    


    <!-- http://www.foodpairing.com/ontologies/foodpairing-kg#icat:000055 -->


    <owl:NamedIndividual rdf:about="http://www.foodpairing.com/ontologies/foodpairing-kg#icat:000055">
        <rdf:type rdf:resource="http://www.foodpairing.com/ontologies/foodpairing-kg#IngredientCategory"/>
        <rdf:type rdf:resource="http://www.w3.org/2004/02/skos/core#Concept"/>
        <skos:broader rdf:resource="http://www.foodpairing.com/ontologies/foodpairing-kg#icat:000048"/>
        <skos:definition xml:lang="en">Encompasses aged cheeses with a firm and dry texture, typically characterized by intense flavors and a long aging process.</skos:definition>
        <skos:prefLabel xml:lang="en">Hard Cheese</skos:prefLabel>
    </owl:NamedIndividual>
    


    <!-- http://www.foodpairing.com/ontologies/foodpairing-kg#icat:000056 -->


    <owl:NamedIndividual rdf:about="http://www.foodpairing.com/ontologies/foodpairing-kg#icat:000056">
        <rdf:type rdf:resource="http://www.foodpairing.com/ontologies/foodpairing-kg#IngredientCategory"/>
        <rdf:type rdf:resource="http://www.w3.org/2004/02/skos/core#Concept"/>
        <skos:broader rdf:resource="http://www.foodpairing.com/ontologies/foodpairing-kg#icat:000048"/>
        <skos:definition xml:lang="en">Refers to cheeses that have been colored or aged with the addition of red cultures or bacteria, resulting in distinct flavors.</skos:definition>
        <skos:prefLabel xml:lang="en">Red Cheese</skos:prefLabel>
    </owl:NamedIndividual>
    


    <!-- http://www.foodpairing.com/ontologies/foodpairing-kg#icat:000057 -->


    <owl:NamedIndividual rdf:about="http://www.foodpairing.com/ontologies/foodpairing-kg#icat:000057">
        <rdf:type rdf:resource="http://www.foodpairing.com/ontologies/foodpairing-kg#IngredientCategory"/>
        <rdf:type rdf:resource="http://www.w3.org/2004/02/skos/core#Concept"/>
        <skos:broader rdf:resource="http://www.foodpairing.com/ontologies/foodpairing-kg#icat:000048"/>
        <skos:definition xml:lang="en">Relates to cheeses with a semi-firm texture and flavors that range from mild to sharp, often suitable for slicing or grating.</skos:definition>
        <skos:prefLabel xml:lang="en">Semi-hard Cheese</skos:prefLabel>
    </owl:NamedIndividual>
    


    <!-- http://www.foodpairing.com/ontologies/foodpairing-kg#icat:000058 -->


    <owl:NamedIndividual rdf:about="http://www.foodpairing.com/ontologies/foodpairing-kg#icat:000058">
        <rdf:type rdf:resource="http://www.foodpairing.com/ontologies/foodpairing-kg#IngredientCategory"/>
        <rdf:type rdf:resource="http://www.w3.org/2004/02/skos/core#Concept"/>
        <skos:broader rdf:resource="http://www.foodpairing.com/ontologies/foodpairing-kg#icat:000048"/>
        <skos:definition xml:lang="en">Encompasses cheeses with a semi-soft or springy texture, offering a balance between firmness and creaminess.</skos:definition>
        <skos:prefLabel xml:lang="en">Semi-soft Cheese</skos:prefLabel>
    </owl:NamedIndividual>
    


    <!-- http://www.foodpairing.com/ontologies/foodpairing-kg#icat:000059 -->


    <owl:NamedIndividual rdf:about="http://www.foodpairing.com/ontologies/foodpairing-kg#icat:000059">
        <rdf:type rdf:resource="http://www.foodpairing.com/ontologies/foodpairing-kg#IngredientCategory"/>
        <rdf:type rdf:resource="http://www.w3.org/2004/02/skos/core#Concept"/>
        <skos:broader rdf:resource="http://www.foodpairing.com/ontologies/foodpairing-kg#icat:000048"/>
        <skos:definition xml:lang="en">Refers to cheeses with a soft and spreadable texture, often creamy and mild in flavor.</skos:definition>
        <skos:prefLabel xml:lang="en">Soft Cheese</skos:prefLabel>
    </owl:NamedIndividual>
    


    <!-- http://www.foodpairing.com/ontologies/foodpairing-kg#icat:000060 -->


    <owl:NamedIndividual rdf:about="http://www.foodpairing.com/ontologies/foodpairing-kg#icat:000060">
        <rdf:type rdf:resource="http://www.foodpairing.com/ontologies/foodpairing-kg#IngredientCategory"/>
        <rdf:type rdf:resource="http://www.w3.org/2004/02/skos/core#Concept"/>
        <skos:broader rdf:resource="http://www.foodpairing.com/ontologies/foodpairing-kg#icat:000009"/>
        <skos:definition xml:lang="en">Refers to beverages containing alcohol, including various types of beer, wine, spirits, and cocktails.</skos:definition>
        <skos:prefLabel xml:lang="en">Alcoholic Drink</skos:prefLabel>
    </owl:NamedIndividual>
    


    <!-- http://www.foodpairing.com/ontologies/foodpairing-kg#icat:000061 -->


    <owl:NamedIndividual rdf:about="http://www.foodpairing.com/ontologies/foodpairing-kg#icat:000061">
        <rdf:type rdf:resource="http://www.foodpairing.com/ontologies/foodpairing-kg#IngredientCategory"/>
        <rdf:type rdf:resource="http://www.w3.org/2004/02/skos/core#Concept"/>
        <skos:broader rdf:resource="http://www.foodpairing.com/ontologies/foodpairing-kg#icat:000009"/>
        <skos:definition xml:lang="en">Includes beverages without alcohol, such as soft drinks, juices, water, coffee, tea, and non-alcoholic cocktails.</skos:definition>
        <skos:prefLabel xml:lang="en">Non-alcoholic Drink</skos:prefLabel>
    </owl:NamedIndividual>
    


    <!-- http://www.foodpairing.com/ontologies/foodpairing-kg#icat:000062 -->


    <owl:NamedIndividual rdf:about="http://www.foodpairing.com/ontologies/foodpairing-kg#icat:000062">
        <rdf:type rdf:resource="http://www.foodpairing.com/ontologies/foodpairing-kg#IngredientCategory"/>
        <rdf:type rdf:resource="http://www.w3.org/2004/02/skos/core#Concept"/>
        <skos:broader rdf:resource="http://www.foodpairing.com/ontologies/foodpairing-kg#icat:000060"/>
        <skos:definition xml:lang="en">Encompasses a wide range of fermented alcoholic beverages made from grains, typically barley, flavored with hops and yeast.</skos:definition>
        <skos:prefLabel xml:lang="en">Beers</skos:prefLabel>
    </owl:NamedIndividual>
    


    <!-- http://www.foodpairing.com/ontologies/foodpairing-kg#icat:000063 -->


    <owl:NamedIndividual rdf:about="http://www.foodpairing.com/ontologies/foodpairing-kg#icat:000063">
        <rdf:type rdf:resource="http://www.foodpairing.com/ontologies/foodpairing-kg#IngredientCategory"/>
        <rdf:type rdf:resource="http://www.w3.org/2004/02/skos/core#Concept"/>
        <skos:broader rdf:resource="http://www.foodpairing.com/ontologies/foodpairing-kg#icat:000060"/>
        <skos:definition xml:lang="en">Refers to a category of alcoholic beverages characterized by a bitter taste, often produced by botanical ingredients or hops.</skos:definition>
        <skos:prefLabel xml:lang="en">Bitter</skos:prefLabel>
    </owl:NamedIndividual>
    


    <!-- http://www.foodpairing.com/ontologies/foodpairing-kg#icat:000064 -->


    <owl:NamedIndividual rdf:about="http://www.foodpairing.com/ontologies/foodpairing-kg#icat:000064">
        <rdf:type rdf:resource="http://www.foodpairing.com/ontologies/foodpairing-kg#IngredientCategory"/>
        <rdf:type rdf:resource="http://www.w3.org/2004/02/skos/core#Concept"/>
        <skos:broader rdf:resource="http://www.foodpairing.com/ontologies/foodpairing-kg#icat:000060"/>
        <skos:definition xml:lang="en">Encompasses distilled alcoholic beverages with a higher alcohol content, often flavored and consumed in small quantities.</skos:definition>
        <skos:prefLabel xml:lang="en">Liquors</skos:prefLabel>
    </owl:NamedIndividual>
    


    <!-- http://www.foodpairing.com/ontologies/foodpairing-kg#icat:000065 -->


    <owl:NamedIndividual rdf:about="http://www.foodpairing.com/ontologies/foodpairing-kg#icat:000065">
        <rdf:type rdf:resource="http://www.foodpairing.com/ontologies/foodpairing-kg#IngredientCategory"/>
        <rdf:type rdf:resource="http://www.w3.org/2004/02/skos/core#Concept"/>
        <skos:broader rdf:resource="http://www.foodpairing.com/ontologies/foodpairing-kg#icat:000060"/>
        <skos:definition xml:lang="en">Refers to a broad category of distilled alcoholic beverages, including liquors, whiskey, vodka, rum, gin, tequila, and others.</skos:definition>
        <skos:prefLabel xml:lang="en">Spirits</skos:prefLabel>
    </owl:NamedIndividual>
    


    <!-- http://www.foodpairing.com/ontologies/foodpairing-kg#icat:000066 -->


    <owl:NamedIndividual rdf:about="http://www.foodpairing.com/ontologies/foodpairing-kg#icat:000066">
        <rdf:type rdf:resource="http://www.foodpairing.com/ontologies/foodpairing-kg#IngredientCategory"/>
        <rdf:type rdf:resource="http://www.w3.org/2004/02/skos/core#Concept"/>
        <skos:broader rdf:resource="http://www.foodpairing.com/ontologies/foodpairing-kg#icat:000060"/>
        <skos:definition xml:lang="en">Includes alcoholic beverages produced by fermenting grapes or other fruits, offering a wide range of flavors, colors, and styles.</skos:definition>
        <skos:prefLabel xml:lang="en">Wines</skos:prefLabel>
    </owl:NamedIndividual>
    


    <!-- http://www.foodpairing.com/ontologies/foodpairing-kg#icat:000067 -->


    <owl:NamedIndividual rdf:about="http://www.foodpairing.com/ontologies/foodpairing-kg#icat:000067">
        <rdf:type rdf:resource="http://www.foodpairing.com/ontologies/foodpairing-kg#IngredientCategory"/>
        <rdf:type rdf:resource="http://www.w3.org/2004/02/skos/core#Concept"/>
        <skos:broader rdf:resource="http://www.foodpairing.com/ontologies/foodpairing-kg#icat:000065"/>
        <skos:definition xml:lang="en">Refers to distilled spirits made from fermented grapes, such as brandy, cognac, and pisco.</skos:definition>
        <skos:prefLabel xml:lang="en">Grape-based Spirits</skos:prefLabel>
    </owl:NamedIndividual>
    


    <!-- http://www.foodpairing.com/ontologies/foodpairing-kg#icat:000068 -->


    <owl:NamedIndividual rdf:about="http://www.foodpairing.com/ontologies/foodpairing-kg#icat:000068">
        <rdf:type rdf:resource="http://www.foodpairing.com/ontologies/foodpairing-kg#IngredientCategory"/>
        <rdf:type rdf:resource="http://www.w3.org/2004/02/skos/core#Concept"/>
        <skos:broader rdf:resource="http://www.foodpairing.com/ontologies/foodpairing-kg#icat:000065"/>
        <skos:definition xml:lang="en">Encompasses distilled spirits made from sources other than grapes, such as whiskey, rum, vodka, and tequila.</skos:definition>
        <skos:prefLabel xml:lang="en">Non Grape-based Spirits</skos:prefLabel>
    </owl:NamedIndividual>
    


    <!-- http://www.foodpairing.com/ontologies/foodpairing-kg#icat:000069 -->


    <owl:NamedIndividual rdf:about="http://www.foodpairing.com/ontologies/foodpairing-kg#icat:000069">
        <rdf:type rdf:resource="http://www.foodpairing.com/ontologies/foodpairing-kg#IngredientCategory"/>
        <rdf:type rdf:resource="http://www.w3.org/2004/02/skos/core#Concept"/>
        <skos:broader rdf:resource="http://www.foodpairing.com/ontologies/foodpairing-kg#icat:000065"/>
        <skos:definition xml:lang="en">Relates to distilled alcoholic beverages made specifically from agave plants, including mezcal and tequila.</skos:definition>
        <skos:prefLabel xml:lang="en">Mezcal And Tequila</skos:prefLabel>
    </owl:NamedIndividual>
    


    <!-- http://www.foodpairing.com/ontologies/foodpairing-kg#icat:000070 -->


    <owl:NamedIndividual rdf:about="http://www.foodpairing.com/ontologies/foodpairing-kg#icat:000070">
        <rdf:type rdf:resource="http://www.foodpairing.com/ontologies/foodpairing-kg#IngredientCategory"/>
        <rdf:type rdf:resource="http://www.w3.org/2004/02/skos/core#Concept"/>
        <skos:broader rdf:resource="http://www.foodpairing.com/ontologies/foodpairing-kg#icat:000065"/>
        <skos:definition xml:lang="en">Includes distilled spirits flavored with juniper berries and other botanical ingredients, such as gin and jenever.</skos:definition>
        <skos:prefLabel xml:lang="en">Gin And Jenever</skos:prefLabel>
    </owl:NamedIndividual>
    


    <!-- http://www.foodpairing.com/ontologies/foodpairing-kg#icat:000071 -->


    <owl:NamedIndividual rdf:about="http://www.foodpairing.com/ontologies/foodpairing-kg#icat:000071">
        <rdf:type rdf:resource="http://www.foodpairing.com/ontologies/foodpairing-kg#IngredientCategory"/>
        <rdf:type rdf:resource="http://www.w3.org/2004/02/skos/core#Concept"/>
        <skos:broader rdf:resource="http://www.foodpairing.com/ontologies/foodpairing-kg#icat:000065"/>
        <skos:definition xml:lang="en">Refers to a distilled alcoholic beverage made from sugarcane byproducts, typically aged in oak barrels for flavor development.</skos:definition>
        <skos:prefLabel xml:lang="en">Rum</skos:prefLabel>
    </owl:NamedIndividual>
    


    <!-- http://www.foodpairing.com/ontologies/foodpairing-kg#icat:000072 -->


    <owl:NamedIndividual rdf:about="http://www.foodpairing.com/ontologies/foodpairing-kg#icat:000072">
        <rdf:type rdf:resource="http://www.foodpairing.com/ontologies/foodpairing-kg#IngredientCategory"/>
        <rdf:type rdf:resource="http://www.w3.org/2004/02/skos/core#Concept"/>
        <skos:broader rdf:resource="http://www.foodpairing.com/ontologies/foodpairing-kg#icat:000065"/>
        <skos:definition xml:lang="en">Encompasses a neutral-tasting distilled spirit typically made from grains or potatoes, often used as a base for cocktails.</skos:definition>
        <skos:prefLabel xml:lang="en">Vodka</skos:prefLabel>
    </owl:NamedIndividual>
    


    <!-- http://www.foodpairing.com/ontologies/foodpairing-kg#icat:000073 -->


    <owl:NamedIndividual rdf:about="http://www.foodpairing.com/ontologies/foodpairing-kg#icat:000073">
        <rdf:type rdf:resource="http://www.foodpairing.com/ontologies/foodpairing-kg#IngredientCategory"/>
        <rdf:type rdf:resource="http://www.w3.org/2004/02/skos/core#Concept"/>
        <skos:broader rdf:resource="http://www.foodpairing.com/ontologies/foodpairing-kg#icat:000065"/>
        <skos:definition xml:lang="en">Relates to distilled alcoholic beverages made from fermented grain mash, aged in wooden casks, and varying in flavor profiles.</skos:definition>
        <skos:prefLabel xml:lang="en">Whisky</skos:prefLabel>
    </owl:NamedIndividual>
    


    <!-- http://www.foodpairing.com/ontologies/foodpairing-kg#icat:000074 -->


    <owl:NamedIndividual rdf:about="http://www.foodpairing.com/ontologies/foodpairing-kg#icat:000074">
        <rdf:type rdf:resource="http://www.foodpairing.com/ontologies/foodpairing-kg#IngredientCategory"/>
        <rdf:type rdf:resource="http://www.w3.org/2004/02/skos/core#Concept"/>
        <skos:broader rdf:resource="http://www.foodpairing.com/ontologies/foodpairing-kg#icat:000061"/>
        <skos:definition xml:lang="en">Includes various coffee products, such as whole beans, ground coffee, instant coffee, and coffee-based beverages.</skos:definition>
        <skos:prefLabel xml:lang="en">Coffees</skos:prefLabel>
    </owl:NamedIndividual>
    


    <!-- http://www.foodpairing.com/ontologies/foodpairing-kg#icat:000075 -->


    <owl:NamedIndividual rdf:about="http://www.foodpairing.com/ontologies/foodpairing-kg#icat:000075">
        <rdf:type rdf:resource="http://www.foodpairing.com/ontologies/foodpairing-kg#IngredientCategory"/>
        <rdf:type rdf:resource="http://www.w3.org/2004/02/skos/core#Concept"/>
        <skos:broader rdf:resource="http://www.foodpairing.com/ontologies/foodpairing-kg#icat:000061"/>
        <skos:definition xml:lang="en">Refers to beverages containing stimulant ingredients like caffeine or taurine, often consumed to provide a temporary energy boost.</skos:definition>
        <skos:prefLabel xml:lang="en">Energy Drinks</skos:prefLabel>
    </owl:NamedIndividual>
    


    <!-- http://www.foodpairing.com/ontologies/foodpairing-kg#icat:000076 -->


    <owl:NamedIndividual rdf:about="http://www.foodpairing.com/ontologies/foodpairing-kg#icat:000076">
        <rdf:type rdf:resource="http://www.foodpairing.com/ontologies/foodpairing-kg#IngredientCategory"/>
        <rdf:type rdf:resource="http://www.w3.org/2004/02/skos/core#Concept"/>
        <skos:broader rdf:resource="http://www.foodpairing.com/ontologies/foodpairing-kg#icat:000061"/>
        <skos:definition xml:lang="en">Encompasses waters infused with flavors, often derived from fruits, herbs, or botanical extracts, offering a refreshing taste.</skos:definition>
        <skos:prefLabel xml:lang="en">Flavoured Waters</skos:prefLabel>
    </owl:NamedIndividual>
    


    <!-- http://www.foodpairing.com/ontologies/foodpairing-kg#icat:000077 -->


    <owl:NamedIndividual rdf:about="http://www.foodpairing.com/ontologies/foodpairing-kg#icat:000077">
        <rdf:type rdf:resource="http://www.foodpairing.com/ontologies/foodpairing-kg#IngredientCategory"/>
        <rdf:type rdf:resource="http://www.w3.org/2004/02/skos/core#Concept"/>
        <skos:broader rdf:resource="http://www.foodpairing.com/ontologies/foodpairing-kg#icat:000061"/>
        <skos:definition xml:lang="en">Refers to a beverage made by steeping ingredients like herbs, fruits, or flowers in hot water, creating flavored and aromatic drinks.</skos:definition>
        <skos:prefLabel xml:lang="en">Infusion</skos:prefLabel>
    </owl:NamedIndividual>
    


    <!-- http://www.foodpairing.com/ontologies/foodpairing-kg#icat:000078 -->


    <owl:NamedIndividual rdf:about="http://www.foodpairing.com/ontologies/foodpairing-kg#icat:000078">
        <rdf:type rdf:resource="http://www.foodpairing.com/ontologies/foodpairing-kg#IngredientCategory"/>
        <rdf:type rdf:resource="http://www.w3.org/2004/02/skos/core#Concept"/>
        <skos:broader rdf:resource="http://www.foodpairing.com/ontologies/foodpairing-kg#icat:000061"/>
        <skos:definition xml:lang="en">Includes the extracted liquids from fruits or vegetables, often consumed as beverages or used as ingredients in recipes.</skos:definition>
        <skos:prefLabel xml:lang="en">Juices</skos:prefLabel>
    </owl:NamedIndividual>
    


    <!-- http://www.foodpairing.com/ontologies/foodpairing-kg#icat:000079 -->


    <owl:NamedIndividual rdf:about="http://www.foodpairing.com/ontologies/foodpairing-kg#icat:000079">
        <rdf:type rdf:resource="http://www.foodpairing.com/ontologies/foodpairing-kg#IngredientCategory"/>
        <rdf:type rdf:resource="http://www.w3.org/2004/02/skos/core#Concept"/>
        <skos:broader rdf:resource="http://www.foodpairing.com/ontologies/foodpairing-kg#icat:000061"/>
        <skos:definition xml:lang="en">Encompasses beverages made from the leaves of the Camellia sinensis plant, offering various flavors and caffeine content.</skos:definition>
        <skos:prefLabel xml:lang="en">Tea</skos:prefLabel>
    </owl:NamedIndividual>
    


    <!-- http://www.foodpairing.com/ontologies/foodpairing-kg#icat:000080 -->


    <owl:NamedIndividual rdf:about="http://www.foodpairing.com/ontologies/foodpairing-kg#icat:000080">
        <rdf:type rdf:resource="http://www.foodpairing.com/ontologies/foodpairing-kg#IngredientCategory"/>
        <rdf:type rdf:resource="http://www.w3.org/2004/02/skos/core#Concept"/>
        <skos:broader rdf:resource="http://www.foodpairing.com/ontologies/foodpairing-kg#icat:000061"/>
        <skos:definition xml:lang="en">Refers to non-alcoholic carbonated beverages, commonly known as sodas or pop, with a wide range of flavors and sweetness levels.</skos:definition>
        <skos:prefLabel xml:lang="en">Soft Drinks</skos:prefLabel>
    </owl:NamedIndividual>
    


    <!-- http://www.foodpairing.com/ontologies/foodpairing-kg#icat:000081 -->


    <owl:NamedIndividual rdf:about="http://www.foodpairing.com/ontologies/foodpairing-kg#icat:000081">
        <rdf:type rdf:resource="http://www.foodpairing.com/ontologies/foodpairing-kg#IngredientCategory"/>
        <rdf:type rdf:resource="http://www.w3.org/2004/02/skos/core#Concept"/>
        <skos:broader rdf:resource="http://www.foodpairing.com/ontologies/foodpairing-kg#icat:000080"/>
        <skos:definition xml:lang="en">Encompasses chilled tea-based beverages, often served with ice, and may be sweetened or flavored with fruits or herbs.</skos:definition>
        <skos:prefLabel xml:lang="en">Iced Tea</skos:prefLabel>
    </owl:NamedIndividual>
    


    <!-- http://www.foodpairing.com/ontologies/foodpairing-kg#icat:000082 -->


    <owl:NamedIndividual rdf:about="http://www.foodpairing.com/ontologies/foodpairing-kg#icat:000082">
        <rdf:type rdf:resource="http://www.foodpairing.com/ontologies/foodpairing-kg#IngredientCategory"/>
        <rdf:type rdf:resource="http://www.w3.org/2004/02/skos/core#Concept"/>
        <skos:broader rdf:resource="http://www.foodpairing.com/ontologies/foodpairing-kg#icat:000010"/>
        <skos:definition xml:lang="en">Relates to the sensory perception resulting from the combination of taste and aroma in food and beverages.</skos:definition>
        <skos:prefLabel xml:lang="en">Flavour</skos:prefLabel>
    </owl:NamedIndividual>
    


    <!-- http://www.foodpairing.com/ontologies/foodpairing-kg#icat:000083 -->


    <owl:NamedIndividual rdf:about="http://www.foodpairing.com/ontologies/foodpairing-kg#icat:000083">
        <rdf:type rdf:resource="http://www.foodpairing.com/ontologies/foodpairing-kg#IngredientCategory"/>
        <rdf:type rdf:resource="http://www.w3.org/2004/02/skos/core#Concept"/>
        <skos:broader rdf:resource="http://www.foodpairing.com/ontologies/foodpairing-kg#icat:000011"/>
        <skos:definition xml:lang="en">Refers to macronutrients that are a concentrated source of energy, such as butter, lard, and oils, used in cooking and baking.</skos:definition>
        <skos:prefLabel xml:lang="en">Fats</skos:prefLabel>
    </owl:NamedIndividual>
    


    <!-- http://www.foodpairing.com/ontologies/foodpairing-kg#icat:000084 -->


    <owl:NamedIndividual rdf:about="http://www.foodpairing.com/ontologies/foodpairing-kg#icat:000084">
        <rdf:type rdf:resource="http://www.foodpairing.com/ontologies/foodpairing-kg#IngredientCategory"/>
        <rdf:type rdf:resource="http://www.w3.org/2004/02/skos/core#Concept"/>
        <skos:broader rdf:resource="http://www.foodpairing.com/ontologies/foodpairing-kg#icat:000011"/>
        <skos:definition xml:lang="en">Includes various liquid fats derived from plants or animals, often used for cooking, frying, and as dressings or flavorings.</skos:definition>
        <skos:prefLabel xml:lang="en">Oils</skos:prefLabel>
    </owl:NamedIndividual>
    


    <!-- http://www.foodpairing.com/ontologies/foodpairing-kg#icat:000085 -->


    <owl:NamedIndividual rdf:about="http://www.foodpairing.com/ontologies/foodpairing-kg#icat:000085">
        <rdf:type rdf:resource="http://www.foodpairing.com/ontologies/foodpairing-kg#IngredientCategory"/>
        <rdf:type rdf:resource="http://www.w3.org/2004/02/skos/core#Concept"/>
        <skos:broader rdf:resource="http://www.foodpairing.com/ontologies/foodpairing-kg#icat:000012"/>
        <skos:definition xml:lang="en">Encompasses substances added to food products to enhance taste, texture, appearance, or extend shelf life, such as preservatives or emulsifiers.</skos:definition>
        <skos:prefLabel xml:lang="en">Additives</skos:prefLabel>
    </owl:NamedIndividual>
    


    <!-- http://www.foodpairing.com/ontologies/foodpairing-kg#icat:000086 -->


    <owl:NamedIndividual rdf:about="http://www.foodpairing.com/ontologies/foodpairing-kg#icat:000086">
        <rdf:type rdf:resource="http://www.foodpairing.com/ontologies/foodpairing-kg#IngredientCategory"/>
        <rdf:type rdf:resource="http://www.w3.org/2004/02/skos/core#Concept"/>
        <skos:broader rdf:resource="http://www.foodpairing.com/ontologies/foodpairing-kg#icat:000012"/>
        <skos:definition xml:lang="en">Refers to substances used to add or enhance color in food and beverages, such as natural or synthetic food dyes.</skos:definition>
        <skos:prefLabel xml:lang="en">Colouring</skos:prefLabel>
    </owl:NamedIndividual>
    


    <!-- http://www.foodpairing.com/ontologies/foodpairing-kg#icat:000087 -->


    <owl:NamedIndividual rdf:about="http://www.foodpairing.com/ontologies/foodpairing-kg#icat:000087">
        <rdf:type rdf:resource="http://www.foodpairing.com/ontologies/foodpairing-kg#IngredientCategory"/>
        <rdf:type rdf:resource="http://www.w3.org/2004/02/skos/core#Concept"/>
        <skos:broader rdf:resource="http://www.foodpairing.com/ontologies/foodpairing-kg#icat:000012"/>
        <skos:definition xml:lang="en">Relates to the distinct taste or aroma of a food or beverage, often achieved through natural or artificial flavorings.</skos:definition>
        <skos:prefLabel xml:lang="en">Flavor</skos:prefLabel>
    </owl:NamedIndividual>
    


    <!-- http://www.foodpairing.com/ontologies/foodpairing-kg#icat:000088 -->


    <owl:NamedIndividual rdf:about="http://www.foodpairing.com/ontologies/foodpairing-kg#icat:000088">
        <rdf:type rdf:resource="http://www.foodpairing.com/ontologies/foodpairing-kg#IngredientCategory"/>
        <rdf:type rdf:resource="http://www.w3.org/2004/02/skos/core#Concept"/>
        <skos:broader rdf:resource="http://www.foodpairing.com/ontologies/foodpairing-kg#icat:000014"/>
        <skos:definition xml:lang="en">Encompasses small, edible fruits, often colorful and packed with antioxidants, such as strawberries, blueberries, and raspberries.</skos:definition>
        <skos:prefLabel xml:lang="en">Berries</skos:prefLabel>
    </owl:NamedIndividual>
    


    <!-- http://www.foodpairing.com/ontologies/foodpairing-kg#icat:000089 -->


    <owl:NamedIndividual rdf:about="http://www.foodpairing.com/ontologies/foodpairing-kg#icat:000089">
        <rdf:type rdf:resource="http://www.foodpairing.com/ontologies/foodpairing-kg#IngredientCategory"/>
        <rdf:type rdf:resource="http://www.w3.org/2004/02/skos/core#Concept"/>
        <skos:broader rdf:resource="http://www.foodpairing.com/ontologies/foodpairing-kg#icat:000014"/>
        <skos:definition xml:lang="en">Refers to a group of fruits characterized by their acidic taste and high vitamin C content, including oranges, lemons, and grapefruits.</skos:definition>
        <skos:prefLabel xml:lang="en">Citrus Fruits</skos:prefLabel>
    </owl:NamedIndividual>
    


    <!-- http://www.foodpairing.com/ontologies/foodpairing-kg#icat:000090 -->


    <owl:NamedIndividual rdf:about="http://www.foodpairing.com/ontologies/foodpairing-kg#icat:000090">
        <rdf:type rdf:resource="http://www.foodpairing.com/ontologies/foodpairing-kg#IngredientCategory"/>
        <rdf:type rdf:resource="http://www.w3.org/2004/02/skos/core#Concept"/>
        <skos:broader rdf:resource="http://www.foodpairing.com/ontologies/foodpairing-kg#icat:000014"/>
        <skos:definition xml:lang="en">Encompasses fruits with a hard, outer rind and soft inner flesh, such as melons, cucumbers, and squash.</skos:definition>
        <skos:prefLabel xml:lang="en">Pepo Fruits</skos:prefLabel>
    </owl:NamedIndividual>
    


    <!-- http://www.foodpairing.com/ontologies/foodpairing-kg#icat:000091 -->


    <owl:NamedIndividual rdf:about="http://www.foodpairing.com/ontologies/foodpairing-kg#icat:000091">
        <rdf:type rdf:resource="http://www.foodpairing.com/ontologies/foodpairing-kg#IngredientCategory"/>
        <rdf:type rdf:resource="http://www.w3.org/2004/02/skos/core#Concept"/>
        <skos:broader rdf:resource="http://www.foodpairing.com/ontologies/foodpairing-kg#icat:000014"/>
        <skos:definition xml:lang="en">Relates to fruits with a central core containing seeds, often sweet and juicy, such as apples, pears, and quinces.</skos:definition>
        <skos:prefLabel xml:lang="en">Pome Fruits</skos:prefLabel>
    </owl:NamedIndividual>
    


    <!-- http://www.foodpairing.com/ontologies/foodpairing-kg#icat:000092 -->


    <owl:NamedIndividual rdf:about="http://www.foodpairing.com/ontologies/foodpairing-kg#icat:000092">
        <rdf:type rdf:resource="http://www.foodpairing.com/ontologies/foodpairing-kg#IngredientCategory"/>
        <rdf:type rdf:resource="http://www.w3.org/2004/02/skos/core#Concept"/>
        <skos:broader rdf:resource="http://www.foodpairing.com/ontologies/foodpairing-kg#icat:000014"/>
        <skos:definition xml:lang="en">Includes fruits with a single hard seed or pit surrounded by juicy flesh, such as peaches, plums, cherries, and apricots.</skos:definition>
        <skos:prefLabel xml:lang="en">Stone Fruits</skos:prefLabel>
    </owl:NamedIndividual>
    


    <!-- http://www.foodpairing.com/ontologies/foodpairing-kg#icat:000093 -->


    <owl:NamedIndividual rdf:about="http://www.foodpairing.com/ontologies/foodpairing-kg#icat:000093">
        <rdf:type rdf:resource="http://www.foodpairing.com/ontologies/foodpairing-kg#IngredientCategory"/>
        <rdf:type rdf:resource="http://www.w3.org/2004/02/skos/core#Concept"/>
        <skos:broader rdf:resource="http://www.foodpairing.com/ontologies/foodpairing-kg#icat:000014"/>
        <skos:definition xml:lang="en">Refers to a diverse group of fruits grown in tropical regions, often exotic in appearance and flavors, such as mangoes, pineapples, and papayas.</skos:definition>
        <skos:prefLabel xml:lang="en">Tropical Fruits</skos:prefLabel>
    </owl:NamedIndividual>
    


    <!-- http://www.foodpairing.com/ontologies/foodpairing-kg#icat:000094 -->


    <owl:NamedIndividual rdf:about="http://www.foodpairing.com/ontologies/foodpairing-kg#icat:000094">
        <rdf:type rdf:resource="http://www.foodpairing.com/ontologies/foodpairing-kg#IngredientCategory"/>
        <rdf:type rdf:resource="http://www.w3.org/2004/02/skos/core#Concept"/>
        <skos:broader rdf:resource="http://www.foodpairing.com/ontologies/foodpairing-kg#icat:000015"/>
        <skos:definition xml:lang="en">Encompasses herbs used primarily for cooking and flavoring dishes, such as basil, thyme, rosemary, and parsley.</skos:definition>
        <skos:prefLabel xml:lang="en">Culinairy Herbs</skos:prefLabel>
    </owl:NamedIndividual>
    


    <!-- http://www.foodpairing.com/ontologies/foodpairing-kg#icat:000095 -->


    <owl:NamedIndividual rdf:about="http://www.foodpairing.com/ontologies/foodpairing-kg#icat:000095">
        <rdf:type rdf:resource="http://www.foodpairing.com/ontologies/foodpairing-kg#IngredientCategory"/>
        <rdf:type rdf:resource="http://www.w3.org/2004/02/skos/core#Concept"/>
        <skos:broader rdf:resource="http://www.foodpairing.com/ontologies/foodpairing-kg#icat:000015"/>
        <skos:definition xml:lang="en">Refers to herbs used for their potential health benefits or medicinal properties, such as chamomile, echinacea, and ginseng.</skos:definition>
        <skos:prefLabel xml:lang="en">Medicinal Herbs</skos:prefLabel>
    </owl:NamedIndividual>
    


    <!-- http://www.foodpairing.com/ontologies/foodpairing-kg#icat:000096 -->


    <owl:NamedIndividual rdf:about="http://www.foodpairing.com/ontologies/foodpairing-kg#icat:000096">
        <rdf:type rdf:resource="http://www.foodpairing.com/ontologies/foodpairing-kg#IngredientCategory"/>
        <rdf:type rdf:resource="http://www.w3.org/2004/02/skos/core#Concept"/>
        <skos:broader rdf:resource="http://www.foodpairing.com/ontologies/foodpairing-kg#icat:000016"/>
        <skos:definition xml:lang="en">Relates to substances or compounds used for medical purposes, including over-the-counter drugs or prescription medications.</skos:definition>
        <skos:prefLabel xml:lang="en">Drug Or Medicine</skos:prefLabel>
    </owl:NamedIndividual>
    


    <!-- http://www.foodpairing.com/ontologies/foodpairing-kg#icat:000097 -->


    <owl:NamedIndividual rdf:about="http://www.foodpairing.com/ontologies/foodpairing-kg#icat:000097">
        <rdf:type rdf:resource="http://www.foodpairing.com/ontologies/foodpairing-kg#IngredientCategory"/>
        <rdf:type rdf:resource="http://www.w3.org/2004/02/skos/core#Concept"/>
        <skos:broader rdf:resource="http://www.foodpairing.com/ontologies/foodpairing-kg#icat:000016"/>
        <skos:definition xml:lang="en">Encompasses products consumed to supplement the diet and provide additional nutrients, vitamins, or minerals.</skos:definition>
        <skos:prefLabel xml:lang="en">Dietary Supplement</skos:prefLabel>
    </owl:NamedIndividual>
    


    <!-- http://www.foodpairing.com/ontologies/foodpairing-kg#icat:000098 -->


    <owl:NamedIndividual rdf:about="http://www.foodpairing.com/ontologies/foodpairing-kg#icat:000098">
        <rdf:type rdf:resource="http://www.foodpairing.com/ontologies/foodpairing-kg#IngredientCategory"/>
        <rdf:type rdf:resource="http://www.w3.org/2004/02/skos/core#Concept"/>
        <skos:broader rdf:resource="http://www.foodpairing.com/ontologies/foodpairing-kg#icat:000145"/>
        <skos:definition xml:lang="en">Refers to highly concentrated liquids extracted from plants, often used for their scent, flavor, or potential therapeutic properties.</skos:definition>
        <skos:prefLabel xml:lang="en">Essential Oil</skos:prefLabel>
    </owl:NamedIndividual>
    


    <!-- http://www.foodpairing.com/ontologies/foodpairing-kg#icat:000100 -->


    <owl:NamedIndividual rdf:about="http://www.foodpairing.com/ontologies/foodpairing-kg#icat:000100">
        <rdf:type rdf:resource="http://www.foodpairing.com/ontologies/foodpairing-kg#IngredientCategory"/>
        <rdf:type rdf:resource="http://www.w3.org/2004/02/skos/core#Concept"/>
        <skos:broader rdf:resource="http://www.foodpairing.com/ontologies/foodpairing-kg#icat:000017"/>
        <skos:definition xml:lang="en">Includes edible seeds enclosed in a hard shell, such as almonds, walnuts, cashews, and peanuts, often consumed as snacks or used in cooking.</skos:definition>
        <skos:prefLabel xml:lang="en">Nuts</skos:prefLabel>
    </owl:NamedIndividual>
    


    <!-- http://www.foodpairing.com/ontologies/foodpairing-kg#icat:000101 -->


    <owl:NamedIndividual rdf:about="http://www.foodpairing.com/ontologies/foodpairing-kg#icat:000101">
        <rdf:type rdf:resource="http://www.foodpairing.com/ontologies/foodpairing-kg#IngredientCategory"/>
        <rdf:type rdf:resource="http://www.w3.org/2004/02/skos/core#Concept"/>
        <skos:broader rdf:resource="http://www.foodpairing.com/ontologies/foodpairing-kg#icat:000017"/>
        <skos:definition xml:lang="en">Refers to plant-based beverages made from nuts, such as almond milk or cashew milk, often used as a dairy milk substitute.</skos:definition>
        <skos:prefLabel xml:lang="en">Nut Drink</skos:prefLabel>
    </owl:NamedIndividual>
    


    <!-- http://www.foodpairing.com/ontologies/foodpairing-kg#icat:000102 -->


    <owl:NamedIndividual rdf:about="http://www.foodpairing.com/ontologies/foodpairing-kg#icat:000102">
        <rdf:type rdf:resource="http://www.foodpairing.com/ontologies/foodpairing-kg#IngredientCategory"/>
        <rdf:type rdf:resource="http://www.w3.org/2004/02/skos/core#Concept"/>
        <skos:broader rdf:resource="http://www.foodpairing.com/ontologies/foodpairing-kg#icat:000017"/>
        <skos:definition xml:lang="en">Encompasses spreads made from ground nuts, such as peanut butter, almond butter, or hazelnut spread.</skos:definition>
        <skos:prefLabel xml:lang="en">Nut Butter</skos:prefLabel>
    </owl:NamedIndividual>
    


    <!-- http://www.foodpairing.com/ontologies/foodpairing-kg#icat:000103 -->


    <owl:NamedIndividual rdf:about="http://www.foodpairing.com/ontologies/foodpairing-kg#icat:000103">
        <rdf:type rdf:resource="http://www.foodpairing.com/ontologies/foodpairing-kg#IngredientCategory"/>
        <rdf:type rdf:resource="http://www.w3.org/2004/02/skos/core#Concept"/>
        <skos:broader rdf:resource="http://www.foodpairing.com/ontologies/foodpairing-kg#icat:000017"/>
        <skos:definition xml:lang="en">Includes small, edible plant embryos often used as ingredients in cooking, baking, or eaten as snacks, such as sesame seeds, chia seeds, and sunflower seeds.</skos:definition>
        <skos:prefLabel xml:lang="en">Seeds</skos:prefLabel>
    </owl:NamedIndividual>
    


    <!-- http://www.foodpairing.com/ontologies/foodpairing-kg#icat:000104 -->


    <owl:NamedIndividual rdf:about="http://www.foodpairing.com/ontologies/foodpairing-kg#icat:000104">
        <rdf:type rdf:resource="http://www.foodpairing.com/ontologies/foodpairing-kg#IngredientCategory"/>
        <rdf:type rdf:resource="http://www.w3.org/2004/02/skos/core#Concept"/>
        <skos:broader rdf:resource="http://www.foodpairing.com/ontologies/foodpairing-kg#icat:000019"/>
        <skos:definition xml:lang="en">Refers to a branch of cooking related to prepared meat products, such as cured meats, sausages, pâtés, and terrines.</skos:definition>
        <skos:prefLabel xml:lang="en">Charcuterie</skos:prefLabel>
    </owl:NamedIndividual>
    


    <!-- http://www.foodpairing.com/ontologies/foodpairing-kg#icat:000105 -->


    <owl:NamedIndividual rdf:about="http://www.foodpairing.com/ontologies/foodpairing-kg#icat:000105">
        <rdf:type rdf:resource="http://www.foodpairing.com/ontologies/foodpairing-kg#IngredientCategory"/>
        <rdf:type rdf:resource="http://www.w3.org/2004/02/skos/core#Concept"/>
        <skos:broader rdf:resource="http://www.foodpairing.com/ontologies/foodpairing-kg#icat:000019"/>
        <skos:definition xml:lang="en">Encompasses various edible aquatic creatures, often prepared as food, such as salmon, tuna, cod, or trout.</skos:definition>
        <skos:prefLabel xml:lang="en">Fish</skos:prefLabel>
    </owl:NamedIndividual>
    


    <!-- http://www.foodpairing.com/ontologies/foodpairing-kg#icat:000106 -->


    <owl:NamedIndividual rdf:about="http://www.foodpairing.com/ontologies/foodpairing-kg#icat:000106">
        <rdf:type rdf:resource="http://www.foodpairing.com/ontologies/foodpairing-kg#IngredientCategory"/>
        <rdf:type rdf:resource="http://www.w3.org/2004/02/skos/core#Concept"/>
        <skos:broader rdf:resource="http://www.foodpairing.com/ontologies/foodpairing-kg#icat:000019"/>
        <skos:definition xml:lang="en">Includes edible insects consumed as food, such as crickets, mealworms, or grasshoppers, which are part of some cultural cuisines.</skos:definition>
        <skos:prefLabel xml:lang="en">Insects</skos:prefLabel>
    </owl:NamedIndividual>
    


    <!-- http://www.foodpairing.com/ontologies/foodpairing-kg#icat:000107 -->


    <owl:NamedIndividual rdf:about="http://www.foodpairing.com/ontologies/foodpairing-kg#icat:000107">
        <rdf:type rdf:resource="http://www.foodpairing.com/ontologies/foodpairing-kg#IngredientCategory"/>
        <rdf:type rdf:resource="http://www.w3.org/2004/02/skos/core#Concept"/>
        <skos:broader rdf:resource="http://www.foodpairing.com/ontologies/foodpairing-kg#icat:000019"/>
        <skos:definition xml:lang="en">Refers to the flesh of animals used as food, such as beef, pork, lamb, or poultry, which can be cooked in various ways.</skos:definition>
        <skos:prefLabel xml:lang="en">Meats</skos:prefLabel>
    </owl:NamedIndividual>
    


    <!-- http://www.foodpairing.com/ontologies/foodpairing-kg#icat:000108 -->


    <owl:NamedIndividual rdf:about="http://www.foodpairing.com/ontologies/foodpairing-kg#icat:000108">
        <rdf:type rdf:resource="http://www.foodpairing.com/ontologies/foodpairing-kg#IngredientCategory"/>
        <rdf:type rdf:resource="http://www.w3.org/2004/02/skos/core#Concept"/>
        <skos:broader rdf:resource="http://www.foodpairing.com/ontologies/foodpairing-kg#icat:000019"/>
        <skos:definition xml:lang="en">Encompasses protein-rich foods derived from plants, such as legumes, tofu, tempeh, seitan, and plant-based meat alternatives.</skos:definition>
        <skos:prefLabel xml:lang="en">Plant-based Proteins</skos:prefLabel>
    </owl:NamedIndividual>
    


    <!-- http://www.foodpairing.com/ontologies/foodpairing-kg#icat:000109 -->


    <owl:NamedIndividual rdf:about="http://www.foodpairing.com/ontologies/foodpairing-kg#icat:000109">
        <rdf:type rdf:resource="http://www.foodpairing.com/ontologies/foodpairing-kg#IngredientCategory"/>
        <rdf:type rdf:resource="http://www.w3.org/2004/02/skos/core#Concept"/>
        <skos:broader rdf:resource="http://www.foodpairing.com/ontologies/foodpairing-kg#icat:000019"/>
        <skos:definition xml:lang="en">Refers to various edible creatures from the sea, including fish, shellfish (such as shrimp, lobster, or crab), and mollusks (such as clams, oysters, or mussels).</skos:definition>
        <skos:prefLabel xml:lang="en">Seafoods</skos:prefLabel>
    </owl:NamedIndividual>
    


    <!-- http://www.foodpairing.com/ontologies/foodpairing-kg#icat:000110 -->


    <owl:NamedIndividual rdf:about="http://www.foodpairing.com/ontologies/foodpairing-kg#icat:000110">
        <rdf:type rdf:resource="http://www.foodpairing.com/ontologies/foodpairing-kg#IngredientCategory"/>
        <rdf:type rdf:resource="http://www.w3.org/2004/02/skos/core#Concept"/>
        <skos:broader rdf:resource="http://www.foodpairing.com/ontologies/foodpairing-kg#icat:000021"/>
        <skos:definition xml:lang="en">Includes crispy snack foods made from potatoes, corn, or other vegetables, often flavored and fried or baked.</skos:definition>
        <skos:prefLabel xml:lang="en">Chips And Crisps</skos:prefLabel>
    </owl:NamedIndividual>
    


    <!-- http://www.foodpairing.com/ontologies/foodpairing-kg#icat:000111 -->


    <owl:NamedIndividual rdf:about="http://www.foodpairing.com/ontologies/foodpairing-kg#icat:000111">
        <rdf:type rdf:resource="http://www.foodpairing.com/ontologies/foodpairing-kg#IngredientCategory"/>
        <rdf:type rdf:resource="http://www.w3.org/2004/02/skos/core#Concept"/>
        <skos:broader rdf:resource="http://www.foodpairing.com/ontologies/foodpairing-kg#icat:000021"/>
        <skos:definition xml:lang="en">Refers to a type of corn kernel that puffs up and becomes light and crispy when heated, commonly consumed as a snack.</skos:definition>
        <skos:prefLabel xml:lang="en">Popcorn</skos:prefLabel>
    </owl:NamedIndividual>
    


    <!-- http://www.foodpairing.com/ontologies/foodpairing-kg#icat:000112 -->


    <owl:NamedIndividual rdf:about="http://www.foodpairing.com/ontologies/foodpairing-kg#icat:000112">
        <rdf:type rdf:resource="http://www.foodpairing.com/ontologies/foodpairing-kg#IngredientCategory"/>
        <rdf:type rdf:resource="http://www.w3.org/2004/02/skos/core#Concept"/>
        <skos:broader rdf:resource="http://www.foodpairing.com/ontologies/foodpairing-kg#icat:000021"/>
        <skos:definition xml:lang="en">Encompasses snack foods made from rice, such as rice cakes, rice crackers, or puffed rice snacks, often flavored or seasoned.</skos:definition>
        <skos:prefLabel xml:lang="en">Rice Snacks</skos:prefLabel>
    </owl:NamedIndividual>
    


    <!-- http://www.foodpairing.com/ontologies/foodpairing-kg#icat:000113 -->


    <owl:NamedIndividual rdf:about="http://www.foodpairing.com/ontologies/foodpairing-kg#icat:000113">
        <rdf:type rdf:resource="http://www.foodpairing.com/ontologies/foodpairing-kg#IngredientCategory"/>
        <rdf:type rdf:resource="http://www.w3.org/2004/02/skos/core#Concept"/>
        <skos:broader rdf:resource="http://www.foodpairing.com/ontologies/foodpairing-kg#icat:000023"/>
        <skos:definition xml:lang="en">Includes spices derived from anise and licorice plants, offering distinctive flavors often used in culinary and confectionery preparations.</skos:definition>
        <skos:prefLabel xml:lang="en">Anise And Liquorice Spices</skos:prefLabel>
    </owl:NamedIndividual>
    


    <!-- http://www.foodpairing.com/ontologies/foodpairing-kg#icat:000114 -->


    <owl:NamedIndividual rdf:about="http://www.foodpairing.com/ontologies/foodpairing-kg#icat:000114">
        <rdf:type rdf:resource="http://www.foodpairing.com/ontologies/foodpairing-kg#IngredientCategory"/>
        <rdf:type rdf:resource="http://www.w3.org/2004/02/skos/core#Concept"/>
        <skos:broader rdf:resource="http://www.foodpairing.com/ontologies/foodpairing-kg#icat:000023"/>
        <skos:definition xml:lang="en">Refers to spices with a bitter taste, often used in small quantities to add complexity and depth of flavor to dishes.</skos:definition>
        <skos:prefLabel xml:lang="en">Bitter Spices</skos:prefLabel>
    </owl:NamedIndividual>
    


    <!-- http://www.foodpairing.com/ontologies/foodpairing-kg#icat:000115 -->


    <owl:NamedIndividual rdf:about="http://www.foodpairing.com/ontologies/foodpairing-kg#icat:000115">
        <rdf:type rdf:resource="http://www.foodpairing.com/ontologies/foodpairing-kg#IngredientCategory"/>
        <rdf:type rdf:resource="http://www.w3.org/2004/02/skos/core#Concept"/>
        <skos:broader rdf:resource="http://www.foodpairing.com/ontologies/foodpairing-kg#icat:000023"/>
        <skos:definition xml:lang="en">Encompasses spices derived from citrus fruits, such as lemon zest, orange peel, or lime leaves, adding tangy and aromatic notes.</skos:definition>
        <skos:prefLabel xml:lang="en">Citrus Spices</skos:prefLabel>
    </owl:NamedIndividual>
    


    <!-- http://www.foodpairing.com/ontologies/foodpairing-kg#icat:000116 -->


    <owl:NamedIndividual rdf:about="http://www.foodpairing.com/ontologies/foodpairing-kg#icat:000116">
        <rdf:type rdf:resource="http://www.foodpairing.com/ontologies/foodpairing-kg#IngredientCategory"/>
        <rdf:type rdf:resource="http://www.w3.org/2004/02/skos/core#Concept"/>
        <skos:broader rdf:resource="http://www.foodpairing.com/ontologies/foodpairing-kg#icat:000023"/>
        <skos:definition xml:lang="en">Includes spices with a nutty flavor profile, such as almonds, cashews, or hazelnuts, used to enhance the taste of dishes or desserts.</skos:definition>
        <skos:prefLabel xml:lang="en">Nutty Spices</skos:prefLabel>
    </owl:NamedIndividual>
    


    <!-- http://www.foodpairing.com/ontologies/foodpairing-kg#icat:000117 -->


    <owl:NamedIndividual rdf:about="http://www.foodpairing.com/ontologies/foodpairing-kg#icat:000117">
        <rdf:type rdf:resource="http://www.foodpairing.com/ontologies/foodpairing-kg#IngredientCategory"/>
        <rdf:type rdf:resource="http://www.w3.org/2004/02/skos/core#Concept"/>
        <skos:broader rdf:resource="http://www.foodpairing.com/ontologies/foodpairing-kg#icat:000023"/>
        <skos:definition xml:lang="en">Refers to spices with a strong, sharp, or intense taste, often used to add heat or spiciness to foods, such as chili peppers or mustard seeds.</skos:definition>
        <skos:prefLabel xml:lang="en">Pungent Spices</skos:prefLabel>
    </owl:NamedIndividual>
    


    <!-- http://www.foodpairing.com/ontologies/foodpairing-kg#icat:000118 -->


    <owl:NamedIndividual rdf:about="http://www.foodpairing.com/ontologies/foodpairing-kg#icat:000118">
        <rdf:type rdf:resource="http://www.foodpairing.com/ontologies/foodpairing-kg#IngredientCategory"/>
        <rdf:type rdf:resource="http://www.w3.org/2004/02/skos/core#Concept"/>
        <skos:broader rdf:resource="http://www.foodpairing.com/ontologies/foodpairing-kg#icat:000023"/>
        <skos:definition xml:lang="en">Encompasses spices with a tangy or fruity flavor, such as tamarind, sumac, or dried berries, used to enhance sweet or savory dishes.</skos:definition>
        <skos:prefLabel xml:lang="en">Sour And Fruity Spices</skos:prefLabel>
    </owl:NamedIndividual>
    


    <!-- http://www.foodpairing.com/ontologies/foodpairing-kg#icat:000119 -->


    <owl:NamedIndividual rdf:about="http://www.foodpairing.com/ontologies/foodpairing-kg#icat:000119">
        <rdf:type rdf:resource="http://www.foodpairing.com/ontologies/foodpairing-kg#IngredientCategory"/>
        <rdf:type rdf:resource="http://www.w3.org/2004/02/skos/core#Concept"/>
        <skos:broader rdf:resource="http://www.foodpairing.com/ontologies/foodpairing-kg#icat:000023"/>
        <skos:definition xml:lang="en">Includes blends of different spices and herbs, often used to season various dishes or add flavor to sauces, marinades, or rubs.</skos:definition>
        <skos:prefLabel xml:lang="en">Spice Mixes</skos:prefLabel>
    </owl:NamedIndividual>
    


    <!-- http://www.foodpairing.com/ontologies/foodpairing-kg#icat:000120 -->


    <owl:NamedIndividual rdf:about="http://www.foodpairing.com/ontologies/foodpairing-kg#icat:000120">
        <rdf:type rdf:resource="http://www.foodpairing.com/ontologies/foodpairing-kg#IngredientCategory"/>
        <rdf:type rdf:resource="http://www.w3.org/2004/02/skos/core#Concept"/>
        <skos:broader rdf:resource="http://www.foodpairing.com/ontologies/foodpairing-kg#icat:000023"/>
        <skos:definition xml:lang="en">Refers to spices with a sweet taste or aroma, such as cinnamon, vanilla, or nutmeg, often used in desserts, baked goods, or sweet beverages.</skos:definition>
        <skos:prefLabel xml:lang="en">Sweet Spices</skos:prefLabel>
    </owl:NamedIndividual>
    


    <!-- http://www.foodpairing.com/ontologies/foodpairing-kg#icat:000121 -->


    <owl:NamedIndividual rdf:about="http://www.foodpairing.com/ontologies/foodpairing-kg#icat:000121">
        <rdf:type rdf:resource="http://www.foodpairing.com/ontologies/foodpairing-kg#IngredientCategory"/>
        <rdf:type rdf:resource="http://www.w3.org/2004/02/skos/core#Concept"/>
        <skos:broader rdf:resource="http://www.foodpairing.com/ontologies/foodpairing-kg#icat:000023"/>
        <skos:definition xml:lang="en">Encompasses spices that create a warm and cozy flavor profile, often associated with fall or winter dishes, such as cloves, ginger, or allspice.</skos:definition>
        <skos:prefLabel xml:lang="en">Warm Spices</skos:prefLabel>
    </owl:NamedIndividual>
    


    <!-- http://www.foodpairing.com/ontologies/foodpairing-kg#icat:000122 -->


    <owl:NamedIndividual rdf:about="http://www.foodpairing.com/ontologies/foodpairing-kg#icat:000122">
        <rdf:type rdf:resource="http://www.foodpairing.com/ontologies/foodpairing-kg#IngredientCategory"/>
        <rdf:type rdf:resource="http://www.w3.org/2004/02/skos/core#Concept"/>
        <skos:broader rdf:resource="http://www.foodpairing.com/ontologies/foodpairing-kg#icat:000117"/>
        <skos:definition xml:lang="en">Includes spices derived from various pepper plants, such as black pepper, white pepper, or pink peppercorns, adding heat and pungency to dishes.</skos:definition>
        <skos:prefLabel xml:lang="en">Pepper Spices</skos:prefLabel>
    </owl:NamedIndividual>
    


    <!-- http://www.foodpairing.com/ontologies/foodpairing-kg#icat:000123 -->


    <owl:NamedIndividual rdf:about="http://www.foodpairing.com/ontologies/foodpairing-kg#icat:000123">
        <rdf:type rdf:resource="http://www.foodpairing.com/ontologies/foodpairing-kg#IngredientCategory"/>
        <rdf:type rdf:resource="http://www.w3.org/2004/02/skos/core#Concept"/>
        <skos:broader rdf:resource="http://www.foodpairing.com/ontologies/foodpairing-kg#icat:000117"/>
        <skos:definition xml:lang="en">Refers to spices made from chili peppers, offering varying levels of heat and flavors, often used in spicy dishes or hot sauces.</skos:definition>
        <skos:prefLabel xml:lang="en">Chili Spices</skos:prefLabel>
    </owl:NamedIndividual>
    


    <!-- http://www.foodpairing.com/ontologies/foodpairing-kg#icat:000124 -->


    <owl:NamedIndividual rdf:about="http://www.foodpairing.com/ontologies/foodpairing-kg#icat:000124">
        <rdf:type rdf:resource="http://www.foodpairing.com/ontologies/foodpairing-kg#IngredientCategory"/>
        <rdf:type rdf:resource="http://www.w3.org/2004/02/skos/core#Concept"/>
        <skos:broader rdf:resource="http://www.foodpairing.com/ontologies/foodpairing-kg#icat:000024"/>
        <skos:definition xml:lang="en">Encompasses confectionery products made by heating sugar, often combined with butter, cream, or milk, resulting in a sweet and chewy treat.</skos:definition>
        <skos:prefLabel xml:lang="en">Caramels</skos:prefLabel>
    </owl:NamedIndividual>
    


    <!-- http://www.foodpairing.com/ontologies/foodpairing-kg#icat:000125 -->


    <owl:NamedIndividual rdf:about="http://www.foodpairing.com/ontologies/foodpairing-kg#icat:000125">
        <rdf:type rdf:resource="http://www.foodpairing.com/ontologies/foodpairing-kg#IngredientCategory"/>
        <rdf:type rdf:resource="http://www.w3.org/2004/02/skos/core#Concept"/>
        <skos:broader rdf:resource="http://www.foodpairing.com/ontologies/foodpairing-kg#icat:000024"/>
        <skos:definition xml:lang="en">Refers to a sweet, viscous liquid produced by bees from flower nectar, often used as a natural sweetener and flavoring agent.</skos:definition>
        <skos:prefLabel xml:lang="en">Honeys</skos:prefLabel>
    </owl:NamedIndividual>
    


    <!-- http://www.foodpairing.com/ontologies/foodpairing-kg#icat:000126 -->


    <owl:NamedIndividual rdf:about="http://www.foodpairing.com/ontologies/foodpairing-kg#icat:000126">
        <rdf:type rdf:resource="http://www.foodpairing.com/ontologies/foodpairing-kg#IngredientCategory"/>
        <rdf:type rdf:resource="http://www.w3.org/2004/02/skos/core#Concept"/>
        <skos:broader rdf:resource="http://www.foodpairing.com/ontologies/foodpairing-kg#icat:000024"/>
        <skos:definition xml:lang="en">Includes thick, sweet liquids made by dissolving sugar in water or other liquids, often used as sweeteners or flavorings in beverages or desserts.</skos:definition>
        <skos:prefLabel xml:lang="en">Syrups</skos:prefLabel>
    </owl:NamedIndividual>
    


    <!-- http://www.foodpairing.com/ontologies/foodpairing-kg#icat:000127 -->


    <owl:NamedIndividual rdf:about="http://www.foodpairing.com/ontologies/foodpairing-kg#icat:000127">
        <rdf:type rdf:resource="http://www.foodpairing.com/ontologies/foodpairing-kg#IngredientCategory"/>
        <rdf:type rdf:resource="http://www.w3.org/2004/02/skos/core#Concept"/>
        <skos:broader rdf:resource="http://www.foodpairing.com/ontologies/foodpairing-kg#icat:000025"/>
        <skos:definition xml:lang="en">Encompasses vegetables with edible bulbs, such as onions, garlic, shallots, or fennel, used as aromatic ingredients in cooking.</skos:definition>
        <skos:prefLabel xml:lang="en">Bulb Vegetables</skos:prefLabel>
    </owl:NamedIndividual>
    


    <!-- http://www.foodpairing.com/ontologies/foodpairing-kg#icat:000128 -->


    <owl:NamedIndividual rdf:about="http://www.foodpairing.com/ontologies/foodpairing-kg#icat:000128">
        <rdf:type rdf:resource="http://www.foodpairing.com/ontologies/foodpairing-kg#IngredientCategory"/>
        <rdf:type rdf:resource="http://www.w3.org/2004/02/skos/core#Concept"/>
        <skos:broader rdf:resource="http://www.foodpairing.com/ontologies/foodpairing-kg#icat:000025"/>
        <skos:definition xml:lang="en">Refers to vegetables where the flowers or flower buds are consumed, such as broccoli, cauliflower, artichokes, or capers.</skos:definition>
        <skos:prefLabel xml:lang="en">Flower Vegetables</skos:prefLabel>
    </owl:NamedIndividual>
    


    <!-- http://www.foodpairing.com/ontologies/foodpairing-kg#icat:000129 -->


    <owl:NamedIndividual rdf:about="http://www.foodpairing.com/ontologies/foodpairing-kg#icat:000129">
        <rdf:type rdf:resource="http://www.foodpairing.com/ontologies/foodpairing-kg#IngredientCategory"/>
        <rdf:type rdf:resource="http://www.w3.org/2004/02/skos/core#Concept"/>
        <skos:broader rdf:resource="http://www.foodpairing.com/ontologies/foodpairing-kg#icat:000025"/>
        <skos:definition xml:lang="en">Encompasses vegetables that are botanically classified as fruits, such as tomatoes, cucumbers, eggplants, or bell peppers.</skos:definition>
        <skos:prefLabel xml:lang="en">Fruit Vegetables</skos:prefLabel>
    </owl:NamedIndividual>
    


    <!-- http://www.foodpairing.com/ontologies/foodpairing-kg#icat:000130 -->


    <owl:NamedIndividual rdf:about="http://www.foodpairing.com/ontologies/foodpairing-kg#icat:000130">
        <rdf:type rdf:resource="http://www.foodpairing.com/ontologies/foodpairing-kg#IngredientCategory"/>
        <rdf:type rdf:resource="http://www.w3.org/2004/02/skos/core#Concept"/>
        <skos:broader rdf:resource="http://www.foodpairing.com/ontologies/foodpairing-kg#icat:000025"/>
        <skos:definition xml:lang="en">Includes vegetables where the leaves are the primary edible part, such as cabbage, Swiss chard, or bok choy.</skos:definition>
        <skos:prefLabel xml:lang="en">Leaves Vegetables</skos:prefLabel>
    </owl:NamedIndividual>
    


    <!-- http://www.foodpairing.com/ontologies/foodpairing-kg#icat:000131 -->


    <owl:NamedIndividual rdf:about="http://www.foodpairing.com/ontologies/foodpairing-kg#icat:000131">
        <rdf:type rdf:resource="http://www.foodpairing.com/ontologies/foodpairing-kg#IngredientCategory"/>
        <rdf:type rdf:resource="http://www.w3.org/2004/02/skos/core#Concept"/>
        <skos:broader rdf:resource="http://www.foodpairing.com/ontologies/foodpairing-kg#icat:000025"/>
        <skos:definition xml:lang="en">Encompasses various edible fungi, including mushrooms, truffles, and other types of fungi used in culinary preparations.</skos:definition>
        <skos:prefLabel xml:lang="en">Mushroom And Funghi</skos:prefLabel>
    </owl:NamedIndividual>
    


    <!-- http://www.foodpairing.com/ontologies/foodpairing-kg#icat:000132 -->


    <owl:NamedIndividual rdf:about="http://www.foodpairing.com/ontologies/foodpairing-kg#icat:000132">
        <rdf:type rdf:resource="http://www.foodpairing.com/ontologies/foodpairing-kg#IngredientCategory"/>
        <rdf:type rdf:resource="http://www.w3.org/2004/02/skos/core#Concept"/>
        <skos:broader rdf:resource="http://www.foodpairing.com/ontologies/foodpairing-kg#icat:000025"/>
        <skos:definition xml:lang="en">Refers to vegetables where the root portion is consumed, such as carrots, potatoes, turnips, or radishes, often used in soups or stews.</skos:definition>
        <skos:prefLabel xml:lang="en">Root Vegetables</skos:prefLabel>
    </owl:NamedIndividual>
    


    <!-- http://www.foodpairing.com/ontologies/foodpairing-kg#icat:000133 -->


    <owl:NamedIndividual rdf:about="http://www.foodpairing.com/ontologies/foodpairing-kg#icat:000133">
        <rdf:type rdf:resource="http://www.foodpairing.com/ontologies/foodpairing-kg#IngredientCategory"/>
        <rdf:type rdf:resource="http://www.w3.org/2004/02/skos/core#Concept"/>
        <skos:broader rdf:resource="http://www.foodpairing.com/ontologies/foodpairing-kg#icat:000025"/>
        <skos:definition xml:lang="en">Includes vegetables and algae that grow in the sea or saltwater environments, such as seaweed, kelp, or sea asparagus.</skos:definition>
        <skos:prefLabel xml:lang="en">Sea-grown Vegetables</skos:prefLabel>
    </owl:NamedIndividual>
    


    <!-- http://www.foodpairing.com/ontologies/foodpairing-kg#icat:000134 -->


    <owl:NamedIndividual rdf:about="http://www.foodpairing.com/ontologies/foodpairing-kg#icat:000134">
        <rdf:type rdf:resource="http://www.foodpairing.com/ontologies/foodpairing-kg#IngredientCategory"/>
        <rdf:type rdf:resource="http://www.w3.org/2004/02/skos/core#Concept"/>
        <skos:broader rdf:resource="http://www.foodpairing.com/ontologies/foodpairing-kg#icat:000025"/>
        <skos:definition xml:lang="en">Encompasses vegetables where the seeds or seed pods are the primary edible part, such as beans, peas, or corn.</skos:definition>
        <skos:prefLabel xml:lang="en">Seed Vegetables</skos:prefLabel>
    </owl:NamedIndividual>
    


    <!-- http://www.foodpairing.com/ontologies/foodpairing-kg#icat:000135 -->


    <owl:NamedIndividual rdf:about="http://www.foodpairing.com/ontologies/foodpairing-kg#icat:000135">
        <rdf:type rdf:resource="http://www.foodpairing.com/ontologies/foodpairing-kg#IngredientCategory"/>
        <rdf:type rdf:resource="http://www.w3.org/2004/02/skos/core#Concept"/>
        <skos:broader rdf:resource="http://www.foodpairing.com/ontologies/foodpairing-kg#icat:000025"/>
        <skos:definition xml:lang="en">Refers to young, tender shoots or germinated seeds of various vegetables, often used as a fresh ingredient in salads or sandwiches.</skos:definition>
        <skos:prefLabel xml:lang="en">Sprouts</skos:prefLabel>
    </owl:NamedIndividual>
    


    <!-- http://www.foodpairing.com/ontologies/foodpairing-kg#icat:000136 -->


    <owl:NamedIndividual rdf:about="http://www.foodpairing.com/ontologies/foodpairing-kg#icat:000136">
        <rdf:type rdf:resource="http://www.foodpairing.com/ontologies/foodpairing-kg#IngredientCategory"/>
        <rdf:type rdf:resource="http://www.w3.org/2004/02/skos/core#Concept"/>
        <skos:broader rdf:resource="http://www.foodpairing.com/ontologies/foodpairing-kg#icat:000025"/>
        <skos:definition xml:lang="en">Includes vegetables where the stem or stalk portion is consumed, such as asparagus, celery, or rhubarb.</skos:definition>
        <skos:prefLabel xml:lang="en">Stem Vegetables</skos:prefLabel>
    </owl:NamedIndividual>
    


    <!-- http://www.foodpairing.com/ontologies/foodpairing-kg#icat:000137 -->


    <owl:NamedIndividual rdf:about="http://www.foodpairing.com/ontologies/foodpairing-kg#icat:000137">
        <rdf:type rdf:resource="http://www.foodpairing.com/ontologies/foodpairing-kg#IngredientCategory"/>
        <rdf:type rdf:resource="http://www.w3.org/2004/02/skos/core#Concept"/>
        <skos:broader rdf:resource="http://www.foodpairing.com/ontologies/foodpairing-kg#icat:000025"/>
        <skos:definition xml:lang="en">Refers to vegetables where the enlarged underground stem or tuber is consumed, such as potatoes, yams, or taro.</skos:definition>
        <skos:prefLabel xml:lang="en">Tuber Vegetables</skos:prefLabel>
    </owl:NamedIndividual>
    


    <!-- http://www.foodpairing.com/ontologies/foodpairing-kg#icat:000138 -->


    <owl:NamedIndividual rdf:about="http://www.foodpairing.com/ontologies/foodpairing-kg#icat:000138">
        <rdf:type rdf:resource="http://www.foodpairing.com/ontologies/foodpairing-kg#IngredientCategory"/>
        <rdf:type rdf:resource="http://www.w3.org/2004/02/skos/core#Concept"/>
        <skos:broader rdf:resource="http://www.foodpairing.com/ontologies/foodpairing-kg#icat:000129"/>
        <skos:definition xml:lang="en">Refers to spicy peppers, often used as a seasoning or ingredient to add heat and flavor to dishes.</skos:definition>
        <skos:prefLabel xml:lang="en">Chili</skos:prefLabel>
    </owl:NamedIndividual>
    


    <!-- http://www.foodpairing.com/ontologies/foodpairing-kg#icat:000139 -->


    <owl:NamedIndividual rdf:about="http://www.foodpairing.com/ontologies/foodpairing-kg#icat:000139">
        <rdf:type rdf:resource="http://www.foodpairing.com/ontologies/foodpairing-kg#IngredientCategory"/>
        <rdf:type rdf:resource="http://www.w3.org/2004/02/skos/core#Concept"/>
        <skos:broader rdf:resource="http://www.foodpairing.com/ontologies/foodpairing-kg#icat:000130"/>
        <skos:definition xml:lang="en">Includes a variety of edible leafy vegetables, such as spinach, lettuce, kale, or Swiss chard, often used in salads or cooked as side dishes.</skos:definition>
        <skos:prefLabel xml:lang="en">Leafy Greens</skos:prefLabel>
    </owl:NamedIndividual>
    


    <!-- http://www.foodpairing.com/ontologies/foodpairing-kg#icat:000140 -->


    <owl:NamedIndividual rdf:about="http://www.foodpairing.com/ontologies/foodpairing-kg#icat:000140">
        <rdf:type rdf:resource="http://www.foodpairing.com/ontologies/foodpairing-kg#IngredientCategory"/>
        <rdf:type rdf:resource="http://www.w3.org/2004/02/skos/core#Concept"/>
        <skos:broader rdf:resource="http://www.foodpairing.com/ontologies/foodpairing-kg#icat:000130"/>
        <skos:definition xml:lang="en">Encompasses different types of lettuce, such as romaine, iceberg, or butterhead, often used in salads or as a bed for other ingredients.</skos:definition>
        <skos:prefLabel xml:lang="en">Lettuces</skos:prefLabel>
    </owl:NamedIndividual>
    


    <!-- http://www.foodpairing.com/ontologies/foodpairing-kg#icat:000141 -->


    <owl:NamedIndividual rdf:about="http://www.foodpairing.com/ontologies/foodpairing-kg#icat:000141">
        <rdf:type rdf:resource="http://www.foodpairing.com/ontologies/foodpairing-kg#IngredientCategory"/>
        <rdf:type rdf:resource="http://www.w3.org/2004/02/skos/core#Concept"/>
        <skos:broader rdf:resource="http://www.foodpairing.com/ontologies/foodpairing-kg#icat:000133"/>
        <skos:definition xml:lang="en">Refers to various types of photosynthetic organisms that grow in water, such as seaweed or microalgae, which can be consumed as food or used as ingredients.</skos:definition>
        <skos:prefLabel xml:lang="en">Algae</skos:prefLabel>
    </owl:NamedIndividual>
    


    <!-- http://www.foodpairing.com/ontologies/foodpairing-kg#icat:000142 -->


    <owl:NamedIndividual rdf:about="http://www.foodpairing.com/ontologies/foodpairing-kg#icat:000142">
        <rdf:type rdf:resource="http://www.foodpairing.com/ontologies/foodpairing-kg#IngredientCategory"/>
        <rdf:type rdf:resource="http://www.w3.org/2004/02/skos/core#Concept"/>
        <skos:broader rdf:resource="http://www.foodpairing.com/ontologies/foodpairing-kg#icat:000133"/>
        <skos:definition xml:lang="en">Includes edible vegetables that grow in the sea or saltwater environments, such as seaweed, kelp, or sea asparagus, often used in Asian cuisines.</skos:definition>
        <skos:prefLabel xml:lang="en">Sea Vegetables</skos:prefLabel>
    </owl:NamedIndividual>
    


    <!-- http://www.foodpairing.com/ontologies/foodpairing-kg#icat:000143 -->


    <owl:NamedIndividual rdf:about="http://www.foodpairing.com/ontologies/foodpairing-kg#icat:000143">
        <rdf:type rdf:resource="http://www.foodpairing.com/ontologies/foodpairing-kg#IngredientCategory"/>
        <rdf:type rdf:resource="http://www.w3.org/2004/02/skos/core#Concept"/>
        <skos:definition xml:lang="en">Broths and stocks are flavorful liquids used as a base for soups, sauces, and various dishes. They are created by simmering ingredients like meats, bones, vegetables, and seasonings in water to extract their flavors.</skos:definition>
        <skos:prefLabel xml:lang="en">Broths And Fonds Category</skos:prefLabel>
    </owl:NamedIndividual>
    


    <!-- http://www.foodpairing.com/ontologies/foodpairing-kg#icat:000144 -->


    <owl:NamedIndividual rdf:about="http://www.foodpairing.com/ontologies/foodpairing-kg#icat:000144">
        <rdf:type rdf:resource="http://www.foodpairing.com/ontologies/foodpairing-kg#IngredientCategory"/>
        <rdf:type rdf:resource="http://www.w3.org/2004/02/skos/core#Concept"/>
        <skos:definition xml:lang="en">A dish refers to a prepared and cooked food item that is intended to be consumed as a single serving. It can consist of one or more ingredients that have been combined and cooked together to create a specific flavor, texture, and presentation.</skos:definition>
        <skos:prefLabel xml:lang="en">Dish Category</skos:prefLabel>
    </owl:NamedIndividual>
    


    <!-- http://www.foodpairing.com/ontologies/foodpairing-kg#icat:000145 -->


    <owl:NamedIndividual rdf:about="http://www.foodpairing.com/ontologies/foodpairing-kg#icat:000145">
        <rdf:type rdf:resource="http://www.foodpairing.com/ontologies/foodpairing-kg#IngredientCategory"/>
        <rdf:type rdf:resource="http://www.w3.org/2004/02/skos/core#Concept"/>
        <skos:definition xml:lang="en">Fragrances are aromatic substances (perfums, compounds,...) that are used to add pleasant odors to people, objects, or spaces</skos:definition>
        <skos:prefLabel xml:lang="en">Fragrance Category</skos:prefLabel>
    </owl:NamedIndividual>
    


    <!-- http://www.foodpairing.com/ontologies/foodpairing-kg#icat:000146 -->


    <owl:NamedIndividual rdf:about="http://www.foodpairing.com/ontologies/foodpairing-kg#icat:000146">
        <rdf:type rdf:resource="http://www.foodpairing.com/ontologies/foodpairing-kg#IngredientCategory"/>
        <rdf:type rdf:resource="http://www.w3.org/2004/02/skos/core#Concept"/>
        <skos:definition xml:lang="en">Personal care refers to products that individuals engage in to maintain their personal hygiene, appearance, and overall well-being. Includes hygiene, skin care, hair care, oral care and cosmetics</skos:definition>
        <skos:prefLabel xml:lang="en">Personal Care Category</skos:prefLabel>
    </owl:NamedIndividual>
    


    <!-- http://www.foodpairing.com/ontologies/foodpairing-kg#icat:000147 -->


    <owl:NamedIndividual rdf:about="http://www.foodpairing.com/ontologies/foodpairing-kg#icat:000147">
        <rdf:type rdf:resource="http://www.foodpairing.com/ontologies/foodpairing-kg#IngredientCategory"/>
        <rdf:type rdf:resource="http://www.w3.org/2004/02/skos/core#Concept"/>
        <skos:broader rdf:resource="http://www.foodpairing.com/ontologies/foodpairing-kg#icat:000040"/>
        <skos:definition xml:lang="en">Type of spicy table sauce made from chili peppers or chili pepper extracts.</skos:definition>
        <skos:prefLabel xml:lang="en">Hot Sauce</skos:prefLabel>
    </owl:NamedIndividual>
    


    <!-- http://www.foodpairing.com/ontologies/foodpairing-kg#icat:000148 -->


    <owl:NamedIndividual rdf:about="http://www.foodpairing.com/ontologies/foodpairing-kg#icat:000148">
        <rdf:type rdf:resource="http://www.foodpairing.com/ontologies/foodpairing-kg#IngredientCategory"/>
        <rdf:type rdf:resource="http://www.w3.org/2004/02/skos/core#Concept"/>
        <skos:broader rdf:resource="http://www.foodpairing.com/ontologies/foodpairing-kg#icat:000061"/>
        <skos:definition xml:lang="en">Refers to a specific type of beverage designed to replenish fluids, electrolytes, and provide carbohydrates during or after intense physical activity.</skos:definition>
        <skos:prefLabel xml:lang="en">Sport Drinks</skos:prefLabel>
    </owl:NamedIndividual>
    


    <!-- http://www.foodpairing.com/ontologies/foodpairing-kg#icat:000149 -->


    <owl:NamedIndividual rdf:about="http://www.foodpairing.com/ontologies/foodpairing-kg#icat:000149">
        <rdf:type rdf:resource="http://www.foodpairing.com/ontologies/foodpairing-kg#IngredientCategory"/>
        <rdf:type rdf:resource="http://www.w3.org/2004/02/skos/core#Concept"/>
        <skos:broader rdf:resource="http://www.foodpairing.com/ontologies/foodpairing-kg#icat:000021"/>
        <skos:definition xml:lang="en">Refers to crispy or puffed snack foods made from corn; often flavored or seasoned.</skos:definition>
        <skos:prefLabel xml:lang="en">Corn Snacks</skos:prefLabel>
    </owl:NamedIndividual>
    


    <!-- http://www.foodpairing.com/ontologies/foodpairing-kg#icat:000150 -->


    <owl:NamedIndividual rdf:about="http://www.foodpairing.com/ontologies/foodpairing-kg#icat:000150">
        <rdf:type rdf:resource="http://www.foodpairing.com/ontologies/foodpairing-kg#IngredientCategory"/>
        <rdf:type rdf:resource="http://www.w3.org/2004/02/skos/core#Concept"/>
        <skos:broader rdf:resource="http://www.foodpairing.com/ontologies/foodpairing-kg#icat:000024"/>
        <skos:definition xml:lang="en">Refers to sweet-tasting, soluble carbohydrates added to foods and beverages to provide sweetness, flavor and energy. Includes natural and synthetic sugars.</skos:definition>
        <skos:prefLabel xml:lang="en">Sugars</skos:prefLabel>
    </owl:NamedIndividual>
    


    <!-- http://www.foodpairing.com/ontologies/foodpairing-kg#icat:000151 -->


    <owl:NamedIndividual rdf:about="http://www.foodpairing.com/ontologies/foodpairing-kg#icat:000151">
        <rdf:type rdf:resource="http://www.foodpairing.com/ontologies/foodpairing-kg#IngredientCategory"/>
        <rdf:type rdf:resource="http://www.w3.org/2004/02/skos/core#Concept"/>
        <skos:broader rdf:resource="http://www.foodpairing.com/ontologies/foodpairing-kg#icat:000021"/>
        <skos:definition xml:lang="en">Cookies are small, sweet, baked treats, typically made from a mixture of flour, sugar, butter, and other ingredients. Cookies come in a wide variety of flavors, shapes, and textures, and are enjoyed as a snack.</skos:definition>
        <skos:prefLabel xml:lang="en">Cookies</skos:prefLabel>
    </owl:NamedIndividual>
</rdf:RDF>



<!-- Generated by the OWL API (version 5.1.18) https://github.com/owlcs/owlapi/ -->


